@prefix : <https://w3id.org/def/phenowl#> .
@prefix owl: <http://www.w3.org/2002/07/owl#> .
@prefix rdf: <http://www.w3.org/1999/02/22-rdf-syntax-ns#> .
@prefix xml: <http://www.w3.org/XML/1998/namespace> .
@prefix xsd: <http://www.w3.org/2001/XMLSchema#> .
@prefix rdfs: <http://www.w3.org/2000/01/rdf-schema#> .
@base <https://w3id.org/def/phenowl#> .

<https://w3id.org/def/phenowl> rdf:type owl:Ontology ;
                                owl:versionIRI <https://w3id.org/def/phenowl/1.0.0> ;
                                owl:imports <http://www.opengis.net/ont/geosparql> ,
                                            <http://www.opengis.net/ont/sf> ,
                                            <http://www.w3.org/2006/time#2016> ,
                                            <https://w3id.org/seas/SystemOntology-1.1> ;
                                <http://purl.org/dc/elements/1.1/creator> "Alencar Medeiros, Gabriel H." ,
                                                                          "Soualmia, Lina F." ,
                                                                          "Zanni-Merk, Cecilia" ;
                                <http://purl.org/dc/elements/1.1/title> "PhenOWL : Core Propagation Phenomenon Ontology" ;
                                <http://purl.org/dc/terms/created> "Wed Nov 22nd, 2023" ;
                                <http://purl.org/dc/terms/license> "https://opensource.org/license/mit/" ;
                                <http://purl.org/dc/terms/modified> "Wed Nov 22nd, 2023" ;
                                <http://purl.org/vocab/vann/preferredNamespacePrefix> "phen" ;
                                <http://purl.org/vocab/vann/preferredNamespaceUri> "https://w3id.org/def/phenowl" ;
                                rdfs:comment "The Core Propagation Phenomenon Ontology (PhenOWL) is designed to represent the propagation of any phenomenon in a network, leveraging the spatiotemporal characteristics of propagation from different observation points, with the participation of multiple entities in the process. This ontology will be used in the future in a broader framework for describing, detecting, and predicting the spread of health risks in a network based on heterogeneous textual data." ;
                                owl:versionInfo "1.0.0" .

#################################################################
#    Annotation properties
#################################################################

###  http://purl.org/dc/elements/1.1/contributor
<http://purl.org/dc/elements/1.1/contributor> rdf:type owl:AnnotationProperty .


###  http://purl.org/dc/elements/1.1/creator
<http://purl.org/dc/elements/1.1/creator> rdf:type owl:AnnotationProperty .


###  http://purl.org/dc/elements/1.1/date
<http://purl.org/dc/elements/1.1/date> rdf:type owl:AnnotationProperty .


###  http://purl.org/dc/elements/1.1/description
<http://purl.org/dc/elements/1.1/description> rdf:type owl:AnnotationProperty .


###  http://purl.org/dc/elements/1.1/source
<http://purl.org/dc/elements/1.1/source> rdf:type owl:AnnotationProperty .


###  http://purl.org/dc/elements/1.1/title
<http://purl.org/dc/elements/1.1/title> rdf:type owl:AnnotationProperty .


###  http://purl.org/dc/terms/bibliographicCitation
<http://purl.org/dc/terms/bibliographicCitation> rdf:type owl:AnnotationProperty .


###  http://purl.org/dc/terms/contributor
<http://purl.org/dc/terms/contributor> rdf:type owl:AnnotationProperty .


###  http://purl.org/dc/terms/created
<http://purl.org/dc/terms/created> rdf:type owl:AnnotationProperty .


###  http://purl.org/dc/terms/creator
<http://purl.org/dc/terms/creator> rdf:type owl:AnnotationProperty .


###  http://purl.org/dc/terms/description
<http://purl.org/dc/terms/description> rdf:type owl:AnnotationProperty .


###  http://purl.org/dc/terms/isVersionOf
<http://purl.org/dc/terms/isVersionOf> rdf:type owl:AnnotationProperty .


###  http://purl.org/dc/terms/issued
<http://purl.org/dc/terms/issued> rdf:type owl:AnnotationProperty .


###  http://purl.org/dc/terms/license
<http://purl.org/dc/terms/license> rdf:type owl:AnnotationProperty .


###  http://purl.org/dc/terms/modified
<http://purl.org/dc/terms/modified> rdf:type owl:AnnotationProperty .


###  http://purl.org/dc/terms/rights
<http://purl.org/dc/terms/rights> rdf:type owl:AnnotationProperty .


###  http://purl.org/dc/terms/title
<http://purl.org/dc/terms/title> rdf:type owl:AnnotationProperty .


###  http://purl.org/vocab/vann/preferredNamespacePrefix
<http://purl.org/vocab/vann/preferredNamespacePrefix> rdf:type owl:AnnotationProperty .


###  http://purl.org/vocab/vann/preferredNamespaceUri
<http://purl.org/vocab/vann/preferredNamespaceUri> rdf:type owl:AnnotationProperty .


###  http://swrl.stanford.edu/ontologies/3.3/swrla.owl#isRuleEnabled
<http://swrl.stanford.edu/ontologies/3.3/swrla.owl#isRuleEnabled> rdf:type owl:AnnotationProperty .


###  http://www.w3.org/2001/XMLSchema#pattern
xsd:pattern rdf:type owl:AnnotationProperty .


###  http://www.w3.org/2003/06/sw-vocab-status/ns#term_status
<http://www.w3.org/2003/06/sw-vocab-status/ns#term_status> rdf:type owl:AnnotationProperty .


###  http://www.w3.org/2004/02/skos/core#altLabel
<http://www.w3.org/2004/02/skos/core#altLabel> rdf:type owl:AnnotationProperty ;
                                               rdfs:comment "The range of skos:altLabel is the class of RDF plain literals."@en ,
                                                            "skos:prefLabel, skos:altLabel and skos:hiddenLabel are pairwise disjoint properties."@en ;
                                               rdfs:isDefinedBy <http://www.w3.org/2004/02/skos/core> ;
                                               rdfs:label "alternative label"@en ;
                                               <http://www.w3.org/2004/02/skos/core#definition> "An alternative lexical label for a resource."@en ;
                                               <http://www.w3.org/2004/02/skos/core#example> "Acronyms, abbreviations, spelling variants, and irregular plural/singular forms may be included among the alternative labels for a concept. Mis-spelled terms are normally included as hidden labels (see skos:hiddenLabel)."@en ;
                                               rdfs:subPropertyOf rdfs:label .


###  http://www.w3.org/2004/02/skos/core#changeNote
<http://www.w3.org/2004/02/skos/core#changeNote> rdf:type owl:AnnotationProperty ;
                                                 rdfs:isDefinedBy <http://www.w3.org/2004/02/skos/core> ;
                                                 rdfs:label "change note"@en ;
                                                 <http://www.w3.org/2004/02/skos/core#definition> "A note about a modification to a concept."@en ;
                                                 rdfs:subPropertyOf <http://www.w3.org/2004/02/skos/core#note> .


###  http://www.w3.org/2004/02/skos/core#definition
<http://www.w3.org/2004/02/skos/core#definition> rdf:type owl:AnnotationProperty ;
                                                 rdfs:isDefinedBy <http://www.w3.org/2004/02/skos/core> ;
                                                 rdfs:label "definition"@en ;
                                                 <http://www.w3.org/2004/02/skos/core#definition> "A statement or formal explanation of the meaning of a concept."@en ;
                                                 rdfs:subPropertyOf <http://www.w3.org/2004/02/skos/core#note> .


###  http://www.w3.org/2004/02/skos/core#editorialNote
<http://www.w3.org/2004/02/skos/core#editorialNote> rdf:type owl:AnnotationProperty ;
                                                    rdfs:isDefinedBy <http://www.w3.org/2004/02/skos/core> ;
                                                    rdfs:label "editorial note"@en ;
                                                    <http://www.w3.org/2004/02/skos/core#definition> "A note for an editor, translator or maintainer of the vocabulary."@en ;
                                                    rdfs:subPropertyOf <http://www.w3.org/2004/02/skos/core#note> .


###  http://www.w3.org/2004/02/skos/core#example
<http://www.w3.org/2004/02/skos/core#example> rdf:type owl:AnnotationProperty ;
                                              rdfs:isDefinedBy <http://www.w3.org/2004/02/skos/core> ;
                                              rdfs:label "example"@en ;
                                              <http://www.w3.org/2004/02/skos/core#definition> "An example of the use of a concept."@en ;
                                              rdfs:subPropertyOf <http://www.w3.org/2004/02/skos/core#note> .


###  http://www.w3.org/2004/02/skos/core#hiddenLabel
<http://www.w3.org/2004/02/skos/core#hiddenLabel> rdf:type owl:AnnotationProperty ;
                                                  rdfs:comment "The range of skos:hiddenLabel is the class of RDF plain literals."@en ,
                                                               "skos:prefLabel, skos:altLabel and skos:hiddenLabel are pairwise disjoint properties."@en ;
                                                  rdfs:isDefinedBy <http://www.w3.org/2004/02/skos/core> ;
                                                  rdfs:label "hidden label"@en ;
                                                  <http://www.w3.org/2004/02/skos/core#definition> "A lexical label for a resource that should be hidden when generating visual displays of the resource, but should still be accessible to free text search operations."@en ;
                                                  rdfs:subPropertyOf rdfs:label .


###  http://www.w3.org/2004/02/skos/core#historyNote
<http://www.w3.org/2004/02/skos/core#historyNote> rdf:type owl:AnnotationProperty ;
                                                  rdfs:isDefinedBy <http://www.w3.org/2004/02/skos/core> ;
                                                  rdfs:label "history note"@en ;
                                                  <http://www.w3.org/2004/02/skos/core#definition> "A note about the past state/use/meaning of a concept."@en ;
                                                  rdfs:subPropertyOf <http://www.w3.org/2004/02/skos/core#note> .


###  http://www.w3.org/2004/02/skos/core#note
<http://www.w3.org/2004/02/skos/core#note> rdf:type owl:AnnotationProperty ;
                                           rdfs:isDefinedBy <http://www.w3.org/2004/02/skos/core> ;
                                           rdfs:label "note"@en ;
                                           <http://www.w3.org/2004/02/skos/core#definition> "A general note, for any purpose."@en ;
                                           <http://www.w3.org/2004/02/skos/core#scopeNote> "This property may be used directly, or as a super-property for more specific note types."@en .


###  http://www.w3.org/2004/02/skos/core#prefLabel
<http://www.w3.org/2004/02/skos/core#prefLabel> rdf:type owl:AnnotationProperty ;
                                                rdfs:comment "A resource has no more than one value of skos:prefLabel per language tag, and no more than one value of skos:prefLabel without language tag."@en ,
                                                             "The range of skos:prefLabel is the class of RDF plain literals."@en ,
                                                             """skos:prefLabel, skos:altLabel and skos:hiddenLabel are pairwise
      disjoint properties."""@en ;
                                                rdfs:isDefinedBy <http://www.w3.org/2004/02/skos/core> ;
                                                rdfs:label "preferred label"@en ;
                                                <http://www.w3.org/2004/02/skos/core#definition> "The preferred lexical label for a resource, in a given language."@en ;
                                                rdfs:subPropertyOf rdfs:label .


###  http://www.w3.org/2004/02/skos/core#scopeNote
<http://www.w3.org/2004/02/skos/core#scopeNote> rdf:type owl:AnnotationProperty ;
                                                rdfs:isDefinedBy <http://www.w3.org/2004/02/skos/core> ;
                                                rdfs:label "scope note"@en ;
                                                <http://www.w3.org/2004/02/skos/core#definition> "A note that helps to clarify the meaning and/or the use of a concept."@en ;
                                                rdfs:subPropertyOf <http://www.w3.org/2004/02/skos/core#note> .


#################################################################
#    Datatypes
#################################################################

###  http://www.opengis.net/ont/geosparql#gmlLiteral
<http://www.opengis.net/ont/geosparql#gmlLiteral> rdf:type rdfs:Datatype ;
                                                  <http://purl.org/dc/elements/1.1/contributor> "Matthew Perry" ;
                                                  <http://purl.org/dc/elements/1.1/creator> "OGC GeoSPARQL 1.0 Standard Working Group" ;
                                                  <http://purl.org/dc/elements/1.1/date> "2011-06-16"^^xsd:date ;
                                                  <http://purl.org/dc/elements/1.1/description> """
      A GML serialization of a geometry object.
    """@en ;
                                                  rdfs:comment """
      A GML serialization of a geometry object.
    """@en ;
                                                  rdfs:isDefinedBy <http://www.opengis.net/ont/geosparql> ,
                                                                   <http://www.opengis.net/spec/geosparql/1.0> ;
                                                  rdfs:label "GML Literal"@en ;
                                                  <http://www.w3.org/2004/02/skos/core#definition> """
      A GML serialization of a geometry object.
    """@en ;
                                                  <http://www.w3.org/2004/02/skos/core#prefLabel> "GML Literal"@en .


###  http://www.opengis.net/ont/geosparql#wktLiteral
<http://www.opengis.net/ont/geosparql#wktLiteral> rdf:type rdfs:Datatype ;
                                                  <http://purl.org/dc/elements/1.1/contributor> "Matthew Perry" ;
                                                  <http://purl.org/dc/elements/1.1/creator> "OGC GeoSPARQL 1.0 Standard Working Group" ;
                                                  <http://purl.org/dc/elements/1.1/date> "2011-06-16"^^xsd:date ;
                                                  <http://purl.org/dc/elements/1.1/description> """
      A Well-known Text serialization of a geometry object.
    """@en ;
                                                  rdfs:comment """
      A Well-known Text serialization of a geometry object.
    """@en ;
                                                  rdfs:isDefinedBy <http://www.opengis.net/ont/geosparql> ,
                                                                   <http://www.opengis.net/spec/geosparql/1.0> ;
                                                  rdfs:label "Well-known Text Literal"@en ;
                                                  <http://www.w3.org/2004/02/skos/core#definition> """
      A Well-known Text serialization of a geometry object.
    """@en ;
                                                  <http://www.w3.org/2004/02/skos/core#prefLabel> "Well-known Text Literal"@en .


###  http://www.w3.org/2001/XMLSchema#date
xsd:date rdf:type rdfs:Datatype .


###  http://www.w3.org/2001/XMLSchema#dateTimeStamp
xsd:dateTimeStamp rdfs:label "sello de tiempo"@es .


###  http://www.w3.org/2001/XMLSchema#duration
xsd:duration rdf:type rdfs:Datatype .


###  http://www.w3.org/2001/XMLSchema#gDay
xsd:gDay rdf:type rdfs:Datatype .


###  http://www.w3.org/2001/XMLSchema#gMonth
xsd:gMonth rdf:type rdfs:Datatype .


###  http://www.w3.org/2001/XMLSchema#gYear
xsd:gYear rdf:type rdfs:Datatype .


###  http://www.w3.org/2001/XMLSchema#gYearMonth
xsd:gYearMonth rdf:type rdfs:Datatype .


###  http://www.w3.org/2006/time#generalDay
<http://www.w3.org/2006/time#generalDay> rdf:type rdfs:Datatype ;
                                         rdfs:comment """Day of month - formulated as a text string with a pattern constraint to reproduce the same lexical form as gDay, except that values up to 99 are permitted, in order to support calendars with more than 31 days in a month. 
Note that the value-space is not defined, so a generic OWL2 processor cannot compute ordering relationships of values of this type."""@en ,
                                                      """Día del mes - formulado como una cadena de texto con una restricción patrón para reproducir la misma forma léxica que gDay, excepto que se permiten valores hasta el 99, con el propósito de proporcionar soporte a calendarios con meses con más de 31 días.
            Nótese que el espacio de valores no está definido, por tanto, un procesador genérico de OWL2 no puede computar relaciones de orden de valores de este tipo."""@es ;
                                         rdfs:label "Día generalizado"@es ,
                                                    "Generalized day"@en ;
                                         <http://www.w3.org/2004/02/skos/core#definition> """Day of month - formulated as a text string with a pattern constraint to reproduce the same lexical form as gDay, except that values up to 99 are permitted, in order to support calendars with more than 31 days in a month. 
Note that the value-space is not defined, so a generic OWL2 processor cannot compute ordering relationships of values of this type."""@en ,
                                                                                          """Día del mes - formulado como una cadena de texto con una restricción patrón para reproducir la misma forma léxica que gDay, excepto que se permiten valores hasta el 99, con el propósito de proporcionar soporte a calendarios con meses con más de 31 días.
            Nótese que el espacio de valores no está definido, por tanto, un procesador genérico de OWL2 no puede computar relaciones de orden de valores de este tipo."""@es .


###  http://www.w3.org/2006/time#generalMonth
<http://www.w3.org/2006/time#generalMonth> rdf:type rdfs:Datatype ;
                                           rdfs:comment """Mes del año - formulado como una cadena de texto con una restricción patrón para reproducir la misma forma léxica que gMonth, excepto que se permiten valores hasta el 20, con el propósito de proporcionar soporte a calendarios con años con más de 12 meses.
            Nótese que el espacio de valores no está definido, por tanto, un procesador genérico de OWL2 no puede computar relaciones de orden de valores de este tipo."""@es ,
                                                        """Month of year - formulated as a text string with a pattern constraint to reproduce the same lexical form as gMonth, except that values up to 20 are permitted, in order to support calendars with more than 12 months in the year. 
Note that the value-space is not defined, so a generic OWL2 processor cannot compute ordering relationships of values of this type."""@en ;
                                           rdfs:label "Generalized month"@en ,
                                                      "Mes generalizado"@es ;
                                           <http://www.w3.org/2004/02/skos/core#definition> """Mes del año - formulado como una cadena de texto con una restricción patrón para reproducir la misma forma léxica que gMonth, excepto que se permiten valores hasta el 20, con el propósito de proporcionar soporte a calendarios con años con más de 12 meses.
            Nótese que el espacio de valores no está definido, por tanto, un procesador genérico de OWL2 no puede computar relaciones de orden de valores de este tipo."""@es ,
                                                                                            """Month of year - formulated as a text string with a pattern constraint to reproduce the same lexical form as gMonth, except that values up to 20 are permitted, in order to support calendars with more than 12 months in the year. 
Note that the value-space is not defined, so a generic OWL2 processor cannot compute ordering relationships of values of this type."""@en .


###  http://www.w3.org/2006/time#generalYear
<http://www.w3.org/2006/time#generalYear> rdf:type rdfs:Datatype ;
                                          rdfs:comment """Número de año - formulado como una cadena de texto con una restricción patrón para reproducir la misma forma léxica que gYear, aunque no está restringido a valores del calendario gregoriano.
            Nótese que el espacio de valores no está definido, por tanto, un procesador genérico de OWL2 no puede computar relaciones de orden de valores de este tipo."""@es ,
                                                       """Year number - formulated as a text string with a pattern constraint to reproduce the same lexical form as gYear, but not restricted to values from the Gregorian calendar. 
Note that the value-space is not defined, so a generic OWL2 processor cannot compute ordering relationships of values of this type."""@en ;
                                          rdfs:label "Año generalizado"@es ,
                                                     "Generalized year"@en ;
                                          <http://www.w3.org/2004/02/skos/core#definition> """Número de año - formulado como una cadena de texto con una restricción patrón para reproducir la misma forma léxica que gYear, aunque no está restringido a valores del calendario gregoriano.
            Nótese que el espacio de valores no está definido, por tanto, un procesador genérico de OWL2 no puede computar relaciones de orden de valores de este tipo."""@es ,
                                                                                           """Year number - formulated as a text string with a pattern constraint to reproduce the same lexical form as gYear, but not restricted to values from the Gregorian calendar. 
Note that the value-space is not defined, so a generic OWL2 processor cannot compute ordering relationships of values of this type."""@en .


#################################################################
#    Object Properties
#################################################################

###  http://purl.org/nemo/gufo#broughtAbout
<http://purl.org/nemo/gufo#broughtAbout> rdf:type owl:ObjectProperty ;
                                         rdfs:domain <http://purl.org/nemo/gufo#Event> ;
                                         rdfs:range <http://purl.org/nemo/gufo#Situation> ;
                                         rdfs:comment """Identifies a gufo:Situation that is brought about by the gufo:Event.

Guizzardi et al. (2013) included a notion of \"brings-about\" that related events to a single (\"maximal\") situation, embodying all the effects of the event at the time it ends. This implementation of gufo:broughtAbout diverges from \"brings-about\" in that work because gufo:broughtAbout can be used to relate events to more than one gufo:Situation. Each gufo:Situation identified through gufo:broughtAbout should be understood as an (improper) part of the maximal situation."""@en ;
                                         rdfs:label "broughtAbout"@en .


###  http://purl.org/nemo/gufo#categorizes
<http://purl.org/nemo/gufo#categorizes> rdf:type owl:ObjectProperty ;
                                        rdfs:domain [ owl:intersectionOf ( <http://purl.org/nemo/gufo#Type>
                                                                           [ rdf:type owl:Class ;
                                                                             owl:complementOf <http://purl.org/nemo/gufo#AbstractEntityType>
                                                                           ]
                                                                           [ rdf:type owl:Class ;
                                                                             owl:complementOf <http://purl.org/nemo/gufo#ConcreteEntityType>
                                                                           ]
                                                                         ) ;
                                                      rdf:type owl:Class
                                                    ] ;
                                        rdfs:range <http://purl.org/nemo/gufo#Type> ;
                                        rdfs:comment """Identifies a gufo:Type whose instances may be classified by instances of the categorizing higher-order type.

For example, \"ShipType\" gufo:categorizes \"Ship\". Instances of \"ShipType\" such as \"Supercarrier\" and \"Cargoship\" should be declared subclasses of \"Ship\". OWL 2 punning should be used to capture the two facets of \"Supercarrier\" and \"Cargoship\" in this example: (i) as instances of \"ShipType\", and (ii) as subclasses of \"Ship\".

The categorized type is termed the \"base type\" in the \"powertype pattern\" see Carvalho et al (2017), the higher-order type is often called the \"powertype\".  

gufo:categorizes is the general (unspecific) form of categorization. See  gufo:partitions for a more specific form, in which instances of the categorized type are classified by exactly one instance of the higher-order type. 

The domain is gufo:Type excluding gufo:AbstractIndividualType as well as gufo:ConcreteIndividualTypes because those types are first-order types (their instances are individuals). Only instances of gufo:Type representing higher-order types can categorize a base type.

For further details and formalization of \"categorization\", see Carvalho et al (2017) which combines UFO with MLT (a multi-level modeling theory).  

V. A. Carvalho, J. P. A. Almeida, C. M. Fonseca, and G. Guizzardi, “Multi-level ontology-based conceptual modeling,” Data & Knowledge Engineering, vol. 109, p. 3–24, 2017. <http://dx.doi.org/10.1016/j.datak.2017.03.002>"""@en ;
                                        rdfs:label "categorizes"@en .


###  http://purl.org/nemo/gufo#concernsConstitutedEndurant
<http://purl.org/nemo/gufo#concernsConstitutedEndurant> rdf:type owl:ObjectProperty ;
                                                        rdfs:domain <http://purl.org/nemo/gufo#TemporaryConstitutionSituation> ;
                                                        rdfs:range <http://purl.org/nemo/gufo#Endurant> ;
                                                        rdfs:comment "Identifies the constituted gufo:Endurant in the gufo:TemporaryConstitutionSituation."@en ;
                                                        rdfs:label "concernsConstitutedEndurant"@en .


###  http://purl.org/nemo/gufo#concernsNonRigidType
<http://purl.org/nemo/gufo#concernsNonRigidType> rdf:type owl:ObjectProperty ,
                                                          owl:FunctionalProperty ;
                                                 rdfs:domain <http://purl.org/nemo/gufo#TemporaryInstantiationSituation> ;
                                                 rdfs:range <http://purl.org/nemo/gufo#NonRigidType> ;
                                                 rdfs:comment "Identifies the gufo:NonRigidType that is instantiated by the endurant that stands in a gufo:TemporaryInstantiationSituation."@en ;
                                                 rdfs:label "concernsNonRigidType"@en .


###  http://purl.org/nemo/gufo#concernsQualityType
<http://purl.org/nemo/gufo#concernsQualityType> rdf:type owl:ObjectProperty ,
                                                         owl:FunctionalProperty ;
                                                rdfs:domain <http://purl.org/nemo/gufo#QualityValueAttributionSituation> ;
                                                rdfs:range <http://purl.org/nemo/gufo#EndurantType> ;
                                                rdfs:comment "Identifies the quality type (a gufo:EndurantType subclassing gufo:Quality) whose value is attributed in the gufo:QualityValueAttributionSituation."@en ;
                                                rdfs:label "concernsQualityType"@en .


###  http://purl.org/nemo/gufo#concernsReifiedQualityValue
<http://purl.org/nemo/gufo#concernsReifiedQualityValue> rdf:type owl:ObjectProperty ,
                                                                 owl:FunctionalProperty ;
                                                        rdfs:domain <http://purl.org/nemo/gufo#QualityValueAttributionSituation> ;
                                                        rdfs:range <http://purl.org/nemo/gufo#QualityValue> ;
                                                        rdfs:comment <http://purl.org/nemo/gufo#concernsQualityValue> ,
                                                                     "Identifies the gufo:QualityValue (i.e., the reified quality value) associated with the endurant that stands in the gufo:QualityValueAttributionSituation."@en ;
                                                        rdfs:label "concernsReifiedQualityValue"@en .


###  http://purl.org/nemo/gufo#concernsRelatedEndurant
<http://purl.org/nemo/gufo#concernsRelatedEndurant> rdf:type owl:ObjectProperty ,
                                                             owl:FunctionalProperty ;
                                                    rdfs:domain <http://purl.org/nemo/gufo#TemporaryRelationshipSituation> ;
                                                    rdfs:range <http://purl.org/nemo/gufo#Endurant> ;
                                                    rdfs:comment "Identifies the related gufo:Endurant in the gufo:TemporaryRelationshipSituation."@en ;
                                                    rdfs:label "concernsRelatedEndurant"@en .


###  http://purl.org/nemo/gufo#concernsRelationshipType
<http://purl.org/nemo/gufo#concernsRelationshipType> rdf:type owl:ObjectProperty ,
                                                              owl:FunctionalProperty ;
                                                     rdfs:domain <http://purl.org/nemo/gufo#TemporaryRelationshipSituation> ;
                                                     rdfs:range <http://purl.org/nemo/gufo#RelationshipType> ;
                                                     rdfs:comment "Identifies the gufo:RelationshipType instantiated in the gufo:TemporaryRelationshipSituation."@en ;
                                                     rdfs:label "concernsRelationshipType"@en .


###  http://purl.org/nemo/gufo#concernsTemporaryWhole
<http://purl.org/nemo/gufo#concernsTemporaryWhole> rdf:type owl:ObjectProperty ,
                                                            owl:FunctionalProperty ;
                                                   rdfs:domain <http://purl.org/nemo/gufo#TemporaryParthoodSituation> ;
                                                   rdfs:range <http://purl.org/nemo/gufo#Endurant> ;
                                                   rdfs:comment "Identifies the whole (a gufo:Endurant) of which the endurant that stands in the gufo:TemporaryParthoodSituation is part."@en ;
                                                   rdfs:label "concernsTemporaryWhole"@en .


###  http://purl.org/nemo/gufo#constitutes
<http://purl.org/nemo/gufo#constitutes> rdf:type owl:ObjectProperty ;
                                        rdfs:domain <http://purl.org/nemo/gufo#ConcreteEntity> ;
                                        rdfs:range <http://purl.org/nemo/gufo#ConcreteEntity> ;
                                        rdfs:comment """Identifies a gufo:ConcreteIndividual that is constituted (partially) by the constituent individual.

For example, the gufo:Collection of persons whose members are John, Paul, George, Ringo constituted the beatles, the gufo:Quantity of marble that constitutes the statue of Venus de Milo, and the gufo:Event of Paul raising his arm in a meeting that constitutes his voting (also a gufo:Event).

In case constitution changes in time, see gufo:standsInQualifiedConstitution."""@en ;
                                        rdfs:label "constitutes"@en ;
                                        rdfs:seeAlso <http://purl.org/nemo/gufo#standsInQualifiedConstitution> .


###  http://purl.org/nemo/gufo#contributedToTrigger
<http://purl.org/nemo/gufo#contributedToTrigger> rdf:type owl:ObjectProperty ;
                                                 rdfs:domain <http://purl.org/nemo/gufo#Situation> ;
                                                 rdfs:range <http://purl.org/nemo/gufo#Event> ;
                                                 rdfs:comment """Identifies a gufo:Event that the gufo:Situation contributed to trigger.

Guizzardi et al. (2013) defined a notion of \"triggers\" to relate the situation satisfying all the sufficient and necessary conditions with the triggered  event. This implementation differs from  \"triggers\" as defined in that work because gufo:contributedToTrigger can be used to relate more than one gufo:Situation to a gufo:Event. Each gufo:Situation identified through gufo:contributedToTrigger should be understood as an (improper) part of the situation that triggered the event."""@en ;
                                                 rdfs:label "contributedToTrigger"@en .


###  http://purl.org/nemo/gufo#emergesFrom
<http://purl.org/nemo/gufo#emergesFrom> rdf:type owl:ObjectProperty ;
                                        rdfs:domain <http://purl.org/nemo/gufo#Event> ;
                                        rdfs:range <http://purl.org/nemo/gufo#Scene> ;
                                        rdfs:comment """A gufo:Event is restricted to an area and an interval, both being conteined in a convex spatio-temporal region. In other words, a gufo;Events emerges from within a gufo:Scene.

(i.e. \"Lebron James becoming NBA's all-time top scorer\" gufo:Event hapened in the \"7th February, 2023 in Crypto.com Arena\" gufo:Scene.)""" ;
                                        rdfs:label "emergesFrom" .


###  http://purl.org/nemo/gufo#externallyDependsOn
<http://purl.org/nemo/gufo#externallyDependsOn> rdf:type owl:ObjectProperty ,
                                                         owl:IrreflexiveProperty ;
                                                rdfs:domain <http://purl.org/nemo/gufo#ExtrinsicMode> ;
                                                rdfs:range <http://purl.org/nemo/gufo#Endurant> ;
                                                rdfs:comment """Identifies a gufo:Endurant on which the gufo:ExtrinsicMode depends.

For example, John's duty to return the book he borrowed from Mary (a gufo:ExtrinsicMode) depends externally on Mary.

The identifed gufo:Endurant should  be external to the bearer of the extrinsic mode (see Guizzardi, 2005, p. 239). In other words, the identified endurant should not be a part or an intrisic aspect of the bearer of the extrinsic mode."""@en ;
                                                rdfs:label "externallyDependsOn"@en .


###  http://purl.org/nemo/gufo#hasAssociatedQualityValueType
<http://purl.org/nemo/gufo#hasAssociatedQualityValueType> rdf:type owl:ObjectProperty ;
                                                          rdfs:domain <http://purl.org/nemo/gufo#EndurantType> ;
                                                          rdfs:range <http://purl.org/nemo/gufo#AbstractEntityType> ;
                                                          rdfs:comment """Identifies a quality value type to which the quality type is associated. 

For example, a \"Color\" quality type may be associated with a \"ColorValueInRGB\" quality value type.

It relates a specialization of gufo:Quality (an instance of gufo:EndurantType) to a specialization of gufo:QualityValue  (an instance of gufo:AbstractIndividualType).

To be used only when quality values are reified."""@en ;
                                                          rdfs:label "hasAssociatedQualityValueType"@en .


###  http://purl.org/nemo/gufo#hasBeginPoint
<http://purl.org/nemo/gufo#hasBeginPoint> rdf:type owl:ObjectProperty ;
                                          rdfs:domain <http://purl.org/nemo/gufo#ConcreteEntity> ;
                                          rdfs:range <http://www.w3.org/2006/time#Instant> ;
                                          rdfs:comment """Identifies the begin point for a gufo:ConcreteIndividual, in the case in which time instants are reified. 

In the case of endurants, this identifies the time point when the endurant comes into existence. In the case of events, this identifies the time point when the event starts to take place. In the case of situation, this identifies the time point when the situation begins to hold.

If time instants are not reified, use gufo:hasBeginPointInXSDDate or gufo:hasBeginPointInXSDDateTimeStamp."""@en ;
                                          rdfs:label "hasBeginPoint"@en ;
                                          rdfs:seeAlso <http://purl.org/nemo/gufo#hasBeginPointInXSDDate> ,
                                                       <http://purl.org/nemo/gufo#hasBeginPointInXSDDateTimeStamp> .


###  http://purl.org/nemo/gufo#hasEndPoint
<http://purl.org/nemo/gufo#hasEndPoint> rdf:type owl:ObjectProperty ;
                                        rdfs:domain <http://purl.org/nemo/gufo#ConcreteEntity> ;
                                        rdfs:range <http://www.w3.org/2006/time#Instant> ;
                                        rdfs:comment """Identifies the end point for a gufo:ConcreteIndividual, in the case in which time instants are reified.

In the case of endurants, this identifies the time point when the endurant ceases to exist. In the case of events, this identifies the time point when the event ends. In the case of situation, this identifies the time point when the situation ceases to hold."""@en ;
                                        rdfs:label "hasEndPoint"@en ;
                                        rdfs:seeAlso <http://purl.org/nemo/gufo#hasEndPointInXSDDate> ,
                                                     <http://purl.org/nemo/gufo#hasEndPointInXSDDateTimeStamp> .


###  http://purl.org/nemo/gufo#hasReifiedQualityValue
<http://purl.org/nemo/gufo#hasReifiedQualityValue> rdf:type owl:ObjectProperty ;
                                                   rdfs:domain <http://purl.org/nemo/gufo#ConcreteEntity> ;
                                                   rdfs:range <http://purl.org/nemo/gufo#QualityValue> ;
                                                   rdfs:comment """Identifies an instance of gufo:QualityValue to reflect the perception or conception of a quality in a certain value space. 

Use this property only for quality values that are to be reified in the A-box and associated with a gufo:ConcreteIndividual. Otherwise, use the gufo:hasQualityValue data property and a literal to determine the quality value.

The full representation pattern for quality values involves first identifying a gufo:Quality that inheres in a concrete individual and then associating it with a reified quality value. For example, let us consider the color of Yves Klein's \"Blue Monochrome\" painting made in 1961 (MoMA's object with number 618.1967). In the full pattern, an instance of gufo:Quality that inheres in the physical object (the color of that painting) is associated with a gufo:QualityValue (say the triplet <0, 47, 167> for that painting) through gufo:hasReifiedQualityValue. The full pattern is recommended when different quality spaces are expected to be used for the same quality. For example, the color of that painting could also be associated with a quadruple <100, 72, 0, 35> representing the same color in a CMYK space.

When the full pattern is not required, gufo:hasReifiedQualityValue can also be used to directly associate a concrete individual (without identifying the quality) with a quality value."""@en ;
                                                   rdfs:label "hasReifiedQualityValue"@en ;
                                                   rdfs:seeAlso <http://purl.org/nemo/gufo#hasQualityValue> .


###  http://purl.org/nemo/gufo#historicallyDependsOn
<http://purl.org/nemo/gufo#historicallyDependsOn> rdf:type owl:ObjectProperty ,
                                                           owl:TransitiveProperty ;
                                                  rdfs:domain <http://purl.org/nemo/gufo#ConcreteEntity> ;
                                                  rdfs:range <http://purl.org/nemo/gufo#ConcreteEntity> ;
                                                  rdfs:comment """Identifies a gufo:ConcreteIndividual on which the concrete individual depends historically. 

For example, a person is historically dependent on his/her ancestors.

When used between events, historical dependence encompasses causation (when the event is caused by the other), but also other cases where there is dependence but not causation (when the event brings about a situation that is either insufficient or more than sufficient to trigger the historically dependent event).

For example, Real Madrid's goal in the 60th minute of the 2016 FIFA Club World Cup Final is historically dependent on (and in this case caused by) a penalty kick by Cristiano Ronaldo. The penalty kick itself is historically dependent on (but not caused by) a penalty (the occurrence of the penalty is necessary but not sufficient to cause the penalty kick as authorization of the referee is required). 

Historical dependence is transitive. Hence, in the example above, Real Madrid's goal is historically dependent on the penalty."""@en ;
                                                  rdfs:label "historicallyDependsOn"@en .


###  http://purl.org/nemo/gufo#inheresIn
<http://purl.org/nemo/gufo#inheresIn> rdf:type owl:ObjectProperty ,
                                               owl:FunctionalProperty ,
                                               owl:AsymmetricProperty ,
                                               owl:IrreflexiveProperty ;
                                      rdfs:domain <http://purl.org/nemo/gufo#Aspect> ;
                                      rdfs:range <http://purl.org/nemo/gufo#ConcreteEntity> ;
                                      rdfs:comment """Identifies the gufo:ConcreteIndividual in which the gufo:Aspect inheres. Inherence is a sort of existential dependence. The identified concrete individual is the \"bearer\" of the aspect.

For example, the color of an object inheres in the object and the average speed of a flight inheres in the flight."""@en ;
                                      rdfs:label "inheresIn"@en .


###  http://purl.org/nemo/gufo#isAspectProperPartOf
<http://purl.org/nemo/gufo#isAspectProperPartOf> rdf:type owl:ObjectProperty ;
                                                 rdfs:subPropertyOf <http://purl.org/nemo/gufo#isProperPartOf> ;
                                                 rdf:type owl:TransitiveProperty ;
                                                 rdfs:domain <http://purl.org/nemo/gufo#Aspect> ;
                                                 rdfs:range <http://purl.org/nemo/gufo#Aspect> ;
                                                 rdfs:comment """Identifies a gufo:Aspect of which the aspect is a proper part.

For example, John's obligations towards Mary in the scope of their marriage is an aspect proper part of their marriage  (and same can be said of Mary's extrinsic aspects in the scope of their marriage.)

This property can be used to represent the composition of a relator from extrisinc aspects, but also to represent complex extrisinc aspects.

gufo:isAspectProperPartOf is transitive."""@en ;
                                                 rdfs:label "isAspectProperPartOf"@en .


###  http://purl.org/nemo/gufo#isCollectionMemberOf
<http://purl.org/nemo/gufo#isCollectionMemberOf> rdf:type owl:ObjectProperty ;
                                                 rdfs:subPropertyOf <http://purl.org/nemo/gufo#isObjectProperPartOf> ;
                                                 rdfs:domain <http://purl.org/nemo/gufo#Object> ;
                                                 rdfs:range <http://purl.org/nemo/gufo#Collection> ;
                                                 rdfs:comment """Identifies a gufo:Collection of which the object is a member. 

This is the relation between John and a group of persons, and between a cow and its herd.

gufo:isCollectionMemberOf is intransitive (Guizzardi, 2005, p. 185).

For membership in a gufo:VariableCollection, see gufo:standsInQualifiedParthood."""@en ;
                                                 rdfs:label "isCollectionMemberOf"@en ;
                                                 rdfs:seeAlso <http://purl.org/nemo/gufo#standsInQualifiedParthood> .


###  http://purl.org/nemo/gufo#isComponentOf
<http://purl.org/nemo/gufo#isComponentOf> rdf:type owl:ObjectProperty ;
                                          rdfs:subPropertyOf <http://purl.org/nemo/gufo#isObjectProperPartOf> ;
                                          rdfs:domain <http://purl.org/nemo/gufo#Object> ;
                                          rdfs:range <http://purl.org/nemo/gufo#FunctionalComplex> ;
                                          rdfs:comment """Identifies a gufo:FunctionalComplex of which the object is a component.

For example, the habitation module is a component of the International Space Station, and so are each of the solar panels; Obama's brain is a component of his body, and so is his heart; the engine is a component of the HMS Queen Elizabeth (R08).

gufo:isComponentOf is not transitive in the general case. Particular sub-properties may be transitive (Guizzardi, 2005, p. 183).

When a component may change its relation to be whole, see gufo:standsInQualifiedParthood."""@en ;
                                          rdfs:label "isComponentOf"@en ;
                                          rdfs:seeAlso <http://purl.org/nemo/gufo#standsInQualifiedParthood> .


###  http://purl.org/nemo/gufo#isDerivedFrom
<http://purl.org/nemo/gufo#isDerivedFrom> rdf:type owl:ObjectProperty ;
                                          rdfs:domain [ rdf:type owl:Class ;
                                                        owl:unionOf ( <http://purl.org/nemo/gufo#ComparativeRelationshipType>
                                                                      <http://purl.org/nemo/gufo#MaterialRelationshipType>
                                                                    )
                                                      ] ;
                                          rdfs:range <http://purl.org/nemo/gufo#EndurantType> ;
                                          rdfs:comment """Identifies a gufo:EndurantType from which the material or comparative relation can be derived. The identified gufo:EndurantType should be a subclass of gufo:Aspect, more specifically a subclass of gufo:ExtrinsicAspect in the case of a gufo:MaterialRelationshipType, and a subclass of gufo:IntrinsicAspect in the case of a gufo:ComparativeRelationshipType.

For example, \"marriedWith\" can be derived from \"Marriage\", \"heavierThan\" can be derived from \"Weight\".

See Fonseca et al. (2019)."""@en ;
                                          rdfs:label "isDerivedFrom"@en .


###  http://purl.org/nemo/gufo#isEventProperPartOf
<http://purl.org/nemo/gufo#isEventProperPartOf> rdf:type owl:ObjectProperty ;
                                                rdfs:subPropertyOf <http://purl.org/nemo/gufo#isProperPartOf> ;
                                                rdf:type owl:TransitiveProperty ;
                                                rdfs:domain <http://purl.org/nemo/gufo#AtomicEvent> ,
                                                            <http://purl.org/nemo/gufo#ComplexEvent> ;
                                                rdfs:range <http://purl.org/nemo/gufo#ComplexEvent> ;
                                                rdfs:comment """Identifies a gufo:Event of which the event is part. 

For example, Cristiano Ronaldo's penalty kick is an event proper part of the 2016 FIFA Club World Cup Final, having ocurred in the 60th minute of that match. That match is itself an event proper part of the 2016 FIFA Club World Cup.

The match can be decomposed in different ways. For example, we can identify the participation of each player in the match (instances of gufo:Participation that are proper parts of the match) or decomposed the match using some temporal segmentation (each minute of the match, each of which is a proper part of the match).

gufo:isEventProperPartOf is transitive."""@en ;
                                                rdfs:label "isEventProperPartOf"@en .


###  http://purl.org/nemo/gufo#isObjectProperPartOf
<http://purl.org/nemo/gufo#isObjectProperPartOf> rdf:type owl:ObjectProperty ;
                                                 rdfs:subPropertyOf <http://purl.org/nemo/gufo#isProperPartOf> ;
                                                 rdf:type owl:TransitiveProperty ;
                                                 rdfs:domain <http://purl.org/nemo/gufo#Object> ;
                                                 rdfs:range <http://purl.org/nemo/gufo#Object> ;
                                                 rdfs:comment """Identifies a gufo:Object of which the object is a part.

This is a general parthood relation between objects. Use the various sub-properties provided in order to represent specific types of parthood, each of which has specialized semantics (and different formal properties in this implementation, in particular, transitivity (Guizzardi, 2005, section 5.6)."""@en ;
                                                 rdfs:label "isObjectProperPartOf"@en .


###  http://purl.org/nemo/gufo#isProperPartOf
<http://purl.org/nemo/gufo#isProperPartOf> rdf:type owl:ObjectProperty ,
                                                    owl:TransitiveProperty ;
                                           rdfs:domain owl:Thing ;
                                           rdfs:range owl:Thing ;
                                           rdfs:comment """Identifies a whole of which the entity is a proper part.

gufo:isProperPartOf is the most generic parthood relation in this implementation. Use the various sub-properties provided in order to represent specific types of parthood.

Proper parthood (and each of its sub-properties) is asymmetric and irreflexive. Nevertheless, these characteristics are not declared in this implementation since that would violate rules of OWL 2 DL that guarantee decidability of reasoning. Instead, we have focused only on declaring transitivity where applicable.

Note that gufo:isProperPartOf (as the most general notion of parthood) is transitive, although the various sub-properties may not be transitive."""@en ;
                                           rdfs:label "isProperPartOf"@en .


###  http://purl.org/nemo/gufo#isSituationProperPartOf
<http://purl.org/nemo/gufo#isSituationProperPartOf> rdf:type owl:ObjectProperty ;
                                                    rdfs:subPropertyOf <http://purl.org/nemo/gufo#isProperPartOf> ;
                                                    rdfs:domain <http://purl.org/nemo/gufo#Situation> ;
                                                    rdfs:range <http://purl.org/nemo/gufo#Situation> ;
                                                    rdfs:comment """Identifies a gufo:Situation of which the situation is a part.

Examples include: the situation in which John has influenza is part of the situation in which John has influenza and he is tired; the situation in which John is friends with Mary is part of the situation in which he is friends with Mary and Alice; the situation in which John is married to Alice is part of the situation in which John is married to Alice, while she works at the Free University of Bozen-Bolzano."""@en ;
                                                    rdfs:label "isSituationProperPartOf"@en .


###  http://purl.org/nemo/gufo#isSubCollectionOf
<http://purl.org/nemo/gufo#isSubCollectionOf> rdf:type owl:ObjectProperty ;
                                              rdfs:subPropertyOf <http://purl.org/nemo/gufo#isObjectProperPartOf> ;
                                              rdf:type owl:TransitiveProperty ;
                                              rdfs:domain <http://purl.org/nemo/gufo#Collection> ;
                                              rdfs:range <http://purl.org/nemo/gufo#Collection> ;
                                              rdfs:comment """Identifies a gufo:Collection of which the collection is a sub-collection. All members of the sub-collection are members of the identified super-collection.

gufo:isSubCollectionOf is transitive (Guizzardi, 2005, p. 186).

For parthood involving one or more varied collections, see gufo:standsInQualifiedParthood."""@en ;
                                              rdfs:label "isSubCollectionOf"@en ;
                                              rdfs:seeAlso <http://purl.org/nemo/gufo#standsInQualifiedParthood> .


###  http://purl.org/nemo/gufo#isSubQuantityOf
<http://purl.org/nemo/gufo#isSubQuantityOf> rdf:type owl:ObjectProperty ;
                                            rdfs:subPropertyOf <http://purl.org/nemo/gufo#isObjectProperPartOf> ;
                                            rdf:type owl:TransitiveProperty ;
                                            rdfs:domain <http://purl.org/nemo/gufo#Quantity> ;
                                            rdfs:range <http://purl.org/nemo/gufo#Quantity> ;
                                            rdfs:comment """Identifies a gufo:Quantity of which the quantity is a part.

For example, the quantity of water in a wine glass is a sub-quantity of the wine in that glass.

gufo:isSubQuantityOf is transitive (Guizzardi, 2005, p. 184).

Sub-quantities are always essential parts of their wholes. Thus, gufo:standsInQualifiedParthood is not applicable for sub-quantities."""@en ;
                                            rdfs:label "isSubQuantityOf"@en .


###  http://purl.org/nemo/gufo#manifestedIn
<http://purl.org/nemo/gufo#manifestedIn> rdf:type owl:ObjectProperty ;
                                         rdfs:domain <http://purl.org/nemo/gufo#Aspect> ;
                                         rdfs:range <http://purl.org/nemo/gufo#Event> ;
                                         rdfs:comment """Identifies a gufo:Event in which the gufo:Aspect is manifested.

For example, the passing of an electrical current in a conductor is an event that encompasses the manifestation of an aspect inhering in a copper wire (the wire's  electrical conductivity)."""@en ;
                                         rdfs:label "manifestedIn"@en .


###  http://purl.org/nemo/gufo#mediates
<http://purl.org/nemo/gufo#mediates> rdf:type owl:ObjectProperty ,
                                              owl:AsymmetricProperty ,
                                              owl:IrreflexiveProperty ;
                                     rdfs:domain <http://purl.org/nemo/gufo#Relator> ;
                                     rdfs:range <http://purl.org/nemo/gufo#Endurant> ;
                                     rdfs:comment """Identifies the endurants mediated by a gufo:Relator.

For example, John and Mary's marriage mediates John and Mary."""@en ;
                                     rdfs:label "mediates"@en .


###  http://purl.org/nemo/gufo#participatedIn
<http://purl.org/nemo/gufo#participatedIn> rdf:type owl:ObjectProperty ;
                                           rdfs:domain <http://purl.org/nemo/gufo#Object> ;
                                           rdfs:range <http://purl.org/nemo/gufo#Event> ;
                                           rdfs:comment """Identifies a gufo:Event in which the gufo:Object participated.

Examples include the participation of Freddy Mercury in Queen's Live Aid Concert and the participation of an airplane in a flight."""@en ;
                                           rdfs:label "participatedIn"@en .


###  http://purl.org/nemo/gufo#partitions
<http://purl.org/nemo/gufo#partitions> rdf:type owl:ObjectProperty ;
                                       rdfs:subPropertyOf <http://purl.org/nemo/gufo#categorizes> ;
                                       rdfs:domain [ owl:intersectionOf ( <http://purl.org/nemo/gufo#Type>
                                                                          [ rdf:type owl:Class ;
                                                                            owl:complementOf <http://purl.org/nemo/gufo#AbstractEntityType>
                                                                          ]
                                                                          [ rdf:type owl:Class ;
                                                                            owl:complementOf <http://purl.org/nemo/gufo#ConcreteEntityType>
                                                                          ]
                                                                        ) ;
                                                     rdf:type owl:Class
                                                   ] ;
                                       rdfs:comment """Identifies a gufo:Type whose instances are classified by exactly one instance of the partitioning higher-order type.

For example, \"AnimalSpecies\" gufo:partitions \"Animal\". Instances of \"AnimalSpecies\" such as \"Lion\", \"Hiena\" must be disjoint subclasses of \"Animal\". OWL 2 punning should be used to capture the two facets of \"Lion\" and \"Hiena\" in this example: (i) as instances of \"AnimalSpecies\", and (ii) as  subclasses of \"Animal\".

Note that the partitioned type (in the example \"Animal\") may or may not be declared to be a disjoint union of the explicitly enumerated subclasses (such as \"Lion\", \"Hiena\"). This is because other instances of the higher-order type (\"AnimalSpecies\") may exist that are not explicitly enumerated in the ontology.

The partitioned type is termed the \"base type\" in the \"powertype pattern\" see Carvalho et al (2017), the higher-order type is often called the \"powertype\".  

For further details and formalization of \"partitioning\", see Carvalho et al (2017) which combines UFO with MLT (a multi-level modeling theory).  

V. A. Carvalho, J. P. A. Almeida, C. M. Fonseca, and G. Guizzardi, “Multi-level ontology-based conceptual modeling,” Data & Knowledge Engineering, vol. 109, p. 3–24, 2017. <http://dx.doi.org/10.1016/j.datak.2017.03.002>"""@en ;
                                       rdfs:label "partitions"@en .


###  http://purl.org/nemo/gufo#standsIn
<http://purl.org/nemo/gufo#standsIn> rdf:type owl:ObjectProperty ;
                                     rdfs:domain owl:Thing ;
                                     rdfs:range <http://purl.org/nemo/gufo#Situation> ;
                                     rdfs:comment """Identifies a gufo:Situation in which the entity stands. 

This implementation includes sub-properties of gufo:standsIn to identify situations concerning the attribution of (mutable) values to qualities, variable relationships, the instantiation of non-contingent types, temporary parthood and temporary constitution."""@en ;
                                     rdfs:label "standsIn"@en .


###  http://purl.org/nemo/gufo#standsInQualifiedAttribution
<http://purl.org/nemo/gufo#standsInQualifiedAttribution> rdf:type owl:ObjectProperty ;
                                                         rdfs:subPropertyOf <http://purl.org/nemo/gufo#standsIn> ;
                                                         rdfs:domain <http://purl.org/nemo/gufo#Endurant> ;
                                                         rdfs:range <http://purl.org/nemo/gufo#QualityValueAttributionSituation> ;
                                                         rdfs:comment "Identifies a gufo:QualityValueAttributionSituation in which the endurant stands. The identified gufo:QualityValueAttributionSituation is then used with the gufo:concernsQualityValue data property or the gufo:concernsReifiedQualityValue object property to indicate a quality value attributed to the gufo:Endurant standing in the situation. This forms a pattern to represent that quality values may differ in different situations."@en ;
                                                         rdfs:label "standsInQualifiedAttribution"@en ;
                                                         rdfs:seeAlso <http://purl.org/nemo/gufo#QualityValueAttributionSituation> .


###  http://purl.org/nemo/gufo#standsInQualifiedConstitution
<http://purl.org/nemo/gufo#standsInQualifiedConstitution> rdf:type owl:ObjectProperty ;
                                                          rdfs:subPropertyOf <http://purl.org/nemo/gufo#standsIn> ;
                                                          rdfs:domain <http://purl.org/nemo/gufo#Endurant> ;
                                                          rdfs:range <http://purl.org/nemo/gufo#TemporaryConstitutionSituation> ;
                                                          rdfs:comment """Identifies a gufo:TemporaryConstitutionSituation in which an endurant stands temporarily (as a constituent). The identified gufo:TemporaryConstitutionSituation is further related with an endurant (the whole) through the gufo:concernsConstitutedEndurant object property. This forms a pattern to represent temporary constitution, in which the relationships between constituents and constituted endurant vary in different situations.

Consider, for example, a group of people (understood as a gufo:FixedCollection) constituting a band (understood as a gufo:FunctionalComplex). In this case, any change in the membership of the group (e.g., the replacement of one person) creates a different group of people. Therefore, the band's constitution can change in time, and the pattern using gufo:TemporaryConstitutionSituation is applicable."""@en ;
                                                          rdfs:label "standsInQualifiedConstitution"@en ;
                                                          rdfs:seeAlso <http://purl.org/nemo/gufo#TemporaryConstitutionSituation> .


###  http://purl.org/nemo/gufo#standsInQualifiedInstantiation
<http://purl.org/nemo/gufo#standsInQualifiedInstantiation> rdf:type owl:ObjectProperty ;
                                                           rdfs:subPropertyOf <http://purl.org/nemo/gufo#standsIn> ;
                                                           rdfs:domain <http://purl.org/nemo/gufo#Endurant> ;
                                                           rdfs:range <http://purl.org/nemo/gufo#TemporaryInstantiationSituation> ;
                                                           rdfs:comment "Identifies a gufo:TemporaryInstantiationSituation in which the endurant stands. The identified gufo:TemporaryInstantiationSituation is further related with a gufo:NonRigidType through the gufo:concernsNonRigidType object property. This forms a pattern to represent the contigent instantiation of a non-rigid type by the endurant, in which case instantiation may vary in different situations."@en ;
                                                           rdfs:label "standsInQualifiedInstantiation"@en ;
                                                           rdfs:seeAlso <http://purl.org/nemo/gufo#TemporaryInstantiationSituation> .


###  http://purl.org/nemo/gufo#standsInQualifiedParthood
<http://purl.org/nemo/gufo#standsInQualifiedParthood> rdf:type owl:ObjectProperty ;
                                                      rdfs:subPropertyOf <http://purl.org/nemo/gufo#standsIn> ;
                                                      rdfs:domain <http://purl.org/nemo/gufo#Endurant> ;
                                                      rdfs:range <http://purl.org/nemo/gufo#TemporaryParthoodSituation> ;
                                                      rdfs:comment "Identifies a gufo:TemporaryParthoodSituation in which the endurant stands (as a temporary part). The identified gufo:TemporaryParthoodSituation is further related with an endurant (the whole) through the gufo:concernsTemporaryWhole object property. This forms a pattern to represent temporary parthood, in which the relationships between parts and wholes vary in different situations. In particular, this pattern is useful in case parts may be separated from their wholes, attached to other wholes, replaced."@en ;
                                                      rdfs:label "standsInQualifiedParthood"@en ;
                                                      rdfs:seeAlso <http://purl.org/nemo/gufo#TemporaryParthoodSituation> .


###  http://purl.org/nemo/gufo#standsInQualifiedRelationship
<http://purl.org/nemo/gufo#standsInQualifiedRelationship> rdf:type owl:ObjectProperty ;
                                                          rdfs:subPropertyOf <http://purl.org/nemo/gufo#standsIn> ;
                                                          rdfs:domain <http://purl.org/nemo/gufo#Endurant> ;
                                                          rdfs:range <http://purl.org/nemo/gufo#TemporaryRelationshipSituation> ;
                                                          rdfs:comment """Identifies a gufo:TemporaryRelationshipSituation in which the endurant stands. The identified gufo:TemporaryRelationshipSituation is then used with the gufo:concernsRelatedEndurant and the gufo:concernsRelationshipType object properties to indicate the related element and the type of relationship that applies. This forms a pattern to represent that relationships that may change in different situations. For example, \"heavierThan\" may change when the objects involved gain or lose weight.

For material relations, prefer the use of gufo:Relator."""@en ;
                                                          rdfs:label "standsInQualifiedRelationship"@en ;
                                                          rdfs:seeAlso <http://purl.org/nemo/gufo#Relator> ,
                                                                       <http://purl.org/nemo/gufo#TemporaryRelationshipSituation> .


###  http://purl.org/nemo/gufo#wasCreatedIn
<http://purl.org/nemo/gufo#wasCreatedIn> rdf:type owl:ObjectProperty ;
                                         rdfs:domain <http://purl.org/nemo/gufo#Endurant> ;
                                         rdfs:range <http://purl.org/nemo/gufo#Event> ;
                                         rdfs:comment """Identifies the gufo:Event which brought the gufo:Endurant into existence. 

For example, a musical piece is created in an act of composition (or in an event that is part of it), a piece of legislation is created in a complex legislative process.

Benevides et al. (2019) only discussed creation of objects; gufo:wasCreatedIn is extended to endurants in general. Further, in that work \"createdBy\" required the event to \"bring about\" a situation in which the created object is present. We relax this requirement here, such that the object may be created and terminated in the scope of the identified gufo:Event.

A. B. Benevides, J. R. Bourguet, G. Guizzardi, R. Penãloza, and J. P. A. Almeida, “Representing a reference foundational ontology of events in SROIQ,” Applied ontology, vol. 14, iss. 3, p. 293–334, 2019. <http://dx.doi.org/10.3233/AO-190214>"""@en ;
                                         rdfs:label "wasCreatedIn"@en .


###  http://purl.org/nemo/gufo#wasTerminatedIn
<http://purl.org/nemo/gufo#wasTerminatedIn> rdf:type owl:ObjectProperty ;
                                            rdfs:domain <http://purl.org/nemo/gufo#Endurant> ;
                                            rdfs:range <http://purl.org/nemo/gufo#Event> ;
                                            rdfs:comment """Identifies the gufo:Event in which the gufo:Endurant was brought to an end. 

For example, the Space Shuttle Challenger (OV-099) (a gufo:FunctionalComplex) was destroyed during the launch of its tenth flight (a gufo:Event). 

Benevides et al. (2019) only discussed termination of objects; gufo:wasCreatedIn is extended to endurants in general. This means that a gufo:Relator (such as a marriage) can be declared terminated. Further, in that work \"terminatedBy\" required the event to be \"triggered\" by a situation in which the terminated object is present. We relax this requirement here, such that the object may be created and terminated in the scope of the identified gufo:Event.

A. B. Benevides, J. R. Bourguet, G. Guizzardi, R. Penãloza, and J. P. A. Almeida, “Representing a reference foundational ontology of events in SROIQ,” Applied ontology, vol. 14, iss. 3, p. 293–334, 2019. <http://dx.doi.org/10.3233/AO-190214>"""@en ;
                                            rdfs:label "wasTerminatedIn"@en .


###  http://www.opengis.net/ont/geosparql#defaultGeometry
<http://www.opengis.net/ont/geosparql#defaultGeometry> rdf:type owl:ObjectProperty ;
                                                       rdfs:subPropertyOf <http://www.opengis.net/ont/geosparql#hasGeometry> ;
                                                       rdfs:domain <http://www.opengis.net/ont/geosparql#Feature> ;
                                                       rdfs:range <http://www.opengis.net/ont/geosparql#Geometry> ;
                                                       <http://purl.org/dc/elements/1.1/contributor> "Matthew Perry" ;
                                                       <http://purl.org/dc/elements/1.1/creator> "OGC GeoSPARQL 1.0 Standard Working Group" ;
                                                       <http://purl.org/dc/elements/1.1/date> "2011-06-16"^^xsd:date ;
                                                       <http://purl.org/dc/elements/1.1/description> """
      The default geometry to be used in spatial calculations.
      It is Usually the most detailed geometry.
    """@en ;
                                                       rdfs:comment """
      The default geometry to be used in spatial calculations.
      It is Usually the most detailed geometry.
    """@en ;
                                                       rdfs:isDefinedBy <http://www.opengis.net/ont/geosparql> ,
                                                                        <http://www.opengis.net/spec/geosparql/1.0> ;
                                                       rdfs:label "defaultGeometry"@en ;
                                                       <http://www.w3.org/2004/02/skos/core#definition> """
      The default geometry to be used in spatial calculations.
      It is Usually the most detailed geometry.
    """@en ;
                                                       <http://www.w3.org/2004/02/skos/core#prefLabel> "defaultGeometry"@en .


###  http://www.opengis.net/ont/geosparql#ehContains
<http://www.opengis.net/ont/geosparql#ehContains> rdf:type owl:ObjectProperty ;
                                                  rdfs:domain <http://www.opengis.net/ont/geosparql#SpatialObject> ;
                                                  rdfs:range <http://www.opengis.net/ont/geosparql#SpatialObject> ;
                                                  <http://purl.org/dc/elements/1.1/contributor> "Matthew Perry" ;
                                                  <http://purl.org/dc/elements/1.1/creator> "OGC GeoSPARQL 1.0 Standard Working Group" ;
                                                  <http://purl.org/dc/elements/1.1/date> "2011-06-16"^^xsd:date ;
                                                  <http://purl.org/dc/elements/1.1/description> """
      Exists if the subject SpatialObject spatially contains the 
      object SpatialObject. DE-9IM: T*TFF*FF*
    """@en ;
                                                  rdfs:comment """
      Exists if the subject SpatialObject spatially contains the 
      object SpatialObject. DE-9IM: T*TFF*FF*
    """@en ;
                                                  rdfs:isDefinedBy <http://www.opengis.net/ont/geosparql> ,
                                                                   <http://www.opengis.net/spec/geosparql/1.0> ;
                                                  rdfs:label "contains"@en ;
                                                  <http://www.w3.org/2004/02/skos/core#definition> """
      Exists if the subject SpatialObject spatially contains the 
      object SpatialObject. DE-9IM: T*TFF*FF*
    """@en ;
                                                  <http://www.w3.org/2004/02/skos/core#prefLabel> "contains"@en .


###  http://www.opengis.net/ont/geosparql#ehCoveredBy
<http://www.opengis.net/ont/geosparql#ehCoveredBy> rdf:type owl:ObjectProperty ;
                                                   rdfs:domain <http://www.opengis.net/ont/geosparql#SpatialObject> ;
                                                   rdfs:range <http://www.opengis.net/ont/geosparql#SpatialObject> ;
                                                   <http://purl.org/dc/elements/1.1/contributor> "Matthew Perry" ;
                                                   <http://purl.org/dc/elements/1.1/creator> "OGC GeoSPARQL 1.0 Standard Working Group" ;
                                                   <http://purl.org/dc/elements/1.1/date> "2011-06-16"^^xsd:date ;
                                                   <http://purl.org/dc/elements/1.1/description> """
      Exists if the subject SpatialObject is spatially covered 
      by the object SpatialObject. DE-9IM: TFF*TFT**
    """@en ;
                                                   rdfs:comment """
      Exists if the subject SpatialObject is spatially covered 
      by the object SpatialObject. DE-9IM: TFF*TFT**
    """@en ;
                                                   rdfs:isDefinedBy <http://www.opengis.net/ont/geosparql> ,
                                                                    <http://www.opengis.net/spec/geosparql/1.0> ;
                                                   rdfs:label "coveredBy"@en ;
                                                   <http://www.w3.org/2004/02/skos/core#definition> """
      Exists if the subject SpatialObject is spatially covered 
      by the object SpatialObject. DE-9IM: TFF*TFT**
    """@en ;
                                                   <http://www.w3.org/2004/02/skos/core#prefLabel> "coveredBy"@en .


###  http://www.opengis.net/ont/geosparql#ehCovers
<http://www.opengis.net/ont/geosparql#ehCovers> rdf:type owl:ObjectProperty ;
                                                rdfs:domain <http://www.opengis.net/ont/geosparql#SpatialObject> ;
                                                rdfs:range <http://www.opengis.net/ont/geosparql#SpatialObject> ;
                                                <http://purl.org/dc/elements/1.1/contributor> "Matthew Perry" ;
                                                <http://purl.org/dc/elements/1.1/creator> "OGC GeoSPARQL 1.0 Standard Working Group" ;
                                                <http://purl.org/dc/elements/1.1/date> "2011-06-16"^^xsd:date ;
                                                <http://purl.org/dc/elements/1.1/description> """
      Exists if the subject SpatialObject spatially covers the 
      object SpatialObject. DE-9IM: T*TFT*FF*
    """@en ;
                                                rdfs:comment """
      Exists if the subject SpatialObject spatially covers the 
      object SpatialObject. DE-9IM: T*TFT*FF*
    """@en ;
                                                rdfs:isDefinedBy <http://www.opengis.net/ont/geosparql> ,
                                                                 <http://www.opengis.net/spec/geosparql/1.0> ;
                                                rdfs:label "covers"@en ;
                                                <http://www.w3.org/2004/02/skos/core#definition> """
      Exists if the subject SpatialObject spatially covers the 
      object SpatialObject. DE-9IM: T*TFT*FF*
    """@en ;
                                                <http://www.w3.org/2004/02/skos/core#prefLabel> "covers"@en .


###  http://www.opengis.net/ont/geosparql#ehDisjoint
<http://www.opengis.net/ont/geosparql#ehDisjoint> rdf:type owl:ObjectProperty ;
                                                  rdfs:domain <http://www.opengis.net/ont/geosparql#SpatialObject> ;
                                                  rdfs:range <http://www.opengis.net/ont/geosparql#SpatialObject> ;
                                                  <http://purl.org/dc/elements/1.1/contributor> "Matthew Perry" ;
                                                  <http://purl.org/dc/elements/1.1/creator> "OGC GeoSPARQL 1.0 Standard Working Group" ;
                                                  <http://purl.org/dc/elements/1.1/date> "2011-06-16"^^xsd:date ;
                                                  <http://purl.org/dc/elements/1.1/description> """
      Exists if the subject SpatialObject is spatially disjoint
      from the object SpatialObject. DE-9IM: FF*FF****
    """@en ;
                                                  rdfs:comment """
      Exists if the subject SpatialObject is spatially disjoint
      from the object SpatialObject. DE-9IM: FF*FF****
    """@en ;
                                                  rdfs:isDefinedBy <http://www.opengis.net/ont/geosparql> ,
                                                                   <http://www.opengis.net/spec/geosparql/1.0> ;
                                                  rdfs:label "disjoint"@en ;
                                                  <http://www.w3.org/2004/02/skos/core#definition> """
      Exists if the subject SpatialObject is spatially disjoint
      from the object SpatialObject. DE-9IM: FF*FF****
    """@en ;
                                                  <http://www.w3.org/2004/02/skos/core#prefLabel> "disjoint"@en .


###  http://www.opengis.net/ont/geosparql#ehEquals
<http://www.opengis.net/ont/geosparql#ehEquals> rdf:type owl:ObjectProperty ;
                                                rdfs:domain <http://www.opengis.net/ont/geosparql#SpatialObject> ;
                                                rdfs:range <http://www.opengis.net/ont/geosparql#SpatialObject> ;
                                                <http://purl.org/dc/elements/1.1/contributor> "Matthew Perry" ;
                                                <http://purl.org/dc/elements/1.1/creator> "OGC GeoSPARQL 1.0 Standard Working Group" ;
                                                <http://purl.org/dc/elements/1.1/date> "2011-06-16"^^xsd:date ;
                                                <http://purl.org/dc/elements/1.1/description> """
      Exists if the subject SpatialObject spatially equals the 
      object SpatialObject. DE-9IM: TFFFTFFFT
    """@en ;
                                                rdfs:comment """
      Exists if the subject SpatialObject spatially equals the 
      object SpatialObject. DE-9IM: TFFFTFFFT
    """@en ;
                                                rdfs:isDefinedBy <http://www.opengis.net/ont/geosparql> ,
                                                                 <http://www.opengis.net/spec/geosparql/1.0> ;
                                                rdfs:label "equals"@en ;
                                                <http://www.w3.org/2004/02/skos/core#definition> """
      Exists if the subject SpatialObject spatially equals the 
      object SpatialObject. DE-9IM: TFFFTFFFT
    """@en ;
                                                <http://www.w3.org/2004/02/skos/core#prefLabel> "equals"@en .


###  http://www.opengis.net/ont/geosparql#ehInside
<http://www.opengis.net/ont/geosparql#ehInside> rdf:type owl:ObjectProperty ;
                                                rdfs:domain <http://www.opengis.net/ont/geosparql#SpatialObject> ;
                                                rdfs:range <http://www.opengis.net/ont/geosparql#SpatialObject> ;
                                                <http://purl.org/dc/elements/1.1/contributor> "Matthew Perry" ;
                                                <http://purl.org/dc/elements/1.1/creator> "OGC GeoSPARQL 1.0 Standard Working Group" ;
                                                <http://purl.org/dc/elements/1.1/date> "2011-06-16"^^xsd:date ;
                                                <http://purl.org/dc/elements/1.1/description> """
      Exists if the subject SpatialObject is spatially inside 
      the object SpatialObject. DE-9IM: TFF*FFT**
    """@en ;
                                                rdfs:comment """
      Exists if the subject SpatialObject is spatially inside 
      the object SpatialObject. DE-9IM: TFF*FFT**
    """@en ;
                                                rdfs:isDefinedBy <http://www.opengis.net/ont/geosparql> ,
                                                                 <http://www.opengis.net/spec/geosparql/1.0> ;
                                                rdfs:label "inside"@en ;
                                                <http://www.w3.org/2004/02/skos/core#definition> """
      Exists if the subject SpatialObject is spatially inside 
      the object SpatialObject. DE-9IM: TFF*FFT**
    """@en ;
                                                <http://www.w3.org/2004/02/skos/core#prefLabel> "inside"@en .


###  http://www.opengis.net/ont/geosparql#ehMeet
<http://www.opengis.net/ont/geosparql#ehMeet> rdf:type owl:ObjectProperty ;
                                              rdfs:domain <http://www.opengis.net/ont/geosparql#SpatialObject> ;
                                              rdfs:range <http://www.opengis.net/ont/geosparql#SpatialObject> ;
                                              <http://purl.org/dc/elements/1.1/contributor> "Matthew Perry" ;
                                              <http://purl.org/dc/elements/1.1/creator> "OGC GeoSPARQL 1.0 Standard Working Group" ;
                                              <http://purl.org/dc/elements/1.1/date> "2011-06-16"^^xsd:date ;
                                              <http://purl.org/dc/elements/1.1/description> """
      Exists if the subject SpatialObject spatially meets the 
      object SpatialObject. 
      DE-9IM: FT******* ^ F**T***** ^ F***T****
    """@en ;
                                              rdfs:comment """
      Exists if the subject SpatialObject spatially meets the 
      object SpatialObject. 
      DE-9IM: FT******* ^ F**T***** ^ F***T****
    """@en ;
                                              rdfs:isDefinedBy <http://www.opengis.net/ont/geosparql> ,
                                                               <http://www.opengis.net/spec/geosparql/1.0> ;
                                              rdfs:label "meet"@en ;
                                              <http://www.w3.org/2004/02/skos/core#definition> """
      Exists if the subject SpatialObject spatially meets the 
      object SpatialObject. 
      DE-9IM: FT******* ^ F**T***** ^ F***T****
    """@en ;
                                              <http://www.w3.org/2004/02/skos/core#prefLabel> "meet"@en .


###  http://www.opengis.net/ont/geosparql#ehOverlap
<http://www.opengis.net/ont/geosparql#ehOverlap> rdf:type owl:ObjectProperty ;
                                                 rdfs:domain <http://www.opengis.net/ont/geosparql#SpatialObject> ;
                                                 rdfs:range <http://www.opengis.net/ont/geosparql#SpatialObject> ;
                                                 <http://purl.org/dc/elements/1.1/contributor> "Matthew Perry" ;
                                                 <http://purl.org/dc/elements/1.1/creator> "OGC GeoSPARQL 1.0 Standard Working Group" ;
                                                 <http://purl.org/dc/elements/1.1/date> "2011-06-16"^^xsd:date ;
                                                 <http://purl.org/dc/elements/1.1/description> """
      Exists if the subject SpatialObject spatially overlaps the 
      object SpatialObject. DE-9IM: T*T***T**
    """@en ;
                                                 rdfs:comment """
      Exists if the subject SpatialObject spatially overlaps the 
      object SpatialObject. DE-9IM: T*T***T**
    """@en ;
                                                 rdfs:isDefinedBy <http://www.opengis.net/ont/geosparql> ,
                                                                  <http://www.opengis.net/spec/geosparql/1.0> ;
                                                 rdfs:label "overlap"@en ;
                                                 <http://www.w3.org/2004/02/skos/core#definition> """
      Exists if the subject SpatialObject spatially overlaps the 
      object SpatialObject. DE-9IM: T*T***T**
    """@en ;
                                                 <http://www.w3.org/2004/02/skos/core#prefLabel> "overlap"@en .


###  http://www.opengis.net/ont/geosparql#hasGeometry
<http://www.opengis.net/ont/geosparql#hasGeometry> rdf:type owl:ObjectProperty ;
                                                   rdfs:domain <http://www.opengis.net/ont/geosparql#Feature> ;
                                                   rdfs:range <http://www.opengis.net/ont/geosparql#Geometry> ;
                                                   <http://purl.org/dc/elements/1.1/contributor> "Matthew Perry" ;
                                                   <http://purl.org/dc/elements/1.1/creator> "OGC GeoSPARQL 1.0 Standard Working Group" ;
                                                   <http://purl.org/dc/elements/1.1/date> "2011-06-16"^^xsd:date ;
                                                   <http://purl.org/dc/elements/1.1/description> """
      A spatial representation for a given feature.
    """@en ;
                                                   rdfs:comment """
      A spatial representation for a given feature.
    """@en ;
                                                   rdfs:isDefinedBy <http://www.opengis.net/ont/geosparql> ,
                                                                    <http://www.opengis.net/spec/geosparql/1.0> ;
                                                   rdfs:label "hasGeometry"@en ;
                                                   <http://www.w3.org/2004/02/skos/core#definition> """
      A spatial representation for a given feature.
    """@en ;
                                                   <http://www.w3.org/2004/02/skos/core#prefLabel> "hasGeometry"@en .


###  http://www.opengis.net/ont/geosparql#rcc8dc
<http://www.opengis.net/ont/geosparql#rcc8dc> rdf:type owl:ObjectProperty ,
                                                       owl:SymmetricProperty ;
                                              rdfs:domain <http://www.opengis.net/ont/geosparql#SpatialObject> ;
                                              rdfs:range <http://www.opengis.net/ont/geosparql#SpatialObject> ;
                                              <http://purl.org/dc/elements/1.1/contributor> "Matthew Perry" ;
                                              <http://purl.org/dc/elements/1.1/creator> "OGC GeoSPARQL 1.0 Standard Working Group" ;
                                              <http://purl.org/dc/elements/1.1/date> "2011-06-16"^^xsd:date ;
                                              <http://purl.org/dc/elements/1.1/description> """
      Exists if the subject SpatialObject is spatially disjoint
      from the object SpatialObject. DE-9IM: FFTFFTTTT
    """@en ;
                                              rdfs:comment """
      Exists if the subject SpatialObject is spatially disjoint
      from the object SpatialObject. DE-9IM: FFTFFTTTT
    """@en ;
                                              rdfs:isDefinedBy <http://www.opengis.net/ont/geosparql> ,
                                                               <http://www.opengis.net/spec/geosparql/1.0> ;
                                              rdfs:label "disconnected"@en ;
                                              <http://www.w3.org/2004/02/skos/core#definition> """
      Exists if the subject SpatialObject is spatially disjoint
      from the object SpatialObject. DE-9IM: FFTFFTTTT
    """@en ;
                                              <http://www.w3.org/2004/02/skos/core#prefLabel> "disconnected"@en .


###  http://www.opengis.net/ont/geosparql#rcc8ec
<http://www.opengis.net/ont/geosparql#rcc8ec> rdf:type owl:ObjectProperty ,
                                                       owl:SymmetricProperty ;
                                              rdfs:domain <http://www.opengis.net/ont/geosparql#SpatialObject> ;
                                              rdfs:range <http://www.opengis.net/ont/geosparql#SpatialObject> ;
                                              <http://purl.org/dc/elements/1.1/contributor> "Matthew Perry" ;
                                              <http://purl.org/dc/elements/1.1/creator> "OGC GeoSPARQL 1.0 Standard Working Group" ;
                                              <http://purl.org/dc/elements/1.1/date> "2011-06-16"^^xsd:date ;
                                              <http://purl.org/dc/elements/1.1/description> """
      Exists if the subject SpatialObject spatially meets the 
      object SpatialObject. DE-9IM: FFTFTTTTT
    """@en ;
                                              rdfs:comment """
      Exists if the subject SpatialObject spatially meets the 
      object SpatialObject. DE-9IM: FFTFTTTTT
    """@en ;
                                              rdfs:isDefinedBy <http://www.opengis.net/ont/geosparql> ,
                                                               <http://www.opengis.net/spec/geosparql/1.0> ;
                                              rdfs:label "externally connected"@en ;
                                              <http://www.w3.org/2004/02/skos/core#definition> """
      Exists if the subject SpatialObject spatially meets the 
      object SpatialObject. DE-9IM: FFTFTTTTT
    """@en ;
                                              <http://www.w3.org/2004/02/skos/core#prefLabel> "externally connected"@en .


###  http://www.opengis.net/ont/geosparql#rcc8eq
<http://www.opengis.net/ont/geosparql#rcc8eq> rdf:type owl:ObjectProperty ,
                                                       owl:SymmetricProperty ,
                                                       owl:TransitiveProperty ;
                                              rdfs:domain <http://www.opengis.net/ont/geosparql#SpatialObject> ;
                                              rdfs:range <http://www.opengis.net/ont/geosparql#SpatialObject> ;
                                              <http://purl.org/dc/elements/1.1/contributor> "Matthew Perry" ;
                                              <http://purl.org/dc/elements/1.1/creator> "OGC GeoSPARQL 1.0 Standard Working Group" ;
                                              <http://purl.org/dc/elements/1.1/date> "2011-06-16"^^xsd:date ;
                                              <http://purl.org/dc/elements/1.1/description> """
      Exists if the subject SpatialObject spatially equals the 
      object SpatialObject. DE-9IM: TFFFTFFFT
    """@en ;
                                              rdfs:comment """
      Exists if the subject SpatialObject spatially equals the 
      object SpatialObject. DE-9IM: TFFFTFFFT
    """@en ;
                                              rdfs:isDefinedBy <http://www.opengis.net/ont/geosparql> ,
                                                               <http://www.opengis.net/spec/geosparql/1.0> ;
                                              rdfs:label "equals"@en ;
                                              <http://www.w3.org/2004/02/skos/core#definition> """
      Exists if the subject SpatialObject spatially equals the 
      object SpatialObject. DE-9IM: TFFFTFFFT
    """@en ;
                                              <http://www.w3.org/2004/02/skos/core#prefLabel> "equals"@en .


###  http://www.opengis.net/ont/geosparql#rcc8ntpp
<http://www.opengis.net/ont/geosparql#rcc8ntpp> rdf:type owl:ObjectProperty ;
                                                owl:inverseOf <http://www.opengis.net/ont/geosparql#rcc8ntppi> ;
                                                rdf:type owl:TransitiveProperty ;
                                                rdfs:domain <http://www.opengis.net/ont/geosparql#SpatialObject> ;
                                                rdfs:range <http://www.opengis.net/ont/geosparql#SpatialObject> ;
                                                <http://purl.org/dc/elements/1.1/contributor> "Matthew Perry" ;
                                                <http://purl.org/dc/elements/1.1/creator> "OGC GeoSPARQL 1.0 Standard Working Group" ;
                                                <http://purl.org/dc/elements/1.1/date> "2011-06-16"^^xsd:date ;
                                                <http://purl.org/dc/elements/1.1/description> """
      Exists if the subject SpatialObject is spatially inside 
      the object SpatialObject. DE-9IM: TFFTFFTTT
    """@en ;
                                                rdfs:comment """
      Exists if the subject SpatialObject is spatially inside 
      the object SpatialObject. DE-9IM: TFFTFFTTT
    """@en ;
                                                rdfs:isDefinedBy <http://www.opengis.net/ont/geosparql> ,
                                                                 <http://www.opengis.net/spec/geosparql/1.0> ;
                                                rdfs:label "non-tangential proper part"@en ;
                                                <http://www.w3.org/2004/02/skos/core#definition> """
      Exists if the subject SpatialObject is spatially inside 
      the object SpatialObject. DE-9IM: TFFTFFTTT
    """@en ;
                                                <http://www.w3.org/2004/02/skos/core#prefLabel> "non-tangential proper part"@en .


###  http://www.opengis.net/ont/geosparql#rcc8ntppi
<http://www.opengis.net/ont/geosparql#rcc8ntppi> rdf:type owl:ObjectProperty ,
                                                          owl:TransitiveProperty ;
                                                 rdfs:domain <http://www.opengis.net/ont/geosparql#SpatialObject> ;
                                                 rdfs:range <http://www.opengis.net/ont/geosparql#SpatialObject> ;
                                                 <http://purl.org/dc/elements/1.1/contributor> "Matthew Perry" ;
                                                 <http://purl.org/dc/elements/1.1/creator> "OGC GeoSPARQL 1.0 Standard Working Group" ;
                                                 <http://purl.org/dc/elements/1.1/date> "2011-06-16"^^xsd:date ;
                                                 <http://purl.org/dc/elements/1.1/description> """
      Exists if the subject SpatialObject spatially contains the 
      object SpatialObject. DE-9IM: TTTFFTFFT
    """@en ;
                                                 rdfs:comment """
      Exists if the subject SpatialObject spatially contains the 
      object SpatialObject. DE-9IM: TTTFFTFFT
    """@en ;
                                                 rdfs:isDefinedBy <http://www.opengis.net/ont/geosparql> ,
                                                                  <http://www.opengis.net/spec/geosparql/1.0> ;
                                                 rdfs:label "non-tangential proper part inverse"@en ;
                                                 <http://www.w3.org/2004/02/skos/core#definition> """
      Exists if the subject SpatialObject spatially contains the 
      object SpatialObject. DE-9IM: TTTFFTFFT
    """@en ;
                                                 <http://www.w3.org/2004/02/skos/core#prefLabel> "non-tangential proper part inverse"@en .


###  http://www.opengis.net/ont/geosparql#rcc8po
<http://www.opengis.net/ont/geosparql#rcc8po> rdf:type owl:ObjectProperty ,
                                                       owl:SymmetricProperty ;
                                              rdfs:domain <http://www.opengis.net/ont/geosparql#SpatialObject> ;
                                              rdfs:range <http://www.opengis.net/ont/geosparql#SpatialObject> ;
                                              <http://purl.org/dc/elements/1.1/contributor> "Matthew Perry" ;
                                              <http://purl.org/dc/elements/1.1/creator> "OGC GeoSPARQL 1.0 Standard Working Group" ;
                                              <http://purl.org/dc/elements/1.1/date> "2011-06-16"^^xsd:date ;
                                              <http://purl.org/dc/elements/1.1/description> """
      Exists if the subject SpatialObject spatially overlaps the 
      object SpatialObject. DE-9IM: TTTTTTTTT
    """@en ;
                                              rdfs:comment """
      Exists if the subject SpatialObject spatially overlaps the 
      object SpatialObject. DE-9IM: TTTTTTTTT
    """@en ;
                                              rdfs:isDefinedBy <http://www.opengis.net/ont/geosparql> ,
                                                               <http://www.opengis.net/spec/geosparql/1.0> ;
                                              rdfs:label "partially overlapping"@en ;
                                              <http://www.w3.org/2004/02/skos/core#definition> """
      Exists if the subject SpatialObject spatially overlaps the 
      object SpatialObject. DE-9IM: TTTTTTTTT
    """@en ;
                                              <http://www.w3.org/2004/02/skos/core#prefLabel> "partially overlapping"@en .


###  http://www.opengis.net/ont/geosparql#rcc8tpp
<http://www.opengis.net/ont/geosparql#rcc8tpp> rdf:type owl:ObjectProperty ;
                                               owl:inverseOf <http://www.opengis.net/ont/geosparql#rcc8tppi> ;
                                               rdf:type owl:TransitiveProperty ;
                                               rdfs:domain <http://www.opengis.net/ont/geosparql#SpatialObject> ;
                                               rdfs:range <http://www.opengis.net/ont/geosparql#SpatialObject> ;
                                               <http://purl.org/dc/elements/1.1/contributor> "Matthew Perry" ;
                                               <http://purl.org/dc/elements/1.1/creator> "OGC GeoSPARQL 1.0 Standard Working Group" ;
                                               <http://purl.org/dc/elements/1.1/date> "2011-06-16"^^xsd:date ;
                                               <http://purl.org/dc/elements/1.1/description> """
      Exists if the subject SpatialObject is spatially covered 
      by the object SpatialObject. DE-9IM: TFFTTFTTT
    """@en ;
                                               rdfs:comment """
      Exists if the subject SpatialObject is spatially covered 
      by the object SpatialObject. DE-9IM: TFFTTFTTT
    """@en ;
                                               rdfs:isDefinedBy <http://www.opengis.net/ont/geosparql> ,
                                                                <http://www.opengis.net/spec/geosparql/1.0> ;
                                               rdfs:label "tangential proper part"@en ;
                                               <http://www.w3.org/2004/02/skos/core#definition> """
      Exists if the subject SpatialObject is spatially covered 
      by the object SpatialObject. DE-9IM: TFFTTFTTT
    """@en ;
                                               <http://www.w3.org/2004/02/skos/core#prefLabel> "tangential proper part"@en .


###  http://www.opengis.net/ont/geosparql#rcc8tppi
<http://www.opengis.net/ont/geosparql#rcc8tppi> rdf:type owl:ObjectProperty ,
                                                         owl:TransitiveProperty ;
                                                rdfs:domain <http://www.opengis.net/ont/geosparql#SpatialObject> ;
                                                rdfs:range <http://www.opengis.net/ont/geosparql#SpatialObject> ;
                                                <http://purl.org/dc/elements/1.1/contributor> "Matthew Perry" ;
                                                <http://purl.org/dc/elements/1.1/creator> "OGC GeoSPARQL 1.0 Standard Working Group" ;
                                                <http://purl.org/dc/elements/1.1/date> "2011-06-16"^^xsd:date ;
                                                <http://purl.org/dc/elements/1.1/description> """
      Exists if the subject SpatialObject spatially covers the 
      object SpatialObject. DE-9IM: TTTFTTFFT
    """@en ;
                                                rdfs:comment """
      Exists if the subject SpatialObject spatially covers the 
      object SpatialObject. DE-9IM: TTTFTTFFT
    """@en ;
                                                rdfs:isDefinedBy <http://www.opengis.net/ont/geosparql> ,
                                                                 <http://www.opengis.net/spec/geosparql/1.0> ;
                                                rdfs:label "tangential proper part inverse"@en ;
                                                <http://www.w3.org/2004/02/skos/core#definition> """
      Exists if the subject SpatialObject spatially covers the 
      object SpatialObject. DE-9IM: TTTFTTFFT
    """@en ;
                                                <http://www.w3.org/2004/02/skos/core#prefLabel> "tangential proper part inverse"@en .


###  http://www.opengis.net/ont/geosparql#sfContains
<http://www.opengis.net/ont/geosparql#sfContains> rdf:type owl:ObjectProperty ;
                                                  rdfs:domain <http://www.opengis.net/ont/geosparql#SpatialObject> ;
                                                  rdfs:range <http://www.opengis.net/ont/geosparql#SpatialObject> ;
                                                  <http://purl.org/dc/elements/1.1/contributor> "Matthew Perry" ;
                                                  <http://purl.org/dc/elements/1.1/creator> "OGC GeoSPARQL 1.0 Standard Working Group" ;
                                                  <http://purl.org/dc/elements/1.1/date> "2011-06-16"^^xsd:date ;
                                                  <http://purl.org/dc/elements/1.1/description> """
      Exists if the subject SpatialObject spatially contains the 
      object SpatialObject. DE-9IM: T*****FF*
    """@en ;
                                                  rdfs:comment """
      Exists if the subject SpatialObject spatially contains the 
      object SpatialObject. DE-9IM: T*****FF*
    """@en ;
                                                  rdfs:isDefinedBy <http://www.opengis.net/ont/geosparql> ,
                                                                   <http://www.opengis.net/spec/geosparql/1.0> ;
                                                  rdfs:label "contains"@en ;
                                                  <http://www.w3.org/2004/02/skos/core#definition> """
      Exists if the subject SpatialObject spatially contains the 
      object SpatialObject. DE-9IM: T*****FF*
    """@en ;
                                                  <http://www.w3.org/2004/02/skos/core#prefLabel> "contains"@en .


###  http://www.opengis.net/ont/geosparql#sfCrosses
<http://www.opengis.net/ont/geosparql#sfCrosses> rdf:type owl:ObjectProperty ;
                                                 rdfs:domain <http://www.opengis.net/ont/geosparql#SpatialObject> ;
                                                 rdfs:range <http://www.opengis.net/ont/geosparql#SpatialObject> ;
                                                 <http://purl.org/dc/elements/1.1/contributor> "Matthew Perry" ;
                                                 <http://purl.org/dc/elements/1.1/creator> "OGC GeoSPARQL 1.0 Standard Working Group" ;
                                                 <http://purl.org/dc/elements/1.1/date> "2011-06-16"^^xsd:date ;
                                                 <http://purl.org/dc/elements/1.1/description> """
      Exists if the subject SpatialObject spatially crosses the 
      object SpatialObject. DE-9IM: T*T******
    """@en ;
                                                 rdfs:comment """
      Exists if the subject SpatialObject spatially crosses the 
      object SpatialObject. DE-9IM: T*T******
    """@en ;
                                                 rdfs:isDefinedBy <http://www.opengis.net/ont/geosparql> ,
                                                                  <http://www.opengis.net/spec/geosparql/1.0> ;
                                                 rdfs:label "crosses"@en ;
                                                 <http://www.w3.org/2004/02/skos/core#definition> """
      Exists if the subject SpatialObject spatially crosses the 
      object SpatialObject. DE-9IM: T*T******
    """@en ;
                                                 <http://www.w3.org/2004/02/skos/core#prefLabel> "crosses"@en .


###  http://www.opengis.net/ont/geosparql#sfDisjoint
<http://www.opengis.net/ont/geosparql#sfDisjoint> rdf:type owl:ObjectProperty ;
                                                  rdfs:domain <http://www.opengis.net/ont/geosparql#SpatialObject> ;
                                                  rdfs:range <http://www.opengis.net/ont/geosparql#SpatialObject> ;
                                                  <http://purl.org/dc/elements/1.1/contributor> "Matthew Perry" ;
                                                  <http://purl.org/dc/elements/1.1/creator> "OGC GeoSPARQL 1.0 Standard Working Group" ;
                                                  <http://purl.org/dc/elements/1.1/date> "2011-06-16"^^xsd:date ;
                                                  <http://purl.org/dc/elements/1.1/description> """
      Exists if the subject SpatialObject is spatially disjoint 
      from the object SpatialObject. DE-9IM: FF*FF****
    """@en ;
                                                  rdfs:comment """
      Exists if the subject SpatialObject is spatially disjoint 
      from the object SpatialObject. DE-9IM: FF*FF****
    """@en ;
                                                  rdfs:isDefinedBy <http://www.opengis.net/ont/geosparql> ,
                                                                   <http://www.opengis.net/spec/geosparql/1.0> ;
                                                  rdfs:label "disjoint"@en ;
                                                  <http://www.w3.org/2004/02/skos/core#definition> """
      Exists if the subject SpatialObject is spatially disjoint 
      from the object SpatialObject. DE-9IM: FF*FF****
    """@en ;
                                                  <http://www.w3.org/2004/02/skos/core#prefLabel> "disjoint"@en .


###  http://www.opengis.net/ont/geosparql#sfEquals
<http://www.opengis.net/ont/geosparql#sfEquals> rdf:type owl:ObjectProperty ;
                                                rdfs:domain <http://www.opengis.net/ont/geosparql#SpatialObject> ;
                                                rdfs:range <http://www.opengis.net/ont/geosparql#SpatialObject> ;
                                                <http://purl.org/dc/elements/1.1/contributor> "Matthew Perry" ;
                                                <http://purl.org/dc/elements/1.1/creator> "OGC GeoSPARQL 1.0 Standard Working Group" ;
                                                <http://purl.org/dc/elements/1.1/date> "2011-06-16"^^xsd:date ;
                                                <http://purl.org/dc/elements/1.1/description> """
      Exists if the subject SpatialObject spatially equals the 
      object SpatialObject. DE-9IM: TFFFTFFFT
    """@en ;
                                                rdfs:comment """
      Exists if the subject SpatialObject spatially equals the 
      object SpatialObject. DE-9IM: TFFFTFFFT
    """@en ;
                                                rdfs:isDefinedBy <http://www.opengis.net/ont/geosparql> ,
                                                                 <http://www.opengis.net/spec/geosparql/1.0> ;
                                                rdfs:label "equals"@en ;
                                                <http://www.w3.org/2004/02/skos/core#definition> """
      Exists if the subject SpatialObject spatially equals the 
      object SpatialObject. DE-9IM: TFFFTFFFT
    """@en ;
                                                <http://www.w3.org/2004/02/skos/core#prefLabel> "equals"@en .


###  http://www.opengis.net/ont/geosparql#sfIntersects
<http://www.opengis.net/ont/geosparql#sfIntersects> rdf:type owl:ObjectProperty ;
                                                    rdfs:domain <http://www.opengis.net/ont/geosparql#SpatialObject> ;
                                                    rdfs:range <http://www.opengis.net/ont/geosparql#SpatialObject> ;
                                                    <http://purl.org/dc/elements/1.1/contributor> "Matthew Perry" ;
                                                    <http://purl.org/dc/elements/1.1/creator> "OGC GeoSPARQL 1.0 Standard Working Group" ;
                                                    <http://purl.org/dc/elements/1.1/date> "2011-06-16"^^xsd:date ;
                                                    <http://purl.org/dc/elements/1.1/description> """
      Exists if the subject SpatialObject is not spatially disjoint 
      from the object SpatialObject.
      DE-9IM: T******** ^ *T******* ^ ***T***** ^ ****T**** 
    """@en ;
                                                    rdfs:comment """
      Exists if the subject SpatialObject is not spatially disjoint 
      from the object SpatialObject.
      DE-9IM: T******** ^ *T******* ^ ***T***** ^ ****T**** 
    """@en ;
                                                    rdfs:isDefinedBy <http://www.opengis.net/ont/geosparql> ,
                                                                     <http://www.opengis.net/spec/geosparql/1.0> ;
                                                    rdfs:label "intersects"@en ;
                                                    <http://www.w3.org/2004/02/skos/core#definition> """
      Exists if the subject SpatialObject is not spatially disjoint 
      from the object SpatialObject.
      DE-9IM: T******** ^ *T******* ^ ***T***** ^ ****T**** 
    """@en ;
                                                    <http://www.w3.org/2004/02/skos/core#prefLabel> "intersects"@en .


###  http://www.opengis.net/ont/geosparql#sfOverlaps
<http://www.opengis.net/ont/geosparql#sfOverlaps> rdf:type owl:ObjectProperty ;
                                                  rdfs:domain <http://www.opengis.net/ont/geosparql#SpatialObject> ;
                                                  rdfs:range <http://www.opengis.net/ont/geosparql#SpatialObject> ;
                                                  <http://purl.org/dc/elements/1.1/contributor> "Matthew Perry" ;
                                                  <http://purl.org/dc/elements/1.1/creator> "OGC GeoSPARQL 1.0 Standard Working Group" ;
                                                  <http://purl.org/dc/elements/1.1/date> "2011-06-16"^^xsd:date ;
                                                  <http://purl.org/dc/elements/1.1/description> """
      Exists if the subject SpatialObject spatially overlaps the 
      object SpatialObject. DE-9IM: T*T***T** 
    """@en ;
                                                  rdfs:comment """
      Exists if the subject SpatialObject spatially overlaps the 
      object SpatialObject. DE-9IM: T*T***T** 
    """@en ;
                                                  rdfs:isDefinedBy <http://www.opengis.net/ont/geosparql> ,
                                                                   <http://www.opengis.net/spec/geosparql/1.0> ;
                                                  rdfs:label "overlaps"@en ;
                                                  <http://www.w3.org/2004/02/skos/core#definition> """
      Exists if the subject SpatialObject spatially overlaps the 
      object SpatialObject. DE-9IM: T*T***T** 
    """@en ;
                                                  <http://www.w3.org/2004/02/skos/core#prefLabel> "overlaps"@en .


###  http://www.opengis.net/ont/geosparql#sfTouches
<http://www.opengis.net/ont/geosparql#sfTouches> rdf:type owl:ObjectProperty ;
                                                 rdfs:domain <http://www.opengis.net/ont/geosparql#SpatialObject> ;
                                                 rdfs:range <http://www.opengis.net/ont/geosparql#SpatialObject> ;
                                                 <http://purl.org/dc/elements/1.1/contributor> "Matthew Perry" ;
                                                 <http://purl.org/dc/elements/1.1/creator> "OGC GeoSPARQL 1.0 Standard Working Group" ;
                                                 <http://purl.org/dc/elements/1.1/date> "2011-06-16"^^xsd:date ;
                                                 <http://purl.org/dc/elements/1.1/description> """
      Exists if the subject SpatialObject spatially touches the 
      object SpatialObject.
      DE-9IM: FT******* ^ F**T***** ^ F***T****
    """@en ;
                                                 rdfs:comment """
      Exists if the subject SpatialObject spatially touches the 
      object SpatialObject.
      DE-9IM: FT******* ^ F**T***** ^ F***T****
    """@en ;
                                                 rdfs:isDefinedBy <http://www.opengis.net/ont/geosparql> ,
                                                                  <http://www.opengis.net/spec/geosparql/1.0> ;
                                                 rdfs:label "touches"@en ;
                                                 <http://www.w3.org/2004/02/skos/core#definition> """
      Exists if the subject SpatialObject spatially touches the 
      object SpatialObject.
      DE-9IM: FT******* ^ F**T***** ^ F***T****
    """@en ;
                                                 <http://www.w3.org/2004/02/skos/core#prefLabel> "touches"@en .


###  http://www.opengis.net/ont/geosparql#sfWithin
<http://www.opengis.net/ont/geosparql#sfWithin> rdf:type owl:ObjectProperty ;
                                                rdfs:domain <http://www.opengis.net/ont/geosparql#SpatialObject> ;
                                                rdfs:range <http://www.opengis.net/ont/geosparql#SpatialObject> ;
                                                <http://purl.org/dc/elements/1.1/contributor> "Matthew Perry" ;
                                                <http://purl.org/dc/elements/1.1/creator> "OGC GeoSPARQL 1.0 Standard Working Group" ;
                                                <http://purl.org/dc/elements/1.1/date> "2011-06-16"^^xsd:date ;
                                                <http://purl.org/dc/elements/1.1/description> """
      Exists if the subject SpatialObject is spatially within the 
      object SpatialObject. DE-9IM: T*F**F***
    """@en ;
                                                rdfs:comment """
      Exists if the subject SpatialObject is spatially within the 
      object SpatialObject. DE-9IM: T*F**F***
    """@en ;
                                                rdfs:isDefinedBy <http://www.opengis.net/ont/geosparql> ,
                                                                 <http://www.opengis.net/spec/geosparql/1.0> ;
                                                rdfs:label "within"@en ;
                                                <http://www.w3.org/2004/02/skos/core#definition> """
      Exists if the subject SpatialObject is spatially within the 
      object SpatialObject. DE-9IM: T*F**F***
    """@en ;
                                                <http://www.w3.org/2004/02/skos/core#prefLabel> "within"@en .


###  http://www.w3.org/2004/02/skos/core#broadMatch
<http://www.w3.org/2004/02/skos/core#broadMatch> rdf:type owl:ObjectProperty ;
                                                 rdfs:subPropertyOf <http://www.w3.org/2004/02/skos/core#broader> ,
                                                                    <http://www.w3.org/2004/02/skos/core#mappingRelation> ;
                                                 owl:inverseOf <http://www.w3.org/2004/02/skos/core#narrowMatch> ;
                                                 rdfs:isDefinedBy <http://www.w3.org/2004/02/skos/core> ;
                                                 rdfs:label "has broader match"@en ;
                                                 <http://www.w3.org/2004/02/skos/core#definition> "skos:broadMatch is used to state a hierarchical mapping link between two conceptual resources in different concept schemes."@en .


###  http://www.w3.org/2004/02/skos/core#broader
<http://www.w3.org/2004/02/skos/core#broader> rdf:type owl:ObjectProperty ;
                                              rdfs:subPropertyOf <http://www.w3.org/2004/02/skos/core#broaderTransitive> ;
                                              owl:inverseOf <http://www.w3.org/2004/02/skos/core#narrower> ;
                                              rdfs:comment "Broader concepts are typically rendered as parents in a concept hierarchy (tree)."@en ;
                                              rdfs:isDefinedBy <http://www.w3.org/2004/02/skos/core> ;
                                              rdfs:label "has broader"@en ;
                                              <http://www.w3.org/2004/02/skos/core#definition> "Relates a concept to a concept that is more general in meaning."@en ;
                                              <http://www.w3.org/2004/02/skos/core#scopeNote> "By convention, skos:broader is only used to assert an immediate (i.e. direct) hierarchical link between two conceptual resources."@en .


###  http://www.w3.org/2004/02/skos/core#broaderTransitive
<http://www.w3.org/2004/02/skos/core#broaderTransitive> rdf:type owl:ObjectProperty ;
                                                        rdfs:subPropertyOf <http://www.w3.org/2004/02/skos/core#semanticRelation> ;
                                                        owl:inverseOf <http://www.w3.org/2004/02/skos/core#narrowerTransitive> ;
                                                        rdf:type owl:TransitiveProperty ;
                                                        rdfs:isDefinedBy <http://www.w3.org/2004/02/skos/core> ;
                                                        rdfs:label "has broader transitive"@en ;
                                                        <http://www.w3.org/2004/02/skos/core#definition> "skos:broaderTransitive is a transitive superproperty of skos:broader." ;
                                                        <http://www.w3.org/2004/02/skos/core#scopeNote> "By convention, skos:broaderTransitive is not used to make assertions. Rather, the properties can be used to draw inferences about the transitive closure of the hierarchical relation, which is useful e.g. when implementing a simple query expansion algorithm in a search application."@en .


###  http://www.w3.org/2004/02/skos/core#closeMatch
<http://www.w3.org/2004/02/skos/core#closeMatch> rdf:type owl:ObjectProperty ;
                                                 rdfs:subPropertyOf <http://www.w3.org/2004/02/skos/core#mappingRelation> ;
                                                 rdf:type owl:SymmetricProperty ;
                                                 rdfs:isDefinedBy <http://www.w3.org/2004/02/skos/core> ;
                                                 rdfs:label "has close match"@en ;
                                                 <http://www.w3.org/2004/02/skos/core#definition> "skos:closeMatch is used to link two concepts that are sufficiently similar that they can be used interchangeably in some information retrieval applications. In order to avoid the possibility of \"compound errors\" when combining mappings across more than two concept schemes, skos:closeMatch is not declared to be a transitive property."@en .


###  http://www.w3.org/2004/02/skos/core#exactMatch
<http://www.w3.org/2004/02/skos/core#exactMatch> rdf:type owl:ObjectProperty ;
                                                 rdfs:subPropertyOf <http://www.w3.org/2004/02/skos/core#closeMatch> ;
                                                 rdf:type owl:SymmetricProperty ,
                                                          owl:TransitiveProperty ;
                                                 rdfs:comment "skos:exactMatch is disjoint with each of the properties skos:broadMatch and skos:relatedMatch."@en ;
                                                 rdfs:isDefinedBy <http://www.w3.org/2004/02/skos/core> ;
                                                 rdfs:label "has exact match"@en ;
                                                 <http://www.w3.org/2004/02/skos/core#definition> "skos:exactMatch is used to link two concepts, indicating a high degree of confidence that the concepts can be used interchangeably across a wide range of information retrieval applications. skos:exactMatch is a transitive property, and is a sub-property of skos:closeMatch."@en .


###  http://www.w3.org/2004/02/skos/core#hasTopConcept
<http://www.w3.org/2004/02/skos/core#hasTopConcept> rdf:type owl:ObjectProperty ;
                                                    owl:inverseOf <http://www.w3.org/2004/02/skos/core#topConceptOf> ;
                                                    rdfs:domain <http://www.w3.org/2004/02/skos/core#ConceptScheme> ;
                                                    rdfs:range <http://www.w3.org/2004/02/skos/core#Concept> ;
                                                    rdfs:isDefinedBy <http://www.w3.org/2004/02/skos/core> ;
                                                    rdfs:label "has top concept"@en ;
                                                    <http://www.w3.org/2004/02/skos/core#definition> "Relates, by convention, a concept scheme to a concept which is topmost in the broader/narrower concept hierarchies for that scheme, providing an entry point to these hierarchies."@en .


###  http://www.w3.org/2004/02/skos/core#inScheme
<http://www.w3.org/2004/02/skos/core#inScheme> rdf:type owl:ObjectProperty ;
                                               rdfs:range <http://www.w3.org/2004/02/skos/core#ConceptScheme> ;
                                               rdfs:isDefinedBy <http://www.w3.org/2004/02/skos/core> ;
                                               rdfs:label "is in scheme"@en ;
                                               <http://www.w3.org/2004/02/skos/core#definition> "Relates a resource (for example a concept) to a concept scheme in which it is included."@en ;
                                               <http://www.w3.org/2004/02/skos/core#scopeNote> "A concept may be a member of more than one concept scheme."@en .


###  http://www.w3.org/2004/02/skos/core#mappingRelation
<http://www.w3.org/2004/02/skos/core#mappingRelation> rdf:type owl:ObjectProperty ;
                                                      rdfs:subPropertyOf <http://www.w3.org/2004/02/skos/core#semanticRelation> ;
                                                      rdfs:comment "These concept mapping relations mirror semantic relations, and the data model defined below is similar (with the exception of skos:exactMatch) to the data model defined for semantic relations. A distinct vocabulary is provided for concept mapping relations, to provide a convenient way to differentiate links within a concept scheme from links between concept schemes. However, this pattern of usage is not a formal requirement of the SKOS data model, and relies on informal definitions of best practice."@en ;
                                                      rdfs:isDefinedBy <http://www.w3.org/2004/02/skos/core> ;
                                                      rdfs:label "is in mapping relation with"@en ;
                                                      <http://www.w3.org/2004/02/skos/core#definition> "Relates two concepts coming, by convention, from different schemes, and that have comparable meanings"@en .


###  http://www.w3.org/2004/02/skos/core#member
<http://www.w3.org/2004/02/skos/core#member> rdf:type owl:ObjectProperty ;
                                             rdfs:domain <http://www.w3.org/2004/02/skos/core#Collection> ;
                                             rdfs:range [ rdf:type owl:Class ;
                                                          owl:unionOf ( <http://www.w3.org/2004/02/skos/core#Collection>
                                                                        <http://www.w3.org/2004/02/skos/core#Concept>
                                                                      )
                                                        ] ;
                                             rdfs:isDefinedBy <http://www.w3.org/2004/02/skos/core> ;
                                             rdfs:label "has member"@en ;
                                             <http://www.w3.org/2004/02/skos/core#definition> "Relates a collection to one of its members."@en .


###  http://www.w3.org/2004/02/skos/core#memberList
<http://www.w3.org/2004/02/skos/core#memberList> rdf:type owl:ObjectProperty ,
                                                          owl:FunctionalProperty ;
                                                 rdfs:domain <http://www.w3.org/2004/02/skos/core#OrderedCollection> ;
                                                 rdfs:range rdf:List ;
                                                 rdfs:comment """For any resource, every item in the list given as the value of the
      skos:memberList property is also a value of the skos:member property."""@en ;
                                                 rdfs:isDefinedBy <http://www.w3.org/2004/02/skos/core> ;
                                                 rdfs:label "has member list"@en ;
                                                 <http://www.w3.org/2004/02/skos/core#definition> "Relates an ordered collection to the RDF list containing its members."@en .


###  http://www.w3.org/2004/02/skos/core#narrowMatch
<http://www.w3.org/2004/02/skos/core#narrowMatch> rdf:type owl:ObjectProperty ;
                                                  rdfs:subPropertyOf <http://www.w3.org/2004/02/skos/core#mappingRelation> ,
                                                                     <http://www.w3.org/2004/02/skos/core#narrower> ;
                                                  rdfs:isDefinedBy <http://www.w3.org/2004/02/skos/core> ;
                                                  rdfs:label "has narrower match"@en ;
                                                  <http://www.w3.org/2004/02/skos/core#definition> "skos:narrowMatch is used to state a hierarchical mapping link between two conceptual resources in different concept schemes."@en .


###  http://www.w3.org/2004/02/skos/core#narrower
<http://www.w3.org/2004/02/skos/core#narrower> rdf:type owl:ObjectProperty ;
                                               rdfs:subPropertyOf <http://www.w3.org/2004/02/skos/core#narrowerTransitive> ;
                                               rdfs:comment "Narrower concepts are typically rendered as children in a concept hierarchy (tree)."@en ;
                                               rdfs:isDefinedBy <http://www.w3.org/2004/02/skos/core> ;
                                               rdfs:label "has narrower"@en ;
                                               <http://www.w3.org/2004/02/skos/core#definition> "Relates a concept to a concept that is more specific in meaning."@en ;
                                               <http://www.w3.org/2004/02/skos/core#scopeNote> "By convention, skos:broader is only used to assert an immediate (i.e. direct) hierarchical link between two conceptual resources."@en .


###  http://www.w3.org/2004/02/skos/core#narrowerTransitive
<http://www.w3.org/2004/02/skos/core#narrowerTransitive> rdf:type owl:ObjectProperty ;
                                                         rdfs:subPropertyOf <http://www.w3.org/2004/02/skos/core#semanticRelation> ;
                                                         rdf:type owl:TransitiveProperty ;
                                                         rdfs:isDefinedBy <http://www.w3.org/2004/02/skos/core> ;
                                                         rdfs:label "has narrower transitive"@en ;
                                                         <http://www.w3.org/2004/02/skos/core#definition> "skos:narrowerTransitive is a transitive superproperty of skos:narrower." ;
                                                         <http://www.w3.org/2004/02/skos/core#scopeNote> "By convention, skos:narrowerTransitive is not used to make assertions. Rather, the properties can be used to draw inferences about the transitive closure of the hierarchical relation, which is useful e.g. when implementing a simple query expansion algorithm in a search application."@en .


###  http://www.w3.org/2004/02/skos/core#related
<http://www.w3.org/2004/02/skos/core#related> rdf:type owl:ObjectProperty ;
                                              rdfs:subPropertyOf <http://www.w3.org/2004/02/skos/core#semanticRelation> ;
                                              rdf:type owl:SymmetricProperty ;
                                              rdfs:comment "skos:related is disjoint with skos:broaderTransitive"@en ;
                                              rdfs:isDefinedBy <http://www.w3.org/2004/02/skos/core> ;
                                              rdfs:label "has related"@en ;
                                              <http://www.w3.org/2004/02/skos/core#definition> "Relates a concept to a concept with which there is an associative semantic relationship."@en .


###  http://www.w3.org/2004/02/skos/core#relatedMatch
<http://www.w3.org/2004/02/skos/core#relatedMatch> rdf:type owl:ObjectProperty ;
                                                   rdfs:subPropertyOf <http://www.w3.org/2004/02/skos/core#mappingRelation> ,
                                                                      <http://www.w3.org/2004/02/skos/core#related> ;
                                                   rdf:type owl:SymmetricProperty ;
                                                   rdfs:isDefinedBy <http://www.w3.org/2004/02/skos/core> ;
                                                   rdfs:label "has related match"@en ;
                                                   <http://www.w3.org/2004/02/skos/core#definition> "skos:relatedMatch is used to state an associative mapping link between two conceptual resources in different concept schemes."@en .


###  http://www.w3.org/2004/02/skos/core#semanticRelation
<http://www.w3.org/2004/02/skos/core#semanticRelation> rdf:type owl:ObjectProperty ;
                                                       rdfs:domain <http://www.w3.org/2004/02/skos/core#Concept> ;
                                                       rdfs:range <http://www.w3.org/2004/02/skos/core#Concept> ;
                                                       rdfs:isDefinedBy <http://www.w3.org/2004/02/skos/core> ;
                                                       rdfs:label "is in semantic relation with"@en ;
                                                       <http://www.w3.org/2004/02/skos/core#definition> "Links a concept to a concept related by meaning."@en ;
                                                       <http://www.w3.org/2004/02/skos/core#scopeNote> "This property should not be used directly, but as a super-property for all properties denoting a relationship of meaning between concepts."@en .


###  http://www.w3.org/2004/02/skos/core#topConceptOf
<http://www.w3.org/2004/02/skos/core#topConceptOf> rdf:type owl:ObjectProperty ;
                                                   rdfs:subPropertyOf <http://www.w3.org/2004/02/skos/core#inScheme> ;
                                                   rdfs:domain <http://www.w3.org/2004/02/skos/core#Concept> ;
                                                   rdfs:range <http://www.w3.org/2004/02/skos/core#ConceptScheme> ;
                                                   rdfs:isDefinedBy <http://www.w3.org/2004/02/skos/core> ;
                                                   rdfs:label "is top concept in scheme"@en ;
                                                   <http://www.w3.org/2004/02/skos/core#definition> "Relates a concept to the concept scheme that it is a top level concept of."@en .


###  http://www.w3.org/2006/time#after
<http://www.w3.org/2006/time#after> rdf:type owl:ObjectProperty ;
                                    owl:inverseOf <http://www.w3.org/2006/time#before> ;
                                    rdfs:domain <http://www.w3.org/2006/time#TemporalEntity> ;
                                    rdfs:range <http://www.w3.org/2006/time#TemporalEntity> ;
                                    rdfs:comment "Asume una dirección en el tiempo. Si una entidad temporal T1 está después de otra entidad temporal T2, entonces el principio de T1 está después del final de T2."@es ,
                                                 "The subject is a temporal entity that occurs after the object. If a temporal entity T1 is after another temporal entity T2, then the beginning of T1 is after the end of T2."@en ;
                                    rdfs:label "después"@es ,
                                               "is after"@en ;
                                    <http://www.w3.org/2004/02/skos/core#definition> "Asume una dirección en el tiempo. Si una entidad temporal T1 está después de otra entidad temporal T2, entonces el principio de T1 está después del final de T2."@es ,
                                                                                     "Gives directionality to time. If a temporal entity T1 is after another temporal entity T2, then the beginning of T1 is after the end of T2."@en .


###  http://www.w3.org/2006/time#before
<http://www.w3.org/2006/time#before> rdf:type owl:ObjectProperty ,
                                              owl:TransitiveProperty ;
                                     rdfs:domain <http://www.w3.org/2006/time#TemporalEntity> ;
                                     rdfs:range <http://www.w3.org/2006/time#TemporalEntity> ;
                                     rdfs:comment "Asume una dirección en el tiempo. Si una entidad temporal T1 está antes que otra entidad temporal T2, entonces el final de T1 está antes que el principio de T2. Así, \"antes\" se puede considerar básica para instantes y derivada para intervalos."@es ,
                                                  "The subject is a temporal entity that occurs before the object. If a temporal entity T1 is before another temporal entity T2, then the end of T1 is before the beginning of T2. Thus, \"before\" can be considered to be basic to instants and derived for intervals."@en ;
                                     rdfs:label "antes"@es ,
                                                "is before"@en ;
                                     <http://www.w3.org/2004/02/skos/core#definition> "Asume una dirección en el tiempo. Si una entidad temporal T1 está antes que otra entidad temporal T2, entonces el final de T1 está antes que el principio de T2. Así, \"antes\" se puede considerar básica para instantes y derivada para intervalos."@es ,
                                                                                      "Gives directionality to time. If a temporal entity T1 is before another temporal entity T2, then the end of T1 is before the beginning of T2. Thus, \"before\" can be considered to be basic to instants and derived for intervals."@en .


###  http://www.w3.org/2006/time#dayOfWeek
<http://www.w3.org/2006/time#dayOfWeek> rdf:type owl:ObjectProperty ;
                                        rdfs:domain <http://www.w3.org/2006/time#GeneralDateTimeDescription> ;
                                        rdfs:range <http://www.w3.org/2006/time#DayOfWeek> ;
                                        rdfs:comment "The day of week, whose value is a member of the class time:DayOfWeek"@en ,
                                                     "El día de la semana, cuyo valor es un miembro de la clase 'día de la semana'." ;
                                        rdfs:label "day of week"@en ,
                                                   "día de la semana"@es ;
                                        <http://www.w3.org/2004/02/skos/core#definition> "El día de la semana, cuyo valor es un miembro de la clase 'día de la semana'."@es ,
                                                                                         "The day of week, whose value is a member of the class time:DayOfWeek"@en .


###  http://www.w3.org/2006/time#hasBeginning
<http://www.w3.org/2006/time#hasBeginning> rdf:type owl:ObjectProperty ;
                                           rdfs:subPropertyOf <http://www.w3.org/2006/time#hasTime> ;
                                           rdfs:domain <http://www.w3.org/2006/time#TemporalEntity> ;
                                           rdfs:range <http://www.w3.org/2006/time#Instant> ;
                                           rdfs:comment "Beginning of a temporal entity"@en ,
                                                        "Comienzo de una entidad temporal."@es ;
                                           rdfs:label "has beginning"@en ,
                                                      "tiene principio"@es ;
                                           <http://www.w3.org/2004/02/skos/core#definition> "Beginning of a temporal entity."@en ,
                                                                                            "Comienzo de una entidad temporal."@es .


###  http://www.w3.org/2006/time#hasDateTimeDescription
<http://www.w3.org/2006/time#hasDateTimeDescription> rdf:type owl:ObjectProperty ;
                                                     rdfs:domain <http://www.w3.org/2006/time#DateTimeInterval> ;
                                                     rdfs:range <http://www.w3.org/2006/time#GeneralDateTimeDescription> ;
                                                     rdfs:comment "Valor de intervalo de fecha-hora expresado como un valor estructurado. El principio y el final del intervalo coincide con los límites del elemento más corto en la descripción."@es ,
                                                                  "Value of DateTimeInterval expressed as a structured value. The beginning and end of the interval coincide with the limits of the shortest element in the description."@en ;
                                                     rdfs:label "has Date-Time description"@en ,
                                                                "tiene descripción fecha-hora"@es ;
                                                     <http://www.w3.org/2004/02/skos/core#definition> "Valor de intervalo de fecha-hora expresado como un valor estructurado. El principio y el final del intervalo coincide con los límites del elemento más corto en la descripción."@es ,
                                                                                                      "Value of DateTimeInterval expressed as a structured value. The beginning and end of the interval coincide with the limits of the shortest element in the description."@en .


###  http://www.w3.org/2006/time#hasDuration
<http://www.w3.org/2006/time#hasDuration> rdf:type owl:ObjectProperty ;
                                          rdfs:subPropertyOf <http://www.w3.org/2006/time#hasTemporalDuration> ;
                                          rdfs:range <http://www.w3.org/2006/time#Duration> ;
                                          rdfs:comment "Duración de una entidad temporal, expresada como un valor escalado o un valor nominal."@es ,
                                                       "Duration of a temporal entity, expressed as a scaled value or nominal value"@en ;
                                          rdfs:label "has duration"@en ,
                                                     "tiene duración"@es ;
                                          <http://www.w3.org/2004/02/skos/core#definition> "Duración de una entidad temporal, evento o actividad, o cosa, expresada como un valor escalado."@es ,
                                                                                           "Duration of a temporal entity, event or activity, or thing, expressed as a scaled value"@en .


###  http://www.w3.org/2006/time#hasDurationDescription
<http://www.w3.org/2006/time#hasDurationDescription> rdf:type owl:ObjectProperty ;
                                                     rdfs:subPropertyOf <http://www.w3.org/2006/time#hasTemporalDuration> ;
                                                     rdfs:range <http://www.w3.org/2006/time#GeneralDurationDescription> ;
                                                     rdfs:comment "Duración de una entidad temporal, expresada utilizando una descripción estructurada."@es ,
                                                                  "Duration of a temporal entity, expressed using a structured description"@en ;
                                                     rdfs:label "has duration description"@en ,
                                                                "tiene descripción de duración"@es ;
                                                     <http://www.w3.org/2004/02/skos/core#definition> "Duración de una entidad temporal, expresada utilizando una descripción estructurada."@es ,
                                                                                                      "Duration of a temporal entity, expressed using a structured description"@en .


###  http://www.w3.org/2006/time#hasEnd
<http://www.w3.org/2006/time#hasEnd> rdf:type owl:ObjectProperty ;
                                     rdfs:subPropertyOf <http://www.w3.org/2006/time#hasTime> ;
                                     rdfs:domain <http://www.w3.org/2006/time#TemporalEntity> ;
                                     rdfs:range <http://www.w3.org/2006/time#Instant> ;
                                     rdfs:comment "End of a temporal entity."@en ,
                                                  "Final de una entidad temporal."@es ;
                                     rdfs:label "has end"@en ,
                                                "tiene fin"@es ;
                                     <http://www.w3.org/2004/02/skos/core#definition> "End of a temporal entity."@en ,
                                                                                      "Final de una entidad temporal."@es .


###  http://www.w3.org/2006/time#hasTRS
<http://www.w3.org/2006/time#hasTRS> rdf:type owl:ObjectProperty ,
                                              owl:FunctionalProperty ;
                                     rdfs:domain [ rdf:type owl:Class ;
                                                   owl:unionOf ( <http://www.w3.org/2006/time#GeneralDurationDescription>
                                                                 <http://www.w3.org/2006/time#TemporalPosition>
                                                               )
                                                 ] ;
                                     rdfs:range <http://www.w3.org/2006/time#TRS> ;
                                     rdfs:comment "El sistema de referencia temporal utilizado por una posición temporal o descripción de extensión."@es ,
                                                  "The temporal reference system used by a temporal position or extent description. "@en ;
                                     rdfs:label "Temporal reference system used"@en ,
                                                "sistema de referencia temporal utilizado"@es ;
                                     <http://www.w3.org/2004/02/skos/core#definition> "El sistema de referencia temporal utilizado por una posición temporal o descripción de extensión."@es ,
                                                                                      "The temporal reference system used by a temporal position or extent description. "@en .


###  http://www.w3.org/2006/time#hasTemporalDuration
<http://www.w3.org/2006/time#hasTemporalDuration> rdf:type owl:ObjectProperty ;
                                                  rdfs:domain <http://www.w3.org/2006/time#TemporalEntity> ;
                                                  rdfs:range <http://www.w3.org/2006/time#TemporalDuration> ;
                                                  rdfs:comment "Duración de una entidad temporal."@es ,
                                                               "Duration of a temporal entity."@en ;
                                                  rdfs:label "has temporal duration"@en ,
                                                             "tiene duración temporal"@es ;
                                                  <http://www.w3.org/2004/02/skos/core#definition> "Duración de una entidad temporal."@es ,
                                                                                                   "Duration of a temporal entity."@en .


###  http://www.w3.org/2006/time#hasTime
<http://www.w3.org/2006/time#hasTime> rdf:type owl:ObjectProperty ;
                                      rdfs:range <http://www.w3.org/2006/time#TemporalEntity> ;
                                      rdfs:comment "Proporciona soporte a la asociación de una entidad temporal (instante o intervalo) a cualquier cosa."@es ,
                                                   "Supports the association of a temporal entity (instant or interval) to any thing"@en ;
                                      rdfs:label "has time"@en ,
                                                 "tiene tiempo"@es ;
                                      <http://www.w3.org/2004/02/skos/core#definition> "Proporciona soporte a la asociación de una entidad temporal (instante o intervalo) a cualquier cosa."@es ,
                                                                                       "Supports the association of a temporal entity (instant or interval) to any thing"@en ;
                                      <http://www.w3.org/2004/02/skos/core#editorialNote> "Característica arriesgada -añadida en la revisión del 2017 que no ha sido todavía utilizada de forma amplia."@es ,
                                                                                          "Feature at risk - added in 2017 revision, and not yet widely used. "@en .


###  http://www.w3.org/2006/time#inDateTime
<http://www.w3.org/2006/time#inDateTime> rdf:type owl:ObjectProperty ;
                                         rdfs:subPropertyOf <http://www.w3.org/2006/time#inTemporalPosition> ;
                                         rdfs:domain <http://www.w3.org/2006/time#Instant> ;
                                         rdfs:range <http://www.w3.org/2006/time#GeneralDateTimeDescription> ;
                                         rdfs:comment "Posición de un instante, expresada utilizando una descripción estructurada."@es ,
                                                      "Position of an instant, expressed using a structured description"@en ;
                                         rdfs:label "en descripción de fecha-hora"@es ,
                                                    "in date-time description"@en ;
                                         <http://www.w3.org/2004/02/skos/core#definition> "Posición de un instante, expresada utilizando una descripción estructurada."@es ,
                                                                                          "Position of an instant, expressed using a structured description"@en .


###  http://www.w3.org/2006/time#inTemporalPosition
<http://www.w3.org/2006/time#inTemporalPosition> rdf:type owl:ObjectProperty ;
                                                 rdfs:domain <http://www.w3.org/2006/time#Instant> ;
                                                 rdfs:range <http://www.w3.org/2006/time#TemporalPosition> ;
                                                 rdfs:comment "Posición de un instante de tiempo."@es ,
                                                              "Position of a time instant"@en ;
                                                 rdfs:label "Temporal position"@en ,
                                                            "posición temporal"@es ;
                                                 <http://www.w3.org/2004/02/skos/core#definition> "Posición de un instante de tiempo."@es ,
                                                                                                  "Position of a time instant"@en .


###  http://www.w3.org/2006/time#inTimePosition
<http://www.w3.org/2006/time#inTimePosition> rdf:type owl:ObjectProperty ;
                                             rdfs:subPropertyOf <http://www.w3.org/2006/time#inTemporalPosition> ;
                                             rdfs:domain <http://www.w3.org/2006/time#Instant> ;
                                             rdfs:range <http://www.w3.org/2006/time#TimePosition> ;
                                             rdfs:comment "Posición de un instante, expresada como una coordenada temporal o un valor nominal."@es ,
                                                          "Position of an instant, expressed as a temporal coordinate or nominal value"@en ;
                                             rdfs:label "Time position"@en ,
                                                        "posición de tiempo"@es ;
                                             <http://www.w3.org/2004/02/skos/core#definition> "Posición de un instante, expresada como una coordenada temporal o un valor nominal."@es ,
                                                                                              "Position of a time instant expressed as a TimePosition"@en .


###  http://www.w3.org/2006/time#inside
<http://www.w3.org/2006/time#inside> rdf:type owl:ObjectProperty ;
                                     rdfs:domain <http://www.w3.org/2006/time#Interval> ;
                                     rdfs:range <http://www.w3.org/2006/time#Instant> ;
                                     rdfs:comment "An instant that falls inside the interval. It is not intended to include beginnings and ends of intervals."@en ,
                                                  "Un instante que cae dentro del intervalo. Se asume que no es ni el principio ni el final de ningún intervalo."@es ;
                                     rdfs:label "has time instant inside"@en ,
                                                "tiene instante de tiempo dentro"@es ;
                                     <http://www.w3.org/2004/02/skos/core#definition> "An instant that falls inside the interval. It is not intended to include beginnings and ends of intervals."@en ,
                                                                                      "Un instante que cae dentro del intervalo. Se asume que no es ni el principio ni el final de ningún intervalo."@es .


###  http://www.w3.org/2006/time#intervalAfter
<http://www.w3.org/2006/time#intervalAfter> rdf:type owl:ObjectProperty ;
                                            rdfs:subPropertyOf <http://www.w3.org/2006/time#after> ,
                                                               <http://www.w3.org/2006/time#intervalDisjoint> ;
                                            owl:inverseOf <http://www.w3.org/2006/time#intervalBefore> ;
                                            rdfs:domain <http://www.w3.org/2006/time#ProperInterval> ;
                                            rdfs:range <http://www.w3.org/2006/time#ProperInterval> ;
                                            rdfs:comment "If a proper interval T1 is intervalAfter another proper interval T2, then the beginning of T1 is after the end of T2."@en ,
                                                         "Si un intervalo propio T1 es posterior a otro intervalo propio T2, entonces el principio de T1 está después que el final de T2." ;
                                            rdfs:label "interval after"@en ,
                                                       "intervalo posterior"@es ;
                                            <http://www.w3.org/2004/02/skos/core#definition> "If a proper interval T1 is intervalAfter another proper interval T2, then the beginning of T1 is after the end of T2."@en ,
                                                                                             "Si un intervalo propio T1 es posterior a otro intervalo propio T2, entonces el principio de T1 está después que el final de T2."@es .


###  http://www.w3.org/2006/time#intervalBefore
<http://www.w3.org/2006/time#intervalBefore> rdf:type owl:ObjectProperty ;
                                             rdfs:subPropertyOf <http://www.w3.org/2006/time#before> ,
                                                                <http://www.w3.org/2006/time#intervalDisjoint> ;
                                             rdfs:domain <http://www.w3.org/2006/time#ProperInterval> ;
                                             rdfs:range <http://www.w3.org/2006/time#ProperInterval> ;
                                             rdfs:comment "If a proper interval T1 is intervalBefore another proper interval T2, then the end of T1 is before the beginning of T2."@en ,
                                                          "Si un intervalo propio T1 está antes que otro intervalo propio T2, entonces el final de T1 está antes que el principio de T2."@es ;
                                             rdfs:label "interval before"@en ,
                                                        "intervalo anterior"@es ;
                                             <http://www.w3.org/2004/02/skos/core#definition> "If a proper interval T1 is intervalBefore another proper interval T2, then the end of T1 is before the beginning of T2."@en ,
                                                                                              "Si un intervalo propio T1 está antes que otro intervalo propio T2, entonces el final de T1 está antes que el principio de T2."@es .


###  http://www.w3.org/2006/time#intervalContains
<http://www.w3.org/2006/time#intervalContains> rdf:type owl:ObjectProperty ;
                                               owl:inverseOf <http://www.w3.org/2006/time#intervalDuring> ;
                                               rdfs:domain <http://www.w3.org/2006/time#ProperInterval> ;
                                               rdfs:range <http://www.w3.org/2006/time#ProperInterval> ;
                                               rdfs:comment "If a proper interval T1 is intervalContains another proper interval T2, then the beginning of T1 is before the beginning of T2, and the end of T1 is after the end of T2."@en ,
                                                            "Si un intervalo propio T1 contiene otro intervalo propio T2, entonces el principio de T1 está antes que el principio de T2, y el final de T1 está después del final de T2."@es ;
                                               rdfs:label "interval contains"@en ,
                                                          "intervalo contiene"@es ;
                                               <http://www.w3.org/2004/02/skos/core#definition> "If a proper interval T1 is intervalContains another proper interval T2, then the beginning of T1 is before the beginning of T2, and the end of T1 is after the end of T2."@en ,
                                                                                                "Si un intervalo propio T1 contiene otro intervalo propio T2, entonces el principio de T1 está antes que el principio de T2, y el final de T1 está después del final de T2."@es .


###  http://www.w3.org/2006/time#intervalDisjoint
<http://www.w3.org/2006/time#intervalDisjoint> rdf:type owl:ObjectProperty ;
                                               rdfs:domain <http://www.w3.org/2006/time#ProperInterval> ;
                                               rdfs:range <http://www.w3.org/2006/time#ProperInterval> ;
                                               rdfs:comment "If a proper interval T1 is intervalDisjoint another proper interval T2, then the beginning of T1 is after the end of T2, or the end of T1 is before the beginning of T2, i.e. the intervals do not overlap in any way, but their ordering relationship is not known."@en ,
                                                            "Si un intervalo propio T1 es disjunto con otro intervalo propio T2, entonces el principio de T1 está después del final de T2, o el final de T1 está antes que el principio de T2, es decir, los intervalos no se solapan de ninguna forma, aunque su relación de orden no se conozca."@es ;
                                               rdfs:label "interval disjoint"@en ,
                                                          "intervalo disjunto"@es ;
                                               <http://www.w3.org/2004/02/skos/core#definition> "If a proper interval T1 is intervalDisjoint another proper interval T2, then the beginning of T1 is after the end of T2, or the end of T1 is before the beginning of T2, i.e. the intervals do not overlap in any way, but their ordering relationship is not known."@en ,
                                                                                                "Si un intervalo propio T1 es disjunto con otro intervalo propio T2, entonces el principio de T1 está después del final de T2, o el final de T1 está antes que el principio de T2, es decir, los intervalos no se solapan de ninguna forma, aunque su relación de orden no se conozca."@es ;
                                               <http://www.w3.org/2004/02/skos/core#note> "Esta relación entre intervalos no estaba incluida en las 13 relaciones básicas definidas por Allen (1984), pero está definida en T.3 como la unión de 'intervalo anterior' con 'intervalo posterior'. Sin embargo, esto está fuera de la expresividad de OWL2, por tanto, está implementado como una propiedad explícita, con 'intervalo anterior' e 'intervalo posterior' como sub-propiedades."@es ,
                                                                                          "This interval relation is not included in the 13 basic relationships defined in Allen (1984), but is defined in (T.3) as the union of :intervalBefore v :intervalAfter . However, that is outside OWL2 expressivity, so is implemented as an explicit property, with :intervalBefore , :intervalAfter as sub-properties"@en .


###  http://www.w3.org/2006/time#intervalDuring
<http://www.w3.org/2006/time#intervalDuring> rdf:type owl:ObjectProperty ;
                                             rdfs:subPropertyOf <http://www.w3.org/2006/time#intervalIn> ;
                                             rdfs:domain <http://www.w3.org/2006/time#ProperInterval> ;
                                             rdfs:range <http://www.w3.org/2006/time#ProperInterval> ;
                                             rdfs:comment "If a proper interval T1 is intervalDuring another proper interval T2, then the beginning of T1 is after the beginning of T2, and the end of T1 is before the end of T2."@en ,
                                                          "Si un intervalo propio T1 está durante otro intervalo propio T2, entonces del principio de T1 está después del principio de T2, y el final de T1 está antes que el final de T2."@es ;
                                             rdfs:label "interval during"@en ,
                                                        "intervalo durante"@es ;
                                             <http://www.w3.org/2004/02/skos/core#definition> "If a proper interval T1 is intervalDuring another proper interval T2, then the beginning of T1 is after the beginning of T2, and the end of T1 is before the end of T2."@en ,
                                                                                              "Si un intervalo propio T1 está durante otro intervalo propio T2, entonces del principio de T1 está después del principio de T2, y el final de T1 está antes que el final de T2."@es .


###  http://www.w3.org/2006/time#intervalEquals
<http://www.w3.org/2006/time#intervalEquals> rdf:type owl:ObjectProperty ,
                                                      owl:SymmetricProperty ;
                                             rdfs:domain <http://www.w3.org/2006/time#ProperInterval> ;
                                             rdfs:range <http://www.w3.org/2006/time#ProperInterval> ;
                                             owl:propertyDisjointWith <http://www.w3.org/2006/time#intervalIn> ;
                                             rdfs:comment "If a proper interval T1 is intervalEquals another proper interval T2, then the beginning of T1 is coincident with the beginning of T2, and the end of T1 is coincident with the end of T2."@en ,
                                                          "Si un intervalo propio T1 es igual a otro intervalo propio T2, entonces el principio de T1 coincide con el principio de T2, y el final de T1 coincide con el final de T2."@es ;
                                             rdfs:label "interval equals"@en ,
                                                        "intervalo igual"@es ;
                                             <http://www.w3.org/2004/02/skos/core#definition> "If a proper interval T1 is intervalEquals another proper interval T2, then the beginning of T1 is coincident with the beginning of T2, and the end of T1 is coincident with the end of T2."@en ,
                                                                                              "Si un intervalo propio T1 es igual a otro intervalo propio T2, entonces el principio de T1 coincide con el principio de T2, y el final de T1 coincide con el final de T2."@es .


###  http://www.w3.org/2006/time#intervalFinishedBy
<http://www.w3.org/2006/time#intervalFinishedBy> rdf:type owl:ObjectProperty ;
                                                 owl:inverseOf <http://www.w3.org/2006/time#intervalFinishes> ;
                                                 rdfs:domain <http://www.w3.org/2006/time#ProperInterval> ;
                                                 rdfs:range <http://www.w3.org/2006/time#ProperInterval> ;
                                                 rdfs:comment "If a proper interval T1 is intervalFinishedBy another proper interval T2, then the beginning of T1 is before the beginning of T2, and the end of T1 is coincident with the end of T2."@en ,
                                                              "Si un intervalo propio T1 está terminado por otro intervalo propio T2, entonces el principio de T1 está antes que el principio de T2, y el final de T1 coincide con el final de T2."@es ;
                                                 rdfs:label "interval finished by"@en ,
                                                            "intervalo terminado por"@es ;
                                                 <http://www.w3.org/2004/02/skos/core#definition> "If a proper interval T1 is intervalFinishedBy another proper interval T2, then the beginning of T1 is before the beginning of T2, and the end of T1 is coincident with the end of T2."@en ,
                                                                                                  "Si un intervalo propio T1 está terminado por otro intervalo propio T2, entonces el principio de T1 está antes que el principio de T2, y el final de T1 coincide con el final de T2."@es .


###  http://www.w3.org/2006/time#intervalFinishes
<http://www.w3.org/2006/time#intervalFinishes> rdf:type owl:ObjectProperty ;
                                               rdfs:subPropertyOf <http://www.w3.org/2006/time#intervalIn> ;
                                               rdfs:domain <http://www.w3.org/2006/time#ProperInterval> ;
                                               rdfs:range <http://www.w3.org/2006/time#ProperInterval> ;
                                               rdfs:comment "If a proper interval T1 is intervalFinishes another proper interval T2, then the beginning of T1 is after the beginning of T2, and the end of T1 is coincident with the end of T2."@en ,
                                                            "Si un intervalo propio T1 termina otro intervalo propio T2, entonces del principio de T1 está después del principio de T2, y el final de T1 coincide con el final de T2."@es ;
                                               rdfs:label "interval finishes"@en ,
                                                          "intervalo termina"@es ;
                                               <http://www.w3.org/2004/02/skos/core#definition> "If a proper interval T1 is intervalFinishes another proper interval T2, then the beginning of T1 is after the beginning of T2, and the end of T1 is coincident with the end of T2."@en ,
                                                                                                "Si un intervalo propio T1 termina otro intervalo propio T2, entonces del principio de T1 está después del principio de T2, y el final de T1 coincide con el final de T2."@es .


###  http://www.w3.org/2006/time#intervalIn
<http://www.w3.org/2006/time#intervalIn> rdf:type owl:ObjectProperty ;
                                         rdfs:domain <http://www.w3.org/2006/time#ProperInterval> ;
                                         rdfs:range <http://www.w3.org/2006/time#ProperInterval> ;
                                         rdfs:comment "If a proper interval T1 is intervalIn another proper interval T2, then the beginning of T1 is after the beginning of T2 or is coincident with the beginning of T2, and the end of T1 is before the end of T2, or is coincident with the end of T2, except that end of T1 may not be coincident with the end of T2 if the beginning of T1 is coincident with the beginning of T2."@en ,
                                                      "Si un intervalo propio T1 es un intervalo interior a otro intervalo propio T2, entonces el principio de T1 está después del principio de T2 o coincide con el principio de T2, y el final de T1 está antes que el final de T2, o coincide con el final de T2, excepto que el final de T1 puede no coincidir con el final de T2 si el principio de T1 coincide con el principio de T2."@es ;
                                         rdfs:label "interval in"@en ,
                                                    "intervalo interior"@es ;
                                         <http://www.w3.org/2004/02/skos/core#definition> "If a proper interval T1 is intervalIn another proper interval T2, then the beginning of T1 is after the beginning of T2 or is coincident with the beginning of T2, and the end of T1 is before the end of T2, or is coincident with the end of T2, except that end of T1 may not be coincident with the end of T2 if the beginning of T1 is coincident with the beginning of T2."@en ,
                                                                                          "Si un intervalo propio T1 es un intervalo interior a otro intervalo propio T2, entonces el principio de T1 está después del principio de T2 o coincide con el principio de T2, y el final de T1 está antes que el final de T2, o coincide con el final de T2, excepto que el final de T1 puede no coincidir con el final de T2 si el principio de T1 coincide con el principio de T2."@es ;
                                         <http://www.w3.org/2004/02/skos/core#note> "Esta relación entre intervalos no estaba incluida en las 13 relaciones básicas definidas por Allen (1984), pero se hace referencia a ella como \"una relación importante\" en Allen y Ferguson (1997). Es la unión disjunta de 'intervalo empieza', 'intervalo durante' y con 'intervalo termina'. Sin embargo, esto está fuera de la expresividad de OWL2, por tanto, se implementa como una propiedad explícita, con 'intervalo empieza', 'intervalo durante' e 'intervalo termina' como sub-propiedades."@es ,
                                                                                    "This interval relation is not included in the 13 basic relationships defined in Allen (1984), but is referred to as 'an important relationship' in Allen and Ferguson (1997). It is the disjoint union of :intervalStarts v :intervalDuring v :intervalFinishes . However, that is outside OWL2 expressivity, so is implemented as an explicit property, with :intervalStarts , :intervalDuring , :intervalFinishes as sub-properties"@en .


###  http://www.w3.org/2006/time#intervalMeets
<http://www.w3.org/2006/time#intervalMeets> rdf:type owl:ObjectProperty ;
                                            owl:inverseOf <http://www.w3.org/2006/time#intervalMetBy> ;
                                            rdfs:domain <http://www.w3.org/2006/time#ProperInterval> ;
                                            rdfs:range <http://www.w3.org/2006/time#ProperInterval> ;
                                            rdfs:comment "If a proper interval T1 is intervalMeets another proper interval T2, then the end of T1 is coincident with the beginning of T2."@en ,
                                                         "Si un intervalo propio T1 se encuentra con otro intervalo propio T2, entonces el final de T1 coincide con el principio de T2."@es ;
                                            rdfs:label "interval meets"@en ,
                                                       "intervalo se encuentra"@es ;
                                            <http://www.w3.org/2004/02/skos/core#definition> "If a proper interval T1 is intervalMeets another proper interval T2, then the end of T1 is coincident with the beginning of T2."@en ,
                                                                                             "Si un intervalo propio T1 se encuentra con otro intervalo propio T2, entonces el final de T1 coincide con el principio de T2."@es .


###  http://www.w3.org/2006/time#intervalMetBy
<http://www.w3.org/2006/time#intervalMetBy> rdf:type owl:ObjectProperty ;
                                            rdfs:domain <http://www.w3.org/2006/time#ProperInterval> ;
                                            rdfs:range <http://www.w3.org/2006/time#ProperInterval> ;
                                            rdfs:comment "If a proper interval T1 is intervalMetBy another proper interval T2, then the beginning of T1 is coincident with the end of T2."@en ,
                                                         "Si un intervalo propio T1 es 'intervalo encontrado por' otro intervalo propio T2, entonces el principio de T1 coincide con el final de T2."@es ;
                                            rdfs:label "interval met by"@en ,
                                                       "intervalo encontrado por"@es ;
                                            <http://www.w3.org/2004/02/skos/core#definition> "If a proper interval T1 is intervalMetBy another proper interval T2, then the beginning of T1 is coincident with the end of T2."@en ,
                                                                                             "Si un intervalo propio T1 es 'intervalo encontrado por' otro intervalo propio T2, entonces el principio de T1 coincide con el final de T2."@es .


###  http://www.w3.org/2006/time#intervalOverlappedBy
<http://www.w3.org/2006/time#intervalOverlappedBy> rdf:type owl:ObjectProperty ;
                                                   owl:inverseOf <http://www.w3.org/2006/time#intervalOverlaps> ;
                                                   rdfs:domain <http://www.w3.org/2006/time#ProperInterval> ;
                                                   rdfs:range <http://www.w3.org/2006/time#ProperInterval> ;
                                                   rdfs:comment "If a proper interval T1 is intervalOverlappedBy another proper interval T2, then the beginning of T1 is after the beginning of T2, the beginning of T1 is before the end of T2, and the end of T1 is after the end of T2."@en ,
                                                                "Si un intervalo propio T1 es 'intervalo solapado por' otro intervalo propio T2, entonces el principio de T1 es posterior al principio de T2, y el principio de T1 es anterior al final de T2, y el final de T1 es posterior al final de T2."@es ;
                                                   rdfs:label "interval overlapped by"@en ,
                                                              "intervalo solapado por"@es ;
                                                   <http://www.w3.org/2004/02/skos/core#definition> "If a proper interval T1 is intervalOverlappedBy another proper interval T2, then the beginning of T1 is after the beginning of T2, the beginning of T1 is before the end of T2, and the end of T1 is after the end of T2."@en ,
                                                                                                    "Si un intervalo propio T1 es 'intervalo solapado por' otro intervalo propio T2, entonces el principio de T1 es posterior al principio de T2, y el principio de T1 es anterior al final de T2, y el final de T1 es posterior al final de T2."@es .


###  http://www.w3.org/2006/time#intervalOverlaps
<http://www.w3.org/2006/time#intervalOverlaps> rdf:type owl:ObjectProperty ;
                                               rdfs:domain <http://www.w3.org/2006/time#ProperInterval> ;
                                               rdfs:range <http://www.w3.org/2006/time#ProperInterval> ;
                                               rdfs:comment "Asume una dirección en el tiempo. Si una entidad temporal T1 está después de otra entidad temporal T2, entonces el principio de T1 está después del final de T2."@es ,
                                                            "If a proper interval T1 is intervalOverlaps another proper interval T2, then the beginning of T1 is before the beginning of T2, the end of T1 is after the beginning of T2, and the end of T1 is before the end of T2."@en ,
                                                            "Si un intervalo propio T1 se solapa con otro intervalo propio T2, entonces el principio de T1 es anterior al principio de T2, el final de T1 es posterior al principio de T2, y el final de T1 es anterior al final de T2."@es ;
                                               rdfs:label "interval overlaps"@en ,
                                                          "intervalo se solapa"@es ;
                                               <http://www.w3.org/2004/02/skos/core#definition> "If a proper interval T1 is intervalOverlaps another proper interval T2, then the beginning of T1 is before the beginning of T2, the end of T1 is after the beginning of T2, and the end of T1 is before the end of T2."@en ,
                                                                                                "Si un intervalo propio T1 se solapa con otro intervalo propio T2, entonces el principio de T1 es anterior al principio de T2, el final de T1 es posterior al principio de T2, y el final de T1 es anterior al final de T2."@es .


###  http://www.w3.org/2006/time#intervalStartedBy
<http://www.w3.org/2006/time#intervalStartedBy> rdf:type owl:ObjectProperty ;
                                                owl:inverseOf <http://www.w3.org/2006/time#intervalStarts> ;
                                                rdfs:domain <http://www.w3.org/2006/time#ProperInterval> ;
                                                rdfs:range <http://www.w3.org/2006/time#ProperInterval> ;
                                                rdfs:comment "If a proper interval T1 is intervalStarted another proper interval T2, then the beginning of T1 is coincident with the beginning of T2, and the end of T1 is after the end of T2."@en ,
                                                             "Si un intervalo propio T1 es empezado por otro intervalo propio T2, entonces el principio de T1 coincide con el principio de T2, y el final de T1 es posterior al final de T2."@es ;
                                                rdfs:label "interval started by"@en ;
                                                <http://www.w3.org/2004/02/skos/core#definition> "If a proper interval T1 is intervalStarted another proper interval T2, then the beginning of T1 is coincident with the beginning of T2, and the end of T1 is after the end of T2."@en ,
                                                                                                 "Si un intervalo propio T1 es empezado por otro intervalo propio T2, entonces el principio de T1 coincide con el principio de T2, y el final de T1 es posterior al final de T2."@es .


###  http://www.w3.org/2006/time#intervalStarts
<http://www.w3.org/2006/time#intervalStarts> rdf:type owl:ObjectProperty ;
                                             rdfs:subPropertyOf <http://www.w3.org/2006/time#intervalIn> ;
                                             rdfs:domain <http://www.w3.org/2006/time#ProperInterval> ;
                                             rdfs:range <http://www.w3.org/2006/time#ProperInterval> ;
                                             rdfs:comment "If a proper interval T1 is intervalStarts another proper interval T2, then the beginning of T1 is coincident with the beginning of T2, and the end of T1 is before the end of T2."@en ,
                                                          "Si un intervalo propio T1 empieza otro intervalo propio T2, entonces del principio de T1 con el principio de T2, y el final de T1 es anterior al final de T2."@es ;
                                             rdfs:label "interval starts"@en ,
                                                        "intervalo empieza"@es ;
                                             <http://www.w3.org/2004/02/skos/core#definition> "If a proper interval T1 is intervalStarts another proper interval T2, then the beginning of T1 is coincident with the beginning of T2, and the end of T1 is before the end of T2."@en ,
                                                                                              "Si un intervalo propio T1 empieza otro intervalo propio T2, entonces del principio de T1 con el final de T2, y el final de T1 es anterior al final de T2."@es .


###  http://www.w3.org/2006/time#monthOfYear
<http://www.w3.org/2006/time#monthOfYear> rdf:type owl:ObjectProperty ;
                                          rdfs:domain <http://www.w3.org/2006/time#GeneralDateTimeDescription> ;
                                          rdfs:range <http://www.w3.org/2006/time#MonthOfYear> ;
                                          rdfs:comment "El mes del año, cuyo valor es un miembro de la clase 'mes del año'."@es ,
                                                       "The month of the year, whose value is a member of the class time:MonthOfYear"@en ;
                                          rdfs:label "mes del año"@es ,
                                                     "month of year"@en ;
                                          <http://www.w3.org/2004/02/skos/core#definition> "El mes del año, cuyo valor es un miembro de la clase 'mes del año'."@es ,
                                                                                           "The month of the year, whose value is a member of the class time:MonthOfYear"@en ;
                                          <http://www.w3.org/2004/02/skos/core#editorialNote> "Característica arriesgada - añadida en la revisión de 2017, y todavía no ampliamente utilizada."@es ,
                                                                                              "Feature at risk - added in 2017 revision, and not yet widely used. "@en .


###  http://www.w3.org/2006/time#timeZone
<http://www.w3.org/2006/time#timeZone> rdf:type owl:ObjectProperty ;
                                       rdfs:domain <http://www.w3.org/2006/time#GeneralDateTimeDescription> ;
                                       rdfs:range <http://www.w3.org/2006/time#TimeZone> ;
                                       rdfs:comment "The time zone for clock elements in the temporal position"@en ;
                                       rdfs:label "en huso horario"@es ,
                                                  "in time zone"@en ;
                                       <http://www.w3.org/2004/02/skos/core#historyNote> """En la versión original de OWL-Time de 2006, el rango de 'en huso horario' se definió en un espacio de nombres diferente \"http://www.w3.org/2006/timezone#\".
            Un axioma de alineación permite que los datos codificados de acuerdo con la versión anterior sean consistentes con la ontología actualizada."""@es ,
                                                                                         """In the original 2006 version of OWL-Time, the range of time:timeZone was a TimeZone class in a separate namespace \"http://www.w3.org/2006/timezone#\". 
An alignment axiom 
	tzont:TimeZone rdfs:subClassOf time:TimeZone . 
allows data encoded according to the previous version to be consistent with the updated ontology. """ ;
                                       <http://www.w3.org/2004/02/skos/core#note> """IANA mantiene una base de datos de husos horarios. Éstas están bien mantenidas y generalmente se consideran autorizadas, pero los ítems individuales no están disponibles en URIs individuales, por tanto, no se pueden utilizar directamente en datos expresados utilizando OWL-Time.
            La BDPedia proporciona un conjunto de recursos correspondientes a los husos horarios de IANA, con una URI para cada uno (por ejemplo, http://dbpedia.org/resource/Australia/Eucla). El Servicio de Reloj Mundial también proporciona una lista de husos horarios con la descripción de cada uno de los disponibles como una página Web individual con una URI adecuada individual (por ejemplo, https://www.timeanddate.com/time/zones/acwst). Éstos, y otros recursos similares, se puden usar como un valor de la propiedad 'huso horario'."""@es ,
                                                                                  """IANA maintains a database of timezones. These are well maintained and generally considered authoritative, but individual items are not available at individual URIs, so cannot be used directly in data expressed using OWL-Time.

DBPedia provides a set of resources corresponding to the IANA timezones, with a URI for each (e.g. http://dbpedia.org/resource/Australia/Eucla). The World Clock service also provides a list of time zones with the description of each available as an individual webpage with a convenient individual URI (e.g. https://www.timeanddate.com/time/zones/acwst). These or other, similar, resources might be used as a value of the time:timeZone property.""" .


###  http://www.w3.org/2006/time#unitType
<http://www.w3.org/2006/time#unitType> rdf:type owl:ObjectProperty ;
                                       rdfs:domain [ rdf:type owl:Class ;
                                                     owl:unionOf ( <http://www.w3.org/2006/time#Duration>
                                                                   <http://www.w3.org/2006/time#GeneralDateTimeDescription>
                                                                 )
                                                   ] ;
                                       rdfs:range <http://www.w3.org/2006/time#TemporalUnit> ;
                                       rdfs:comment "La unidad de tiempo que proporciona la precisión de un valor fecha-hora o la escala de una extensión temporal."@es ,
                                                    "The temporal unit which provides the precision of a date-time value or scale of a temporal extent"@en ;
                                       rdfs:label "temporal unit type"@en ,
                                                  "tipo de unidad temporal"@es .


###  https://w3id.org/def/phenowl#characterizes
:characterizes rdf:type owl:ObjectProperty ;
               rdfs:domain <http://purl.org/nemo/gufo#Entity> ;
               rdfs:range :Phenomenon ;
               rdfs:comment "\"Identify gufo:Individuals/entities that characterize (are crucial to the existence) of a given phen:Phenomenon.\"" ;
               rdfs:label "Characterizes" .


###  https://w3id.org/def/phenowl#fromPhenomenon
:fromPhenomenon rdf:type owl:ObjectProperty ,
                         owl:FunctionalProperty ;
                rdfs:domain :PhenomenonOccurrence ;
                rdfs:range :Phenomenon ;
                rdfs:comment """Identifies the phen:Phenomenon that gives the occurrence phen:PhenomenonOccurrence.


I.e. A phen:PhenomenonOccurence \"Occurence of a Hurricane in Paris\" is an occurrence of the phen:Phenomenon \"Hurricane\".""" ;
                rdfs:label "fromPhenomenon" .


###  https://w3id.org/def/phenowl#happensIn
:happensIn rdf:type owl:ObjectProperty ;
           rdfs:domain :Observation ;
           rdfs:range <https://w3id.org/seas/System> ;
           rdfs:comment "Identifies the seas:System where the phen:Observation happens." ;
           rdfs:label "Happens In" .


###  https://w3id.org/def/phenowl#hasPresence
:hasPresence rdf:type owl:ObjectProperty ;
             rdfs:domain <http://purl.org/nemo/gufo#Entity> ;
             rdfs:range :Presence ;
             rdfs:comment "Relates an instance of gufo:Individual/entity to its spatiotemporal presence." ;
             rdfs:label "Has Presence" .


###  https://w3id.org/def/phenowl#hasSTValidPath
:hasSTValidPath rdf:type owl:ObjectProperty ,
                         owl:AsymmetricProperty ;
                rdfs:domain :Observation ;
                rdfs:range :Observation ;
                rdfs:comment """Represents a valid spatial-temporal path between two observations.


I.e. From the same phen:PhenomenonOccurrence \"Hurricane in France on 2019\", we may have different phen:Observations like \"Hurricane observed in Rouen on November,2019\" and \"Hurricane observed in Paris on December,2019\". We may say that there is a possibility that the Hurricane went from Rouen to Paris, so there is a valid spatial-temporal path between the first and the second observation.""" ;
                rdfs:label "Has Spatial-Temporal Valid Path" .


###  https://w3id.org/def/phenowl#hasSpatialObject
:hasSpatialObject rdf:type owl:ObjectProperty ;
                  rdfs:domain <http://purl.org/nemo/gufo#Object> ;
                  rdfs:range <http://www.opengis.net/ont/geosparql#SpatialObject> ;
                  rdfs:comment """Relies a gufo:Object to parts of it's geo:SpatialObject.

I.e. A gufo:Object \"Country\" could be related to one geo:SpatialObject that delimits its entire zone, or it could be related to many geo:SpatialObjects for each gufo:Object \"City\" that forms the \"Country\".""" ;
                  rdfs:label "Has Spatial Object" .


###  https://w3id.org/def/phenowl#hasTimeInterval
:hasTimeInterval rdf:type owl:ObjectProperty ;
                 rdfs:domain <http://purl.org/nemo/gufo#ConcreteEntity> ;
                 rdfs:range <http://www.w3.org/2006/time#ProperInterval> ;
                 rdfs:comment "is an additional property to facilitate the application of Allen's interval algebra of the proper time interval between the start and end point of the gufo:ConcreteEntity" ;
                 rdfs:label "Entity's Proper Time Interaval" .


###  https://w3id.org/def/phenowl#observationOf
:observationOf rdf:type owl:ObjectProperty ,
                        owl:FunctionalProperty ;
               rdfs:domain :Observation ;
               rdfs:range :PhenomenonOccurrence ;
               rdfs:comment """Identifies the phen:PhenomenonOccurence observed in the phen:Observation.

I.e. From the same phen:PhenomenonOccurrence \"Hurricane in France on 2019\", we may have different phen:Observations like \"Hurricane observed in Rouen on November,2019\" and \"Hurricane observed in Paris on December,2019\"""" ;
               rdfs:label "Observation" .


###  https://w3id.org/def/phenowl#observationalPresenceIn
:observationalPresenceIn rdf:type owl:ObjectProperty ;
                         rdfs:domain :Presence ;
                         rdfs:range :Observation ;
                         rdfs:comment """Relates the phen:Presence of multiple gufo:Individuals in a phen:Observation.

I.e. \"Vacines\", \"Pantients of COVID-19\" and \"Pneumonia\" gufo:Indifiduals were present (phen:Presence) on december of 2020 in the phen:Observation \"Spread of COVID-19 in Paris on december of 2020\".""" ;
                         rdfs:label "Observational Presence In" .


###  https://w3id.org/def/phenowl#spatialPresenceIn
:spatialPresenceIn rdf:type owl:ObjectProperty ;
                   rdfs:domain :Presence ;
                   rdfs:range <http://www.opengis.net/ont/geosparql#SpatialObject> ;
                   rdfs:comment "Indicates the presence phen:Presence in a spatial region geo:SpatialObject." ;
                   rdfs:label "Spatial Presence In" .


###  https://w3id.org/seas/connectedThrough
<https://w3id.org/seas/connectedThrough> rdf:type owl:ObjectProperty ;
                                         owl:inverseOf <https://w3id.org/seas/connectsSystem> ;
                                         rdfs:domain <https://w3id.org/seas/System> ;
                                         rdfs:range <https://w3id.org/seas/Connection> ;
                                         owl:propertyChainAxiom ( <https://w3id.org/seas/connectsAt>
                                                                  <https://w3id.org/seas/connectsSystemThrough>
                                                                ) ;
                                         rdfs:comment "Links a system to one of its connections to other systems."@en ;
                                         rdfs:isDefinedBy <https://w3id.org/seas/SystemOntology> ;
                                         rdfs:label "connected through"@en ;
                                         <http://www.w3.org/2003/06/sw-vocab-status/ns#term_status> "stable" .


###  https://w3id.org/seas/connectedTo
<https://w3id.org/seas/connectedTo> rdf:type owl:ObjectProperty ,
                                             owl:SymmetricProperty ;
                                    rdfs:domain <https://w3id.org/seas/System> ;
                                    rdfs:range <https://w3id.org/seas/System> ;
                                    rdfs:comment """Links a system to a system it is connected to.

Connected systems interact in some way. The exact meaning of _interact_ is defined by sub properties of `seas:connectedTo`.

For example, for the electricity to directly flow between an electric vehicle service equipment and an electric vehicle, then they must be linked by property `seas:exchangesElectricityWith`: 

```
seas:exchangesElectricityWith rdfs:subPropertyOf seas:connectedTo .

<electric_vehicle> seas:exchangesElectricityWith <electric_vehicle_service_equipment> .
```

Property `seas:connectedTo` is symmetric:

```
if x seas:connectedTo y, then it is true that y seas:connectedTo x.
```

This property can be qualified using class `seas:Connection`, which connects the two systems.

If there is a connection between several systems, then one may infer these systems are pairwise connected."""@en ;
                                    rdfs:isDefinedBy <https://w3id.org/seas/SystemOntology> ;
                                    rdfs:label "connected to"@en ;
                                    <http://www.w3.org/2003/06/sw-vocab-status/ns#term_status> "stable" .


###  https://w3id.org/seas/connectionPointOf
<https://w3id.org/seas/connectionPointOf> rdf:type owl:ObjectProperty ;
                                          owl:inverseOf <https://w3id.org/seas/connectsAt> ;
                                          rdf:type owl:FunctionalProperty ;
                                          rdfs:domain <https://w3id.org/seas/ConnectionPoint> ;
                                          rdfs:range <https://w3id.org/seas/System> ;
                                          rdfs:comment "Links a connection point to the one and only one system it belongs to."@en ;
                                          rdfs:isDefinedBy <https://w3id.org/seas/SystemOntology> ;
                                          rdfs:label "connection point to"@en ;
                                          <http://www.w3.org/2003/06/sw-vocab-status/ns#term_status> "stable" .


###  https://w3id.org/seas/connectsAt
<https://w3id.org/seas/connectsAt> rdf:type owl:ObjectProperty ,
                                            owl:InverseFunctionalProperty ;
                                   rdfs:domain <https://w3id.org/seas/System> ;
                                   rdfs:range <https://w3id.org/seas/ConnectionPoint> ;
                                   rdfs:comment "Links a system to one of the connection points at which it connects."@en ;
                                   rdfs:isDefinedBy <https://w3id.org/seas/SystemOntology> ;
                                   rdfs:label "connects at"@en ;
                                   <http://www.w3.org/2003/06/sw-vocab-status/ns#term_status> "stable" .


###  https://w3id.org/seas/connectsSystem
<https://w3id.org/seas/connectsSystem> rdf:type owl:ObjectProperty ;
                                       rdfs:domain <https://w3id.org/seas/Connection> ;
                                       rdfs:range <https://w3id.org/seas/System> ;
                                       owl:propertyChainAxiom ( <https://w3id.org/seas/connectsSystemAt>
                                                                <https://w3id.org/seas/connectionPointOf>
                                                              ) ;
                                       rdfs:comment "Links a connection to one of the systems it connects."@en ;
                                       rdfs:isDefinedBy <https://w3id.org/seas/SystemOntology> ;
                                       rdfs:label "connects system"@en ;
                                       <http://www.w3.org/2003/06/sw-vocab-status/ns#term_status> "stable" .


###  https://w3id.org/seas/connectsSystemAt
<https://w3id.org/seas/connectsSystemAt> rdf:type owl:ObjectProperty ;
                                         owl:inverseOf <https://w3id.org/seas/connectsSystemThrough> ;
                                         rdfs:domain <https://w3id.org/seas/Connection> ;
                                         rdfs:range <https://w3id.org/seas/ConnectionPoint> ;
                                         rdfs:comment "Links a connection to one of the connection points at which it connects a system."@en ;
                                         rdfs:isDefinedBy <https://w3id.org/seas/SystemOntology> ;
                                         rdfs:label "connects system at"@en ;
                                         <http://www.w3.org/2003/06/sw-vocab-status/ns#term_status> "stable" .


###  https://w3id.org/seas/connectsSystemThrough
<https://w3id.org/seas/connectsSystemThrough> rdf:type owl:ObjectProperty ;
                                              rdfs:domain <https://w3id.org/seas/ConnectionPoint> ;
                                              rdfs:range <https://w3id.org/seas/Connection> ;
                                              rdfs:comment "Links a connection point to one of the connections through which it connects its system."@en ;
                                              rdfs:isDefinedBy <https://w3id.org/seas/SystemOntology> ;
                                              rdfs:label "connects system through"@en ;
                                              <http://www.w3.org/2003/06/sw-vocab-status/ns#term_status> "stable" .


###  https://w3id.org/seas/hasSubSystem
<https://w3id.org/seas/hasSubSystem> rdf:type owl:ObjectProperty ;
                                     owl:inverseOf <https://w3id.org/seas/subSystemOf> ;
                                     rdf:type owl:InverseFunctionalProperty ;
                                     rdfs:domain <https://w3id.org/seas/System> ;
                                     rdfs:range <https://w3id.org/seas/System> ;
                                     rdfs:comment "Links a system to one of its sub systems."@en ;
                                     rdfs:isDefinedBy <https://w3id.org/seas/SystemOntology> ;
                                     rdfs:label "has sub system"@en ;
                                     <http://www.w3.org/2003/06/sw-vocab-status/ns#term_status> "stable" .


###  https://w3id.org/seas/subSystemOf
<https://w3id.org/seas/subSystemOf> rdf:type owl:ObjectProperty ,
                                             owl:FunctionalProperty ;
                                    rdfs:domain <https://w3id.org/seas/System> ;
                                    rdfs:range <https://w3id.org/seas/System> ;
                                    rdfs:comment """Links a system to its super system.

Properties of subsystems somehow contribute to the properties of the super system. The exact meaning of _contribute_ is defined by sub properties of `seas:subSystemOf`.

For example, if a fridge is a subsystem of a kitchen, then its consumption power contributes to the consumption power of the kitchen. 

Property `seas:subSystemOf` is functional, and should be asymmetric:

```
if x seas:subSystemOf y1 and x seas:subSystemOf y2, then y1 and y2 refer to the same resource.
if x seas:subSystemOf y, then it can't be the case that y seas:subSystemOf x.
```

The asymmetric aspect of property `seas:subSystemOf` would prevents a system from being its own sub-system. Unfortunately, OWL 2 DL disallow a non-simple property (e.g., a functional property) from being asymmetric, see OWL 2 Syntax section 11.

If it was possible that both the fridge and the kitchen be sub systems of a common super system, say, the house, then the consumption power of the fridge would contribute twice to the consumption power of the house. The functional aspect of property `seas:subSystemOf` prevents this undesired effect. 

Due to the open world assumption of RDF, it is not possible to model the closed set of sub systems of a system using property `seas:subSystemOf`.
"""@en ;
                                    rdfs:isDefinedBy <https://w3id.org/seas/SystemOntology> ;
                                    rdfs:label "sub system of"@en ;
                                    <http://www.w3.org/2003/06/sw-vocab-status/ns#term_status> "stable" .


#################################################################
#    Data properties
#################################################################

###  http://purl.org/nemo/gufo#concernsQualityValue
<http://purl.org/nemo/gufo#concernsQualityValue> rdf:type owl:DatatypeProperty ;
                                                 rdfs:domain <http://purl.org/nemo/gufo#QualityValueAttributionSituation> ;
                                                 rdfs:comment """Determines a quality value associated with the gufo:ConcreteIndividual that stands in the gufo:QualityValueAttributionSituation.

Use gufo:concernsReifiedQualityValue instead when quality values are refied.

It is recommended that subproperties of gufo:concernsQualityValue are created, possibly identifying the datatype to be used. For example, \"concernsTemperatureValue\" could be defined as a sub-property of gufo:concernsQualityValue with range xsd:double."""@en ;
                                                 rdfs:label "concernsQualityValue"@en ;
                                                 rdfs:seeAlso <http://purl.org/nemo/gufo#concernsReifiedQualityValue> .


###  http://purl.org/nemo/gufo#hasBeginPointInXSDDate
<http://purl.org/nemo/gufo#hasBeginPointInXSDDate> rdf:type owl:DatatypeProperty ,
                                                            owl:FunctionalProperty ;
                                                   rdfs:domain <http://purl.org/nemo/gufo#ConcreteEntity> ;
                                                   rdfs:range xsd:date ;
                                                   rdfs:comment """Determines the begin point for a gufo:ConcreteIndividual, using a xsd:date literal.

In the case of endurants, gufo:asBeginPointInXSDDate determines the time point when the endurant comes into existence. In the case of events, this data property determines the time point when the event starts to take place. In the case of situation, it determines the time point when the situation begins to hold.

Use gufo:hasBeginPoint instead when temporal entities are reified."""@en ;
                                                   rdfs:label "hasBeginPointInXSDDate"@en ;
                                                   rdfs:seeAlso <http://purl.org/nemo/gufo#hasBeginPoint> ,
                                                                <http://purl.org/nemo/gufo#hasBeginPointInXSDDateTimeStamp> .


###  http://purl.org/nemo/gufo#hasBeginPointInXSDDateTimeStamp
<http://purl.org/nemo/gufo#hasBeginPointInXSDDateTimeStamp> rdf:type owl:DatatypeProperty ,
                                                                     owl:FunctionalProperty ;
                                                            rdfs:domain <http://purl.org/nemo/gufo#ConcreteEntity> ;
                                                            rdfs:range xsd:dateTimeStamp ;
                                                            rdfs:comment """Determines the begin point for a gufo:ConcreteIndividual, using a xsd:dateTimeStamp literal.

In the case of endurants, gufo:hasBeginPointInXSDDateTimeStamp determines the time point when the endurant comes into existence. In the case of events, this data property determines the time point when the event starts to take place. In the case of situation, it determines the time point when the situation begins to hold.

Use gufo:hasBeginPoint instead when temporal entities are reified."""@en ;
                                                            rdfs:label "hasBeginPointInXSDDateTimeStamp"@en ;
                                                            rdfs:seeAlso <http://purl.org/nemo/gufo#hasBeginPoint> ,
                                                                         <http://purl.org/nemo/gufo#hasBeginPointInXSDDate> .


###  http://purl.org/nemo/gufo#hasEndPointInXSDDate
<http://purl.org/nemo/gufo#hasEndPointInXSDDate> rdf:type owl:DatatypeProperty ,
                                                          owl:FunctionalProperty ;
                                                 rdfs:domain <http://purl.org/nemo/gufo#ConcreteEntity> ;
                                                 rdfs:range xsd:date ;
                                                 rdfs:comment """Determines the end point for a gufo:ConcreteIndividual using a xsd:date literal.
 
In the case of endurants, gufo:hasEndPointInXSDDate determines the time point when the endurant ceases to exist. In the case of events, this data property determines the time point when the event ends. In the case of situation, it determines the time point when the situation ceases to hold.

Use gufo:hasEndPoint instead when temporal entities are reified."""@en ;
                                                 rdfs:label "hasEndPointInXSDDate"@en ;
                                                 rdfs:seeAlso <http://purl.org/nemo/gufo#hasEndPoint> ,
                                                              <http://purl.org/nemo/gufo#hasEndPointInXSDDateTimeStamp> .


###  http://purl.org/nemo/gufo#hasEndPointInXSDDateTimeStamp
<http://purl.org/nemo/gufo#hasEndPointInXSDDateTimeStamp> rdf:type owl:DatatypeProperty ,
                                                                   owl:FunctionalProperty ;
                                                          rdfs:domain <http://purl.org/nemo/gufo#ConcreteEntity> ;
                                                          rdfs:range xsd:dateTimeStamp ;
                                                          rdfs:comment """Determines the end point for a gufo:ConcreteIndividual using a xsd:dateTimeStamp literal.
 
In the case of endurants, gufo:hasEndPointInXSDDateTimeStamp determines the time point when the endurant ceases to exist. In the case of events, this data property determines the time point when the event ends. In the case of situation, it determines the time point when the situation ceases to hold.

Use gufo:hasEndPoint instead when temporal entities are reified."""@en ;
                                                          rdfs:label "hasEndPointInXSDDateTimeStamp"@en ;
                                                          rdfs:seeAlso <http://purl.org/nemo/gufo#hasEndPoint> ,
                                                                       <http://purl.org/nemo/gufo#hasEndPointInXSDDate> .


###  http://purl.org/nemo/gufo#hasQualityValue
<http://purl.org/nemo/gufo#hasQualityValue> rdf:type owl:DatatypeProperty ;
                                            rdfs:domain <http://purl.org/nemo/gufo#ConcreteEntity> ;
                                            rdfs:comment """Determines a quality value associated with the concrete individual.

Use gufo:hasReifiedQualityValue instead when quality values are reified.

It is recommended that subproperties of gufo:hasQualityValue are created, possibly identifying the datatype to be used. For example, \"hasTemperatureValue\" could be defined as a sub-property of gufo:hasQualityValue whose domain is \"Temperature\" (specializing gufo:Quality) and whose range is xsd:double."""@en ;
                                            rdfs:label "hasQualityValue"@en ;
                                            rdfs:seeAlso <http://purl.org/nemo/gufo#hasReifiedQualityValue> .


###  http://purl.org/nemo/gufo#hasValueComponent
<http://purl.org/nemo/gufo#hasValueComponent> rdf:type owl:DatatypeProperty ;
                                              rdfs:domain <http://purl.org/nemo/gufo#QualityValue> ;
                                              rdfs:comment """This property is used for quality values that are defined in terms of a multidimensional quality structure (such as color conceived in terms of hue, saturation and brightness). Each value component of a quality value (a particular value for hue, a particular value for saturation, a particular value for brightness) is determined with this property. 

It is recommended that subproperties of gufo:hasValueComponent are created to indicate values for particular dimensions, possibly identifying the datatype to be used. For example \"hasHueComponent\", \"hasSaturationComponent\" and \"hasBrightnessComponent\" could be used as data properties specializing gufo:hasValueComponent with the xsd:double datatype."""@en ;
                                              rdfs:label "hasValueComponent"@en .


###  http://www.opengis.net/ont/geosparql#asGML
<http://www.opengis.net/ont/geosparql#asGML> rdf:type owl:DatatypeProperty ;
                                             rdfs:subPropertyOf <http://www.opengis.net/ont/geosparql#hasSerialization> ;
                                             rdfs:domain <http://www.opengis.net/ont/geosparql#Geometry> ;
                                             rdfs:range <http://www.opengis.net/ont/geosparql#gmlLiteral> ;
                                             <http://purl.org/dc/elements/1.1/contributor> "Matthew Perry" ;
                                             <http://purl.org/dc/elements/1.1/creator> "OGC GeoSPARQL 1.0 Standard Working Group" ;
                                             <http://purl.org/dc/elements/1.1/date> "2011-06-16"^^xsd:date ;
                                             <http://purl.org/dc/elements/1.1/description> """
      The GML serialization of a geometry
    """@en ;
                                             rdfs:comment """
      The GML serialization of a geometry
    """@en ;
                                             rdfs:isDefinedBy <http://www.opengis.net/ont/geosparql> ,
                                                              <http://www.opengis.net/spec/geosparql/1.0> ;
                                             rdfs:label "asGML"@en ;
                                             <http://www.w3.org/2004/02/skos/core#definition> """
      The GML serialization of a geometry
    """@en ;
                                             <http://www.w3.org/2004/02/skos/core#prefLabel> "asGML"@en .


###  http://www.opengis.net/ont/geosparql#asWKT
<http://www.opengis.net/ont/geosparql#asWKT> rdf:type owl:DatatypeProperty ;
                                             rdfs:subPropertyOf <http://www.opengis.net/ont/geosparql#hasSerialization> ;
                                             rdfs:domain <http://www.opengis.net/ont/geosparql#Geometry> ;
                                             rdfs:range <http://www.opengis.net/ont/geosparql#wktLiteral> ;
                                             <http://purl.org/dc/elements/1.1/contributor> "Matthew Perry" ;
                                             <http://purl.org/dc/elements/1.1/creator> "OGC GeoSPARQL 1.0 Standard Working Group" ;
                                             <http://purl.org/dc/elements/1.1/date> "2011-06-16"^^xsd:date ;
                                             <http://purl.org/dc/elements/1.1/description> """
      The WKT serialization of a geometry
    """@en ;
                                             rdfs:comment """
      The WKT serialization of a geometry
    """@en ;
                                             rdfs:isDefinedBy <http://www.opengis.net/ont/geosparql> ,
                                                              <http://www.opengis.net/spec/geosparql/1.0> ;
                                             rdfs:label "asWKT"@en ;
                                             <http://www.w3.org/2004/02/skos/core#definition> """
      The WKT serialization of a geometry
    """@en ;
                                             <http://www.w3.org/2004/02/skos/core#prefLabel> "asWKT"@en .


###  http://www.opengis.net/ont/geosparql#coordinateDimension
<http://www.opengis.net/ont/geosparql#coordinateDimension> rdf:type owl:DatatypeProperty ;
                                                           rdfs:domain <http://www.opengis.net/ont/geosparql#Geometry> ;
                                                           rdfs:range xsd:integer ;
                                                           <http://purl.org/dc/elements/1.1/contributor> "Matthew Perry" ;
                                                           <http://purl.org/dc/elements/1.1/creator> "OGC GeoSPARQL 1.0 Standard Working Group" ;
                                                           <http://purl.org/dc/elements/1.1/date> "2011-06-16"^^xsd:date ;
                                                           <http://purl.org/dc/elements/1.1/description> """
      The number of measurements or axes needed to describe the position of this
      geometry in a coordinate system.
    """@en ;
                                                           rdfs:comment """
      The number of measurements or axes needed to describe the position of this
      geometry in a coordinate system.
    """@en ;
                                                           rdfs:isDefinedBy <http://www.opengis.net/ont/geosparql> ,
                                                                            <http://www.opengis.net/spec/geosparql/1.0> ;
                                                           rdfs:label "coordinateDimension"@en ;
                                                           <http://www.w3.org/2004/02/skos/core#definition> """
      The number of measurements or axes needed to describe the position of this
      geometry in a coordinate system.
    """@en ;
                                                           <http://www.w3.org/2004/02/skos/core#prefLabel> "coordinateDimension"@en .


###  http://www.opengis.net/ont/geosparql#dimension
<http://www.opengis.net/ont/geosparql#dimension> rdf:type owl:DatatypeProperty ;
                                                 rdfs:domain <http://www.opengis.net/ont/geosparql#Geometry> ;
                                                 rdfs:range xsd:integer ;
                                                 <http://purl.org/dc/elements/1.1/contributor> "Matthew Perry" ;
                                                 <http://purl.org/dc/elements/1.1/creator> "OGC GeoSPARQL 1.0 Standard Working Group" ;
                                                 <http://purl.org/dc/elements/1.1/date> "2011-06-16"^^xsd:date ;
                                                 <http://purl.org/dc/elements/1.1/description> """
      The topological dimension of this geometric object, which 
      must be less than or equal to the coordinate dimension. 
      In non-homogeneous collections, this will return the largest 
      topological dimension of the contained objects.
    """@en ;
                                                 rdfs:comment """
      The topological dimension of this geometric object, which 
      must be less than or equal to the coordinate dimension. 
      In non-homogeneous collections, this will return the largest 
      topological dimension of the contained objects.
    """@en ;
                                                 rdfs:isDefinedBy <http://www.opengis.net/ont/geosparql> ,
                                                                  <http://www.opengis.net/spec/geosparql/1.0> ;
                                                 rdfs:label "dimension"@en ;
                                                 <http://www.w3.org/2004/02/skos/core#definition> """
      The topological dimension of this geometric object, which 
      must be less than or equal to the coordinate dimension. 
      In non-homogeneous collections, this will return the largest 
      topological dimension of the contained objects.
    """@en ;
                                                 <http://www.w3.org/2004/02/skos/core#prefLabel> "dimension"@en .


###  http://www.opengis.net/ont/geosparql#hasSerialization
<http://www.opengis.net/ont/geosparql#hasSerialization> rdf:type owl:DatatypeProperty ;
                                                        rdfs:domain <http://www.opengis.net/ont/geosparql#Geometry> ;
                                                        rdfs:range rdfs:Literal ;
                                                        <http://purl.org/dc/elements/1.1/contributor> "Matthew Perry" ;
                                                        <http://purl.org/dc/elements/1.1/creator> "OGC GeoSPARQL 1.0 Standard Working Group" ;
                                                        <http://purl.org/dc/elements/1.1/date> "2011-06-16"^^xsd:date ;
                                                        <http://purl.org/dc/elements/1.1/description> """
      Connects a geometry object with its text-based serialization.
    """@en ;
                                                        rdfs:comment """
      Connects a geometry object with its text-based serialization.
    """@en ;
                                                        rdfs:isDefinedBy <http://www.opengis.net/ont/geosparql> ,
                                                                         <http://www.opengis.net/spec/geosparql/1.0> ;
                                                        rdfs:label "has serialization"@en ;
                                                        <http://www.w3.org/2004/02/skos/core#definition> """
      Connects a geometry object with its text-based serialization.
    """@en ;
                                                        <http://www.w3.org/2004/02/skos/core#prefLabel> "has serialization"@en .


###  http://www.opengis.net/ont/geosparql#isEmpty
<http://www.opengis.net/ont/geosparql#isEmpty> rdf:type owl:DatatypeProperty ;
                                               rdfs:domain <http://www.opengis.net/ont/geosparql#Geometry> ;
                                               rdfs:range xsd:boolean ;
                                               <http://purl.org/dc/elements/1.1/contributor> "Matthew Perry" ;
                                               <http://purl.org/dc/elements/1.1/creator> "OGC GeoSPARQL 1.0 Standard Working Group" ;
                                               <http://purl.org/dc/elements/1.1/date> "2011-06-16"^^xsd:date ;
                                               <http://purl.org/dc/elements/1.1/description> """
      (true) if this geometric object is the empty Geometry. If 
      true, then this geometric object represents the empty point 
      set for the coordinate space.
    """@en ;
                                               rdfs:comment """
      (true) if this geometric object is the empty Geometry. If 
      true, then this geometric object represents the empty point 
      set for the coordinate space.
    """@en ;
                                               rdfs:isDefinedBy <http://www.opengis.net/ont/geosparql> ,
                                                                <http://www.opengis.net/spec/geosparql/1.0> ;
                                               rdfs:label "isEmpty"@en ;
                                               <http://www.w3.org/2004/02/skos/core#definition> """
      (true) if this geometric object is the empty Geometry. If 
      true, then this geometric object represents the empty point 
      set for the coordinate space.
    """@en ;
                                               <http://www.w3.org/2004/02/skos/core#prefLabel> "isEmpty"@en .


###  http://www.opengis.net/ont/geosparql#isSimple
<http://www.opengis.net/ont/geosparql#isSimple> rdf:type owl:DatatypeProperty ;
                                                rdfs:domain <http://www.opengis.net/ont/geosparql#Geometry> ;
                                                rdfs:range xsd:boolean ;
                                                <http://purl.org/dc/elements/1.1/contributor> "Matthew Perry" ;
                                                <http://purl.org/dc/elements/1.1/creator> "OGC GeoSPARQL 1.0 Standard Working Group" ;
                                                <http://purl.org/dc/elements/1.1/date> "2011-06-16"^^xsd:date ;
                                                <http://purl.org/dc/elements/1.1/description> """
      (true) if this geometric object has no anomalous geometric 
      points, such as self intersection or self tangency.
    """@en ;
                                                rdfs:comment """
      (true) if this geometric object has no anomalous geometric 
      points, such as self intersection or self tangency.
    """@en ;
                                                rdfs:isDefinedBy <http://www.opengis.net/ont/geosparql> ,
                                                                 <http://www.opengis.net/spec/geosparql/1.0> ;
                                                rdfs:label "isSimple"@en ;
                                                <http://www.w3.org/2004/02/skos/core#definition> """
      (true) if this geometric object has no anomalous geometric 
      points, such as self intersection or self tangency.
    """@en ;
                                                <http://www.w3.org/2004/02/skos/core#prefLabel> "isSimple"@en .


###  http://www.opengis.net/ont/geosparql#spatialDimension
<http://www.opengis.net/ont/geosparql#spatialDimension> rdf:type owl:DatatypeProperty ;
                                                        rdfs:domain <http://www.opengis.net/ont/geosparql#Geometry> ;
                                                        rdfs:range xsd:integer ;
                                                        <http://purl.org/dc/elements/1.1/contributor> "Matthew Perry" ;
                                                        <http://purl.org/dc/elements/1.1/creator> "OGC GeoSPARQL 1.0 Standard Working Group" ;
                                                        <http://purl.org/dc/elements/1.1/date> "2011-06-16"^^xsd:date ;
                                                        <http://purl.org/dc/elements/1.1/description> """
      The number of measurements or axes needed to describe the spatial position of 
      this geometry in a coordinate system.
    """@en ;
                                                        rdfs:comment """
      The number of measurements or axes needed to describe the spatial position of 
      this geometry in a coordinate system.
    """@en ;
                                                        rdfs:isDefinedBy <http://www.opengis.net/ont/geosparql> ,
                                                                         <http://www.opengis.net/spec/geosparql/1.0> ;
                                                        rdfs:label "spatialDimension"@en ;
                                                        <http://www.w3.org/2004/02/skos/core#definition> """
      The number of measurements or axes needed to describe the spatial position of 
      this geometry in a coordinate system.
    """@en ;
                                                        <http://www.w3.org/2004/02/skos/core#prefLabel> "spatialDimension"@en .


###  http://www.w3.org/2004/02/skos/core#notation
<http://www.w3.org/2004/02/skos/core#notation> rdf:type owl:DatatypeProperty ;
                                               rdfs:isDefinedBy <http://www.w3.org/2004/02/skos/core> ;
                                               rdfs:label "notation"@en ;
                                               <http://www.w3.org/2004/02/skos/core#definition> "A notation, also known as classification code, is a string of characters such as \"T58.5\" or \"303.4833\" used to uniquely identify a concept within the scope of a given concept scheme."@en ;
                                               <http://www.w3.org/2004/02/skos/core#scopeNote> "By convention, skos:notation is used with a typed literal in the object position of the triple."@en .


###  http://www.w3.org/2006/time#day
<http://www.w3.org/2006/time#day> rdf:type owl:DatatypeProperty ;
                                  rdfs:domain <http://www.w3.org/2006/time#GeneralDateTimeDescription> ;
                                  rdfs:comment """Day position in a calendar-clock system.

The range of this property is not specified, so can be replaced by any specific representation of a calendar day from any calendar. """@en ,
                                               "Posición de día en un sistema calendario-reloj."@es ;
                                  rdfs:label "day"@en ,
                                             "día"@es ;
                                  <http://www.w3.org/2004/02/skos/core#definition> """Day position in a calendar-clock system.

The range of this property is not specified, so can be replaced by any specific representation of a calendar day from any calendar. """@en ,
                                                                                   """Posición de día en un sistema calendario-reloj.

El rango de esta propiedad no está especificado, por tanto, se puede reemplazar por una representación específica de un día de calendario de cualquier calendario."""@es .


###  http://www.w3.org/2006/time#dayOfYear
<http://www.w3.org/2006/time#dayOfYear> rdf:type owl:DatatypeProperty ;
                                        rdfs:domain <http://www.w3.org/2006/time#GeneralDateTimeDescription> ;
                                        rdfs:range xsd:nonNegativeInteger ;
                                        rdfs:comment "El número de día en el año."@es ,
                                                     "The number of the day within the year"@en ;
                                        rdfs:label "day of year"@en ,
                                                   "día del año"@es ;
                                        <http://www.w3.org/2004/02/skos/core#definition> "El número de día en el año."@es ,
                                                                                         "The number of the day within the year"@en .


###  http://www.w3.org/2006/time#days
<http://www.w3.org/2006/time#days> rdf:type owl:DatatypeProperty ;
                                   rdfs:domain <http://www.w3.org/2006/time#GeneralDurationDescription> ;
                                   rdfs:range xsd:decimal ;
                                   rdfs:comment "Longitud de, o elemento de la longitud de, una extensión temporal expresada en días."@es ,
                                                "length of, or element of the length of, a temporal extent expressed in days"@en ;
                                   rdfs:label "days duration"@en ,
                                              "duración en días"@es ;
                                   <http://www.w3.org/2004/02/skos/core#definition> "Longitud de, o elemento de la longitud de, una extensión temporal expresada en días."@es ,
                                                                                    "length of, or element of the length of, a temporal extent expressed in days"@en .


###  http://www.w3.org/2006/time#hasXSDDuration
<http://www.w3.org/2006/time#hasXSDDuration> rdf:type owl:DatatypeProperty ;
                                             rdfs:domain <http://www.w3.org/2006/time#TemporalEntity> ;
                                             rdfs:range xsd:duration ;
                                             rdfs:comment "Extensión de una entidad temporal, expresada utilizando xsd:duration."@es ,
                                                          "Extent of a temporal entity, expressed using xsd:duration"@en ;
                                             rdfs:label "has XSD duration"@en ,
                                                        "tiene duración XSD"@es ;
                                             <http://www.w3.org/2004/02/skos/core#definition> "Extensión de una entidad temporal, expresada utilizando xsd:duration."@es ,
                                                                                              "Extent of a temporal entity, expressed using xsd:duration"@en ;
                                             <http://www.w3.org/2004/02/skos/core#editorialNote> "Característica arriesgada - añadida en la revisión de 2017, y todavía no ampliamente utilizada."@es ,
                                                                                                 "Feature at risk - added in 2017 revision, and not yet widely used. "@en .


###  http://www.w3.org/2006/time#hour
<http://www.w3.org/2006/time#hour> rdf:type owl:DatatypeProperty ;
                                   rdfs:domain <http://www.w3.org/2006/time#GeneralDateTimeDescription> ;
                                   rdfs:range xsd:nonNegativeInteger ;
                                   rdfs:comment "Hour position in a calendar-clock system."@en ,
                                                "Posición de hora en un sistema calendario-reloj."@es ;
                                   rdfs:label "hora"@es ,
                                              "hour"@en ;
                                   <http://www.w3.org/2004/02/skos/core#definition> "Hour position in a calendar-clock system."@en ,
                                                                                    "Posición de hora en un sistema calendario-reloj."@es .


###  http://www.w3.org/2006/time#hours
<http://www.w3.org/2006/time#hours> rdf:type owl:DatatypeProperty ;
                                    rdfs:domain <http://www.w3.org/2006/time#GeneralDurationDescription> ;
                                    rdfs:range xsd:decimal ;
                                    rdfs:comment "Longitud de, o elemento de la longitud de, una extensión temporal expresada en horas."@es ,
                                                 "length of, or element of the length of, a temporal extent expressed in hours"@en ;
                                    rdfs:label "duración en horas"@es ,
                                               "hours duration"@en ;
                                    <http://www.w3.org/2004/02/skos/core#definition> "Longitud de, o elemento de la longitud de, una extensión temporal expresada en horas."@es ,
                                                                                     "length of, or element of the length of, a temporal extent expressed in hours"@en .


###  http://www.w3.org/2006/time#inXSDDate
<http://www.w3.org/2006/time#inXSDDate> rdf:type owl:DatatypeProperty ;
                                        rdfs:domain <http://www.w3.org/2006/time#Instant> ;
                                        rdfs:range xsd:date ;
                                        rdfs:comment "Posición de un instante, expresado utilizando xsd:date."@es ,
                                                     "Position of an instant, expressed using xsd:date"@en ;
                                        rdfs:label "en fecha XSD"@es ,
                                                   "in XSD date"@en ;
                                        <http://www.w3.org/2004/02/skos/core#definition> "Posición de un instante, expresado utilizando xsd:date."@es ,
                                                                                         "Position of an instant, expressed using xsd:date"@en .


###  http://www.w3.org/2006/time#inXSDDateTime
<http://www.w3.org/2006/time#inXSDDateTime> rdf:type owl:DatatypeProperty ;
                                            rdfs:domain <http://www.w3.org/2006/time#Instant> ;
                                            rdfs:range xsd:dateTime ;
                                            rdfs:comment "Posición de un instante, expresado utilizando xsd:dateTime."@es ,
                                                         "Position of an instant, expressed using xsd:dateTime"@en ;
                                            rdfs:label "en fecha-tiempo XSD"@es ,
                                                       "in XSD Date-Time"@en ;
                                            owl:deprecated "true"^^xsd:boolean ;
                                            <http://www.w3.org/2004/02/skos/core#definition> "Posición de un instante, expresado utilizando xsd:dateTime."@es ,
                                                                                             "Position of an instant, expressed using xsd:dateTime"@en ;
                                            <http://www.w3.org/2004/02/skos/core#note> "La propiedad 'en fecha-hora XSD' ha sido reemplazada por 'en fecha-sello de tiempo XSD' que hace obligatorio el campo 'huso horario'."@es ,
                                                                                       "The property :inXSDDateTime is replaced by :inXSDDateTimeStamp which makes the time-zone field mandatory."@en .


###  http://www.w3.org/2006/time#inXSDDateTimeStamp
<http://www.w3.org/2006/time#inXSDDateTimeStamp> rdf:type owl:DatatypeProperty ;
                                                 rdfs:domain <http://www.w3.org/2006/time#Instant> ;
                                                 rdfs:range xsd:dateTimeStamp ;
                                                 rdfs:comment "Posición de un instante, expresado utilizando xsd:dateTimeStamp."@es ,
                                                              "Position of an instant, expressed using xsd:dateTimeStamp"@en ;
                                                 rdfs:label "en fecha-sello de tiempo XSD"@es ,
                                                            "in XSD Date-Time-Stamp"@en ;
                                                 <http://www.w3.org/2004/02/skos/core#definition> "Posición de un instante, expresado utilizando xsd:dateTimeStamp."@es ,
                                                                                                  "Position of an instant, expressed using xsd:dateTimeStamp"@en .


###  http://www.w3.org/2006/time#inXSDgYear
<http://www.w3.org/2006/time#inXSDgYear> rdf:type owl:DatatypeProperty ;
                                         rdfs:domain <http://www.w3.org/2006/time#Instant> ;
                                         rdfs:range xsd:gYear ;
                                         rdfs:comment "Posición de un instante, expresado utilizando xsd:gYear."@es ,
                                                      "Position of an instant, expressed using xsd:gYear"@en ;
                                         rdfs:label "en año gregoriano XSD"@es ,
                                                    "in XSD g-Year"@en ;
                                         <http://www.w3.org/2004/02/skos/core#definition> "Posición de un instante, expresado utilizando xsd:gYear."@es ,
                                                                                          "Position of an instant, expressed using xsd:gYear"@en .


###  http://www.w3.org/2006/time#inXSDgYearMonth
<http://www.w3.org/2006/time#inXSDgYearMonth> rdf:type owl:DatatypeProperty ;
                                              rdfs:domain <http://www.w3.org/2006/time#Instant> ;
                                              rdfs:range xsd:gYearMonth ;
                                              rdfs:comment "Posición de un instante, expresado utilizando xsd:gYearMonth."@es ,
                                                           "Position of an instant, expressed using xsd:gYearMonth"@en ;
                                              rdfs:label "en año-mes gregoriano XSD"@es ,
                                                         "in XSD g-YearMonth"@en ;
                                              <http://www.w3.org/2004/02/skos/core#definition> "Posición de un instante, expresado utilizando xsd:gYearMonth."@es ,
                                                                                               "Position of an instant, expressed using xsd:gYearMonth"@en .


###  http://www.w3.org/2006/time#minute
<http://www.w3.org/2006/time#minute> rdf:type owl:DatatypeProperty ;
                                     rdfs:domain <http://www.w3.org/2006/time#GeneralDateTimeDescription> ;
                                     rdfs:range xsd:nonNegativeInteger ;
                                     rdfs:comment "Minute position in a calendar-clock system."@en ,
                                                  "Posición de minuto en un sistema calendario-reloj."@es ;
                                     rdfs:label "minute"@en ,
                                                "minuto"@es ;
                                     <http://www.w3.org/2004/02/skos/core#definition> "Minute position in a calendar-clock system."@en ,
                                                                                      "Posición de minuto en un sistema calendario-reloj."@es .


###  http://www.w3.org/2006/time#minutes
<http://www.w3.org/2006/time#minutes> rdf:type owl:DatatypeProperty ;
                                      rdfs:domain <http://www.w3.org/2006/time#GeneralDurationDescription> ;
                                      rdfs:range xsd:decimal ;
                                      rdfs:comment "Longitud de, o elemento de la longitud de, una extensión temporal expresada en minutos."@es ,
                                                   "length, or element of, a temporal extent expressed in minutes"@en ;
                                      rdfs:label "minutes"@en ,
                                                 "minutos"@es ;
                                      <http://www.w3.org/2004/02/skos/core#definition> "Longitud de, o elemento de la longitud de, una extensión temporal expresada en minutos."@es ,
                                                                                       "length, or element of, a temporal extent expressed in minutes"@en .


###  http://www.w3.org/2006/time#month
<http://www.w3.org/2006/time#month> rdf:type owl:DatatypeProperty ;
                                    rdfs:domain <http://www.w3.org/2006/time#GeneralDateTimeDescription> ;
                                    rdfs:comment """Month position in a calendar-clock system.

The range of this property is not specified, so can be replaced by any specific representation of a calendar month from any calendar. """@en ,
                                                 """Posición de mes en un sistema calendario-reloj.
    El rango de esta propiedad no está especificado, por tanto, se puede reemplazar por cualquier representación específica de un mes de calendario de un calendario cualquiera."""@es ;
                                    rdfs:label "mes"@es ,
                                               "month"@en ;
                                    <http://www.w3.org/2004/02/skos/core#definition> """Month position in a calendar-clock system.

The range of this property is not specified, so can be replaced by any specific representation of a calendar month from any calendar. """@en ,
                                                                                     """Posición de mes en un sistema calendario-reloj.
            El rango de esta propiedad no está especificado, por tanto, se puede reemplazar por cualquier representación específica de un mes de calendario de un calendario cualquiera."""@es .


###  http://www.w3.org/2006/time#months
<http://www.w3.org/2006/time#months> rdf:type owl:DatatypeProperty ;
                                     rdfs:domain <http://www.w3.org/2006/time#GeneralDurationDescription> ;
                                     rdfs:range xsd:decimal ;
                                     rdfs:comment "Longitud de, o elemento de la longitud de, una extensión temporal expresada en meses."@es ,
                                                  "length of, or element of the length of, a temporal extent expressed in months"@en ;
                                     rdfs:label "duración en meses"@es ,
                                                "months duration"@en ;
                                     <http://www.w3.org/2004/02/skos/core#definition> "Longitud de, o elemento de la longitud de, una extensión temporal expresada en meses."@es ,
                                                                                      "length of, or element of the length of, a temporal extent expressed in months"@en .


###  http://www.w3.org/2006/time#nominalPosition
<http://www.w3.org/2006/time#nominalPosition> rdf:type owl:DatatypeProperty ;
                                              rdfs:domain <http://www.w3.org/2006/time#TimePosition> ;
                                              rdfs:range xsd:string ;
                                              rdfs:comment "El valor (nominal) que indica posición temporal en un sistema de referencia ordinal."@es ,
                                                           "The (nominal) value indicating temporal position in an ordinal reference system "@en ;
                                              rdfs:label "Name of temporal position"@en ,
                                                         "nombre de posición temporal"@es ;
                                              <http://www.w3.org/2004/02/skos/core#definition> "El valor (nominal) que indica posición temporal en un sistema de referencia ordinal."@es ,
                                                                                               "The (nominal) value indicating temporal position in an ordinal reference system "@en .


###  http://www.w3.org/2006/time#numericDuration
<http://www.w3.org/2006/time#numericDuration> rdf:type owl:DatatypeProperty ;
                                              rdfs:domain <http://www.w3.org/2006/time#Duration> ;
                                              rdfs:range xsd:decimal ;
                                              rdfs:comment "Valor de una extensión temporal expresada como un número decimal escalado por una unidad de tiempo."@es ,
                                                           "Value of a temporal extent expressed as a decimal number scaled by a temporal unit"@en ;
                                              rdfs:label "Numeric value of temporal duration"@en ,
                                                         "valor numérico de duración temporal"@es ;
                                              <http://www.w3.org/2004/02/skos/core#definition> "Valor de una extensión temporal expresada como un número decimal escalado por una unidad de tiempo."@es ,
                                                                                               "Value of a temporal extent expressed as a decimal number scaled by a temporal unit"@en .


###  http://www.w3.org/2006/time#numericPosition
<http://www.w3.org/2006/time#numericPosition> rdf:type owl:DatatypeProperty ;
                                              rdfs:domain <http://www.w3.org/2006/time#TimePosition> ;
                                              rdfs:range xsd:decimal ;
                                              rdfs:comment "El valor (numérico) que indica posición temporal en un sistema de referencia ordinal."@es ,
                                                           "The (numeric) value indicating position within a temporal coordinate system "@en ;
                                              rdfs:label "Numeric value of temporal position"@en ,
                                                         "valor numérico de posición temporal"@es ;
                                              <http://www.w3.org/2004/02/skos/core#definition> "El valor (numérico) que indica posición temporal en un sistema de referencia ordinal."@es ,
                                                                                               "The (numeric) value indicating position within a temporal coordinate system "@en .


###  http://www.w3.org/2006/time#second
<http://www.w3.org/2006/time#second> rdf:type owl:DatatypeProperty ;
                                     rdfs:domain <http://www.w3.org/2006/time#GeneralDateTimeDescription> ;
                                     rdfs:range xsd:decimal ;
                                     rdfs:comment "Posición de segundo en un sistema calendario-reloj."@es ,
                                                  "Second position in a calendar-clock system."@en ;
                                     rdfs:label "second"@en ,
                                                "segundo"@es .


###  http://www.w3.org/2006/time#seconds
<http://www.w3.org/2006/time#seconds> rdf:type owl:DatatypeProperty ;
                                      rdfs:domain <http://www.w3.org/2006/time#GeneralDurationDescription> ;
                                      rdfs:range xsd:decimal ;
                                      rdfs:comment "Longitud de, o elemento de la longitud de, una extensión temporal expresada en segundos."@es ,
                                                   "length of, or element of the length of, a temporal extent expressed in seconds"@en ;
                                      rdfs:label "duración en segundos"@es ,
                                                 "seconds duration"@en ;
                                      rdfs:seeAlso <http://www.bipm.org/en/publications/si-brochure/second.html> .


###  http://www.w3.org/2006/time#week
<http://www.w3.org/2006/time#week> rdf:type owl:DatatypeProperty ;
                                   rdfs:domain <http://www.w3.org/2006/time#GeneralDateTimeDescription> ;
                                   rdfs:range xsd:nonNegativeInteger ;
                                   rdfs:comment "Número de semana en el año."@es ,
                                                "Week number within the year."@en ;
                                   rdfs:label "semana"@es ,
                                              "week"@en ;
                                   <http://www.w3.org/2004/02/skos/core#note> "Weeks are numbered differently depending on the calendar in use and the local language or cultural conventions (locale). ISO-8601 specifies that the first week of the year includes at least four days, and that Monday is the first day of the week. In that system, week 1 is the week that contains the first Thursday in the year."@en ;
                                   <http://www.w3.org/2004/02/skos/core#scopeNote> "Las semanas están numeradas de forma diferente dependiendo del calendario en uso y de las convenciones lingüísticas y culturales locales (locale en inglés). El ISO-8601 especifica que la primera semana del año incluye al menos cuatro días, y que el lunes es el primer día de la semana. En ese sistema, la semana 1 es la semana que contiene el primer jueves del año."@es .


###  http://www.w3.org/2006/time#weeks
<http://www.w3.org/2006/time#weeks> rdf:type owl:DatatypeProperty ;
                                    rdfs:domain <http://www.w3.org/2006/time#GeneralDurationDescription> ;
                                    rdfs:range xsd:decimal ;
                                    rdfs:comment "Longitud de, o elemento de la longitud de, una extensión temporal expresada en semanas."@es ,
                                                 "length of, or element of the length of, a temporal extent expressed in weeks"@en ;
                                    rdfs:label "duración en semanas"@es ,
                                               "weeks duration"@en .


###  http://www.w3.org/2006/time#xsdDateTime
<http://www.w3.org/2006/time#xsdDateTime> rdf:type owl:DatatypeProperty ;
                                          rdfs:domain <http://www.w3.org/2006/time#DateTimeInterval> ;
                                          rdfs:range xsd:dateTime ;
                                          rdfs:comment "Valor de 'intervalo de fecha-hora' expresado como un valor compacto."@es ,
                                                       "Value of DateTimeInterval expressed as a compact value."@en ;
                                          rdfs:label "has XSD date-time"@en ,
                                                     "tiene fecha-hora XSD"@es ;
                                          owl:deprecated "true"^^xsd:boolean ;
                                          <http://www.w3.org/2004/02/skos/core#note> "Using xsd:dateTime in this place means that the duration of the interval is implicit: it corresponds to the length of the smallest non-zero element of the date-time literal. However, this rule cannot be used for intervals whose duration is more than one rank smaller than the starting time - e.g. the first minute or second of a day, the first hour of a month, or the first day of a year. In these cases the desired interval cannot be distinguished from the interval corresponding to the next rank up. Because of this essential ambiguity, use of this property is not recommended and it is deprecated."@en ,
                                                                                     "Utilizando xsd:dateTime en este lugar significa que la duración del intervalo está implícita: se corresponde con la longitud del elemento más pequeño distinto de cero del literal fecha-hora. Sin embargo, esta regla no se puede utilizar para intervalos cuya duración es mayor que un rango más pequeño que el tiempo de comienzo - p.ej. el primer minuto o segundo del día, la primera hora del mes, o el primer día del año. En estos casos el intervalo deseado no se puede distinguir del intervalo correspondiente al próximo rango más alto. Debido a esta ambigüedad esencial, no se recomienda el uso de esta propiedad y está desaprobada." .


###  http://www.w3.org/2006/time#year
<http://www.w3.org/2006/time#year> rdf:type owl:DatatypeProperty ;
                                   rdfs:domain <http://www.w3.org/2006/time#GeneralDateTimeDescription> ;
                                   rdfs:comment """Posición de año en un sistema calendario-reloj.

l rango de esta propiedad no está especificado, por tanto, se puede reemplazar por cualquier representación específica de un año de calendario de un calendario cualquiera."""@es ,
                                                """Year position in a calendar-clock system.

The range of this property is not specified, so can be replaced by any specific representation of a calendar year from any calendar. """@en ;
                                   rdfs:label "year"@en .


###  http://www.w3.org/2006/time#years
<http://www.w3.org/2006/time#years> rdf:type owl:DatatypeProperty ;
                                    rdfs:domain <http://www.w3.org/2006/time#GeneralDurationDescription> ;
                                    rdfs:range xsd:decimal ;
                                    rdfs:comment "Longitud de, o elemento de la longitud de, una extensión temporal expresada en años."@es ,
                                                 "length of, or element of the length of, a temporal extent expressed in years"@en ;
                                    rdfs:label "duración en años"@es ,
                                               "years duration"@en .


#################################################################
#    Classes
#################################################################

###  http://purl.org/nemo/gufo#AbstractEntity
<http://purl.org/nemo/gufo#AbstractEntity> rdf:type owl:Class ;
                                           rdfs:subClassOf <http://purl.org/nemo/gufo#Entity> ;
                                           owl:disjointWith <http://purl.org/nemo/gufo#ConcreteEntity> ;
                                           rdfs:comment """A gufo:Individual that does not exist in space-time in the same way as a gufo:ConcreteIndividual does. A gufo:AbstractIndividual has no spatiotemporal qualities in its own right. Hence, it does not make sense to ask how much space it now occupies (Gideon, 2018) and when it was created or destroyed.

Examples include the number ten, the null set, and the proposition that 'Obama was the president of the United States'.

Rosen, Gideon, \"Abstract Objects\", The Stanford Encyclopedia of Philosophy (Winter 2018 Edition), Edward N. Zalta (ed.), <https://plato.stanford.edu/archives/win2018/entries/abstract-objects/>"""@en ;
                                           rdfs:label "AbstractIndividual"@en .


###  http://purl.org/nemo/gufo#AbstractEntityType
<http://purl.org/nemo/gufo#AbstractEntityType> rdf:type owl:Class ;
                                               rdfs:subClassOf <http://purl.org/nemo/gufo#Type> ;
                                               owl:disjointWith <http://purl.org/nemo/gufo#ConcreteEntityType> ,
                                                                <http://purl.org/nemo/gufo#RelationshipType> ;
                                               rdfs:comment """A gufo:Type whose instances are abstract individuals.

Instances of gufo:AbstractIndividualType are subclasses of gufo:AbstractIndividual.

Examples include the types \"NaturalNumber\", \"Set\", \"Proposition\"."""@en ;
                                               rdfs:label "AbstractIndividualType"@en .


###  http://purl.org/nemo/gufo#AntiRigidType
<http://purl.org/nemo/gufo#AntiRigidType> rdf:type owl:Class ;
                                          rdfs:subClassOf <http://purl.org/nemo/gufo#NonRigidType> ;
                                          owl:disjointWith <http://purl.org/nemo/gufo#SemiRigidType> ;
                                          rdfs:comment """A gufo:NonRigidType that applies contingently to all its instances (see Guizzardi, 2005, chapter 4).

Examples include the gufo:Phase \"Child\", the gufo:PhaseMixin \"InfantAnimal\", the gufo:Role \"Student\", and the gufo:RoleMixin \"Customer\"."""@en ;
                                          rdfs:label "AntiRigidType"@en .


###  http://purl.org/nemo/gufo#Aspect
<http://purl.org/nemo/gufo#Aspect> rdf:type owl:Class ;
                                   rdfs:subClassOf <http://purl.org/nemo/gufo#Endurant> ;
                                   owl:disjointWith <http://purl.org/nemo/gufo#Object> ;
                                   owl:disjointUnionOf ( <http://purl.org/nemo/gufo#ExtrinsicAspect>
                                                         <http://purl.org/nemo/gufo#IntrinsicAspect>
                                                       ) ;
                                   rdfs:comment """A gufo:Endurant that depends on at least one other concrete individual for its existence. A gufo:Aspect is a characteristic or trait of a concrete individual that is itself conceived as an individual. 

Examples include: intrinsic physical aspects, such as the Moon's mass, Lassie's fur color; mental dispositions, such as Bob's math skills, his belief that the number one is odd; as well as relational aspects, such as John's love for Mary and the marriage between John and Mary. 

The specific sort of existential dependence connecting aspects to their bearers is called inherence.

Corresponds to \"Moment\" in Guizzardi (2005). 

Also termed \"property instance\", \"particularized property\", \"individual accident\", or \"(variable) trope\" in the philosophical literature."""@en ;
                                   rdfs:label "Aspect"@en .


###  http://purl.org/nemo/gufo#AtomicEvent
<http://purl.org/nemo/gufo#AtomicEvent> rdf:type owl:Class ;
                                        rdfs:subClassOf <http://purl.org/nemo/gufo#Event> .


###  http://purl.org/nemo/gufo#Category
<http://purl.org/nemo/gufo#Category> rdf:type owl:Class ;
                                     rdfs:subClassOf <http://purl.org/nemo/gufo#NonSortal> ,
                                                     <http://purl.org/nemo/gufo#RigidType> ;
                                     rdfs:comment """A gufo:EndurantType that is both non-sortal and rigid. It captures essential properties that apply to instances of different kinds.

For example, \"PhysicalObject\" may be considered a gufo:Category, encompassing objects such as cars, planets, trees. \"Agent\" may be a gufo:Category that classifies both people and organizations."""@en ;
                                     rdfs:label "Category"@en .


###  http://purl.org/nemo/gufo#Collection
<http://purl.org/nemo/gufo#Collection> rdf:type owl:Class ;
                                       rdfs:subClassOf <http://purl.org/nemo/gufo#Object> ;
                                       owl:disjointUnionOf ( <http://purl.org/nemo/gufo#FixedCollection>
                                                             <http://purl.org/nemo/gufo#VariableCollection>
                                                           ) ;
                                       rdfs:comment """A complex gufo:Object whose parts (the members of the collection) have a uniform structure (i.e., members are conceived as playing the same role in the collection). Collections may have a fixed or variable membership, which can be asserted using gufo:FixedCollection and gufo:VariableCollection respectively.

Examples include a deck of cards, a pile of bricks, a forest (conceived as a collection of trees), and a group of people.

Collections in many cases constitute a functional complex. For example, a pile of bricks may constitute a wall, a group of people may constitute a football team.

A gufo:Collection may be decomposed into \"smaller\" collections. For instance, a group of people may be decomposed into a group of English speakers and a group of Italian speakers. Sub collections may or may not share members among them."""@en ;
                                       rdfs:label "Collection"@en .


###  http://purl.org/nemo/gufo#ComparativeRelationshipType
<http://purl.org/nemo/gufo#ComparativeRelationshipType> rdf:type owl:Class ;
                                                        rdfs:subClassOf <http://purl.org/nemo/gufo#RelationshipType> ;
                                                        owl:disjointWith <http://purl.org/nemo/gufo#MaterialRelationshipType> ;
                                                        rdfs:comment """A gufo:RelationshipType derived from intrinsic aspects of the related entities.

For example, \"heavierThan\", \"olderThan\". 

For a gufo:ComparativeRelationshipType it is recommended to identify the types of intrinsic aspects from which it is derived (see gufo:isDerivedFrom). For example \"heavierThan\" is derived from the \"Weight\" quality type.

Note that, in the case of relationships that may change in different circumstances or times, the use of a qualified relation pattern enables indicating the period of time in which the relationship holds. See gufo:TemporaryRelationshipSituation.

Corresponds to \"comparative formal relation\" in Guizzardi (2005) and \"Comparative Relation\" in Fonseca et al. (2019)."""@en ;
                                                        rdfs:label "ComparativeRelationshipType"@en ;
                                                        rdfs:seeAlso <http://purl.org/nemo/gufo#isDerivedFrom> .


###  http://purl.org/nemo/gufo#ComplexEvent
<http://purl.org/nemo/gufo#ComplexEvent> rdf:type owl:Class ;
                                         rdfs:subClassOf <http://purl.org/nemo/gufo#Event> .


###  http://purl.org/nemo/gufo#ConcreteEntity
<http://purl.org/nemo/gufo#ConcreteEntity> rdf:type owl:Class ;
                                           rdfs:subClassOf <http://purl.org/nemo/gufo#Entity> ;
                                           owl:disjointUnionOf ( <http://purl.org/nemo/gufo#Endurant>
                                                                 <http://purl.org/nemo/gufo#Event>
                                                                 <http://purl.org/nemo/gufo#Situation>
                                                               ) ;
                                           rdfs:comment """A gufo:Individual that exists in space-time. 

Concrete individuals comprise not only object-like entities (a car, a mountain, a person, a marriage, a belief), but also events (a business meeting, a soccer match) and situations (the situation in which a person weighs 80 kilograms, the situation in which a bank account is overdrawn)."""@en ;
                                           rdfs:label "ConcreteIndividual"@en .


###  http://purl.org/nemo/gufo#ConcreteEntityType
<http://purl.org/nemo/gufo#ConcreteEntityType> rdf:type owl:Class ;
                                               rdfs:subClassOf <http://purl.org/nemo/gufo#Type> ;
                                               owl:disjointWith <http://purl.org/nemo/gufo#RelationshipType> ;
                                               rdfs:comment """A gufo:Type whose instances are concrete individuals.

Instances of gufo:ConcreteIndividualType are subclasses of gufo:ConcreteIndividual.

Examples include the gufo:Kind \"Person\", the gufo:Category \"Physical Object\", the gufo:EventType \"Business Meeting\"."""@en ;
                                               rdfs:label "ConcreteIndividualType"@en .


###  http://purl.org/nemo/gufo#Endurant
<http://purl.org/nemo/gufo#Endurant> rdf:type owl:Class ;
                                     rdfs:subClassOf <http://purl.org/nemo/gufo#ConcreteEntity> ;
                                     owl:disjointUnionOf ( <http://purl.org/nemo/gufo#Aspect>
                                                           <http://purl.org/nemo/gufo#Object>
                                                         ) ;
                                     rdfs:comment """A gufo:ConcreteIndividual that endures in time and may change qualitatively while keeping its identity. 

Examples include: ordinary objects of everyday experience, such as a person, a house, and a car; reified relationships, such as a marriage, a rental contract, and a person's love for another; and existentially-dependent aspects of objects, such as a car's weight, a person's language skills, and a house's color. 

Also termed \"continuant\" in the philosophical literature."""@en ;
                                     rdfs:label "Endurant"@en .


###  http://purl.org/nemo/gufo#EndurantType
<http://purl.org/nemo/gufo#EndurantType> rdf:type owl:Class ;
                                         rdfs:subClassOf <http://purl.org/nemo/gufo#ConcreteEntityType> ;
                                         owl:disjointWith <http://purl.org/nemo/gufo#EventType> ,
                                                          <http://purl.org/nemo/gufo#SituationType> ;
                                         owl:disjointUnionOf ( <http://purl.org/nemo/gufo#NonRigidType>
                                                               <http://purl.org/nemo/gufo#RigidType>
                                                             ) ,
                                                             ( <http://purl.org/nemo/gufo#NonSortal>
                                                               <http://purl.org/nemo/gufo#Sortal>
                                                             ) ;
                                         rdfs:comment """A gufo:Type whose instances are endurants. 

Instances of gufo:EndurantType are subclasses of gufo:Endurant.

Examples include the object kind \"Person\", the phase \"Child\", the relator kind \"Marriage\".

See Guizzardi et al. (2018) for details concerning the taxonomy of endurant types included here."""@en ;
                                         rdfs:label "EndurantType"@en .


###  http://purl.org/nemo/gufo#Entity
<http://purl.org/nemo/gufo#Entity> rdf:type owl:Class ;
                                   owl:disjointWith <http://purl.org/nemo/gufo#Type> ;
                                   owl:disjointUnionOf ( <http://purl.org/nemo/gufo#AbstractEntity>
                                                         <http://purl.org/nemo/gufo#ConcreteEntity>
                                                       ) ;
                                   rdfs:comment """An entity that (unlike a gufo:Type) cannot be instantiated.

Individuals may be either concrete (e.g., the Earth, Mick Jagger, Brazil, the 1985 Mexico City Earthquake) or abstract (e.g., the number two, the proposition that 'three is a prime number').

Also known as \"particular\" in the philosophical literature."""@en ;
                                   rdfs:label "Individual"@en .


###  http://purl.org/nemo/gufo#Event
<http://purl.org/nemo/gufo#Event> rdf:type owl:Class ;
                                  rdfs:subClassOf <http://purl.org/nemo/gufo#Perdurants> ;
                                  rdfs:comment """A gufo:ConcreteIndividual that 'occurs' or 'happens' in time. They may be instantaneous or long-running. Events are those \"things that happen to or are performed by\" (Casati and Varzi, 2015) endurants. 

Examples include actions and processes, such as a business meeting, a communicative act, a soccer match, a goal kick, the clicking of a mouse button; as well as natural occurrences such as an earthquake, the fall of the meteor that caused the extinction of the dinosaurs.

Also termed \"happening\", \"occurrence\", \"perdurant\" or \"occurrent\" in the philosophical literature.

Casati, R. & Varzi, A. (2015). Events. In E.N. Zalta (Ed.), The Stanford Encyclopedia of Philosophy (Winter 2015 ed.). 19 Metaphysics Research Lab, Stanford University. https://plato.stanford.edu/archives/win2015/entries/events/"""@en ;
                                  rdfs:label "Event"@en ;
                                  rdfs:seeAlso <http://purl.org/nemo/gufo#participatedIn> .


###  http://purl.org/nemo/gufo#EventType
<http://purl.org/nemo/gufo#EventType> rdf:type owl:Class ;
                                      rdfs:subClassOf <http://purl.org/nemo/gufo#PerdurantType> ;
                                      owl:disjointWith <http://purl.org/nemo/gufo#SituationType> ;
                                      rdfs:comment """A gufo:Type whose instances are events.

Instances of gufo:EventType are subclasses of gufo:Event.

Examples include \"Business Meeting\", \"Birth\", \"Musical Performance\"."""@en ;
                                      rdfs:label "EventType"@en .


###  http://purl.org/nemo/gufo#ExtrinsicAspect
<http://purl.org/nemo/gufo#ExtrinsicAspect> rdf:type owl:Class ;
                                            rdfs:subClassOf <http://purl.org/nemo/gufo#Aspect> ;
                                            owl:disjointWith <http://purl.org/nemo/gufo#IntrinsicAspect> ;
                                            owl:disjointUnionOf ( <http://purl.org/nemo/gufo#ExtrinsicMode>
                                                                  <http://purl.org/nemo/gufo#Relator>
                                                                ) ;
                                            rdfs:comment """A gufo:Aspect that depends on one or more concrete individuals.

Extrinsic (or \"relational\") aspects are reified relationships, e.g., John and Mary's marriage, Mary's employment contract at Nasa, or parts of those relationships, e.g., John's obligations towards Mary in the scope of the marriage, Mary's reciprocal claims, Mary's obligations towards John, John's reciprocal claims. Extrinsic aspects can also be reified one-sided relationships, e.g., John's admiration for Obama (which depends on Obama but does not characterize him).

Corresponds to \"Extrinsic Moment\" in Fonseca et al (2019). Encompasses \"Externally Depedent Mode\", \"Qua Individual\" and \"Relator\" in Guizzardi (2005)."""@en ;
                                            rdfs:label "ExtrinsicAspect"@en .


###  http://purl.org/nemo/gufo#ExtrinsicMode
<http://purl.org/nemo/gufo#ExtrinsicMode> rdf:type owl:Class ;
                                          rdfs:subClassOf <http://purl.org/nemo/gufo#ExtrinsicAspect> ,
                                                          [ rdf:type owl:Restriction ;
                                                            owl:onProperty <http://purl.org/nemo/gufo#externallyDependsOn> ;
                                                            owl:someValuesFrom <http://purl.org/nemo/gufo#ConcreteEntity>
                                                          ] ,
                                                          [ rdf:type owl:Restriction ;
                                                            owl:onProperty <http://purl.org/nemo/gufo#inheresIn> ;
                                                            owl:qualifiedCardinality "1"^^xsd:nonNegativeInteger ;
                                                            owl:onClass <http://purl.org/nemo/gufo#ConcreteEntity>
                                                          ] ;
                                          owl:disjointWith <http://purl.org/nemo/gufo#Relator> ;
                                          rdfs:comment """A gufo:ExtrinsicAspect that inheres in a concrete individual and depends on others for its existence.

A gufo:ExtrinsicMode can be understood as a reified one-sided relationship, such as John's admiration for Mary.

Corresponds to \"Extrinsic Moment\" in Fonseca et al (2019). Encompasses what \"Externally Dependent Mode\", \"Qua Individual\" and \"Relator\" in Guizzardi (2005)."""@en ;
                                          rdfs:label "ExtrinsicMode"@en ;
                                          rdfs:seeAlso <http://purl.org/nemo/gufo#externallyDependsOn> ,
                                                       <http://purl.org/nemo/gufo#inheresIn> .


###  http://purl.org/nemo/gufo#FixedCollection
<http://purl.org/nemo/gufo#FixedCollection> rdf:type owl:Class ;
                                            rdfs:subClassOf <http://purl.org/nemo/gufo#Collection> ;
                                            owl:disjointWith <http://purl.org/nemo/gufo#VariableCollection> ;
                                            rdfs:comment """A gufo:Collection for which no change in membership is possible.

Such a collection obeys an extensional principle of identity, i.e., two fixed collections are the same if, and only if, they have the same members.

Consider, for example, a group of people understood as a gufo:FixedCollection. In this case, any change in the membership of the group (e.g., the addition of one person) would in fact create a different group of people. In this case, the gufo:FixedCollection may be contrasted with the complexes they constitute. For instance, The Beatles (the band conceived as a gufo:FunctionalComplex) was in a certain circumstance constituted by the collection {John, Paul, George, Pete} and in another one constituted by the collection {John, Paul, George, Ringo}. The replacement of Pete Best by Ringo Star does not alter the identity of the band, but creates a  different group of people."""@en ;
                                            rdfs:label "FixedCollection"@en ;
                                            rdfs:seeAlso <http://purl.org/nemo/gufo#isCollectionMemberOf> ,
                                                         <http://purl.org/nemo/gufo#isSubCollectionOf> .


###  http://purl.org/nemo/gufo#FunctionalComplex
<http://purl.org/nemo/gufo#FunctionalComplex> rdf:type owl:Class ;
                                              rdfs:subClassOf <http://purl.org/nemo/gufo#Object> ;
                                              rdfs:comment <http://purl.org/nemo/gufo#isComponentOf> ,
                                                           """A complex gufo:Object whose parts (components) play different roles in its composition. 

For example, a person could be considered a gufo:FunctionalComplex with the various organs (heart, brain, lungs, etc.) playing different roles. Another example is a scrum team, which is composed by people playing the roles of scrum master, product owner, developer, etc.

To explicitly capture temporary components, use gufo:TemporaryParthoodSituation."""@en ;
                                              rdfs:label "FunctionalComplex"@en ;
                                              rdfs:seeAlso <http://purl.org/nemo/gufo#TemporaryParthoodSituation> .


###  http://purl.org/nemo/gufo#History
<http://purl.org/nemo/gufo#History> rdf:type owl:Class ;
                                    rdfs:subClassOf <http://purl.org/nemo/gufo#Perdurants> .


###  http://purl.org/nemo/gufo#IntrinsicAspect
<http://purl.org/nemo/gufo#IntrinsicAspect> rdf:type owl:Class ;
                                            rdfs:subClassOf <http://purl.org/nemo/gufo#Aspect> ,
                                                            [ rdf:type owl:Restriction ;
                                                              owl:onProperty <http://purl.org/nemo/gufo#inheresIn> ;
                                                              owl:qualifiedCardinality "1"^^xsd:nonNegativeInteger ;
                                                              owl:onClass <http://purl.org/nemo/gufo#ConcreteEntity>
                                                            ] ;
                                            owl:disjointUnionOf ( <http://purl.org/nemo/gufo#IntrinsicMode>
                                                                  <http://purl.org/nemo/gufo#Quality>
                                                                ) ;
                                            rdfs:comment """A gufo:Aspect that depends on a single concrete individual in which it inheres. 

Examples include intrinsic physical aspects, such as the Moon's mass, Lassie's fur color; the fragility of John Lennon's glasses; mental dispositions, such as Bob's math skills, his belief that the number one is odd.

A gufo:IntrinsicAspect is classified as a gufo:Quality (e.g., an apple's weight, the height of the Statue of Liberty) if it is measurable by a certain value space, or as a gufo:IntrinsicMode (e.g. Bob's belief that the Eiffel Tower is in Paris) otherwise.

Corresponds to \"Instrinsic Moment\" in Guizzardi (2005). Different from Guizzardi (2005), here we consider that aspects can inhere in concrete individuals in general, and not only in endurants."""@en ;
                                            rdfs:label "IntrinsicAspect"@en ;
                                            rdfs:seeAlso <http://purl.org/nemo/gufo#inheresIn> .


###  http://purl.org/nemo/gufo#IntrinsicMode
<http://purl.org/nemo/gufo#IntrinsicMode> rdf:type owl:Class ;
                                          rdfs:subClassOf <http://purl.org/nemo/gufo#IntrinsicAspect> ;
                                          owl:disjointWith <http://purl.org/nemo/gufo#Quality> ;
                                          rdfs:comment """A gufo:IntrinsicAspect that is not measurable.

For example, Bob's belief that the Eiffel Tower is in Paris, his math skills, his headache.

Corresponds to \"Mode\" in Guizzardi (2005)."""@en ;
                                          rdfs:label "IntrinsicMode"@en .


###  http://purl.org/nemo/gufo#Kind
<http://purl.org/nemo/gufo#Kind> rdf:type owl:Class ;
                                 rdfs:subClassOf <http://purl.org/nemo/gufo#RigidType> ,
                                                 <http://purl.org/nemo/gufo#Sortal> ;
                                 owl:disjointWith <http://purl.org/nemo/gufo#SubKind> ;
                                 rdfs:comment """A gufo:EndurantType that is both sortal and rigid. It provides a uniform principle of identity for its instances. Every gufo:Endurant instantiates one and only one gufo:Kind. 

Examples include kinds of ordinary objects of everyday experience, such as: \"Person\", \"House\", \"Car\"; kinds of relators, such as \"Marriage\", \"RentalContract\"; kinds of existentially-dependent aspects of objects, such as \"Weight\", \"Belief\", \"Vulnerability\"."""@en ;
                                 rdfs:label "Kind"@en .


###  http://purl.org/nemo/gufo#MaterialRelationshipType
<http://purl.org/nemo/gufo#MaterialRelationshipType> rdf:type owl:Class ;
                                                     rdfs:subClassOf <http://purl.org/nemo/gufo#RelationshipType> ;
                                                     rdfs:comment """A gufo:RelationshipType derived from extrinsic aspects of the related entities.

For example, \"marriedWith\", \"employedBy\", \"enrolledIn\", \"admires\". 

For a gufo:MaterialRelationshipType it is recommended to identify the type of extrinsic aspect from which the material relationship type is derived (see gufo:isDerivedFrom). For example \"marriedWith\" can be derived from the \"Marriage\" relator type, \"employedBy\" can be derived from the \"Employment\" relator type.

Encompasses \"Material Relation\" in Guizzardi (2005) and corresponds to \"Material Relation\" in Fonseca et al. (2019)."""@en ;
                                                     rdfs:label "MaterialRelationshipType"@en ;
                                                     rdfs:seeAlso <http://purl.org/nemo/gufo#isDerivedFrom> .


###  http://purl.org/nemo/gufo#Mixin
<http://purl.org/nemo/gufo#Mixin> rdf:type owl:Class ;
                                  rdfs:subClassOf <http://purl.org/nemo/gufo#NonSortal> ,
                                                  <http://purl.org/nemo/gufo#SemiRigidType> ;
                                  rdfs:comment """A gufo:EndurantType that is both non-sortal and semi-rigid. As a semi-rigid type, it applies necessarily to some of its instances and contingently to some others. As a non-sortal, it captures properties shared by instances of different kinds.

For example, the type \"FemaleAnimal\" may be considered a gufo:Mixin as it applies necessarily to animals of certain species, e.g., lions and sharks, while it applies contingently to animals of other species such as clownfish and mushroom corals (which may change sex given certain conditions)."""@en ;
                                  rdfs:label "Mixin"@en .


###  http://purl.org/nemo/gufo#NonRigidType
<http://purl.org/nemo/gufo#NonRigidType> rdf:type owl:Class ;
                                         rdfs:subClassOf <http://purl.org/nemo/gufo#EndurantType> ;
                                         owl:disjointWith <http://purl.org/nemo/gufo#RigidType> ;
                                         owl:disjointUnionOf ( <http://purl.org/nemo/gufo#AntiRigidType>
                                                               <http://purl.org/nemo/gufo#SemiRigidType>
                                                             ) ;
                                         rdfs:comment """A gufo:EndurantType that does not apply necessarily to at least one of its instances (see Guizzardi, 2005, chapter 4).

Examples include anti-rigid types, such as the role \"Student\" and the phase \"Child\", and semi-rigid types, such as the mixin \"MusicalArtist\" (which necessarily characterizes bands, but contingently characterizes people) and the mixin \"FemaleAnimal\" (which is necessarily characterizes female dogs, but contigently characterizes clownfish)."""@en ;
                                         rdfs:label "NonRigidType"@en .


###  http://purl.org/nemo/gufo#NonSortal
<http://purl.org/nemo/gufo#NonSortal> rdf:type owl:Class ;
                                      rdfs:subClassOf <http://purl.org/nemo/gufo#EndurantType> ;
                                      owl:disjointWith <http://purl.org/nemo/gufo#Sortal> ;
                                      rdfs:comment """A gufo:EndurantType that applies to individuals of different kinds (see Guizzardi, 2005, chapter 4).

Non-sortals do not provide a uniform principle of identity for their instances; instead, they just classify things that share common properties but which obey different principles of identity.

Also termed \"dispersive\" types in the philosophical literature."""@en ;
                                      rdfs:label "NonSortal"@en .


###  http://purl.org/nemo/gufo#Object
<http://purl.org/nemo/gufo#Object> rdf:type owl:Class ;
                                   rdfs:subClassOf <http://purl.org/nemo/gufo#Endurant> ;
                                   rdfs:comment """A gufo:Endurant that does not depend on another endurant for its existence (excluding its essential parts and aspects). 

Examples of objects include ordinary physical entities, such as a dog, a house, a tomato, a car, Alan Turing, but also socially-defined entities such as The Rolling Stones, the European Union, the Brazilian 1988 Constitution.

Guizzardi (2005) also included the more abstract notion of \"Substantial\", which generalizes both objects and amounts of matter. That notion was left out from this implementation, together with the notion of amount of matter. Support for the representation of maximally-self-connected amounts of matter is given by gufo:Quantity."""@en ;
                                   rdfs:label "Object"@en .


###  http://purl.org/nemo/gufo#Participation
<http://purl.org/nemo/gufo#Participation> rdf:type owl:Class ;
                                          rdfs:subClassOf <http://purl.org/nemo/gufo#Event> ,
                                                          [ rdf:type owl:Restriction ;
                                                            owl:onProperty [ owl:inverseOf <http://purl.org/nemo/gufo#participatedIn>
                                                                           ] ;
                                                            owl:qualifiedCardinality "1"^^xsd:nonNegativeInteger ;
                                                            owl:onClass <http://purl.org/nemo/gufo#Object>
                                                          ] ;
                                          rdfs:comment """A gufo:Event that depends on a single object. 

Participations can be used to partition an event into portions, each of which depend exclusively on a single object. Consider a business meeting with multiple participants, including John and Mary. John's participation in the meeting encompasses all events that are part of the meeting and that depend solely on him. Likewise, Mary's participation encompasses all events that are part of the meeting and that depend solely on her. Similarly, in Brutus’ stabbing of Caesar, we may identify the participations of Brutus, of Caesar, and of the dagger."""@en ;
                                          rdfs:label "Participation"@en ;
                                          rdfs:seeAlso <http://purl.org/nemo/gufo#participatedIn> .


###  http://purl.org/nemo/gufo#PerdurantType
<http://purl.org/nemo/gufo#PerdurantType> rdf:type owl:Class ;
                                          rdfs:subClassOf <http://purl.org/nemo/gufo#ConcreteEntityType> .


###  http://purl.org/nemo/gufo#Perdurants
<http://purl.org/nemo/gufo#Perdurants> rdf:type owl:Class ;
                                       rdfs:subClassOf <http://purl.org/nemo/gufo#ConcreteEntity> .


###  http://purl.org/nemo/gufo#Phase
<http://purl.org/nemo/gufo#Phase> rdf:type owl:Class ;
                                  rdfs:subClassOf <http://purl.org/nemo/gufo#AntiRigidType> ,
                                                  <http://purl.org/nemo/gufo#Sortal> ;
                                  owl:disjointWith <http://purl.org/nemo/gufo#Role> ;
                                  rdfs:comment """A gufo:EndurantType that is both sortal and anti-rigid. It is defined by instrinsic but contingent instantiation conditions. Phases are relationally independent types that capturec instrinsic properties shared by instances of a given kind.

For example, \"Child\" may be considered a gufo:Phase as a subclass of the gufo:Kind \"Person\", instantiated by persons younger than 12. Another example is the type \"IllPerson\", which may be considered a gufo:Phase that is instantiated whenever an instance of \"Disease\" (a gufo:IntrinsicMode) inheres in a person."""@en ;
                                  rdfs:label "Phase"@en .


###  http://purl.org/nemo/gufo#PhaseMixin
<http://purl.org/nemo/gufo#PhaseMixin> rdf:type owl:Class ;
                                       rdfs:subClassOf <http://purl.org/nemo/gufo#AntiRigidType> ,
                                                       <http://purl.org/nemo/gufo#NonSortal> ;
                                       owl:disjointWith <http://purl.org/nemo/gufo#RoleMixin> ;
                                       rdfs:comment """A gufo:EndurantType that is both non-sortal and anti-rigid. It is defined by instrinsic but contingent instantiation conditions. Phase mixins are relationally independent types that capture instrinsic properties shared by instances of different kinds.

For example, \"LivingAnimal\" may be considered a gufo:PhaseMixin as a superclass of the phases \"LivingPerson\" (specializing the gufo:Kind \"Person\") and \"LivingDog\" (specializing the gufo:Kind \"Dog\")."""@en ;
                                       rdfs:label "PhaseMixin"@en .


###  http://purl.org/nemo/gufo#Quality
<http://purl.org/nemo/gufo#Quality> rdf:type owl:Class ;
                                    rdfs:subClassOf <http://purl.org/nemo/gufo#IntrinsicAspect> ;
                                    rdfs:comment """A gufo:IntrinsicAspect that is measurable by some value spaces. A quality may be used to compare individuals, on the basis of the value it takes in a certain quality space (for instance, a position within the RGB spectrum).

Examples include the weight of a person, the name of organization, the color of a car, and the duration of a concert."""@en ;
                                    rdfs:label "Quality"@en .


###  http://purl.org/nemo/gufo#QualityValue
<http://purl.org/nemo/gufo#QualityValue> rdf:type owl:Class ;
                                         rdfs:subClassOf <http://purl.org/nemo/gufo#AbstractEntity> ;
                                         rdfs:comment """A gufo:AbstractIndividual that can be associated with a gufo:Quality reflecting the perception or conception of the quality in a certain value space. 

Instances of gufo:QualityValue include the rational number 2.5 when used to conceive of the acidity of a portion of wine (in a pH scale), the tuple <38.8897,-77.0089> when used to conceive of the location of a building (in a space formed by latitude and longitude), or the triplet <0,0,0> when used to conceive of the color of a physical object (in a trimensional space formed by red, green and blue color components).  

Corresponds to \"Quale\" in Guizzardi (2005). 

Use this class only for quality values (qualia) that are to be reified in the A-box and associated with a gufo:ConcreteIndividual through the object property gufo:hasReifiedQualityValue. Otherwise, use the gufo:hasQualityValue data property and a literal to determine the quality value."""@en ;
                                         rdfs:label "QualityValue"@en ;
                                         rdfs:seeAlso <http://purl.org/nemo/gufo#hasReifiedQualityValue> .


###  http://purl.org/nemo/gufo#QualityValueAttributionSituation
<http://purl.org/nemo/gufo#QualityValueAttributionSituation> rdf:type owl:Class ;
                                                             rdfs:subClassOf <http://purl.org/nemo/gufo#Situation> ,
                                                                             [ rdf:type owl:Class ;
                                                                               owl:unionOf ( [ rdf:type owl:Restriction ;
                                                                                               owl:onProperty <http://purl.org/nemo/gufo#concernsReifiedQualityValue> ;
                                                                                               owl:qualifiedCardinality "1"^^xsd:nonNegativeInteger ;
                                                                                               owl:onClass <http://purl.org/nemo/gufo#QualityValue>
                                                                                             ]
                                                                                             [ rdf:type owl:Restriction ;
                                                                                               owl:onProperty <http://purl.org/nemo/gufo#concernsQualityValue> ;
                                                                                               owl:cardinality "1"^^xsd:nonNegativeInteger
                                                                                             ]
                                                                                           )
                                                                             ] ,
                                                                             [ rdf:type owl:Restriction ;
                                                                               owl:onProperty <http://purl.org/nemo/gufo#concernsQualityType> ;
                                                                               owl:qualifiedCardinality "1"^^xsd:nonNegativeInteger ;
                                                                               owl:onClass <http://purl.org/nemo/gufo#EndurantType>
                                                                             ] ,
                                                                             [ rdf:type owl:Restriction ;
                                                                               owl:onProperty [ owl:inverseOf <http://purl.org/nemo/gufo#standsInQualifiedAttribution>
                                                                                              ] ;
                                                                               owl:qualifiedCardinality "1"^^xsd:nonNegativeInteger ;
                                                                               owl:onClass <http://purl.org/nemo/gufo#Endurant>
                                                                             ] ;
                                                             owl:disjointWith <http://purl.org/nemo/gufo#TemporaryConstitutionSituation> ,
                                                                              <http://purl.org/nemo/gufo#TemporaryInstantiationSituation> ,
                                                                              <http://purl.org/nemo/gufo#TemporaryParthoodSituation> ,
                                                                              <http://purl.org/nemo/gufo#TemporaryRelationshipSituation> ;
                                                             rdfs:comment """A gufo:Situation in which a quality value is temporarily attributed to a gufo:Endurant.

A gufo:QualityValueAttributionSituation should be used only for mutable qualities, i.e. those whose value can vary in time.

Examples include: the situation in which the value of a bitcoin in Euros is 6.526,12, which lasted from 10/12/2019 to 11/12/2019; the situation in which the weight of Mike Tyson was 100 kg; and the situation in which the color of Einstein' hair was grey.

This is a reification of the quality value attribution (in a solution that is similar to the qualified relation pattern  http://patterns.dataincubator.org/book/qualified-relation.html )"""@en ;
                                                             rdfs:label "QualityValueAttributionSituation"@en ;
                                                             rdfs:seeAlso <http://purl.org/nemo/gufo#concernsQualityValue> ,
                                                                          <http://purl.org/nemo/gufo#concernsReifiedQualityValue> .


###  http://purl.org/nemo/gufo#Quantity
<http://purl.org/nemo/gufo#Quantity> rdf:type owl:Class ;
                                     rdfs:subClassOf <http://purl.org/nemo/gufo#Object> ;
                                     rdfs:comment """A complex gufo:Object that is a maximally-connected portion of stuff. A gufo:Quantity has a fixed constitution, and thus, removing or adding a sub-quantity would result in a different quantity.

Examples include the portion of wine in a wine tank, a lump of clay, the gold that constitutes a wedding ring.

Also termed \"quantity of matter\", \"objectified portion of matter\", \"piece\" in the philosophical literature."""@en ;
                                     rdfs:label "Quantity"@en ;
                                     rdfs:seeAlso <http://purl.org/nemo/gufo#isSubQuantityOf> .


###  http://purl.org/nemo/gufo#RelationshipType
<http://purl.org/nemo/gufo#RelationshipType> rdf:type owl:Class ;
                                             rdfs:subClassOf <http://purl.org/nemo/gufo#Type> ;
                                             rdfs:comment """A gufo:Type whose instances are ordered pairs of related entities. Instances of gufo:RelationshipType are object properties in UFO-based ontologies.

The object properties \"marriedWith\" and \"enrolledIn\" are examples of material relationship types. The object properties \"heavierThan\", \"olderThan\" are examples of comparative relationship types.

The use of gufo:RelationshipType and its subclasses requires OWL 2 punning.

Corresponds to \"Relation\" in Guizzardi (2005) and Fonseca et al. (2019)."""@en ;
                                             rdfs:label "RelationshipType"@en .


###  http://purl.org/nemo/gufo#Relator
<http://purl.org/nemo/gufo#Relator> rdf:type owl:Class ;
                                    rdfs:subClassOf <http://purl.org/nemo/gufo#ExtrinsicAspect> ,
                                                    [ rdf:type owl:Restriction ;
                                                      owl:onProperty <http://purl.org/nemo/gufo#mediates> ;
                                                      owl:minQualifiedCardinality "2"^^xsd:nonNegativeInteger ;
                                                      owl:onClass <http://purl.org/nemo/gufo#Endurant>
                                                    ] ;
                                    rdfs:comment """A gufo:ExtrinsicAspect that connects (involves, mediates) two or more concrete individuals. Relators are reified relationships composed of reciprocal extrinsic modes.

Examples of relators include John and Mary's marriage (composed of John's obligations towards Mary in the scope of the marriage, Mary's reciprocal claims, Mary's obligations towards John, John's reciprocal claims), Mary's employment contract at Nasa, a covalent bond between two atoms."""@en ;
                                    rdfs:label "Relator"@en ;
                                    rdfs:seeAlso <http://purl.org/nemo/gufo#mediates> .


###  http://purl.org/nemo/gufo#RigidType
<http://purl.org/nemo/gufo#RigidType> rdf:type owl:Class ;
                                      rdfs:subClassOf <http://purl.org/nemo/gufo#EndurantType> ;
                                      rdfs:comment """A gufo:EndurantType which applies necessarily to its instances (see Guizzardi, 2005, chapter 4).

Examples include the types \"Agent\", \"Person\", \"Animal\", \"PhysicalObject\", \"Car\", and \"Tree\"."""@en ;
                                      rdfs:label "RigidType"@en .


###  http://purl.org/nemo/gufo#Role
<http://purl.org/nemo/gufo#Role> rdf:type owl:Class ;
                                 rdfs:subClassOf <http://purl.org/nemo/gufo#AntiRigidType> ,
                                                 <http://purl.org/nemo/gufo#Sortal> ;
                                 rdfs:comment """A gufo:EndurantType that both sortal and anti-rigid. It is defined by relational instantiation conditions. Roles are relationally dependent types, capturing relational properties shared by instances of a given kind.

For example, \"Student\" may be considered a gufo:Role as a subclass of the gufo:Kind \"Person\", instantiated by all persons enrolled in a school. \""""@en ;
                                 rdfs:label "Role"@en .


###  http://purl.org/nemo/gufo#RoleMixin
<http://purl.org/nemo/gufo#RoleMixin> rdf:type owl:Class ;
                                      rdfs:subClassOf <http://purl.org/nemo/gufo#AntiRigidType> ,
                                                      <http://purl.org/nemo/gufo#NonSortal> ;
                                      rdfs:comment """A gufo:EndurantType that is both non-sortal and anti-rigid. It is defined by relational instantiation conditions. Role mixins are relationally dependent types, capturing relational properties shared by instances of different kinds.

For example, \"Customer\" may be considered a gufo:RoleMixin as a superclass of the roles \"CorporateCustomer\" (specializing the gufo:Kind \"BusinessOrganization\") and \"PersonalCustomer\" (specializing the gufo:Kind \"Person\")."""@en ;
                                      rdfs:label "RoleMixin"@en .


###  http://purl.org/nemo/gufo#Scene
<http://purl.org/nemo/gufo#Scene> rdf:type owl:Class ;
                                  rdfs:subClassOf <http://purl.org/nemo/gufo#Perdurants> .


###  http://purl.org/nemo/gufo#SemiRigidType
<http://purl.org/nemo/gufo#SemiRigidType> rdf:type owl:Class ;
                                          rdfs:subClassOf <http://purl.org/nemo/gufo#NonRigidType> ;
                                          rdfs:comment "A gufo:NonRigidType that applies necessarily to some of its instances and contingently to some others (see Guizzardi, 2005, chapter 4)."@en ;
                                          rdfs:label "SemiRigidType"@en .


###  http://purl.org/nemo/gufo#Situation
<http://purl.org/nemo/gufo#Situation> rdf:type owl:Class ;
                                      rdfs:subClassOf <http://purl.org/nemo/gufo#Perdurants> ;
                                      rdfs:comment """A gufo:ConcreteIndividual that is a particular configuration of a part of reality which can be understood as a whole and in which entities stand in relations. A situation may be counterfactual or actual. An actual situation (or in other words, a \"fact\") \"obtains\" in a certain time instant or during a time interval.

Note that, in Guizzardi et al. (2013), situations were considered to obtain at a specific point in time. Here, instead, they obtain in a time interval when begin and end points differ.

The various subclasses of Situation in this implementation are used to capture \"mutable\" facts which obtain during some time and fail to obtain at other times. This includes the contingent instantiation of non-rigid types (e.g., as someone is a child at one point in time and a teenager later), the attribution of value to mutable qualities (such as a person's weight) and temporary participation in part-whole relations for replaceable parts (such as a car's tires). Other subclasses may be created to capture domain-specific notions such as \"HazardousSituation\", \"PersonHasFever\"."""@en ;
                                      rdfs:label "Situation"@en .


###  http://purl.org/nemo/gufo#SituationType
<http://purl.org/nemo/gufo#SituationType> rdf:type owl:Class ;
                                          rdfs:subClassOf <http://purl.org/nemo/gufo#PerdurantType> ;
                                          rdfs:comment """A gufo:Type whose instances are situations.

Instances of gufo:SituationType are subclasses of gufo:Situation.

Examples include \"HazardousSituation\", \"PersonHasFever\",  \"PersonIsStudent\"."""@en ;
                                          rdfs:label "SituationType"@en .


###  http://purl.org/nemo/gufo#Sortal
<http://purl.org/nemo/gufo#Sortal> rdf:type owl:Class ;
                                   rdfs:subClassOf <http://purl.org/nemo/gufo#EndurantType> ;
                                   rdfs:comment "A gufo:EndurantType which carries (or supplies) a principle of identity for its instances  (see Guizzardi, 2005, chapter 4)."@en ;
                                   rdfs:label "Sortal"@en .


###  http://purl.org/nemo/gufo#SubKind
<http://purl.org/nemo/gufo#SubKind> rdf:type owl:Class ;
                                    rdfs:subClassOf <http://purl.org/nemo/gufo#RigidType> ,
                                                    <http://purl.org/nemo/gufo#Sortal> ;
                                    rdfs:comment """A gufo:EndurantType that is both sortal and rigid. It specializes a gufo:Kind carrying the principle of identity supplied by that kind. Every gufo:SubKind should directly or indirectly specialize a gufo:Kind.

For example, the gufo:Kind \"Lion\" may be specialized into the \"Lionness\" and \"Male Lion\" subkinds, while the gufo:Kind \"Computer\" may be specialized into the \"Laptop\" and \"Desktop\" subkinds."""@en ;
                                    rdfs:label "SubKind"@en .


###  http://purl.org/nemo/gufo#TemporaryConstitutionSituation
<http://purl.org/nemo/gufo#TemporaryConstitutionSituation> rdf:type owl:Class ;
                                                           rdfs:subClassOf <http://purl.org/nemo/gufo#Situation> ,
                                                                           [ rdf:type owl:Restriction ;
                                                                             owl:onProperty <http://purl.org/nemo/gufo#concernsConstitutedEndurant> ;
                                                                             owl:qualifiedCardinality "1"^^xsd:nonNegativeInteger ;
                                                                             owl:onClass <http://purl.org/nemo/gufo#Object>
                                                                           ] ,
                                                                           [ rdf:type owl:Restriction ;
                                                                             owl:onProperty [ owl:inverseOf <http://purl.org/nemo/gufo#standsInQualifiedConstitution>
                                                                                            ] ;
                                                                             owl:qualifiedCardinality "1"^^xsd:nonNegativeInteger ;
                                                                             owl:onClass <http://purl.org/nemo/gufo#Object>
                                                                           ] ;
                                                           owl:disjointWith <http://purl.org/nemo/gufo#TemporaryInstantiationSituation> ,
                                                                            <http://purl.org/nemo/gufo#TemporaryRelationshipSituation> ;
                                                           rdfs:comment """A gufo:Situation in which a gufo:Endurant temporarly constitutes another gufo:Endurant.

When constitution of an object may change in time, it may be qualified by the period in time in which the relation applies. 

Examples include: the situation in which the Beatles is constituted by the group composed of {John,Paul,Ringo,George}; and the situation in which the statue of Venus de Milo was constituted by its original quantity of marble (including its arms).

This is a reification of constitution (in a solution that is similar to the qualified relation pattern  http://patterns.dataincubator.org/book/qualified-relation.html)"""@en ;
                                                           rdfs:label "TemporaryConstitutionSituation"@en .


###  http://purl.org/nemo/gufo#TemporaryInstantiationSituation
<http://purl.org/nemo/gufo#TemporaryInstantiationSituation> rdf:type owl:Class ;
                                                            rdfs:subClassOf <http://purl.org/nemo/gufo#Situation> ,
                                                                            [ rdf:type owl:Restriction ;
                                                                              owl:onProperty <http://purl.org/nemo/gufo#concernsNonRigidType> ;
                                                                              owl:qualifiedCardinality "1"^^xsd:nonNegativeInteger ;
                                                                              owl:onClass <http://purl.org/nemo/gufo#NonRigidType>
                                                                            ] ,
                                                                            [ rdf:type owl:Restriction ;
                                                                              owl:onProperty [ owl:inverseOf <http://purl.org/nemo/gufo#standsInQualifiedInstantiation>
                                                                                             ] ;
                                                                              owl:qualifiedCardinality "1"^^xsd:nonNegativeInteger ;
                                                                              owl:onClass <http://purl.org/nemo/gufo#Endurant>
                                                                            ] ;
                                                            owl:disjointWith <http://purl.org/nemo/gufo#TemporaryParthoodSituation> ,
                                                                             <http://purl.org/nemo/gufo#TemporaryRelationshipSituation> ;
                                                            rdfs:comment """A gufo:Situation in which a gufo:Endurant temporarily instantiates a gufo:NonRigidType.

A gufo:TemporaryInstantiationSituation can account for the time period in which a particular instantiation holds.

Examples include: the situation in which Obama instantiates the role of president, which began in 20/01/2009 and lasted until 20/01/2017; the situation in which Coatria instantiates the role of EU Member, which began in 01/07/2013 (and is still on-going); and the situation in which Steve Jobs instantiates the child phase, which began in 24/02/1955 and lasted until 24/02/1965.

This solution is inspired in the qualified relation pattern (http://patterns.dataincubator.org/book/qualified-relation.html)."""@en ;
                                                            rdfs:label "TemporaryInstantiationSituation"@en .


###  http://purl.org/nemo/gufo#TemporaryParthoodSituation
<http://purl.org/nemo/gufo#TemporaryParthoodSituation> rdf:type owl:Class ;
                                                       rdfs:subClassOf <http://purl.org/nemo/gufo#Situation> ,
                                                                       [ rdf:type owl:Restriction ;
                                                                         owl:onProperty <http://purl.org/nemo/gufo#concernsTemporaryWhole> ;
                                                                         owl:qualifiedCardinality "1"^^xsd:nonNegativeInteger ;
                                                                         owl:onClass <http://purl.org/nemo/gufo#Endurant>
                                                                       ] ,
                                                                       [ rdf:type owl:Restriction ;
                                                                         owl:onProperty [ owl:inverseOf <http://purl.org/nemo/gufo#standsInQualifiedParthood>
                                                                                        ] ;
                                                                         owl:qualifiedCardinality "1"^^xsd:nonNegativeInteger ;
                                                                         owl:onClass <http://purl.org/nemo/gufo#Endurant>
                                                                       ] ;
                                                       owl:disjointWith <http://purl.org/nemo/gufo#TemporaryRelationshipSituation> ;
                                                       rdfs:comment """A gufo:Situation in which a gufo:Endurant is temporarily a part of another gufo:Endurant.

A gufo:TemporaryParthoodSituation should only be used for mutable parts. It may be qualified by the period in time in which the relation applies. 

Examples include: the situation in which the United Kingdom is a member of the European Union; the situation in which Messi is a a member of the Barcelona FC squad; the situation in which an engine is part of a car; and the situation in which a transplanted heart is part of a person.

Note that, since every instance of gufo:Quantity or gufo:FixedCollection only has essential parts, the gufo:TemporaryParthoodSituation should not be used to represent these parthood relations.
 
This solution is inspired in the qualified relation pattern (http://patterns.dataincubator.org/book/qualified-relation.html).""" ;
                                                       rdfs:label "TemporaryParthoodSituation"@en .


###  http://purl.org/nemo/gufo#TemporaryRelationshipSituation
<http://purl.org/nemo/gufo#TemporaryRelationshipSituation> rdf:type owl:Class ;
                                                           rdfs:subClassOf <http://purl.org/nemo/gufo#Situation> ,
                                                                           [ rdf:type owl:Restriction ;
                                                                             owl:onProperty <http://purl.org/nemo/gufo#concernsRelatedEndurant> ;
                                                                             owl:someValuesFrom <http://purl.org/nemo/gufo#Endurant>
                                                                           ] ,
                                                                           [ rdf:type owl:Restriction ;
                                                                             owl:onProperty <http://purl.org/nemo/gufo#concernsRelationshipType> ;
                                                                             owl:qualifiedCardinality "1"^^xsd:nonNegativeInteger ;
                                                                             owl:onClass <http://purl.org/nemo/gufo#RelationshipType>
                                                                           ] ,
                                                                           [ rdf:type owl:Restriction ;
                                                                             owl:onProperty [ owl:inverseOf <http://purl.org/nemo/gufo#standsInQualifiedRelationship>
                                                                                            ] ;
                                                                             owl:qualifiedCardinality "1"^^xsd:nonNegativeInteger ;
                                                                             owl:onClass <http://purl.org/nemo/gufo#Endurant>
                                                                           ] ;
                                                           rdfs:comment """A gufo:Situation in which a gufo:Endurant temporarily stands in a relation with another gufo:Endurant (or other endurants in the case of n-ary relationships). 

Reification of a gufo:TemporaryRelationshipSituation allows qualification of the relationship with the period in time in which it applies. 

Examples include: the situation in which Einstein works at the Swiss Patent Office in Bern; the situation in which Elon Musk studies at the University of Pennsylvania; the situation in which John Lennon is married to Yoko Ono; and the situation in which Facebook has a lower market value than Amazon.

For material relationships, prefer the use of gufo:Relator.

This is a reification of the relationship (in a solution that is similar to the qualified relation pattern  http://patterns.dataincubator.org/book/qualified-relation.html)."""@en ;
                                                           rdfs:label "TemporaryRelationshipSituation"@en .


###  http://purl.org/nemo/gufo#Type
<http://purl.org/nemo/gufo#Type> rdf:type owl:Class ;
                                 rdfs:comment """An entity that may be instantiated by (or predicated over) other entities. Types encompass what we often call \"sorts\", \"kinds\", \"categories\", etc. 

Examples include the kind \"Person\", the event type \"Earthquake\", and the abstract individual type \"NaturalNumber\". Relations, such as \"marriedTo\" and \"olderThan\", are also considered as types.

Instances of gufo:Type are classes, and should specialize the taxonomy of individuals of gUFO. For example, \"Person\" is a gufo:Type (more specifically a gufo:Kind), specializing gufo:Object. The mechanism that allows for this is called punning in OWL 2.

Encompasses the notion of \"Universal\" in Guizzardi (2005)."""@en ;
                                 rdfs:label "Type"@en .


###  http://purl.org/nemo/gufo#VariableCollection
<http://purl.org/nemo/gufo#VariableCollection> rdf:type owl:Class ;
                                               rdfs:subClassOf <http://purl.org/nemo/gufo#Collection> ;
                                               rdfs:comment <http://purl.org/nemo/gufo#TemporaryParthoodSituation> ,
                                                            """A gufo:Collection for which change in membership is possible.

Such a collection obeys an intensional principle of identity, i.e., change in membership does not necessarily create a different collection.

For example, KLM's fleet of airplanes could be understood as a gufo:VariableCollection. In this case, when the company acquires (or retires) an airplane, the fleet changes. Note that, in this case, the airplanes are conceptualized as playing the role of \"member of a fleet\". If various roles for the parts of a fleet were envisioned (such as \"cargo airplane\", \"passenger airplane\"), then a fleet would be best understood as a gufo:FunctionalComplex.

See gufo:TemporaryParthoodSituation for the pattern to represent the relation of a variable collection to its temporary parts."""@en ;
                                               rdfs:label "VariableCollection"@en .


###  http://www.opengis.net/ont/geosparql#Feature
<http://www.opengis.net/ont/geosparql#Feature> rdf:type owl:Class ;
                                               rdfs:subClassOf <http://www.opengis.net/ont/geosparql#SpatialObject> ;
                                               owl:disjointWith <http://www.opengis.net/ont/geosparql#Geometry> ;
                                               <http://purl.org/dc/elements/1.1/contributor> "Matthew Perry" ;
                                               <http://purl.org/dc/elements/1.1/creator> "OGC GeoSPARQL 1.0 Standard Working Group" ;
                                               <http://purl.org/dc/elements/1.1/date> "2011-06-16"^^xsd:date ;
                                               <http://purl.org/dc/elements/1.1/description> """
      This class represents the top-level feature type. This class is 
      equivalent to GFI_Feature defined in ISO 19156:2011, and it is 
      superclass of all feature types.
    """@en ;
                                               rdfs:comment """
      This class represents the top-level feature type. This class is 
      equivalent to GFI_Feature defined in ISO 19156:2011, and it is 
      superclass of all feature types.
    """@en ;
                                               rdfs:isDefinedBy <http://www.opengis.net/ont/geosparql> ,
                                                                <http://www.opengis.net/ont/gml> ,
                                                                <http://www.opengis.net/spec/geosparql/1.0> ;
                                               rdfs:label "Feature"@en ;
                                               <http://www.w3.org/2004/02/skos/core#definition> """
      This class represents the top-level feature type. This class is 
      equivalent to GFI_Feature defined in ISO 19156:2011, and it is 
      superclass of all feature types.
    """@en ,
                                                                                                """A discrete spatial phenomenon in a universe of discourse.

Spatial phenomena can generally be thought of as either discrete objects with clear boundaries or as a continuous phenomenon that can be observed everywhere, but does not have natural boundaries. 

Discrete spatial objects may refer to a river, road, country, town, or a research site.

Examples of continuous phenomena, or “spatial fields”, include elevation and qualities.""" ;
                                               <http://www.w3.org/2004/02/skos/core#prefLabel> "Feature"@en .


###  http://www.opengis.net/ont/geosparql#Geometry
<http://www.opengis.net/ont/geosparql#Geometry> rdf:type owl:Class ;
                                                rdfs:subClassOf <http://www.opengis.net/ont/geosparql#SpatialObject> ;
                                                <http://purl.org/dc/elements/1.1/contributor> "Matthew Perry" ;
                                                <http://purl.org/dc/elements/1.1/creator> "OGC GeoSPARQL 1.0 Standard Working Group" ;
                                                <http://purl.org/dc/elements/1.1/date> "2011-06-16"^^xsd:date ;
                                                <http://purl.org/dc/elements/1.1/description> """
      The class represents the top-level geometry type. This class is 
      equivalent to the UML class GM_Object defined in ISO 19107, and 
      it is superclass of all geometry types.
    """@en ;
                                                rdfs:comment """
      The class represents the top-level geometry type. This class is 
      equivalent to the UML class GM_Object defined in ISO 19107, and 
      it is superclass of all geometry types.
    """@en ;
                                                rdfs:isDefinedBy <http://www.opengis.net/ont/geosparql> ,
                                                                 <http://www.opengis.net/ont/gml> ,
                                                                 <http://www.opengis.net/spec/geosparql/1.0> ;
                                                rdfs:label "Geometry"@en ;
                                                <http://www.w3.org/2004/02/skos/core#definition> """
      The class represents the top-level geometry type. This class is 
      equivalent to the UML class GM_Object defined in ISO 19107, and 
      it is superclass of all geometry types.
    """@en ;
                                                <http://www.w3.org/2004/02/skos/core#prefLabel> "Geometry"@en .


###  http://www.opengis.net/ont/geosparql#SpatialObject
<http://www.opengis.net/ont/geosparql#SpatialObject> rdf:type owl:Class ;
                                                     rdfs:subClassOf <http://purl.org/nemo/gufo#Object> ;
                                                     <http://purl.org/dc/elements/1.1/contributor> "Matthew Perry" ;
                                                     <http://purl.org/dc/elements/1.1/creator> "OGC GeoSPARQL 1.0 Standard Working Group" ;
                                                     <http://purl.org/dc/elements/1.1/date> "2011-06-16"^^xsd:date ;
                                                     <http://purl.org/dc/elements/1.1/description> """
      The class spatial-object represents everything that can have 
      a spatial representation. It is superclass of feature and geometry.
    """@en ;
                                                     rdfs:comment """
      The class spatial-object represents everything that can have 
      a spatial representation. It is superclass of feature and geometry.
    """@en ;
                                                     rdfs:isDefinedBy <http://www.opengis.net/ont/geosparql> ,
                                                                      <http://www.opengis.net/ont/gml> ,
                                                                      <http://www.opengis.net/spec/geosparql/1.0> ;
                                                     rdfs:label "SpatialObject"@en ;
                                                     <http://www.w3.org/2004/02/skos/core#definition> """
      The class spatial-object represents everything that can have 
      a spatial representation. It is superclass of feature and geometry.
    """@en ;
                                                     <http://www.w3.org/2004/02/skos/core#prefLabel> "SpatialObject"@en .


###  http://www.opengis.net/ont/gml#AbstractCurveSegment
<http://www.opengis.net/ont/gml#AbstractCurveSegment> rdf:type owl:Class ;
                                                      rdfs:subClassOf <http://www.opengis.net/ont/geosparql#Geometry> ;
                                                      rdfs:isDefinedBy <http://www.opengis.net/ont/gml> ;
                                                      rdfs:label "Abstract Curve Segment"@en .


###  http://www.opengis.net/ont/gml#AbstractGeometricPrimitive
<http://www.opengis.net/ont/gml#AbstractGeometricPrimitive> rdf:type owl:Class ;
                                                            rdfs:subClassOf <http://www.opengis.net/ont/gml#AbstractGeometry> ;
                                                            rdfs:isDefinedBy <http://www.opengis.net/ont/gml> ;
                                                            rdfs:label "Abstract Geometric Primitive"@en .


###  http://www.opengis.net/ont/gml#AbstractGeometry
<http://www.opengis.net/ont/gml#AbstractGeometry> rdf:type owl:Class ;
                                                  rdfs:subClassOf <http://www.opengis.net/ont/geosparql#Geometry> ;
                                                  rdfs:isDefinedBy <http://www.opengis.net/ont/gml> ;
                                                  rdfs:label "Abstract Geometry"@en .


###  http://www.opengis.net/ont/gml#AbstractGriddedSurface
<http://www.opengis.net/ont/gml#AbstractGriddedSurface> rdf:type owl:Class ;
                                                        rdfs:subClassOf <http://www.opengis.net/ont/gml#AbstractParametricCurveSurface> ;
                                                        rdfs:isDefinedBy <http://www.opengis.net/ont/gml> ;
                                                        rdfs:label "Abstract Gridded Surface"@en .


###  http://www.opengis.net/ont/gml#AbstractParametricCurveSurface
<http://www.opengis.net/ont/gml#AbstractParametricCurveSurface> rdf:type owl:Class ;
                                                                rdfs:subClassOf <http://www.opengis.net/ont/gml#AbstractSurfacePatch> ;
                                                                rdfs:isDefinedBy <http://www.opengis.net/ont/gml> ;
                                                                rdfs:label "Abstract Parametric Curve Surface"@en .


###  http://www.opengis.net/ont/gml#AbstractSurfacePatch
<http://www.opengis.net/ont/gml#AbstractSurfacePatch> rdf:type owl:Class ;
                                                      rdfs:subClassOf <http://www.opengis.net/ont/geosparql#Geometry> ;
                                                      rdfs:isDefinedBy <http://www.opengis.net/ont/gml> ;
                                                      rdfs:label "Abstract Surface Patch"@en .


###  http://www.opengis.net/ont/gml#Arc
<http://www.opengis.net/ont/gml#Arc> rdf:type owl:Class ;
                                     rdfs:subClassOf <http://www.opengis.net/ont/gml#ArcString> ;
                                     rdfs:isDefinedBy <http://www.opengis.net/ont/gml> ;
                                     rdfs:label "Arc"@en .


###  http://www.opengis.net/ont/gml#ArcByBulge
<http://www.opengis.net/ont/gml#ArcByBulge> rdf:type owl:Class ;
                                            rdfs:subClassOf <http://www.opengis.net/ont/gml#ArcStringByBulge> ;
                                            rdfs:isDefinedBy <http://www.opengis.net/ont/gml> ;
                                            rdfs:label "Arc by Bulge"@en .


###  http://www.opengis.net/ont/gml#ArcByCenterPoint
<http://www.opengis.net/ont/gml#ArcByCenterPoint> rdf:type owl:Class ;
                                                  rdfs:subClassOf <http://www.opengis.net/ont/gml#AbstractCurveSegment> ;
                                                  rdfs:isDefinedBy <http://www.opengis.net/ont/gml> ;
                                                  rdfs:label "Arc by Center Point"@en .


###  http://www.opengis.net/ont/gml#ArcString
<http://www.opengis.net/ont/gml#ArcString> rdf:type owl:Class ;
                                           rdfs:subClassOf <http://www.opengis.net/ont/gml#AbstractCurveSegment> ;
                                           rdfs:isDefinedBy <http://www.opengis.net/ont/gml> ;
                                           rdfs:label "Arc String"@en .


###  http://www.opengis.net/ont/gml#ArcStringByBulge
<http://www.opengis.net/ont/gml#ArcStringByBulge> rdf:type owl:Class ;
                                                  rdfs:subClassOf <http://www.opengis.net/ont/gml#AbstractCurveSegment> ;
                                                  rdfs:isDefinedBy <http://www.opengis.net/ont/gml> ;
                                                  rdfs:label "Arc String by Bulge"@en .


###  http://www.opengis.net/ont/gml#BSpline
<http://www.opengis.net/ont/gml#BSpline> rdf:type owl:Class ;
                                         rdfs:subClassOf <http://www.opengis.net/ont/gml#SplineCurve> ;
                                         rdfs:isDefinedBy <http://www.opengis.net/ont/gml> ;
                                         rdfs:label "BSpline"@en .


###  http://www.opengis.net/ont/gml#Bezier
<http://www.opengis.net/ont/gml#Bezier> rdf:type owl:Class ;
                                        rdfs:subClassOf <http://www.opengis.net/ont/gml#BSpline> ;
                                        rdfs:isDefinedBy <http://www.opengis.net/ont/gml> ;
                                        rdfs:label "Bezier"@en .


###  http://www.opengis.net/ont/gml#Circle
<http://www.opengis.net/ont/gml#Circle> rdf:type owl:Class ;
                                        rdfs:subClassOf <http://www.opengis.net/ont/gml#Arc> ;
                                        rdfs:isDefinedBy <http://www.opengis.net/ont/gml> ;
                                        rdfs:label "Circle"@en .


###  http://www.opengis.net/ont/gml#CircleByCenterPoint
<http://www.opengis.net/ont/gml#CircleByCenterPoint> rdf:type owl:Class ;
                                                     rdfs:subClassOf <http://www.opengis.net/ont/gml#ArcByCenterPoint> ;
                                                     rdfs:isDefinedBy <http://www.opengis.net/ont/gml> ;
                                                     rdfs:label "CircleByCenterPoint"@en .


###  http://www.opengis.net/ont/gml#Clothoid
<http://www.opengis.net/ont/gml#Clothoid> rdf:type owl:Class ;
                                          rdfs:subClassOf <http://www.opengis.net/ont/gml#AbstractCurveSegment> ;
                                          rdfs:isDefinedBy <http://www.opengis.net/ont/gml> ;
                                          rdfs:label "Clothoid"@en .


###  http://www.opengis.net/ont/gml#Composite
<http://www.opengis.net/ont/gml#Composite> rdf:type owl:Class ;
                                           rdfs:subClassOf <http://www.opengis.net/ont/gml#GeometricComplex> ;
                                           rdfs:isDefinedBy <http://www.opengis.net/ont/gml> ;
                                           rdfs:label "Composite"@en .


###  http://www.opengis.net/ont/gml#CompositeCurve
<http://www.opengis.net/ont/gml#CompositeCurve> rdf:type owl:Class ;
                                                rdfs:subClassOf <http://www.opengis.net/ont/gml#Composite> ,
                                                                <http://www.opengis.net/ont/gml#OrientableCurve> ;
                                                rdfs:isDefinedBy <http://www.opengis.net/ont/gml> ;
                                                rdfs:label "Composite Curve"@en .


###  http://www.opengis.net/ont/gml#CompositeSolid
<http://www.opengis.net/ont/gml#CompositeSolid> rdf:type owl:Class ;
                                                rdfs:subClassOf <http://www.opengis.net/ont/gml#Composite> ,
                                                                <http://www.opengis.net/ont/gml#Solid> ;
                                                rdfs:isDefinedBy <http://www.opengis.net/ont/gml> ;
                                                rdfs:label "Composite Solid"@en .


###  http://www.opengis.net/ont/gml#CompositeSurface
<http://www.opengis.net/ont/gml#CompositeSurface> rdf:type owl:Class ;
                                                  rdfs:subClassOf <http://www.opengis.net/ont/gml#Composite> ,
                                                                  <http://www.opengis.net/ont/gml#OrientableSurface> ;
                                                  rdfs:isDefinedBy <http://www.opengis.net/ont/gml> ;
                                                  rdfs:label "Composite Surface"@en .


###  http://www.opengis.net/ont/gml#Cone
<http://www.opengis.net/ont/gml#Cone> rdf:type owl:Class ;
                                      rdfs:subClassOf <http://www.opengis.net/ont/gml#AbstractGriddedSurface> ;
                                      rdfs:isDefinedBy <http://www.opengis.net/ont/gml> ;
                                      rdfs:label "Cone"@en .


###  http://www.opengis.net/ont/gml#CubicSpline
<http://www.opengis.net/ont/gml#CubicSpline> rdf:type owl:Class ;
                                             rdfs:subClassOf <http://www.opengis.net/ont/gml#PolynomialSpline> ;
                                             rdfs:isDefinedBy <http://www.opengis.net/ont/gml> ;
                                             rdfs:label "Cubic Spline"@en .


###  http://www.opengis.net/ont/gml#Curve
<http://www.opengis.net/ont/gml#Curve> rdf:type owl:Class ;
                                       rdfs:subClassOf <http://www.opengis.net/ont/gml#AbstractGeometricPrimitive> ,
                                                       <http://www.opengis.net/ont/gml#OrientableCurve> ;
                                       rdfs:isDefinedBy <http://www.opengis.net/ont/gml> ;
                                       rdfs:label "Curve"@en .


###  http://www.opengis.net/ont/gml#Cylinder
<http://www.opengis.net/ont/gml#Cylinder> rdf:type owl:Class ;
                                          rdfs:subClassOf <http://www.opengis.net/ont/gml#AbstractGriddedSurface> ;
                                          rdfs:isDefinedBy <http://www.opengis.net/ont/gml> ;
                                          rdfs:label "Cylinder"@en .


###  http://www.opengis.net/ont/gml#Geodesic
<http://www.opengis.net/ont/gml#Geodesic> rdf:type owl:Class ;
                                          rdfs:subClassOf <http://www.opengis.net/ont/gml#GeodesicString> ;
                                          rdfs:isDefinedBy <http://www.opengis.net/ont/gml> ;
                                          rdfs:label "Geodesic"@en .


###  http://www.opengis.net/ont/gml#GeodesicString
<http://www.opengis.net/ont/gml#GeodesicString> rdf:type owl:Class ;
                                                rdfs:subClassOf <http://www.opengis.net/ont/gml#AbstractCurveSegment> ;
                                                rdfs:isDefinedBy <http://www.opengis.net/ont/gml> ;
                                                rdfs:label "Geodesic String"@en .


###  http://www.opengis.net/ont/gml#GeometricComplex
<http://www.opengis.net/ont/gml#GeometricComplex> rdf:type owl:Class ;
                                                  rdfs:subClassOf <http://www.opengis.net/ont/gml#AbstractGeometry> ;
                                                  rdfs:isDefinedBy <http://www.opengis.net/ont/gml> ;
                                                  rdfs:label "Geometric Complex"@en .


###  http://www.opengis.net/ont/gml#LineString
<http://www.opengis.net/ont/gml#LineString> rdf:type owl:Class ;
                                            rdfs:subClassOf <http://www.opengis.net/ont/gml#LineStringSegment> ;
                                            rdfs:isDefinedBy <http://www.opengis.net/ont/gml> ;
                                            rdfs:label "Line String"@en .


###  http://www.opengis.net/ont/gml#LineStringSegment
<http://www.opengis.net/ont/gml#LineStringSegment> rdf:type owl:Class ;
                                                   rdfs:subClassOf <http://www.opengis.net/ont/gml#AbstractCurveSegment> ;
                                                   rdfs:isDefinedBy <http://www.opengis.net/ont/gml> ;
                                                   rdfs:label "Line String Segment"@en .


###  http://www.opengis.net/ont/gml#LinearRing
<http://www.opengis.net/ont/gml#LinearRing> rdf:type owl:Class ;
                                            rdfs:subClassOf <http://www.opengis.net/ont/gml#Ring> ;
                                            rdfs:isDefinedBy <http://www.opengis.net/ont/gml> ;
                                            rdfs:label "Linear Ring"@en .


###  http://www.opengis.net/ont/gml#MultiCurve
<http://www.opengis.net/ont/gml#MultiCurve> rdf:type owl:Class ;
                                            rdfs:subClassOf <http://www.opengis.net/ont/gml#MultiGeometry> ;
                                            rdfs:isDefinedBy <http://www.opengis.net/ont/gml> ;
                                            rdfs:label "Multi-Curve"@en .


###  http://www.opengis.net/ont/gml#MultiGeometry
<http://www.opengis.net/ont/gml#MultiGeometry> rdf:type owl:Class ;
                                               rdfs:subClassOf <http://www.opengis.net/ont/gml#AbstractGeometry> ;
                                               rdfs:isDefinedBy <http://www.opengis.net/ont/gml> ;
                                               rdfs:label "Multi-Geometry"@en .


###  http://www.opengis.net/ont/gml#MultiPoint
<http://www.opengis.net/ont/gml#MultiPoint> rdf:type owl:Class ;
                                            rdfs:subClassOf <http://www.opengis.net/ont/gml#MultiGeometry> ;
                                            rdfs:isDefinedBy <http://www.opengis.net/ont/gml> ;
                                            rdfs:label "Multi-Point"@en .


###  http://www.opengis.net/ont/gml#MultiSolid
<http://www.opengis.net/ont/gml#MultiSolid> rdf:type owl:Class ;
                                            rdfs:subClassOf <http://www.opengis.net/ont/gml#MultiGeometry> ;
                                            rdfs:isDefinedBy <http://www.opengis.net/ont/gml> ;
                                            rdfs:label "Multi-Solid"@en .


###  http://www.opengis.net/ont/gml#MultiSurface
<http://www.opengis.net/ont/gml#MultiSurface> rdf:type owl:Class ;
                                              rdfs:subClassOf <http://www.opengis.net/ont/gml#MultiGeometry> ;
                                              rdfs:isDefinedBy <http://www.opengis.net/ont/gml> ;
                                              rdfs:label "Multi-Surface"@en .


###  http://www.opengis.net/ont/gml#OffsetCurve
<http://www.opengis.net/ont/gml#OffsetCurve> rdf:type owl:Class ;
                                             rdfs:subClassOf <http://www.opengis.net/ont/gml#AbstractCurveSegment> ;
                                             rdfs:isDefinedBy <http://www.opengis.net/ont/gml> ;
                                             rdfs:label "Offset Curve"@en .


###  http://www.opengis.net/ont/gml#OrientableCurve
<http://www.opengis.net/ont/gml#OrientableCurve> rdf:type owl:Class ;
                                                 rdfs:subClassOf <http://www.opengis.net/ont/gml#AbstractGeometricPrimitive> ;
                                                 rdfs:isDefinedBy <http://www.opengis.net/ont/gml> ;
                                                 rdfs:label "Orientable Curve"@en .


###  http://www.opengis.net/ont/gml#OrientableSurface
<http://www.opengis.net/ont/gml#OrientableSurface> rdf:type owl:Class ;
                                                   rdfs:subClassOf <http://www.opengis.net/ont/gml#AbstractGeometricPrimitive> ;
                                                   rdfs:isDefinedBy <http://www.opengis.net/ont/gml> ;
                                                   rdfs:label "Orientable Surface"@en .


###  http://www.opengis.net/ont/gml#Point
<http://www.opengis.net/ont/gml#Point> rdf:type owl:Class ;
                                       rdfs:subClassOf <http://www.opengis.net/ont/gml#AbstractGeometricPrimitive> ;
                                       rdfs:isDefinedBy <http://www.opengis.net/ont/gml> ;
                                       rdfs:label "Point"@en .


###  http://www.opengis.net/ont/gml#Polygon
<http://www.opengis.net/ont/gml#Polygon> rdf:type owl:Class ;
                                         rdfs:subClassOf <http://www.opengis.net/ont/gml#Surface> ;
                                         rdfs:isDefinedBy <http://www.opengis.net/ont/gml> ;
                                         rdfs:label "Polygon"@en .


###  http://www.opengis.net/ont/gml#PolygonPatch
<http://www.opengis.net/ont/gml#PolygonPatch> rdf:type owl:Class ;
                                              rdfs:subClassOf <http://www.opengis.net/ont/gml#AbstractSurfacePatch> ;
                                              rdfs:isDefinedBy <http://www.opengis.net/ont/gml> ;
                                              rdfs:label "Polygon Patch"@en .


###  http://www.opengis.net/ont/gml#PolyhedralSurface
<http://www.opengis.net/ont/gml#PolyhedralSurface> rdf:type owl:Class ;
                                                   rdfs:subClassOf <http://www.opengis.net/ont/gml#Surface> ;
                                                   rdfs:isDefinedBy <http://www.opengis.net/ont/gml> ;
                                                   rdfs:label "Polyhedral Surface"@en .


###  http://www.opengis.net/ont/gml#PolynomialSpline
<http://www.opengis.net/ont/gml#PolynomialSpline> rdf:type owl:Class ;
                                                  rdfs:subClassOf <http://www.opengis.net/ont/gml#SplineCurve> ;
                                                  rdfs:isDefinedBy <http://www.opengis.net/ont/gml> ;
                                                  rdfs:label "Polynomial Spline"@en .


###  http://www.opengis.net/ont/gml#Rectangle
<http://www.opengis.net/ont/gml#Rectangle> rdf:type owl:Class ;
                                           rdfs:subClassOf <http://www.opengis.net/ont/gml#PolygonPatch> ;
                                           rdfs:isDefinedBy <http://www.opengis.net/ont/gml> ;
                                           rdfs:label "Rectangle"@en .


###  http://www.opengis.net/ont/gml#Ring
<http://www.opengis.net/ont/gml#Ring> rdf:type owl:Class ;
                                      rdfs:subClassOf <http://www.opengis.net/ont/gml#CompositeCurve> ;
                                      rdfs:isDefinedBy <http://www.opengis.net/ont/gml> ;
                                      rdfs:label "Ring"@en .


###  http://www.opengis.net/ont/gml#Shell
<http://www.opengis.net/ont/gml#Shell> rdf:type owl:Class ;
                                       rdfs:subClassOf <http://www.opengis.net/ont/gml#CompositeSurface> ;
                                       rdfs:isDefinedBy <http://www.opengis.net/ont/gml> ;
                                       rdfs:label "Shell"@en .


###  http://www.opengis.net/ont/gml#Solid
<http://www.opengis.net/ont/gml#Solid> rdf:type owl:Class ;
                                       rdfs:subClassOf <http://www.opengis.net/ont/gml#AbstractGeometricPrimitive> ;
                                       rdfs:isDefinedBy <http://www.opengis.net/ont/gml> ;
                                       rdfs:label "Solid"@en .


###  http://www.opengis.net/ont/gml#Sphere
<http://www.opengis.net/ont/gml#Sphere> rdf:type owl:Class ;
                                        rdfs:subClassOf <http://www.opengis.net/ont/gml#AbstractGriddedSurface> ;
                                        rdfs:isDefinedBy <http://www.opengis.net/ont/gml> ;
                                        rdfs:label "Sphere"@en .


###  http://www.opengis.net/ont/gml#SplineCurve
<http://www.opengis.net/ont/gml#SplineCurve> rdf:type owl:Class ;
                                             rdfs:subClassOf <http://www.opengis.net/ont/gml#AbstractCurveSegment> ;
                                             rdfs:isDefinedBy <http://www.opengis.net/ont/gml> ;
                                             rdfs:label "Spline Curve"@en .


###  http://www.opengis.net/ont/gml#Surface
<http://www.opengis.net/ont/gml#Surface> rdf:type owl:Class ;
                                         rdfs:subClassOf <http://www.opengis.net/ont/gml#AbstractGeometricPrimitive> ,
                                                         <http://www.opengis.net/ont/gml#OrientableSurface> ;
                                         rdfs:isDefinedBy <http://www.opengis.net/ont/gml> ;
                                         rdfs:label "Surface"@en .


###  http://www.opengis.net/ont/gml#Tin
<http://www.opengis.net/ont/gml#Tin> rdf:type owl:Class ;
                                     rdfs:subClassOf <http://www.opengis.net/ont/gml#TriangulatedSurface> ;
                                     rdfs:isDefinedBy <http://www.opengis.net/ont/gml> ;
                                     rdfs:label "Triangulated Irregular Network"@en .


###  http://www.opengis.net/ont/gml#Triangle
<http://www.opengis.net/ont/gml#Triangle> rdf:type owl:Class ;
                                          rdfs:subClassOf <http://www.opengis.net/ont/gml#PolygonPatch> ;
                                          rdfs:isDefinedBy <http://www.opengis.net/ont/gml> ;
                                          rdfs:label "Triangle"@en .


###  http://www.opengis.net/ont/gml#TriangulatedSurface
<http://www.opengis.net/ont/gml#TriangulatedSurface> rdf:type owl:Class ;
                                                     rdfs:subClassOf <http://www.opengis.net/ont/gml#PolyhedralSurface> ;
                                                     rdfs:isDefinedBy <http://www.opengis.net/ont/gml> ;
                                                     rdfs:label "Triangulated Surface"@en .


###  http://www.w3.org/1999/02/22-rdf-syntax-ns#List
rdf:List rdf:type owl:Class .


###  http://www.w3.org/2004/02/skos/core#Collection
<http://www.w3.org/2004/02/skos/core#Collection> rdf:type owl:Class ;
                                                 owl:disjointWith <http://www.w3.org/2004/02/skos/core#Concept> ,
                                                                  <http://www.w3.org/2004/02/skos/core#ConceptScheme> ;
                                                 rdfs:isDefinedBy <http://www.w3.org/2004/02/skos/core> ;
                                                 rdfs:label "Collection"@en ;
                                                 <http://www.w3.org/2004/02/skos/core#definition> "A meaningful collection of concepts."@en ;
                                                 <http://www.w3.org/2004/02/skos/core#scopeNote> "Labelled collections can be used where you would like a set of concepts to be displayed under a 'node label' in the hierarchy."@en .


###  http://www.w3.org/2004/02/skos/core#Concept
<http://www.w3.org/2004/02/skos/core#Concept> rdf:type owl:Class ;
                                              owl:disjointWith <http://www.w3.org/2004/02/skos/core#ConceptScheme> ;
                                              rdfs:isDefinedBy <http://www.w3.org/2004/02/skos/core> ;
                                              rdfs:label "Concept"@en ;
                                              <http://www.w3.org/2004/02/skos/core#definition> "An idea or notion; a unit of thought."@en .


###  http://www.w3.org/2004/02/skos/core#ConceptScheme
<http://www.w3.org/2004/02/skos/core#ConceptScheme> rdf:type owl:Class ;
                                                    rdfs:isDefinedBy <http://www.w3.org/2004/02/skos/core> ;
                                                    rdfs:label "Concept Scheme"@en ;
                                                    <http://www.w3.org/2004/02/skos/core#definition> "A set of concepts, optionally including statements about semantic relationships between those concepts."@en ;
                                                    <http://www.w3.org/2004/02/skos/core#example> "Thesauri, classification schemes, subject heading lists, taxonomies, 'folksonomies', and other types of controlled vocabulary are all examples of concept schemes. Concept schemes are also embedded in glossaries and terminologies."@en ;
                                                    <http://www.w3.org/2004/02/skos/core#scopeNote> "A concept scheme may be defined to include concepts from different sources."@en .


###  http://www.w3.org/2004/02/skos/core#OrderedCollection
<http://www.w3.org/2004/02/skos/core#OrderedCollection> rdf:type owl:Class ;
                                                        rdfs:subClassOf <http://www.w3.org/2004/02/skos/core#Collection> ;
                                                        rdfs:isDefinedBy <http://www.w3.org/2004/02/skos/core> ;
                                                        rdfs:label "Ordered Collection"@en ;
                                                        <http://www.w3.org/2004/02/skos/core#definition> "An ordered collection of concepts, where both the grouping and the ordering are meaningful."@en ;
                                                        <http://www.w3.org/2004/02/skos/core#scopeNote> "Ordered collections can be used where you would like a set of concepts to be displayed in a specific order, and optionally under a 'node label'."@en .


###  http://www.w3.org/2006/time#DateTimeDescription
<http://www.w3.org/2006/time#DateTimeDescription> rdf:type owl:Class ;
                                                  rdfs:subClassOf <http://www.w3.org/2006/time#GeneralDateTimeDescription> ,
                                                                  [ rdf:type owl:Restriction ;
                                                                    owl:onProperty <http://www.w3.org/2006/time#day> ;
                                                                    owl:allValuesFrom xsd:gDay
                                                                  ] ,
                                                                  [ rdf:type owl:Restriction ;
                                                                    owl:onProperty <http://www.w3.org/2006/time#month> ;
                                                                    owl:allValuesFrom xsd:gMonth
                                                                  ] ,
                                                                  [ rdf:type owl:Restriction ;
                                                                    owl:onProperty <http://www.w3.org/2006/time#year> ;
                                                                    owl:allValuesFrom xsd:gYear
                                                                  ] ;
                                                  rdfs:comment "Descripción de fecha y tiempo estructurada con valores separados para los diferentes elementos de un sistema calendario-reloj. El sistema de referencia temporal está fijado al calendario gregoriano, y el rango de las propiedades año, mes, día restringidas a los correspondientes tipos del XML Schema xsd:gYear, xsd:gMonth y xsd:gDay respectivamente."@es ,
                                                               "Description of date and time structured with separate values for the various elements of a calendar-clock system. The temporal reference system is fixed to Gregorian Calendar, and the range of year, month, day properties restricted to corresponding XML Schema types xsd:gYear, xsd:gMonth and xsd:gDay, respectively."@en ;
                                                  rdfs:label "Date-Time description"@en ,
                                                             "descripción de fecha-tiempo"@es ;
                                                  <http://www.w3.org/2004/02/skos/core#definition> "Descripción de fecha y tiempo estructurada con valores separados para los diferentes elementos de un sistema calendario-reloj. El sistema de referencia temporal está fijado al calendario gregoriano, y el rango de las propiedades año, mes, día restringidas a los correspondientes tipos del XML Schema xsd:gYear, xsd:gMonth y xsd:gDay respectivamente."@es ,
                                                                                                   "Description of date and time structured with separate values for the various elements of a calendar-clock system. The temporal reference system is fixed to Gregorian Calendar, and the range of year, month, day properties restricted to corresponding XML Schema types xsd:gYear, xsd:gMonth and xsd:gDay, respectively."@en .


###  http://www.w3.org/2006/time#DateTimeInterval
<http://www.w3.org/2006/time#DateTimeInterval> rdf:type owl:Class ;
                                               rdfs:subClassOf <http://www.w3.org/2006/time#ProperInterval> ;
                                               rdfs:comment "'intervalo de fecha-hora' es una subclase de 'intervalo propio', definida utilizando el multi-elemento 'descripción de fecha-hora'."@es ,
                                                            "DateTimeInterval is a subclass of ProperInterval, defined using the multi-element DateTimeDescription."@en ;
                                               rdfs:label "Date-time interval"@en ,
                                                          "intervalo de fecha-hora"@es ;
                                               <http://www.w3.org/2004/02/skos/core#definition> "'intervalo de fecha-hora' es una subclase de 'intervalo propio', definida utilizando el multi-elemento 'descripción de fecha-hora'."@es ,
                                                                                                "DateTimeInterval is a subclass of ProperInterval, defined using the multi-element DateTimeDescription."@en ;
                                               <http://www.w3.org/2004/02/skos/core#note> "'intervalo de fecha-hora' se puede utilizar sólo para un intervalo cuyos límites coinciden con un elemento de fecha-hora alineados con el calendario y la zona horaria indicados. Por ejemplo, aunque ambos tienen una duración de un día, el intervalo de 24 horas que empieza en la media noche del comienzo del 8 mayo en Europa Central se puede expresar como un 'intervalo de fecha-hora', el intervalo de 24 horas que empieza a las 1:30pm no."@es ,
                                                                                          ":DateTimeInterval can only be used for an interval whose limits coincide with a date-time element aligned to the calendar and timezone indicated. For example, while both have a duration of one day, the 24-hour interval beginning at midnight at the beginning of 8 May in Central Europe can be expressed as a :DateTimeInterval, but the 24-hour interval starting at 1:30pm cannot."@en .


###  http://www.w3.org/2006/time#DayOfWeek
<http://www.w3.org/2006/time#DayOfWeek> rdf:type owl:Class ;
                                        rdfs:subClassOf owl:Thing ;
                                        rdfs:comment "El día de la semana"@es ,
                                                     "The day of week"@en ;
                                        rdfs:label "Day of week"@en ,
                                                   "día de la semana"@es ;
                                        <http://www.w3.org/2004/02/skos/core#changeNote> """Remove enumeration from definition, in order to allow other days to be used when required in other calendars. 
NOTE: existing days are still present as members of the class, but the class membership is now open. 

In the original OWL-Time the following constraint appeared: 
  owl:oneOf (
      time:Monday
      time:Tuesday
      time:Wednesday
      time:Thursday
      time:Friday
      time:Saturday
      time:Sunday
    ) ;"""@en ;
                                        <http://www.w3.org/2004/02/skos/core#definition> "El día de la semana"@es ,
                                                                                         "The day of week"@en ;
                                        <http://www.w3.org/2004/02/skos/core#note> "La pertenencia a la clase 'día de la semana' está abierta, para permitir longitudes de semana alternativas y diferentes nombres de días."@es ,
                                                                                   "Membership of the class :DayOfWeek is open, to allow for alternative week lengths and different day names."@en .


###  http://www.w3.org/2006/time#Duration
<http://www.w3.org/2006/time#Duration> rdf:type owl:Class ;
                                       rdfs:subClassOf <http://www.w3.org/2006/time#TemporalDuration> ,
                                                       [ rdf:type owl:Restriction ;
                                                         owl:onProperty <http://www.w3.org/2006/time#unitType> ;
                                                         owl:cardinality "1"^^xsd:nonNegativeInteger
                                                       ] ,
                                                       [ rdf:type owl:Restriction ;
                                                         owl:onProperty <http://www.w3.org/2006/time#numericDuration> ;
                                                         owl:cardinality "1"^^xsd:nonNegativeInteger
                                                       ] ;
                                       rdfs:comment "Duración de una extensión temporal expresada como un número escalado por una unidad temporal."@es ,
                                                    "Duration of a temporal extent expressed as a number scaled by a temporal unit"@en ;
                                       rdfs:label "Time duration"@en ,
                                                  "duración de tiempo" ;
                                       <http://www.w3.org/2004/02/skos/core#definition> "Duración de una extensión temporal expresada como un número escalado por una unidad temporal."@es ,
                                                                                        "Duration of a temporal extent expressed as a number scaled by a temporal unit"@en ;
                                       <http://www.w3.org/2004/02/skos/core#note> "Alternativa a 'descripción de tiempo' para proporcionar descripción soporte a una duración temporal diferente a utilizar un sistema de calendario/reloj."@es ,
                                                                                  "Alternative to time:DurationDescription to support description of a temporal duration other than using a calendar/clock system."@en .


###  http://www.w3.org/2006/time#DurationDescription
<http://www.w3.org/2006/time#DurationDescription> rdf:type owl:Class ;
                                                  rdfs:subClassOf <http://www.w3.org/2006/time#GeneralDurationDescription> ,
                                                                  [ rdf:type owl:Restriction ;
                                                                    owl:onProperty <http://www.w3.org/2006/time#days> ;
                                                                    owl:allValuesFrom xsd:decimal
                                                                  ] ,
                                                                  [ rdf:type owl:Restriction ;
                                                                    owl:onProperty <http://www.w3.org/2006/time#hours> ;
                                                                    owl:allValuesFrom xsd:decimal
                                                                  ] ,
                                                                  [ rdf:type owl:Restriction ;
                                                                    owl:onProperty <http://www.w3.org/2006/time#minutes> ;
                                                                    owl:allValuesFrom xsd:decimal
                                                                  ] ,
                                                                  [ rdf:type owl:Restriction ;
                                                                    owl:onProperty <http://www.w3.org/2006/time#months> ;
                                                                    owl:allValuesFrom xsd:decimal
                                                                  ] ,
                                                                  [ rdf:type owl:Restriction ;
                                                                    owl:onProperty <http://www.w3.org/2006/time#seconds> ;
                                                                    owl:allValuesFrom xsd:decimal
                                                                  ] ,
                                                                  [ rdf:type owl:Restriction ;
                                                                    owl:onProperty <http://www.w3.org/2006/time#weeks> ;
                                                                    owl:allValuesFrom xsd:decimal
                                                                  ] ,
                                                                  [ rdf:type owl:Restriction ;
                                                                    owl:onProperty <http://www.w3.org/2006/time#years> ;
                                                                    owl:allValuesFrom xsd:decimal
                                                                  ] ;
                                                  rdfs:comment "Descripción de extensión temporal estructurada con valores separados para los distintos elementos de un sistema de horario-calendario. El sistema de referencia temporal se fija al calendario gregoriano, y el intervalo de cada una de las propiedades numéricas se restringe a xsd:decimal."@es ,
                                                               "Description of temporal extent structured with separate values for the various elements of a calendar-clock system. The temporal reference system is fixed to Gregorian Calendar, and the range of each of the numeric properties is restricted to xsd:decimal"@en ;
                                                  rdfs:label "Duration description"@en ,
                                                             "descripción de duración"@es ;
                                                  <http://www.w3.org/2004/02/skos/core#definition> "Descripción de extensión temporal estructurada con valores separados para los distintos elementos de un sistema de horario-calendario. El sistema de referencia temporal se fija al calendario gregoriano, y el intervalo de cada una de las propiedades numéricas se restringe a xsd:decimal."@es ,
                                                                                                   "Description of temporal extent structured with separate values for the various elements of a calendar-clock system. The temporal reference system is fixed to Gregorian Calendar, and the range of each of the numeric properties is restricted to xsd:decimal"@en ;
                                                  <http://www.w3.org/2004/02/skos/core#note> "En el calendario gregoriano la longitud de los meses no es fija. Por lo tanto, un valor como \"2,5 meses\" no se puede comparar exactamente con una duración similar expresada en términos de semanas o días."@es ,
                                                                                             "In the Gregorian calendar the length of the month is not fixed. Therefore, a value like \"2.5 months\" cannot be exactly compared with a similar duration expressed in terms of weeks or days."@en .


###  http://www.w3.org/2006/time#GeneralDateTimeDescription
<http://www.w3.org/2006/time#GeneralDateTimeDescription> rdf:type owl:Class ;
                                                         rdfs:subClassOf <http://www.w3.org/2006/time#TemporalPosition> ,
                                                                         [ rdf:type owl:Restriction ;
                                                                           owl:onProperty <http://www.w3.org/2006/time#unitType> ;
                                                                           owl:cardinality "1"^^xsd:nonNegativeInteger
                                                                         ] ,
                                                                         [ rdf:type owl:Restriction ;
                                                                           owl:onProperty <http://www.w3.org/2006/time#dayOfWeek> ;
                                                                           owl:maxCardinality "1"^^xsd:nonNegativeInteger
                                                                         ] ,
                                                                         [ rdf:type owl:Restriction ;
                                                                           owl:onProperty <http://www.w3.org/2006/time#monthOfYear> ;
                                                                           owl:maxCardinality "1"^^xsd:nonNegativeInteger
                                                                         ] ,
                                                                         [ rdf:type owl:Restriction ;
                                                                           owl:onProperty <http://www.w3.org/2006/time#timeZone> ;
                                                                           owl:maxCardinality "1"^^xsd:nonNegativeInteger
                                                                         ] ,
                                                                         [ rdf:type owl:Restriction ;
                                                                           owl:onProperty <http://www.w3.org/2006/time#day> ;
                                                                           owl:maxCardinality "1"^^xsd:nonNegativeInteger
                                                                         ] ,
                                                                         [ rdf:type owl:Restriction ;
                                                                           owl:onProperty <http://www.w3.org/2006/time#dayOfYear> ;
                                                                           owl:maxCardinality "1"^^xsd:nonNegativeInteger
                                                                         ] ,
                                                                         [ rdf:type owl:Restriction ;
                                                                           owl:onProperty <http://www.w3.org/2006/time#hour> ;
                                                                           owl:maxCardinality "1"^^xsd:nonNegativeInteger
                                                                         ] ,
                                                                         [ rdf:type owl:Restriction ;
                                                                           owl:onProperty <http://www.w3.org/2006/time#minute> ;
                                                                           owl:maxCardinality "1"^^xsd:nonNegativeInteger
                                                                         ] ,
                                                                         [ rdf:type owl:Restriction ;
                                                                           owl:onProperty <http://www.w3.org/2006/time#month> ;
                                                                           owl:maxCardinality "1"^^xsd:nonNegativeInteger
                                                                         ] ,
                                                                         [ rdf:type owl:Restriction ;
                                                                           owl:onProperty <http://www.w3.org/2006/time#second> ;
                                                                           owl:maxCardinality "1"^^xsd:nonNegativeInteger
                                                                         ] ,
                                                                         [ rdf:type owl:Restriction ;
                                                                           owl:onProperty <http://www.w3.org/2006/time#week> ;
                                                                           owl:maxCardinality "1"^^xsd:nonNegativeInteger
                                                                         ] ,
                                                                         [ rdf:type owl:Restriction ;
                                                                           owl:onProperty <http://www.w3.org/2006/time#year> ;
                                                                           owl:maxCardinality "1"^^xsd:nonNegativeInteger
                                                                         ] ;
                                                         rdfs:comment "Descripción de fecha y hora estructurada con valores separados para los distintos elementos de un sistema calendario-reloj."@es ,
                                                                      "Description of date and time structured with separate values for the various elements of a calendar-clock system"@en ;
                                                         rdfs:label "Generalized date-time description"@en ,
                                                                    "descripción de fecha-hora generalizada"@es ;
                                                         <http://www.w3.org/2004/02/skos/core#definition> "Description of date and time structured with separate values for the various elements of a calendar-clock system"@en ,
                                                                                                          "Descripción de fecha y hora estructurada con valores separados para los distintos elementos de un sistema calendario-reloj." ;
                                                         <http://www.w3.org/2004/02/skos/core#note> "Algunas combinaciones de propiedades son redundantes - por ejemplo, dentro de un 'año' especificado si se proporciona 'día del año' entonces 'día' y 'mes' se pueden computar, y viceversa. Los valores individuales deberían ser consistentes entre ellos y con el calendario, indicado a través del valor de la propiedad 'tiene TRS'."@es ,
                                                                                                    "Some combinations of properties are redundant - for example, within a specified :year if :dayOfYear is provided then :day and :month can be computed, and vice versa. Individual values should be consistent with each other and the calendar, indicated through the value of the :hasTRS property." .


###  http://www.w3.org/2006/time#GeneralDurationDescription
<http://www.w3.org/2006/time#GeneralDurationDescription> rdf:type owl:Class ;
                                                         rdfs:subClassOf <http://www.w3.org/2006/time#TemporalDuration> ,
                                                                         [ rdf:type owl:Restriction ;
                                                                           owl:onProperty <http://www.w3.org/2006/time#hasTRS> ;
                                                                           owl:cardinality "1"^^xsd:nonNegativeInteger
                                                                         ] ,
                                                                         [ rdf:type owl:Restriction ;
                                                                           owl:onProperty <http://www.w3.org/2006/time#days> ;
                                                                           owl:maxCardinality "1"^^xsd:nonNegativeInteger
                                                                         ] ,
                                                                         [ rdf:type owl:Restriction ;
                                                                           owl:onProperty <http://www.w3.org/2006/time#hours> ;
                                                                           owl:maxCardinality "1"^^xsd:nonNegativeInteger
                                                                         ] ,
                                                                         [ rdf:type owl:Restriction ;
                                                                           owl:onProperty <http://www.w3.org/2006/time#minutes> ;
                                                                           owl:maxCardinality "1"^^xsd:nonNegativeInteger
                                                                         ] ,
                                                                         [ rdf:type owl:Restriction ;
                                                                           owl:onProperty <http://www.w3.org/2006/time#months> ;
                                                                           owl:maxCardinality "1"^^xsd:nonNegativeInteger
                                                                         ] ,
                                                                         [ rdf:type owl:Restriction ;
                                                                           owl:onProperty <http://www.w3.org/2006/time#seconds> ;
                                                                           owl:maxCardinality "1"^^xsd:nonNegativeInteger
                                                                         ] ,
                                                                         [ rdf:type owl:Restriction ;
                                                                           owl:onProperty <http://www.w3.org/2006/time#weeks> ;
                                                                           owl:maxCardinality "1"^^xsd:nonNegativeInteger
                                                                         ] ,
                                                                         [ rdf:type owl:Restriction ;
                                                                           owl:onProperty <http://www.w3.org/2006/time#years> ;
                                                                           owl:maxCardinality "1"^^xsd:nonNegativeInteger
                                                                         ] ;
                                                         rdfs:comment "Descripción de extensión temporal estructurada con valores separados para los distintos elementos de un sistema de horario-calendario."@es ,
                                                                      "Description of temporal extent structured with separate values for the various elements of a calendar-clock system."@en ;
                                                         rdfs:label "Generalized duration description"@en ,
                                                                    "descripción de duración generalizada"@es ;
                                                         <http://www.w3.org/2004/02/skos/core#definition> "Descripción de extensión temporal estructurada con valores separados para los distintos elementos de un sistema de horario-calendario."@es ,
                                                                                                          "Description of temporal extent structured with separate values for the various elements of a calendar-clock system."@en ;
                                                         <http://www.w3.org/2004/02/skos/core#note> "La extensión de una duración de tiempo expresada como una 'descripción de duración general' depende del Sistema de Referencia Temporal. En algunos calendarios la longitud de la semana o del mes no es constante a lo largo del año. Por tanto, un valor como \"25 meses\" puede no ser necesariamente ser comparado con un duración similar expresada en términos de semanas o días. Cuando se consideran calendarios que no están basados en el movimiento de la Tierra, se deben tomar incluso más precauciones en la comparación de duraciones."@es ,
                                                                                                    "The extent of a time duration expressed as a GeneralDurationDescription depends on the Temporal Reference System. In some calendars the length of the week or month is not constant within the year. Therefore, a value like \"2.5 months\" may not necessarily be exactly compared with a similar duration expressed in terms of weeks or days. When non-earth-based calendars are considered even more care must be taken in comparing durations."@en .


###  http://www.w3.org/2006/time#Instant
<http://www.w3.org/2006/time#Instant> rdf:type owl:Class ;
                                      rdfs:subClassOf <http://purl.org/nemo/gufo#AbstractEntity> ,
                                                      <http://www.w3.org/2006/time#TemporalEntity> ;
                                      owl:disjointWith <http://www.w3.org/2006/time#ProperInterval> ;
                                      rdfs:comment "A temporal entity with zero extent or duration"@en ,
                                                   "An gufo:AbstractIndividual that reifies time instants. It is used as a target of the gufo:hasBeginPoint and gufo:hasEndPoint object properties."@en ,
                                                   "Una entidad temporal con una extensión o duración cero."@es ;
                                      rdfs:label "Instant"@en ,
                                                 "Time instant"@en ,
                                                 "instante de tiempo."@es ;
                                      <http://www.w3.org/2004/02/skos/core#definition> "A temporal entity with zero extent or duration"@en ,
                                                                                       "Una entidad temporal con una extensión o duración cero."@es .


###  http://www.w3.org/2006/time#Interval
<http://www.w3.org/2006/time#Interval> rdf:type owl:Class ;
                                       rdfs:subClassOf <http://www.w3.org/2006/time#TemporalEntity> ;
                                       rdfs:comment "A temporal entity with an extent or duration"@en ,
                                                    "Una entidad temporal con una extensión o duración."@es ;
                                       rdfs:label "Time interval"@en ,
                                                  "intervalo de tiempo"@es ;
                                       <http://www.w3.org/2004/02/skos/core#definition> "A temporal entity with an extent or duration"@en ,
                                                                                        "Una entidad temporal con una extensión o duración."@es .


###  http://www.w3.org/2006/time#MonthOfYear
<http://www.w3.org/2006/time#MonthOfYear> rdf:type owl:Class ;
                                          rdfs:subClassOf <http://www.w3.org/2006/time#DateTimeDescription> ,
                                                          [ rdf:type owl:Restriction ;
                                                            owl:onProperty <http://www.w3.org/2006/time#unitType> ;
                                                            owl:hasValue <http://www.w3.org/2006/time#unitMonth>
                                                          ] ,
                                                          [ rdf:type owl:Restriction ;
                                                            owl:onProperty <http://www.w3.org/2006/time#day> ;
                                                            owl:cardinality "0"^^xsd:nonNegativeInteger
                                                          ] ,
                                                          [ rdf:type owl:Restriction ;
                                                            owl:onProperty <http://www.w3.org/2006/time#hour> ;
                                                            owl:cardinality "0"^^xsd:nonNegativeInteger
                                                          ] ,
                                                          [ rdf:type owl:Restriction ;
                                                            owl:onProperty <http://www.w3.org/2006/time#minute> ;
                                                            owl:cardinality "0"^^xsd:nonNegativeInteger
                                                          ] ,
                                                          [ rdf:type owl:Restriction ;
                                                            owl:onProperty <http://www.w3.org/2006/time#month> ;
                                                            owl:cardinality "1"^^xsd:nonNegativeInteger
                                                          ] ,
                                                          [ rdf:type owl:Restriction ;
                                                            owl:onProperty <http://www.w3.org/2006/time#second> ;
                                                            owl:cardinality "0"^^xsd:nonNegativeInteger
                                                          ] ,
                                                          [ rdf:type owl:Restriction ;
                                                            owl:onProperty <http://www.w3.org/2006/time#week> ;
                                                            owl:cardinality "0"^^xsd:nonNegativeInteger
                                                          ] ,
                                                          [ rdf:type owl:Restriction ;
                                                            owl:onProperty <http://www.w3.org/2006/time#year> ;
                                                            owl:cardinality "0"^^xsd:nonNegativeInteger
                                                          ] ;
                                          rdfs:comment "El mes del año."@es ,
                                                       "The month of the year"@en ;
                                          rdfs:label "Month of year"@en ,
                                                     "mes del año"@es ;
                                          <http://www.w3.org/2004/02/skos/core#definition> "El mes del año."@es ,
                                                                                           "The month of the year"@en ;
                                          <http://www.w3.org/2004/02/skos/core#editorialNote> "Característica en riesgo - añadida en la revisión de 2017, y no utilizada todavía de forma amplia."@es ,
                                                                                              "Feature at risk - added in 2017 revision, and not yet widely used. "@en ;
                                          <http://www.w3.org/2004/02/skos/core#note> "La pertenencia a la clase 'mes del año' está abierta, a permitir calendarios anuales alternativos y diferentes nombres de meses."@es ,
                                                                                     "Membership of the class :MonthOfYear is open, to allow for alternative annual calendars and different month names."@en .


###  http://www.w3.org/2006/time#ProperInterval
<http://www.w3.org/2006/time#ProperInterval> rdf:type owl:Class ;
                                             rdfs:subClassOf <http://www.w3.org/2006/time#Interval> ;
                                             rdfs:comment "A temporal entity with non-zero extent or duration, i.e. for which the value of the beginning and end are different"@en ,
                                                          "Una entidad temporal con extensión o duración distinta de cero, es decir, para la cual los valores de principio y fin del intervalo son diferentes."@es ;
                                             rdfs:label "Proper interval"@en ,
                                                        "intervalo propio"@es ;
                                             <http://www.w3.org/2004/02/skos/core#definition> "A temporal entity with non-zero extent or duration, i.e. for which the value of the beginning and end are different"@en ,
                                                                                              "Una entidad temporal con extensión o duración distinta de cero, es decir, para la cual los valores de principio y fin del intervalo son diferentes."@es .


###  http://www.w3.org/2006/time#TRS
<http://www.w3.org/2006/time#TRS> rdf:type owl:Class ;
                                  rdfs:comment """A temporal reference system, such as a temporal coordinate system (with an origin, direction, and scale), a calendar-clock combination, or a (possibly hierarchical) ordinal system. 

This is a stub class, representing the set of all temporal reference systems."""@en ,
                                               """Un sistema de referencia temporal, tal como un sistema de coordenadas temporales (con un origen, una dirección y una escala), una combinación calendario-reloj, o un sistema ordinal (posiblemente jerárquico).
        Esta clase comodín representa el conjunto de todos los sistemas de referencia temporal."""@es ;
                                  rdfs:label "Temporal Reference System"@en ,
                                             "sistema de referencia temporal"@es ;
                                  <http://www.w3.org/2004/02/skos/core#definition> """A temporal reference system, such as a temporal coordinate system (with an origin, direction, and scale), a calendar-clock combination, or a (possibly hierarchical) ordinal system. 

This is a stub class, representing the set of all temporal reference systems."""@en ,
                                                                                   """Un sistema de referencia temporal, tal como un sistema de coordenadas temporales (con un origen, una dirección y una escala), una combinación calendario-reloj, o un sistema ordinal (posiblemente jerárquico).
    Esta clase comodín representa el conjunto de todos los sistemas de referencia temporal."""@es ;
                                  <http://www.w3.org/2004/02/skos/core#note> "A taxonomy of temporal reference systems is provided in ISO 19108:2002 [ISO19108], including (a) calendar + clock systems; (b) temporal coordinate systems (i.e. numeric offset from an epoch); (c) temporal ordinal reference systems (i.e. ordered sequence of named intervals, not necessarily of equal duration)."@en ,
                                                                             "En el ISO 19108:2002 [ISO19108] se proporciona una taxonomía de sistemas de referencia temporal, incluyendo (a) sistemas de calendario + reloj; (b) sistemas de coordenadas temporales (es decir, desplazamiento numérico a partir de una época); (c) sistemas de referencia ordinales temporales (es decir, secuencia ordenada de intervalos nombrados, no necesariamente de igual duración)."@es .


###  http://www.w3.org/2006/time#TemporalDuration
<http://www.w3.org/2006/time#TemporalDuration> rdf:type owl:Class ;
                                               rdfs:comment "Extensión de tiempo; duración de un intervalo de tiempo independiente de su posición de inicio particular."@es ,
                                                            "Time extent; duration of a time interval separate from its particular start position"@en ;
                                               rdfs:label "Temporal duration"@en ,
                                                          "duración temporal"@es ;
                                               <http://www.w3.org/2004/02/skos/core#definition> "Extensión de tiempo; duración de un intervalo de tiempo independiente de su posición de inicio particular."@es ,
                                                                                                "Time extent; duration of a time interval separate from its particular start position"@en .


###  http://www.w3.org/2006/time#TemporalEntity
<http://www.w3.org/2006/time#TemporalEntity> rdf:type owl:Class ;
                                             owl:equivalentClass [ rdf:type owl:Class ;
                                                                   owl:unionOf ( <http://www.w3.org/2006/time#Instant>
                                                                                 <http://www.w3.org/2006/time#Interval>
                                                                               )
                                                                 ] ;
                                             rdfs:subClassOf owl:Thing ;
                                             rdfs:comment "A temporal interval or instant."@en ,
                                                          "Un intervalo temporal o un instante."@es ;
                                             rdfs:label "Temporal entity"@en ,
                                                        "entidad temporal"@es ;
                                             <http://www.w3.org/2004/02/skos/core#definition> "A temporal interval or instant."@en ,
                                                                                              "Un intervalo temporal o un instante."@es .


###  http://www.w3.org/2006/time#TemporalPosition
<http://www.w3.org/2006/time#TemporalPosition> rdf:type owl:Class ;
                                               rdfs:subClassOf [ rdf:type owl:Restriction ;
                                                                 owl:onProperty <http://www.w3.org/2006/time#hasTRS> ;
                                                                 owl:cardinality "1"^^xsd:nonNegativeInteger
                                                               ] ;
                                               rdfs:comment "A position on a time-line"@en ,
                                                            "Una posición sobre una línea de tiempo."@es ;
                                               rdfs:label "Temporal position"@en ,
                                                          "posición temporal"@es ;
                                               <http://www.w3.org/2004/02/skos/core#definition> "A position on a time-line"@en ,
                                                                                                "Una posición sobre una línea de tiempo."@es .


###  http://www.w3.org/2006/time#TemporalUnit
<http://www.w3.org/2006/time#TemporalUnit> rdf:type owl:Class ;
                                           rdfs:subClassOf <http://www.w3.org/2006/time#TemporalDuration> ;
                                           rdfs:comment "A standard duration, which provides a scale factor for a time extent, or the granularity or precision for a time position."@en ,
                                                        "Una duración estándar, que proporciona un factor de escala para una extensión de tiempo, o la granularidad o precisión para una posición de tiempo."@es ;
                                           rdfs:label "Temporal unit"@en ,
                                                      "unidad de tiempo"@es ;
                                           <http://www.w3.org/2004/02/skos/core#changeNote> """Remove enumeration from definition, in order to allow other units to be used when required in other coordinate systems. 
NOTE: existing units are still present as members of the class, but the class membership is now open. 

In the original OWL-Time the following constraint appeared: 
  owl:oneOf (
      time:unitSecond
      time:unitMinute
      time:unitHour
      time:unitDay
      time:unitWeek
      time:unitMonth
      time:unitYear
    ) ;"""@en ;
                                           <http://www.w3.org/2004/02/skos/core#definition> "A standard duration, which provides a scale factor for a time extent, or the granularity or precision for a time position."@en ,
                                                                                            "Una duración estándar, que proporciona un factor de escala para una extensión de tiempo, o la granularidad o precisión para una posición de tiempo."@es ;
                                           <http://www.w3.org/2004/02/skos/core#note> "La pertenencia de la clase 'unidad de tiempo' está abierta, para permitir otras unidades de tiempo utilizadas en algunas aplicaciones técnicas (por ejemplo, millones de años o el mes Baha'i)."@es ,
                                                                                      "Membership of the class TemporalUnit is open, to allow for other temporal units used in some technical applications (e.g. millions of years, Baha'i month)."@en .


###  http://www.w3.org/2006/time#TimePosition
<http://www.w3.org/2006/time#TimePosition> rdf:type owl:Class ;
                                           rdfs:subClassOf <http://www.w3.org/2006/time#TemporalPosition> ,
                                                           [ rdf:type owl:Class ;
                                                             owl:unionOf ( [ rdf:type owl:Restriction ;
                                                                             owl:onProperty <http://www.w3.org/2006/time#nominalPosition> ;
                                                                             owl:cardinality "1"^^xsd:nonNegativeInteger
                                                                           ]
                                                                           [ rdf:type owl:Restriction ;
                                                                             owl:onProperty <http://www.w3.org/2006/time#numericPosition> ;
                                                                             owl:cardinality "1"^^xsd:nonNegativeInteger
                                                                           ]
                                                                         )
                                                           ] ;
                                           rdfs:comment "A temporal position described using either a (nominal) value from an ordinal reference system, or a (numeric) value in a temporal coordinate system. "@en ,
                                                        "Una posición temporal descrita utilizando bien un valor (nominal) de un sistema de referencia ordinal, o un valor (numérico) en un sistema de coordenadas temporales."@es ;
                                           rdfs:label "Time position"@en ,
                                                      "posición de tiempo"@es ;
                                           <http://www.w3.org/2004/02/skos/core#definition> "A temporal position described using either a (nominal) value from an ordinal reference system, or a (numeric) value in a temporal coordinate system. "@en ,
                                                                                            "Una posición temporal descrita utilizando bien un valor (nominal) de un sistema de referencia ordinal, o un valor (numérico) en un sistema de coordenadas temporales."@es .


###  http://www.w3.org/2006/time#TimeZone
<http://www.w3.org/2006/time#TimeZone> rdf:type owl:Class ;
                                       rdfs:comment """A Time Zone specifies the amount by which the local time is offset from UTC. 
	A time zone is usually denoted geographically (e.g. Australian Eastern Daylight Time), with a constant value in a given region. 
The region where it applies and the offset from UTC are specified by a locally recognised governing authority."""@en ,
                                                    """Un huso horario especifica la cantidad en que la hora local está desplazada con respecto a UTC.
        Un huso horario normalmente se denota geográficamente (p.ej. el horario de verano del este de Australia), con un valor constante en una región dada.
        La región donde aplica y el desplazamiento desde UTC las especifica una autoridad gubernamental localmente reconocida."""@es ;
                                       rdfs:label "Time Zone"@en ,
                                                  "huso horario"@es ;
                                       <http://www.w3.org/2004/02/skos/core#definition> """A Time Zone specifies the amount by which the local time is offset from UTC. 
	A time zone is usually denoted geographically (e.g. Australian Eastern Daylight Time), with a constant value in a given region. 
The region where it applies and the offset from UTC are specified by a locally recognised governing authority."""@en ,
                                                                                        """Un huso horario especifica la cantidad en que la hora local está desplazada con respecto a UTC.
    Un huso horario normalmente se denota geográficamente (p.ej. el horario de verano del este de Australia), con un valor constante en una región dada.
    La región donde aplica y el desplazamiento desde UTC las especifica una autoridad gubernamental localmente reconocida."""@es ;
                                       <http://www.w3.org/2004/02/skos/core#historyNote> """En la versión original de OWL-Time de 2006, se definió, en un espacio de nombres diferente \"http://www.w3.org/2006/timezone#\", la clase 'huso horario', con varias propiedades específicas correspondientes a un modelo específico de huso horario.
    En la versión actual hay una clase con el mismo nombre local en el espacio de nombres de OWL-Time, eliminando la dependencia del espacio de nombres externo.
    Un axioma de alineación permite que los datos codificados de acuerdo con la versión anterior sean consistentes con la ontología actualizada."""@es ,
                                                                                         """In the original 2006 version of OWL-Time, the TimeZone class, with several properties corresponding to a specific model of time-zones, was defined in a separate namespace \"http://www.w3.org/2006/timezone#\". 

In the current version a class with same local name is put into the main OWL-Time namespace, removing the dependency on the external namespace. 

An alignment axiom 
	tzont:TimeZone rdfs:subClassOf time:TimeZone . 
allows data encoded according to the previous version to be consistent with the updated ontology. """ ;
                                       <http://www.w3.org/2004/02/skos/core#note> """A designated timezone is associated with a geographic region. However, for a particular region the offset from UTC often varies seasonally, and the dates of the changes may vary from year to year. The timezone designation usually changes for the different seasons (e.g. Australian Eastern Standard Time vs. Australian Eastern Daylight Time). Furthermore, the offset for a timezone may change over longer timescales, though its designation might not.  

Detailed guidance about working with time zones is given in http://www.w3.org/TR/timezone/ ."""@en ,
                                                                                  "An ontology for time zone descriptions was described in [owl-time-20060927] and provided as RDF in a separate namespace tzont:. However, that ontology was incomplete in scope, and the example datasets were selective. Furthermore, since the use of a class from an external ontology as the range of an ObjectProperty in OWL-Time creates a dependency, reference to the time zone class has been replaced with the 'stub' class in the normative part of this version of OWL-Time."@en ,
                                                                                  """Un huso horario designado está asociado con una región geográfica. Sin embargo, para una región particular el desplazamiento desde UTC a menudo varía según las estaciones, y las fechas de los cambios pueden variar de un año a otro. La designación de huso horario  normalmente cambia de una estación a otra (por ejemplo, el horario estándar frente al horario de verano ambos del este de Australia). Además, del desplazamiento para un huso horario puede cambiar sobre escalas de tiempo mayores, aunque su designación no lo haga.
    Se puede encontrar una guía detallada sobre el funcionamiento de husos horarios en http://www.w3.org/TR/timezone/.\"@es , \"En [owl-time-20060927] se describió una ontología para descripciones de husos horarios, y se proporcionó en un espacio de nombres separado tzont:. Sin embargo, dicha ontología estaba incompleta en su alcance, y el ejemplo de conjuntos de datos (datasets) era selectivo. Además, puesto que el uso de una clase de una ontología externa como el rango de una propiedad de objeto en OWL-Time crea una dependencia, la referencia a la clase huso horario se ha reemplazado por una clase que viene a ser un \"cajón de sastre\" en la en la parte normativa de esta versión de OWL-Time."""@es ;
                                       <http://www.w3.org/2004/02/skos/core#scopeNote> "En esta implementación 'huso horario' no tiene definidas propiedades. Se debería pensar como una superclase \"abstracta\" de todas las implementaciones de huso horario específicas."@es ,
                                                                                       "In this implementation TimeZone has no properties defined. It should be thought of as an 'abstract' superclass of all specific timezone implementations." .


###  http://www.w3.org/2006/time#Year
<http://www.w3.org/2006/time#Year> rdf:type owl:Class ;
                                   rdfs:subClassOf <http://www.w3.org/2006/time#DurationDescription> ,
                                                   [ rdf:type owl:Restriction ;
                                                     owl:onProperty <http://www.w3.org/2006/time#days> ;
                                                     owl:cardinality "0"^^xsd:nonNegativeInteger
                                                   ] ,
                                                   [ rdf:type owl:Restriction ;
                                                     owl:onProperty <http://www.w3.org/2006/time#hours> ;
                                                     owl:cardinality "0"^^xsd:nonNegativeInteger
                                                   ] ,
                                                   [ rdf:type owl:Restriction ;
                                                     owl:onProperty <http://www.w3.org/2006/time#minutes> ;
                                                     owl:cardinality "0"^^xsd:nonNegativeInteger
                                                   ] ,
                                                   [ rdf:type owl:Restriction ;
                                                     owl:onProperty <http://www.w3.org/2006/time#months> ;
                                                     owl:cardinality "0"^^xsd:nonNegativeInteger
                                                   ] ,
                                                   [ rdf:type owl:Restriction ;
                                                     owl:onProperty <http://www.w3.org/2006/time#seconds> ;
                                                     owl:cardinality "0"^^xsd:nonNegativeInteger
                                                   ] ,
                                                   [ rdf:type owl:Restriction ;
                                                     owl:onProperty <http://www.w3.org/2006/time#weeks> ;
                                                     owl:cardinality "0"^^xsd:nonNegativeInteger
                                                   ] ,
                                                   [ rdf:type owl:Restriction ;
                                                     owl:onProperty <http://www.w3.org/2006/time#years> ;
                                                     owl:cardinality "1"^^xsd:nonNegativeInteger
                                                   ] ;
                                   rdfs:comment "Year duration" ;
                                   rdfs:label "Year"@en ;
                                   owl:deprecated "true"^^xsd:boolean ;
                                   <http://www.w3.org/2004/02/skos/core#definition> "Year duration" ;
                                   <http://www.w3.org/2004/02/skos/core#historyNote> """Year was proposed in the 2006 version of OWL-Time as an example of how DurationDescription could be specialized to allow for a duration to be restricted to a number of years. 

It is deprecated in this edition of OWL-Time. """ ;
                                   <http://www.w3.org/2004/02/skos/core#prefLabel> "Anno"@it ,
                                                                                   "Année (calendrier)"@fr ,
                                                                                   "Ano"@pt ,
                                                                                   "Año"@es ,
                                                                                   "Jaar"@nl ,
                                                                                   "Jahr"@de ,
                                                                                   "Rok"@pl ,
                                                                                   "Year"@en ,
                                                                                   "Год"@ru ,
                                                                                   "سنة"@ar ,
                                                                                   "年"@ja ,
                                                                                   "年"@zh .


###  https://w3id.org/def/phenowl#Observation
:Observation rdf:type owl:Class ;
             rdfs:subClassOf <http://purl.org/nemo/gufo#Perdurants> ;
             rdfs:comment """As a propagation phenomenon is still a general phenomenon (\"
            Smith, David Woodruff. « Phenomenology ». The Stanford Encyclopedia of Philosophy, édité par Edward N. Zalta, Summer 2018, Metaphysics Research Lab, Stanford University, 2018. Stanford Encyclopedia of Philosophy, https://plato.stanford.edu/archives/sum2018/entries/phenomenology/.
            \"), different points of view or observations may result in different experiences. A phen:Observation is a gufo:Perdurant that represents a spatial-temporal perspective of a phen:PhenomenonOccurrence (i.e., two observations from different people may differ in the number of details one can give).

            In practice, a phen:Observation may be used to identify what gufo:Individual are participating in a phen:PhenomenonOccurrence for a given node of the network for a given time interval.

            As phen:Observation designs a spatial-temporal cluster itself, it can be used to track valid spatial-temporal paths between several pairs of phen:Observation.""" ;
             rdfs:label "Observation of Propagation Phenomenon Occurrence" .


###  https://w3id.org/def/phenowl#Phenomenon
:Phenomenon rdf:type owl:Class ;
            rdfs:subClassOf <http://purl.org/nemo/gufo#Perdurants> ;
            rdfs:comment """It is based on the meaning of the Propagation Phenomenon presented by \"Król, Dariusz, Damien Fay, et Bogdan Gabryś, éd. Propagation Phenomena in Real World Networks. Vol. 85. Intelligent Systems Reference Library. Cham: Springer International Publishing, 2015. https://doi.org/10.1007/978-3-319-15916-4.\"
        A phenomenon is a gufo:Perdurant that defines a fact or event of scientific interest susceptible to scientific description and explanation (Merriam-Webster dictionary). It does not define the occurrence of a phenomenon but the study of a type of it (i.e., Epidemic phenomena such as COVID-19, Influenza, etc.). As the mentioned phenomena, the study of a phenomenon may only be valid from the first occurrence of it until the last occurrence of it.""" ;
            rdfs:label "Propagation Phenomenon Type" .


###  https://w3id.org/def/phenowl#PhenomenonOccurrence
:PhenomenonOccurrence rdf:type owl:Class ;
                      rdfs:subClassOf <http://purl.org/nemo/gufo#Perdurants> ;
                      rdfs:comment """A gufo:Perdurant that represents the occurrence of a phen:Phenomenon. Similar to the concept of the occurrence of information being propagated in the social information propagation phenomenon on \"Król, Dariusz, Damien Fay, et Bogdan Gabryś, éd. Propagation Phenomena in Real World Networks. Vol. 85. Intelligent Systems Reference Library. Cham: Springer International Publishing, 2015. https://doi.org/10.1007/978-3-319-15916-4.\". Another example would be an outburst in a network from a particular virus type.

        For example, the occurrence of a hurricane in Paris is different from the occurrence of a hurricane in the United States if they are happening simultaneously. Therefore, they are two different instances of phen:PhenomenonOccurrence of the same phen:Phenomenon (Hurricane).""" ;
                      rdfs:label "Phenomenon Occurrence" .


###  https://w3id.org/def/phenowl#Presence
:Presence rdf:type owl:Class ;
          rdfs:subClassOf <http://purl.org/nemo/gufo#Perdurants> ;
          rdfs:comment "A gufo:Perdurant whose sole purpose is to identify the presence of instances of gufo:Individual in a node of the network or, consequently, in a phen:Observation for a given time interval." ;
          rdfs:label "Presence of entities in a network node" .


###  https://w3id.org/seas/Connection
<https://w3id.org/seas/Connection> rdf:type owl:Class ;
                                   rdfs:subClassOf <http://purl.org/nemo/gufo#Perdurants> ,
                                                   [ rdf:type owl:Restriction ;
                                                     owl:onProperty <https://w3id.org/seas/connectsSystem> ;
                                                     owl:someValuesFrom <https://w3id.org/seas/System>
                                                   ] ,
                                                   [ rdf:type owl:Restriction ;
                                                     owl:onProperty <https://w3id.org/seas/connectsSystemAt> ;
                                                     owl:someValuesFrom <https://w3id.org/seas/ConnectionPoint>
                                                   ] ;
                                   owl:disjointWith <https://w3id.org/seas/ConnectionPoint> ,
                                                    <https://w3id.org/seas/System> ;
                                   rdfs:comment """The class of connections between systems.

This class qualifies property `seas:connectedTo`. 

A connection describes potential interactions between systems. 

For example, a power connection between power systems describes the fact that these systems may exchange electricity.

```
<connection> seas:connectsSystem <electric_vehicle> , <electric_vehicle_service_equipment> .
<electric_vehicle> seas:connectedThrough <connection> .
<electric_vehicle_service_equipment> seas:connectedThrough <connection> .
```

Any two connected systems are connected through a connection. If:

```
<system1> a seas:System .
<system2> a seas:System .
<system1> seas:connectedTo <system2> .
```

then there exists `_:connection` such that:

```
_:connection seas:connectsSystem <system1> , <system2> .
```

A connection can connect more than two systems at the same time.


Figure below illustrates connections of systems:

[![Connections of systems](https://w3id.org/seas/system2.png)](https://w3id.org/seas/system2.png)

"""@en ;
                                   rdfs:isDefinedBy <https://w3id.org/seas/SystemOntology> ;
                                   rdfs:label "Connection"@en ;
                                   <http://www.w3.org/2003/06/sw-vocab-status/ns#term_status> "stable" .


###  https://w3id.org/seas/ConnectionPoint
<https://w3id.org/seas/ConnectionPoint> rdf:type owl:Class ;
                                        rdfs:subClassOf <http://www.opengis.net/ont/geosparql#Feature> ,
                                                        [ rdf:type owl:Restriction ;
                                                          owl:onProperty <https://w3id.org/seas/connectionPointOf> ;
                                                          owl:cardinality "1"^^xsd:nonNegativeInteger
                                                        ] ;
                                        owl:disjointWith <https://w3id.org/seas/System> ;
                                        rdfs:comment """The class of connection points of systems, at which they may be connected to other systems.

This class qualifies properties `seas:connectsSystem` and `seas:connectedThrough`.

A connection point belongs to exactly one system.


For example, an electric vehicle service equipment may have three power connection points: two different kinds of plugs that enable to charge electric vehicles, and a three phase power bus connection point to the grid:

```
<electric_vehicle> seas:connectsAt <plug_high_voltage> , <normal_plug> , <three_phase_connection_point> .
```


Any system connected through a connection is connected at one of its connection points to the connection:
  if:

```
<system> a seas:System .
<system> seas:connectedThrough <connection> .
<connection> a seas:Connection .
```

  then there exists `_:connectionPoint` such that:

```
<system> seas:connectsAt _:connectionPoint .

_:connectionPoint seas:connectsSystemAt <connection> .
```


The system of a connection point that is connected through a connection is itself connected through the connection:. If:

```
<connection> a seas:Connection .
<system> a seas:System .
<connectionPoint> a seas:ConnectionPoint ;
<connectionPoint> seas:connectsSystemThrough <connection> .
```

then it is true that:

```
<connectionPoint> seas:connectionPointOf <system> .
```

Figure below illustrates connection points of systems:

[![Connection points of systems](https://w3id.org/seas/system3.png)](https://w3id.org/seas/system3.png)

"""@en ;
                                        rdfs:isDefinedBy <https://w3id.org/seas/SystemOntology> ;
                                        rdfs:label "Connection Point"@en ;
                                        <http://www.w3.org/2003/06/sw-vocab-status/ns#term_status> "stable" .


###  https://w3id.org/seas/System
<https://w3id.org/seas/System> rdf:type owl:Class ;
                               rdfs:subClassOf <http://www.opengis.net/ont/geosparql#Feature> ;
                               rdfs:comment """The class of systems, i.e., systems virtually isolated from the environment, whose behaviour and interactions with the environment are modeled.

  Systems can be connected to other systems. Connected systems interact in some ways. For example:

```
<electric_vehicle> seas:connectedTo <electric_vehicle_service_equipment> .
```

  Systems can also have subsystems. Properties of subsystems somehow contribute to the properties of the supersystem. For example:

```
<battery> seas:subSystemOf <electric_vehicle> .
```

Figure below illustrates systems and their connections:

[![Systems and their connections](https://w3id.org/seas/system1.png)](https://w3id.org/seas/system1.png)

"""@en ;
                               rdfs:isDefinedBy <https://w3id.org/seas/SystemOntology> ;
                               rdfs:label "System"@en ;
                               <http://www.w3.org/2003/06/sw-vocab-status/ns#term_status> "stable" .


#################################################################
#    Individuals
#################################################################

###  http://www.w3.org/2006/time#Friday
<http://www.w3.org/2006/time#Friday> rdf:type owl:NamedIndividual ,
                                              <http://www.w3.org/2006/time#DayOfWeek> ;
                                     rdfs:label "Friday"@en ;
                                     <http://www.w3.org/2004/02/skos/core#prefLabel> "Freitag"@de ,
                                                                                     "Friday"@en ,
                                                                                     "Piątek"@pl ,
                                                                                     "Sexta-feira"@pt ,
                                                                                     "Vendredi"@fr ,
                                                                                     "Venerdì"@it ,
                                                                                     "Viernes"@es ,
                                                                                     "Vrijdag"@nl ,
                                                                                     "Пятница"@ru ,
                                                                                     "الجمعة"@ar ,
                                                                                     "星期五"@zh ,
                                                                                     "金曜日"@ja .


###  http://www.w3.org/2006/time#Monday
<http://www.w3.org/2006/time#Monday> rdf:type owl:NamedIndividual ,
                                              <http://www.w3.org/2006/time#DayOfWeek> ;
                                     rdfs:label "Monday"@en ;
                                     <http://www.w3.org/2004/02/skos/core#prefLabel> "Lundi"@fr ,
                                                                                     "Lunedì"@it ,
                                                                                     "Lunes"@es ,
                                                                                     "Maandag"@nl ,
                                                                                     "Monday"@en ,
                                                                                     "Montag"@de ,
                                                                                     "Poniedziałek"@pl ,
                                                                                     "Segunda-feira"@pt ,
                                                                                     "Понедельник"@ru ,
                                                                                     "الاثنين"@ar ,
                                                                                     "星期一"@zh ,
                                                                                     "月曜日"@ja .


###  http://www.w3.org/2006/time#Saturday
<http://www.w3.org/2006/time#Saturday> rdf:type owl:NamedIndividual ,
                                                <http://www.w3.org/2006/time#DayOfWeek> ;
                                       rdfs:label "Saturday"@en ;
                                       <http://www.w3.org/2004/02/skos/core#prefLabel> "Sabato"@it ,
                                                                                       "Samedi"@fr ,
                                                                                       "Samstag"@de ,
                                                                                       "Saturday"@en ,
                                                                                       "Sobota"@pl ,
                                                                                       "Sábado"@es ,
                                                                                       "Sábado"@pt ,
                                                                                       "Zaterdag"@nl ,
                                                                                       "Суббота"@ru ,
                                                                                       "السبت"@ar ,
                                                                                       "土曜日"@ja ,
                                                                                       "星期六"@zh .


###  http://www.w3.org/2006/time#Sunday
<http://www.w3.org/2006/time#Sunday> rdf:type owl:NamedIndividual ,
                                              <http://www.w3.org/2006/time#DayOfWeek> ;
                                     rdfs:label "Sunday"@en ;
                                     <http://www.w3.org/2004/02/skos/core#prefLabel> "Dimanche"@fr ,
                                                                                     "Domenica"@it ,
                                                                                     "Domingo"@es ,
                                                                                     "Domingo"@pt ,
                                                                                     "Niedziela"@pl ,
                                                                                     "Sonntag"@de ,
                                                                                     "Sunday"@en ,
                                                                                     "Zondag"@nl ,
                                                                                     "Воскресенье"@ru ,
                                                                                     "الأحد (يوم)"@ar ,
                                                                                     "日曜日"@ja ,
                                                                                     "星期日"@zh .


###  http://www.w3.org/2006/time#Thursday
<http://www.w3.org/2006/time#Thursday> rdf:type owl:NamedIndividual ,
                                                <http://www.w3.org/2006/time#DayOfWeek> ;
                                       rdfs:label "Thursday"@en ;
                                       <http://www.w3.org/2004/02/skos/core#prefLabel> "Czwartek"@pl ,
                                                                                       "Donderdag"@nl ,
                                                                                       "Donnerstag"@de ,
                                                                                       "Giovedì"@it ,
                                                                                       "Jeudi"@fr ,
                                                                                       "Jueves"@es ,
                                                                                       "Quinta-feira"@pt ,
                                                                                       "Thursday"@en ,
                                                                                       "Четверг"@ru ,
                                                                                       "الخميس"@ar ,
                                                                                       "星期四"@zh ,
                                                                                       "木曜日"@ja .


###  http://www.w3.org/2006/time#Tuesday
<http://www.w3.org/2006/time#Tuesday> rdf:type owl:NamedIndividual ,
                                               <http://www.w3.org/2006/time#DayOfWeek> ;
                                      rdfs:label "Tuesday"@en ;
                                      <http://www.w3.org/2004/02/skos/core#prefLabel> "Dienstag"@de ,
                                                                                      "Dinsdag"@nl ,
                                                                                      "Mardi"@fr ,
                                                                                      "Martedì"@it ,
                                                                                      "Martes"@es ,
                                                                                      "Terça-feira"@pt ,
                                                                                      "Tuesday"@en ,
                                                                                      "Wtorek"@pl ,
                                                                                      "Вторник"@ru ,
                                                                                      "الثلاثاء"@ar ,
                                                                                      "星期二"@zh ,
                                                                                      "火曜日"@ja .


###  http://www.w3.org/2006/time#Wednesday
<http://www.w3.org/2006/time#Wednesday> rdf:type owl:NamedIndividual ,
                                                 <http://www.w3.org/2006/time#DayOfWeek> ;
                                        rdfs:label "Wednesday"@en ;
                                        <http://www.w3.org/2004/02/skos/core#prefLabel> "Mercoledì"@it ,
                                                                                        "Mercredi"@fr ,
                                                                                        "Mittwoch"@de ,
                                                                                        "Miércoles"@es ,
                                                                                        "Quarta-feira"@pt ,
                                                                                        "Wednesday"@en ,
                                                                                        "Woensdag"@nl ,
                                                                                        "Środa"@pl ,
                                                                                        "Среда"@ru ,
                                                                                        "الأربعاء"@ar ,
                                                                                        "星期三"@zh ,
                                                                                        "水曜日"@ja .


###  http://www.w3.org/2006/time#unitCentury
<http://www.w3.org/2006/time#unitCentury> rdf:type owl:NamedIndividual ,
                                                   <http://www.w3.org/2006/time#TemporalUnit> ;
                                          <http://www.w3.org/2006/time#days> 0 ;
                                          <http://www.w3.org/2006/time#hours> 0 ;
                                          <http://www.w3.org/2006/time#minutes> 0 ;
                                          <http://www.w3.org/2006/time#months> 0 ;
                                          <http://www.w3.org/2006/time#seconds> 0 ;
                                          <http://www.w3.org/2006/time#weeks> 0 ;
                                          <http://www.w3.org/2006/time#years> 100 ;
                                          rdfs:label "Century (unit of temporal duration)"@en ;
                                          <http://www.w3.org/2004/02/skos/core#prefLabel> "Jahrhundert"@de ,
                                                                                          "century"@en ,
                                                                                          "eeuw"@nl ,
                                                                                          "secolo"@it ,
                                                                                          "siglo"@es ,
                                                                                          "siècle"@fr ,
                                                                                          "stulecie"@pl ,
                                                                                          "século"@pt ,
                                                                                          "век"@ru ,
                                                                                          "قرن واحد"@ar ,
                                                                                          "一世紀"@ja ,
                                                                                          "一个世纪"@zh ,
                                                                                          "한 세기"@kr .


###  http://www.w3.org/2006/time#unitDay
<http://www.w3.org/2006/time#unitDay> rdf:type owl:NamedIndividual ,
                                               <http://www.w3.org/2006/time#TemporalUnit> ;
                                      <http://www.w3.org/2006/time#days> 1 ;
                                      <http://www.w3.org/2006/time#hours> 0 ;
                                      <http://www.w3.org/2006/time#minutes> 0 ;
                                      <http://www.w3.org/2006/time#months> 0 ;
                                      <http://www.w3.org/2006/time#seconds> 0 ;
                                      <http://www.w3.org/2006/time#weeks> 0 ;
                                      <http://www.w3.org/2006/time#years> 0 ;
                                      rdfs:label "Day (unit of temporal duration)"@en ;
                                      <http://www.w3.org/2004/02/skos/core#prefLabel> "Tag"@de ,
                                                                                      "dag"@nl ,
                                                                                      "day"@en ,
                                                                                      "dia"@pt ,
                                                                                      "doba"@pl ,
                                                                                      "día"@es ,
                                                                                      "giorno"@it ,
                                                                                      "jour"@fr ,
                                                                                      "يوماً ما"@ar ,
                                                                                      "ある日"@ja ,
                                                                                      "一天"@zh ,
                                                                                      "언젠가"@kr .


###  http://www.w3.org/2006/time#unitDecade
<http://www.w3.org/2006/time#unitDecade> rdf:type owl:NamedIndividual ,
                                                  <http://www.w3.org/2006/time#TemporalUnit> ;
                                         <http://www.w3.org/2006/time#days> 0 ;
                                         <http://www.w3.org/2006/time#hours> 0 ;
                                         <http://www.w3.org/2006/time#minutes> 0 ;
                                         <http://www.w3.org/2006/time#months> 0 ;
                                         <http://www.w3.org/2006/time#seconds> 0 ;
                                         <http://www.w3.org/2006/time#weeks> 0 ;
                                         <http://www.w3.org/2006/time#years> 10 ;
                                         rdfs:label "Decade (unit of temporal duration)"@en ;
                                         <http://www.w3.org/2004/02/skos/core#prefLabel> "1 열개의"@kr ,
                                                                                         "10年"@ja ,
                                                                                         "Dekade"@de ,
                                                                                         "decade"@en ,
                                                                                         "decennio"@it ,
                                                                                         "decennium"@nl ,
                                                                                         "dekada"@pl ,
                                                                                         "década"@pt ,
                                                                                         "décennie"@fr ,
                                                                                         "una década"@es ,
                                                                                         "одно десятилетие"@ru ,
                                                                                         "عقد واحد"@ar ,
                                                                                         "十年"@zh .


###  http://www.w3.org/2006/time#unitHour
<http://www.w3.org/2006/time#unitHour> rdf:type owl:NamedIndividual ,
                                                <http://www.w3.org/2006/time#TemporalUnit> ;
                                       <http://www.w3.org/2006/time#days> 0 ;
                                       <http://www.w3.org/2006/time#hours> 1 ;
                                       <http://www.w3.org/2006/time#minutes> 0 ;
                                       <http://www.w3.org/2006/time#months> 0 ;
                                       <http://www.w3.org/2006/time#seconds> 0 ;
                                       <http://www.w3.org/2006/time#weeks> 0 ;
                                       <http://www.w3.org/2006/time#years> 0 ;
                                       rdfs:label "Hour (unit of temporal duration)"@en ;
                                       <http://www.w3.org/2004/02/skos/core#prefLabel> "Stunde"@de ,
                                                                                       "godzina"@pl ,
                                                                                       "heure"@fr ,
                                                                                       "hora"@es ,
                                                                                       "hora"@pt ,
                                                                                       "hour"@en ,
                                                                                       "ora"@it ,
                                                                                       "uur"@nl ,
                                                                                       "ساعة واحدة"@ar ,
                                                                                       "一小時"@zh ,
                                                                                       "一時間"@ja ,
                                                                                       "한 시간"@kr ,
                                                                                       "один час\"@ru" .


###  http://www.w3.org/2006/time#unitMillenium
<http://www.w3.org/2006/time#unitMillenium> rdf:type owl:NamedIndividual ,
                                                     <http://www.w3.org/2006/time#TemporalUnit> ;
                                            <http://www.w3.org/2006/time#days> 0 ;
                                            <http://www.w3.org/2006/time#hours> 0 ;
                                            <http://www.w3.org/2006/time#minutes> 0 ;
                                            <http://www.w3.org/2006/time#months> 0 ;
                                            <http://www.w3.org/2006/time#seconds> 0 ;
                                            <http://www.w3.org/2006/time#weeks> 0 ;
                                            <http://www.w3.org/2006/time#years> 1000 ;
                                            rdfs:label "Century (unit of temporal duration)"@en ;
                                            <http://www.w3.org/2004/02/skos/core#prefLabel> "Jahrtausend"@de ,
                                                                                            "milenio"@es ,
                                                                                            "millenium"@en ,
                                                                                            "millennio"@it ,
                                                                                            "millennium"@nl ,
                                                                                            "millénaire"@fr ,
                                                                                            "milênio"@pt ,
                                                                                            "tysiąclecie"@pl ,
                                                                                            "тысячелетие"@ru ,
                                                                                            "الألفية"@ar ,
                                                                                            "ミレニアム"@ja ,
                                                                                            "千年"@zh ,
                                                                                            "밀레니엄"@kr .


###  http://www.w3.org/2006/time#unitMinute
<http://www.w3.org/2006/time#unitMinute> rdf:type owl:NamedIndividual ,
                                                  <http://www.w3.org/2006/time#TemporalUnit> ;
                                         <http://www.w3.org/2006/time#days> 0 ;
                                         <http://www.w3.org/2006/time#hours> 0 ;
                                         <http://www.w3.org/2006/time#minutes> 1 ;
                                         <http://www.w3.org/2006/time#months> 0 ;
                                         <http://www.w3.org/2006/time#seconds> 0 ;
                                         <http://www.w3.org/2006/time#weeks> 0 ;
                                         <http://www.w3.org/2006/time#years> 0 ;
                                         rdfs:label "Minute (unit of temporal duration)"@en ;
                                         <http://www.w3.org/2004/02/skos/core#prefLabel> "Minute"@de ,
                                                                                         "minuta"@pl ,
                                                                                         "minute"@en ,
                                                                                         "minute"@fr ,
                                                                                         "minuto"@es ,
                                                                                         "minuto"@it ,
                                                                                         "minuto"@pt ,
                                                                                         "minuut"@nl ,
                                                                                         "одна минута"@ru ,
                                                                                         "دقيقة واحدة"@ar ,
                                                                                         "一分"@ja ,
                                                                                         "等一下"@zh ,
                                                                                         "분"@kr .


###  http://www.w3.org/2006/time#unitMonth
<http://www.w3.org/2006/time#unitMonth> rdf:type owl:NamedIndividual ,
                                                 <http://www.w3.org/2006/time#TemporalUnit> ;
                                        <http://www.w3.org/2006/time#days> 0 ;
                                        <http://www.w3.org/2006/time#hours> 0 ;
                                        <http://www.w3.org/2006/time#minutes> 0 ;
                                        <http://www.w3.org/2006/time#months> 1 ;
                                        <http://www.w3.org/2006/time#seconds> 0 ;
                                        <http://www.w3.org/2006/time#weeks> 0 ;
                                        <http://www.w3.org/2006/time#years> 0 ;
                                        rdfs:label "Month (unit of temporal duration)"@en ;
                                        <http://www.w3.org/2004/02/skos/core#prefLabel> "Monat"@de ,
                                                                                        "maand"@nl ,
                                                                                        "mes"@es ,
                                                                                        "mese"@it ,
                                                                                        "miesiąc"@pl ,
                                                                                        "mois"@fr ,
                                                                                        "month"@en ,
                                                                                        "один месяц"@ru ,
                                                                                        "شهر واحد"@ar ,
                                                                                        "一か月"@ja ,
                                                                                        "一個月"@zh ,
                                                                                        "한달"@kr .


###  http://www.w3.org/2006/time#unitSecond
<http://www.w3.org/2006/time#unitSecond> rdf:type owl:NamedIndividual ,
                                                  <http://www.w3.org/2006/time#TemporalUnit> ;
                                         <http://www.w3.org/2006/time#days> 0 ;
                                         <http://www.w3.org/2006/time#hours> 0 ;
                                         <http://www.w3.org/2006/time#minutes> 0 ;
                                         <http://www.w3.org/2006/time#months> 0 ;
                                         <http://www.w3.org/2006/time#seconds> 1 ;
                                         <http://www.w3.org/2006/time#weeks> 0 ;
                                         <http://www.w3.org/2006/time#years> 0 ;
                                         rdfs:label "Second (unit of temporal duration)"@en ;
                                         <http://www.w3.org/2004/02/skos/core#prefLabel> "Sekunde"@de ,
                                                                                         "second"@en ,
                                                                                         "seconde"@fr ,
                                                                                         "seconde"@nl ,
                                                                                         "secondo"@it ,
                                                                                         "segundo"@es ,
                                                                                         "segundo"@pt ,
                                                                                         "sekundę"@pl ,
                                                                                         "ثانية واحدة"@ar ,
                                                                                         "一秒"@ja ,
                                                                                         "一秒"@zh ,
                                                                                         "일초"@kr .


###  http://www.w3.org/2006/time#unitWeek
<http://www.w3.org/2006/time#unitWeek> rdf:type owl:NamedIndividual ,
                                                <http://www.w3.org/2006/time#TemporalUnit> ;
                                       <http://www.w3.org/2006/time#days> 0 ;
                                       <http://www.w3.org/2006/time#hours> 0 ;
                                       <http://www.w3.org/2006/time#minutes> 0 ;
                                       <http://www.w3.org/2006/time#months> 0 ;
                                       <http://www.w3.org/2006/time#seconds> 0 ;
                                       <http://www.w3.org/2006/time#weeks> 1 ;
                                       <http://www.w3.org/2006/time#years> 0 ;
                                       rdfs:label "Week (unit of temporal duration)"@en ;
                                       <http://www.w3.org/2004/02/skos/core#prefLabel> "Woche"@de ,
                                                                                       "semaine"@fr ,
                                                                                       "semana"@es ,
                                                                                       "semana"@pt ,
                                                                                       "settimana"@it ,
                                                                                       "tydzień"@pl ,
                                                                                       "week"@en ,
                                                                                       "week"@nl ,
                                                                                       "одна неделя"@ru ,
                                                                                       "سبوع واحد"@ar ,
                                                                                       "一周"@zh ,
                                                                                       "一週間"@ja ,
                                                                                       "일주일"@kr .


###  http://www.w3.org/2006/time#unitYear
<http://www.w3.org/2006/time#unitYear> rdf:type owl:NamedIndividual ,
                                                <http://www.w3.org/2006/time#TemporalUnit> ;
                                       <http://www.w3.org/2006/time#days> 0 ;
                                       <http://www.w3.org/2006/time#hours> 0 ;
                                       <http://www.w3.org/2006/time#minutes> 0 ;
                                       <http://www.w3.org/2006/time#months> 0 ;
                                       <http://www.w3.org/2006/time#seconds> 0 ;
                                       <http://www.w3.org/2006/time#weeks> 0 ;
                                       <http://www.w3.org/2006/time#years> 1 ;
                                       rdfs:label "Year (unit of temporal duration)"@en ;
                                       <http://www.w3.org/2004/02/skos/core#prefLabel> "1 년"@kr ,
                                                                                       "Jahr"@de ,
                                                                                       "an"@fr ,
                                                                                       "anno"@it ,
                                                                                       "ano"@pt ,
                                                                                       "jaar"@nl ,
                                                                                       "rok"@pl ,
                                                                                       "un año"@es ,
                                                                                       "year"@en ,
                                                                                       "один год"@ru ,
                                                                                       "سنة واحدة"@ar ,
                                                                                       "一年"@ja ,
                                                                                       "一年"@zh .


###  https://w3id.org/def/phenowl#t1
:t1 rdf:type owl:NamedIndividual ,
             <http://www.w3.org/2006/time#Instant> .


###  https://w3id.org/def/phenowl#t2
:t2 rdf:type owl:NamedIndividual ,
             <http://www.w3.org/2006/time#Instant> .


###  https://w3id.org/def/phenowl#t3
:t3 rdf:type owl:NamedIndividual ,
             <http://www.w3.org/2006/time#Instant> ;
    <http://www.w3.org/2006/time#after> :t1 .


###  https://w3id.org/def/phenowl#t4
:t4 rdf:type owl:NamedIndividual ,
             <http://www.w3.org/2006/time#Instant> .


[ xsd:pattern "--(0[1-9]|1[0-9]|20)(Z|(\\+|-)((0[0-9]|1[0-3]):[0-5][0-9]|14:00))?"
] .

[ xsd:pattern "---(0[1-9]|[1-9][0-9])(Z|(\\+|-)((0[0-9]|1[0-3]):[0-5][0-9]|14:00))?"
 ] .

[ xsd:pattern "-?([1-9][0-9]{3,}|0[0-9]{3})(Z|(\\+|-)((0[0-9]|1[0-3]):[0-5][0-9]|14:00))?"
 ] .

#################################################################
#    Annotations
#################################################################

<https://w3id.org/seas/BalanceEvaluation> rdfs:comment "Evaluation of the difference between the incoming evaluation and the outgoing evaluation."@en ;
                                           rdfs:isDefinedBy <https://w3id.org/seas/ZoneOntology> ;
                                           rdfs:label "Balance Evaluation" ;
                                           <http://www.w3.org/2003/06/sw-vocab-status/ns#term_status> "testing" .


#################################################################
#    General axioms
#################################################################

[ rdf:type owl:AllDisjointClasses ;
  owl:members ( <http://purl.org/nemo/gufo#Collection>
                <http://purl.org/nemo/gufo#FunctionalComplex>
                <http://purl.org/nemo/gufo#Quantity>
              )
] .


[ rdf:type owl:AllDisjointClasses ;
  owl:members ( <http://purl.org/nemo/gufo#Endurant>
                <http://purl.org/nemo/gufo#Event>
                <http://purl.org/nemo/gufo#Situation>
              )
] .


#################################################################
#    Rules
#################################################################

<http://www.semanticweb.org/alencga1/ontologies/2023/2/PhenOWL/O1> rdf:type <http://www.w3.org/2003/11/swrl#Variable> .

<http://www.semanticweb.org/alencga1/ontologies/2023/2/PhenOWL/PI1> rdf:type <http://www.w3.org/2003/11/swrl#Variable> .

<http://www.semanticweb.org/alencga1/ontologies/2023/2/PhenOWL/PI2> rdf:type <http://www.w3.org/2003/11/swrl#Variable> .

<http://www.semanticweb.org/alencga1/ontologies/2023/2/PhenOWL/SO2> rdf:type <http://www.w3.org/2003/11/swrl#Variable> .

<http://www.semanticweb.org/alencga1/ontologies/2023/2/PhenOWL/PR1> rdf:type <http://www.w3.org/2003/11/swrl#Variable> .

<http://www.semanticweb.org/alencga1/ontologies/2023/2/PhenOWL/S1> rdf:type <http://www.w3.org/2003/11/swrl#Variable> .

<http://www.semanticweb.org/alencga1/ontologies/2023/2/PhenOWL/O2> rdf:type <http://www.w3.org/2003/11/swrl#Variable> .

<http://www.semanticweb.org/alencga1/ontologies/2023/2/PhenOWL/S2> rdf:type <http://www.w3.org/2003/11/swrl#Variable> .

<http://www.semanticweb.org/alencga1/ontologies/2023/2/PhenOWL/t1> rdf:type <http://www.w3.org/2003/11/swrl#Variable> .

<http://www.semanticweb.org/alencga1/ontologies/2023/2/PhenOWL/t2> rdf:type <http://www.w3.org/2003/11/swrl#Variable> .

<http://www.semanticweb.org/alencga1/ontologies/2023/2/PhenOWL/OP2> rdf:type <http://www.w3.org/2003/11/swrl#Variable> .

<http://www.semanticweb.org/alencga1/ontologies/2023/2/PhenOWL/OP1> rdf:type <http://www.w3.org/2003/11/swrl#Variable> .

<http://www.semanticweb.org/alencga1/ontologies/2023/2/PhenOWL/P1> rdf:type <http://www.w3.org/2003/11/swrl#Variable> .

<http://www.semanticweb.org/alencga1/ontologies/2023/2/PhenOWL/GCE> rdf:type <http://www.w3.org/2003/11/swrl#Variable> .

<http://www.semanticweb.org/alencga1/ontologies/2023/2/PhenOWL/SO1> rdf:type <http://www.w3.org/2003/11/swrl#Variable> .

[ <http://swrl.stanford.edu/ontologies/3.3/swrla.owl#isRuleEnabled> "true"^^xsd:boolean ;
   rdfs:comment "Presence of group of Individuals in both node/system and observation (eq equals)" ;
   rdfs:label "S4.3 - Pr in Obs (eq equals)" ;
   rdf:type <http://www.w3.org/2003/11/swrl#Imp> ;
   <http://www.w3.org/2003/11/swrl#body> [ rdf:type <http://www.w3.org/2003/11/swrl#AtomList> ;
                                           rdf:first [ rdf:type <http://www.w3.org/2003/11/swrl#ClassAtom> ;
                                                       <http://www.w3.org/2003/11/swrl#classPredicate> :Observation ;
                                                       <http://www.w3.org/2003/11/swrl#argument1> <http://www.semanticweb.org/alencga1/ontologies/2023/2/PhenOWL/O1>
                                                     ] ;
                                           rdf:rest [ rdf:type <http://www.w3.org/2003/11/swrl#AtomList> ;
                                                      rdf:first [ rdf:type <http://www.w3.org/2003/11/swrl#IndividualPropertyAtom> ;
                                                                  <http://www.w3.org/2003/11/swrl#propertyPredicate> <http://www.w3.org/2006/time#intervalEquals> ;
                                                                  <http://www.w3.org/2003/11/swrl#argument1> <http://www.semanticweb.org/alencga1/ontologies/2023/2/PhenOWL/PI1> ;
                                                                  <http://www.w3.org/2003/11/swrl#argument2> <http://www.semanticweb.org/alencga1/ontologies/2023/2/PhenOWL/PI2>
                                                                ] ;
                                                      rdf:rest [ rdf:type <http://www.w3.org/2003/11/swrl#AtomList> ;
                                                                 rdf:first [ rdf:type <http://www.w3.org/2003/11/swrl#ClassAtom> ;
                                                                             <http://www.w3.org/2003/11/swrl#classPredicate> <http://www.opengis.net/ont/geosparql#SpatialObject> ;
                                                                             <http://www.w3.org/2003/11/swrl#argument1> <http://www.semanticweb.org/alencga1/ontologies/2023/2/PhenOWL/SO2>
                                                                           ] ;
                                                                 rdf:rest [ rdf:type <http://www.w3.org/2003/11/swrl#AtomList> ;
                                                                            rdf:first [ rdf:type <http://www.w3.org/2003/11/swrl#IndividualPropertyAtom> ;
                                                                                        <http://www.w3.org/2003/11/swrl#propertyPredicate> :spatialPresenceIn ;
                                                                                        <http://www.w3.org/2003/11/swrl#argument1> <http://www.semanticweb.org/alencga1/ontologies/2023/2/PhenOWL/PR1> ;
                                                                                        <http://www.w3.org/2003/11/swrl#argument2> <http://www.semanticweb.org/alencga1/ontologies/2023/2/PhenOWL/SO2>
                                                                                      ] ;
                                                                            rdf:rest [ rdf:type <http://www.w3.org/2003/11/swrl#AtomList> ;
                                                                                       rdf:first [ rdf:type <http://www.w3.org/2003/11/swrl#ClassAtom> ;
                                                                                                   <http://www.w3.org/2003/11/swrl#classPredicate> <http://www.w3.org/2006/time#ProperInterval> ;
                                                                                                   <http://www.w3.org/2003/11/swrl#argument1> <http://www.semanticweb.org/alencga1/ontologies/2023/2/PhenOWL/PI1>
                                                                                                 ] ;
                                                                                       rdf:rest [ rdf:type <http://www.w3.org/2003/11/swrl#AtomList> ;
                                                                                                  rdf:first [ rdf:type <http://www.w3.org/2003/11/swrl#ClassAtom> ;
                                                                                                              <http://www.w3.org/2003/11/swrl#classPredicate> <https://w3id.org/seas/System> ;
                                                                                                              <http://www.w3.org/2003/11/swrl#argument1> <http://www.semanticweb.org/alencga1/ontologies/2023/2/PhenOWL/S1>
                                                                                                            ] ;
                                                                                                  rdf:rest [ rdf:type <http://www.w3.org/2003/11/swrl#AtomList> ;
                                                                                                             rdf:first [ rdf:type <http://www.w3.org/2003/11/swrl#ClassAtom> ;
                                                                                                                         <http://www.w3.org/2003/11/swrl#classPredicate> :Presence ;
                                                                                                                         <http://www.w3.org/2003/11/swrl#argument1> <http://www.semanticweb.org/alencga1/ontologies/2023/2/PhenOWL/PR1>
                                                                                                                       ] ;
                                                                                                             rdf:rest [ rdf:type <http://www.w3.org/2003/11/swrl#AtomList> ;
                                                                                                                        rdf:first [ rdf:type <http://www.w3.org/2003/11/swrl#ClassAtom> ;
                                                                                                                                    <http://www.w3.org/2003/11/swrl#classPredicate> <http://www.w3.org/2006/time#ProperInterval> ;
                                                                                                                                    <http://www.w3.org/2003/11/swrl#argument1> <http://www.semanticweb.org/alencga1/ontologies/2023/2/PhenOWL/PI2>
                                                                                                                                  ] ;
                                                                                                                        rdf:rest [ rdf:type <http://www.w3.org/2003/11/swrl#AtomList> ;
                                                                                                                                   rdf:first [ rdf:type <http://www.w3.org/2003/11/swrl#IndividualPropertyAtom> ;
                                                                                                                                               <http://www.w3.org/2003/11/swrl#propertyPredicate> :hasTimeInterval ;
                                                                                                                                               <http://www.w3.org/2003/11/swrl#argument1> <http://www.semanticweb.org/alencga1/ontologies/2023/2/PhenOWL/PR1> ;
                                                                                                                                               <http://www.w3.org/2003/11/swrl#argument2> <http://www.semanticweb.org/alencga1/ontologies/2023/2/PhenOWL/PI2>
                                                                                                                                             ] ;
                                                                                                                                   rdf:rest [ rdf:type <http://www.w3.org/2003/11/swrl#AtomList> ;
                                                                                                                                              rdf:first [ rdf:type <http://www.w3.org/2003/11/swrl#IndividualPropertyAtom> ;
                                                                                                                                                          <http://www.w3.org/2003/11/swrl#propertyPredicate> :hasTimeInterval ;
                                                                                                                                                          <http://www.w3.org/2003/11/swrl#argument1> <http://www.semanticweb.org/alencga1/ontologies/2023/2/PhenOWL/O1> ;
                                                                                                                                                          <http://www.w3.org/2003/11/swrl#argument2> <http://www.semanticweb.org/alencga1/ontologies/2023/2/PhenOWL/PI1>
                                                                                                                                                        ] ;
                                                                                                                                              rdf:rest [ rdf:type <http://www.w3.org/2003/11/swrl#AtomList> ;
                                                                                                                                                         rdf:first [ rdf:type <http://www.w3.org/2003/11/swrl#IndividualPropertyAtom> ;
                                                                                                                                                                     <http://www.w3.org/2003/11/swrl#propertyPredicate> :happensIn ;
                                                                                                                                                                     <http://www.w3.org/2003/11/swrl#argument1> <http://www.semanticweb.org/alencga1/ontologies/2023/2/PhenOWL/O1> ;
                                                                                                                                                                     <http://www.w3.org/2003/11/swrl#argument2> <http://www.semanticweb.org/alencga1/ontologies/2023/2/PhenOWL/S1>
                                                                                                                                                                   ] ;
                                                                                                                                                         rdf:rest [ rdf:type <http://www.w3.org/2003/11/swrl#AtomList> ;
                                                                                                                                                                    rdf:first [ rdf:type <http://www.w3.org/2003/11/swrl#IndividualPropertyAtom> ;
                                                                                                                                                                                <http://www.w3.org/2003/11/swrl#propertyPredicate> <http://www.opengis.net/ont/geosparql#rcc8eq> ;
                                                                                                                                                                                <http://www.w3.org/2003/11/swrl#argument1> <http://www.semanticweb.org/alencga1/ontologies/2023/2/PhenOWL/SO2> ;
                                                                                                                                                                                <http://www.w3.org/2003/11/swrl#argument2> <http://www.semanticweb.org/alencga1/ontologies/2023/2/PhenOWL/S1>
                                                                                                                                                                              ] ;
                                                                                                                                                                    rdf:rest rdf:nil
                                                                                                                                                                  ]
                                                                                                                                                       ]
                                                                                                                                            ]
                                                                                                                                 ]
                                                                                                                      ]
                                                                                                           ]
                                                                                                ]
                                                                                     ]
                                                                          ]
                                                               ]
                                                    ]
                                         ] ;
   <http://www.w3.org/2003/11/swrl#head> [ rdf:type <http://www.w3.org/2003/11/swrl#AtomList> ;
                                           rdf:first [ rdf:type <http://www.w3.org/2003/11/swrl#IndividualPropertyAtom> ;
                                                       <http://www.w3.org/2003/11/swrl#propertyPredicate> :observationalPresenceIn ;
                                                       <http://www.w3.org/2003/11/swrl#argument1> <http://www.semanticweb.org/alencga1/ontologies/2023/2/PhenOWL/PR1> ;
                                                       <http://www.w3.org/2003/11/swrl#argument2> <http://www.semanticweb.org/alencga1/ontologies/2023/2/PhenOWL/O1>
                                                     ] ;
                                           rdf:rest rdf:nil
                                         ]
 ] .

[ <http://swrl.stanford.edu/ontologies/3.3/swrla.owl#isRuleEnabled> "true"^^xsd:boolean ;
   rdfs:comment "Presence of group of Individuals in both node/system and observation (ntpp equals)" ;
   rdfs:label "S4.2 - Pr in Obs (nttp equals)" ;
   rdf:type <http://www.w3.org/2003/11/swrl#Imp> ;
   <http://www.w3.org/2003/11/swrl#body> [ rdf:type <http://www.w3.org/2003/11/swrl#AtomList> ;
                                           rdf:first [ rdf:type <http://www.w3.org/2003/11/swrl#ClassAtom> ;
                                                       <http://www.w3.org/2003/11/swrl#classPredicate> :Observation ;
                                                       <http://www.w3.org/2003/11/swrl#argument1> <http://www.semanticweb.org/alencga1/ontologies/2023/2/PhenOWL/O1>
                                                     ] ;
                                           rdf:rest [ rdf:type <http://www.w3.org/2003/11/swrl#AtomList> ;
                                                      rdf:first [ rdf:type <http://www.w3.org/2003/11/swrl#IndividualPropertyAtom> ;
                                                                  <http://www.w3.org/2003/11/swrl#propertyPredicate> <http://www.w3.org/2006/time#intervalEquals> ;
                                                                  <http://www.w3.org/2003/11/swrl#argument1> <http://www.semanticweb.org/alencga1/ontologies/2023/2/PhenOWL/PI1> ;
                                                                  <http://www.w3.org/2003/11/swrl#argument2> <http://www.semanticweb.org/alencga1/ontologies/2023/2/PhenOWL/PI2>
                                                                ] ;
                                                      rdf:rest [ rdf:type <http://www.w3.org/2003/11/swrl#AtomList> ;
                                                                 rdf:first [ rdf:type <http://www.w3.org/2003/11/swrl#ClassAtom> ;
                                                                             <http://www.w3.org/2003/11/swrl#classPredicate> <http://www.opengis.net/ont/geosparql#SpatialObject> ;
                                                                             <http://www.w3.org/2003/11/swrl#argument1> <http://www.semanticweb.org/alencga1/ontologies/2023/2/PhenOWL/SO2>
                                                                           ] ;
                                                                 rdf:rest [ rdf:type <http://www.w3.org/2003/11/swrl#AtomList> ;
                                                                            rdf:first [ rdf:type <http://www.w3.org/2003/11/swrl#IndividualPropertyAtom> ;
                                                                                        <http://www.w3.org/2003/11/swrl#propertyPredicate> :spatialPresenceIn ;
                                                                                        <http://www.w3.org/2003/11/swrl#argument1> <http://www.semanticweb.org/alencga1/ontologies/2023/2/PhenOWL/PR1> ;
                                                                                        <http://www.w3.org/2003/11/swrl#argument2> <http://www.semanticweb.org/alencga1/ontologies/2023/2/PhenOWL/SO2>
                                                                                      ] ;
                                                                            rdf:rest [ rdf:type <http://www.w3.org/2003/11/swrl#AtomList> ;
                                                                                       rdf:first [ rdf:type <http://www.w3.org/2003/11/swrl#ClassAtom> ;
                                                                                                   <http://www.w3.org/2003/11/swrl#classPredicate> <http://www.w3.org/2006/time#ProperInterval> ;
                                                                                                   <http://www.w3.org/2003/11/swrl#argument1> <http://www.semanticweb.org/alencga1/ontologies/2023/2/PhenOWL/PI1>
                                                                                                 ] ;
                                                                                       rdf:rest [ rdf:type <http://www.w3.org/2003/11/swrl#AtomList> ;
                                                                                                  rdf:first [ rdf:type <http://www.w3.org/2003/11/swrl#ClassAtom> ;
                                                                                                              <http://www.w3.org/2003/11/swrl#classPredicate> <https://w3id.org/seas/System> ;
                                                                                                              <http://www.w3.org/2003/11/swrl#argument1> <http://www.semanticweb.org/alencga1/ontologies/2023/2/PhenOWL/S1>
                                                                                                            ] ;
                                                                                                  rdf:rest [ rdf:type <http://www.w3.org/2003/11/swrl#AtomList> ;
                                                                                                             rdf:first [ rdf:type <http://www.w3.org/2003/11/swrl#ClassAtom> ;
                                                                                                                         <http://www.w3.org/2003/11/swrl#classPredicate> :Presence ;
                                                                                                                         <http://www.w3.org/2003/11/swrl#argument1> <http://www.semanticweb.org/alencga1/ontologies/2023/2/PhenOWL/PR1>
                                                                                                                       ] ;
                                                                                                             rdf:rest [ rdf:type <http://www.w3.org/2003/11/swrl#AtomList> ;
                                                                                                                        rdf:first [ rdf:type <http://www.w3.org/2003/11/swrl#ClassAtom> ;
                                                                                                                                    <http://www.w3.org/2003/11/swrl#classPredicate> <http://www.w3.org/2006/time#ProperInterval> ;
                                                                                                                                    <http://www.w3.org/2003/11/swrl#argument1> <http://www.semanticweb.org/alencga1/ontologies/2023/2/PhenOWL/PI2>
                                                                                                                                  ] ;
                                                                                                                        rdf:rest [ rdf:type <http://www.w3.org/2003/11/swrl#AtomList> ;
                                                                                                                                   rdf:first [ rdf:type <http://www.w3.org/2003/11/swrl#IndividualPropertyAtom> ;
                                                                                                                                               <http://www.w3.org/2003/11/swrl#propertyPredicate> :hasTimeInterval ;
                                                                                                                                               <http://www.w3.org/2003/11/swrl#argument1> <http://www.semanticweb.org/alencga1/ontologies/2023/2/PhenOWL/PR1> ;
                                                                                                                                               <http://www.w3.org/2003/11/swrl#argument2> <http://www.semanticweb.org/alencga1/ontologies/2023/2/PhenOWL/PI2>
                                                                                                                                             ] ;
                                                                                                                                   rdf:rest [ rdf:type <http://www.w3.org/2003/11/swrl#AtomList> ;
                                                                                                                                              rdf:first [ rdf:type <http://www.w3.org/2003/11/swrl#IndividualPropertyAtom> ;
                                                                                                                                                          <http://www.w3.org/2003/11/swrl#propertyPredicate> <http://www.opengis.net/ont/geosparql#rcc8ntpp> ;
                                                                                                                                                          <http://www.w3.org/2003/11/swrl#argument1> <http://www.semanticweb.org/alencga1/ontologies/2023/2/PhenOWL/SO2> ;
                                                                                                                                                          <http://www.w3.org/2003/11/swrl#argument2> <http://www.semanticweb.org/alencga1/ontologies/2023/2/PhenOWL/S1>
                                                                                                                                                        ] ;
                                                                                                                                              rdf:rest [ rdf:type <http://www.w3.org/2003/11/swrl#AtomList> ;
                                                                                                                                                         rdf:first [ rdf:type <http://www.w3.org/2003/11/swrl#IndividualPropertyAtom> ;
                                                                                                                                                                     <http://www.w3.org/2003/11/swrl#propertyPredicate> :hasTimeInterval ;
                                                                                                                                                                     <http://www.w3.org/2003/11/swrl#argument1> <http://www.semanticweb.org/alencga1/ontologies/2023/2/PhenOWL/O1> ;
                                                                                                                                                                     <http://www.w3.org/2003/11/swrl#argument2> <http://www.semanticweb.org/alencga1/ontologies/2023/2/PhenOWL/PI1>
                                                                                                                                                                   ] ;
                                                                                                                                                         rdf:rest [ rdf:type <http://www.w3.org/2003/11/swrl#AtomList> ;
                                                                                                                                                                    rdf:first [ rdf:type <http://www.w3.org/2003/11/swrl#IndividualPropertyAtom> ;
                                                                                                                                                                                <http://www.w3.org/2003/11/swrl#propertyPredicate> :happensIn ;
                                                                                                                                                                                <http://www.w3.org/2003/11/swrl#argument1> <http://www.semanticweb.org/alencga1/ontologies/2023/2/PhenOWL/O1> ;
                                                                                                                                                                                <http://www.w3.org/2003/11/swrl#argument2> <http://www.semanticweb.org/alencga1/ontologies/2023/2/PhenOWL/S1>
                                                                                                                                                                              ] ;
                                                                                                                                                                    rdf:rest rdf:nil
                                                                                                                                                                  ]
                                                                                                                                                       ]
                                                                                                                                            ]
                                                                                                                                 ]
                                                                                                                      ]
                                                                                                           ]
                                                                                                ]
                                                                                     ]
                                                                          ]
                                                               ]
                                                    ]
                                         ] ;
   <http://www.w3.org/2003/11/swrl#head> [ rdf:type <http://www.w3.org/2003/11/swrl#AtomList> ;
                                           rdf:first [ rdf:type <http://www.w3.org/2003/11/swrl#IndividualPropertyAtom> ;
                                                       <http://www.w3.org/2003/11/swrl#propertyPredicate> :observationalPresenceIn ;
                                                       <http://www.w3.org/2003/11/swrl#argument1> <http://www.semanticweb.org/alencga1/ontologies/2023/2/PhenOWL/PR1> ;
                                                       <http://www.w3.org/2003/11/swrl#argument2> <http://www.semanticweb.org/alencga1/ontologies/2023/2/PhenOWL/O1>
                                                     ] ;
                                           rdf:rest rdf:nil
                                         ]
 ] .

[ <http://swrl.stanford.edu/ontologies/3.3/swrla.owl#isRuleEnabled> "true"^^xsd:boolean ;
   rdfs:comment "Presence of group of Individuals in both node/system and observation (tpp equals)" ;
   rdfs:label "S4.1 - Pr in Obs (ttp equals)" ;
   rdf:type <http://www.w3.org/2003/11/swrl#Imp> ;
   <http://www.w3.org/2003/11/swrl#body> [ rdf:type <http://www.w3.org/2003/11/swrl#AtomList> ;
                                           rdf:first [ rdf:type <http://www.w3.org/2003/11/swrl#ClassAtom> ;
                                                       <http://www.w3.org/2003/11/swrl#classPredicate> :Observation ;
                                                       <http://www.w3.org/2003/11/swrl#argument1> <http://www.semanticweb.org/alencga1/ontologies/2023/2/PhenOWL/O1>
                                                     ] ;
                                           rdf:rest [ rdf:type <http://www.w3.org/2003/11/swrl#AtomList> ;
                                                      rdf:first [ rdf:type <http://www.w3.org/2003/11/swrl#IndividualPropertyAtom> ;
                                                                  <http://www.w3.org/2003/11/swrl#propertyPredicate> <http://www.w3.org/2006/time#intervalEquals> ;
                                                                  <http://www.w3.org/2003/11/swrl#argument1> <http://www.semanticweb.org/alencga1/ontologies/2023/2/PhenOWL/PI1> ;
                                                                  <http://www.w3.org/2003/11/swrl#argument2> <http://www.semanticweb.org/alencga1/ontologies/2023/2/PhenOWL/PI2>
                                                                ] ;
                                                      rdf:rest [ rdf:type <http://www.w3.org/2003/11/swrl#AtomList> ;
                                                                 rdf:first [ rdf:type <http://www.w3.org/2003/11/swrl#IndividualPropertyAtom> ;
                                                                             <http://www.w3.org/2003/11/swrl#propertyPredicate> <http://www.opengis.net/ont/geosparql#rcc8tpp> ;
                                                                             <http://www.w3.org/2003/11/swrl#argument1> <http://www.semanticweb.org/alencga1/ontologies/2023/2/PhenOWL/SO2> ;
                                                                             <http://www.w3.org/2003/11/swrl#argument2> <http://www.semanticweb.org/alencga1/ontologies/2023/2/PhenOWL/S1>
                                                                           ] ;
                                                                 rdf:rest [ rdf:type <http://www.w3.org/2003/11/swrl#AtomList> ;
                                                                            rdf:first [ rdf:type <http://www.w3.org/2003/11/swrl#ClassAtom> ;
                                                                                        <http://www.w3.org/2003/11/swrl#classPredicate> <http://www.opengis.net/ont/geosparql#SpatialObject> ;
                                                                                        <http://www.w3.org/2003/11/swrl#argument1> <http://www.semanticweb.org/alencga1/ontologies/2023/2/PhenOWL/SO2>
                                                                                      ] ;
                                                                            rdf:rest [ rdf:type <http://www.w3.org/2003/11/swrl#AtomList> ;
                                                                                       rdf:first [ rdf:type <http://www.w3.org/2003/11/swrl#IndividualPropertyAtom> ;
                                                                                                   <http://www.w3.org/2003/11/swrl#propertyPredicate> :spatialPresenceIn ;
                                                                                                   <http://www.w3.org/2003/11/swrl#argument1> <http://www.semanticweb.org/alencga1/ontologies/2023/2/PhenOWL/PR1> ;
                                                                                                   <http://www.w3.org/2003/11/swrl#argument2> <http://www.semanticweb.org/alencga1/ontologies/2023/2/PhenOWL/SO2>
                                                                                                 ] ;
                                                                                       rdf:rest [ rdf:type <http://www.w3.org/2003/11/swrl#AtomList> ;
                                                                                                  rdf:first [ rdf:type <http://www.w3.org/2003/11/swrl#ClassAtom> ;
                                                                                                              <http://www.w3.org/2003/11/swrl#classPredicate> <http://www.w3.org/2006/time#ProperInterval> ;
                                                                                                              <http://www.w3.org/2003/11/swrl#argument1> <http://www.semanticweb.org/alencga1/ontologies/2023/2/PhenOWL/PI1>
                                                                                                            ] ;
                                                                                                  rdf:rest [ rdf:type <http://www.w3.org/2003/11/swrl#AtomList> ;
                                                                                                             rdf:first [ rdf:type <http://www.w3.org/2003/11/swrl#ClassAtom> ;
                                                                                                                         <http://www.w3.org/2003/11/swrl#classPredicate> <https://w3id.org/seas/System> ;
                                                                                                                         <http://www.w3.org/2003/11/swrl#argument1> <http://www.semanticweb.org/alencga1/ontologies/2023/2/PhenOWL/S1>
                                                                                                                       ] ;
                                                                                                             rdf:rest [ rdf:type <http://www.w3.org/2003/11/swrl#AtomList> ;
                                                                                                                        rdf:first [ rdf:type <http://www.w3.org/2003/11/swrl#ClassAtom> ;
                                                                                                                                    <http://www.w3.org/2003/11/swrl#classPredicate> :Presence ;
                                                                                                                                    <http://www.w3.org/2003/11/swrl#argument1> <http://www.semanticweb.org/alencga1/ontologies/2023/2/PhenOWL/PR1>
                                                                                                                                  ] ;
                                                                                                                        rdf:rest [ rdf:type <http://www.w3.org/2003/11/swrl#AtomList> ;
                                                                                                                                   rdf:first [ rdf:type <http://www.w3.org/2003/11/swrl#ClassAtom> ;
                                                                                                                                               <http://www.w3.org/2003/11/swrl#classPredicate> <http://www.w3.org/2006/time#ProperInterval> ;
                                                                                                                                               <http://www.w3.org/2003/11/swrl#argument1> <http://www.semanticweb.org/alencga1/ontologies/2023/2/PhenOWL/PI2>
                                                                                                                                             ] ;
                                                                                                                                   rdf:rest [ rdf:type <http://www.w3.org/2003/11/swrl#AtomList> ;
                                                                                                                                              rdf:first [ rdf:type <http://www.w3.org/2003/11/swrl#IndividualPropertyAtom> ;
                                                                                                                                                          <http://www.w3.org/2003/11/swrl#propertyPredicate> :hasTimeInterval ;
                                                                                                                                                          <http://www.w3.org/2003/11/swrl#argument1> <http://www.semanticweb.org/alencga1/ontologies/2023/2/PhenOWL/PR1> ;
                                                                                                                                                          <http://www.w3.org/2003/11/swrl#argument2> <http://www.semanticweb.org/alencga1/ontologies/2023/2/PhenOWL/PI2>
                                                                                                                                                        ] ;
                                                                                                                                              rdf:rest [ rdf:type <http://www.w3.org/2003/11/swrl#AtomList> ;
                                                                                                                                                         rdf:first [ rdf:type <http://www.w3.org/2003/11/swrl#IndividualPropertyAtom> ;
                                                                                                                                                                     <http://www.w3.org/2003/11/swrl#propertyPredicate> :hasTimeInterval ;
                                                                                                                                                                     <http://www.w3.org/2003/11/swrl#argument1> <http://www.semanticweb.org/alencga1/ontologies/2023/2/PhenOWL/O1> ;
                                                                                                                                                                     <http://www.w3.org/2003/11/swrl#argument2> <http://www.semanticweb.org/alencga1/ontologies/2023/2/PhenOWL/PI1>
                                                                                                                                                                   ] ;
                                                                                                                                                         rdf:rest [ rdf:type <http://www.w3.org/2003/11/swrl#AtomList> ;
                                                                                                                                                                    rdf:first [ rdf:type <http://www.w3.org/2003/11/swrl#IndividualPropertyAtom> ;
                                                                                                                                                                                <http://www.w3.org/2003/11/swrl#propertyPredicate> :happensIn ;
                                                                                                                                                                                <http://www.w3.org/2003/11/swrl#argument1> <http://www.semanticweb.org/alencga1/ontologies/2023/2/PhenOWL/O1> ;
                                                                                                                                                                                <http://www.w3.org/2003/11/swrl#argument2> <http://www.semanticweb.org/alencga1/ontologies/2023/2/PhenOWL/S1>
                                                                                                                                                                              ] ;
                                                                                                                                                                    rdf:rest rdf:nil
                                                                                                                                                                  ]
                                                                                                                                                       ]
                                                                                                                                            ]
                                                                                                                                 ]
                                                                                                                      ]
                                                                                                           ]
                                                                                                ]
                                                                                     ]
                                                                          ]
                                                               ]
                                                    ]
                                         ] ;
   <http://www.w3.org/2003/11/swrl#head> [ rdf:type <http://www.w3.org/2003/11/swrl#AtomList> ;
                                           rdf:first [ rdf:type <http://www.w3.org/2003/11/swrl#IndividualPropertyAtom> ;
                                                       <http://www.w3.org/2003/11/swrl#propertyPredicate> :observationalPresenceIn ;
                                                       <http://www.w3.org/2003/11/swrl#argument1> <http://www.semanticweb.org/alencga1/ontologies/2023/2/PhenOWL/PR1> ;
                                                       <http://www.w3.org/2003/11/swrl#argument2> <http://www.semanticweb.org/alencga1/ontologies/2023/2/PhenOWL/O1>
                                                     ] ;
                                           rdf:rest rdf:nil
                                         ]
 ] .

[ <http://swrl.stanford.edu/ontologies/3.3/swrla.owl#isRuleEnabled> "true"^^xsd:boolean ;
   rdfs:comment "Valid ST Path from gufo begin point" ;
   rdfs:label "S5.1 - Valid ST Path from gufo" ;
   rdf:type <http://www.w3.org/2003/11/swrl#Imp> ;
   <http://www.w3.org/2003/11/swrl#body> [ rdf:type <http://www.w3.org/2003/11/swrl#AtomList> ;
                                           rdf:first [ rdf:type <http://www.w3.org/2003/11/swrl#ClassAtom> ;
                                                       <http://www.w3.org/2003/11/swrl#classPredicate> :Observation ;
                                                       <http://www.w3.org/2003/11/swrl#argument1> <http://www.semanticweb.org/alencga1/ontologies/2023/2/PhenOWL/O2>
                                                     ] ;
                                           rdf:rest [ rdf:type <http://www.w3.org/2003/11/swrl#AtomList> ;
                                                      rdf:first [ rdf:type <http://www.w3.org/2003/11/swrl#ClassAtom> ;
                                                                  <http://www.w3.org/2003/11/swrl#classPredicate> <https://w3id.org/seas/System> ;
                                                                  <http://www.w3.org/2003/11/swrl#argument1> <http://www.semanticweb.org/alencga1/ontologies/2023/2/PhenOWL/S2>
                                                                ] ;
                                                      rdf:rest [ rdf:type <http://www.w3.org/2003/11/swrl#AtomList> ;
                                                                 rdf:first [ rdf:type <http://www.w3.org/2003/11/swrl#ClassAtom> ;
                                                                             <http://www.w3.org/2003/11/swrl#classPredicate> :Observation ;
                                                                             <http://www.w3.org/2003/11/swrl#argument1> <http://www.semanticweb.org/alencga1/ontologies/2023/2/PhenOWL/O1>
                                                                           ] ;
                                                                 rdf:rest [ rdf:type <http://www.w3.org/2003/11/swrl#AtomList> ;
                                                                            rdf:first [ rdf:type <http://www.w3.org/2003/11/swrl#ClassAtom> ;
                                                                                        <http://www.w3.org/2003/11/swrl#classPredicate> <http://www.w3.org/2006/time#Instant> ;
                                                                                        <http://www.w3.org/2003/11/swrl#argument1> <http://www.semanticweb.org/alencga1/ontologies/2023/2/PhenOWL/t1>
                                                                                      ] ;
                                                                            rdf:rest [ rdf:type <http://www.w3.org/2003/11/swrl#AtomList> ;
                                                                                       rdf:first [ rdf:type <http://www.w3.org/2003/11/swrl#IndividualPropertyAtom> ;
                                                                                                   <http://www.w3.org/2003/11/swrl#propertyPredicate> <http://www.w3.org/2006/time#after> ;
                                                                                                   <http://www.w3.org/2003/11/swrl#argument1> <http://www.semanticweb.org/alencga1/ontologies/2023/2/PhenOWL/t2> ;
                                                                                                   <http://www.w3.org/2003/11/swrl#argument2> <http://www.semanticweb.org/alencga1/ontologies/2023/2/PhenOWL/t1>
                                                                                                 ] ;
                                                                                       rdf:rest [ rdf:type <http://www.w3.org/2003/11/swrl#AtomList> ;
                                                                                                  rdf:first [ rdf:type <http://www.w3.org/2003/11/swrl#ClassAtom> ;
                                                                                                              <http://www.w3.org/2003/11/swrl#classPredicate> :PhenomenonOccurrence ;
                                                                                                              <http://www.w3.org/2003/11/swrl#argument1> <http://www.semanticweb.org/alencga1/ontologies/2023/2/PhenOWL/OP2>
                                                                                                            ] ;
                                                                                                  rdf:rest [ rdf:type <http://www.w3.org/2003/11/swrl#AtomList> ;
                                                                                                             rdf:first [ rdf:type <http://www.w3.org/2003/11/swrl#IndividualPropertyAtom> ;
                                                                                                                         <http://www.w3.org/2003/11/swrl#propertyPredicate> :observationOf ;
                                                                                                                         <http://www.w3.org/2003/11/swrl#argument1> <http://www.semanticweb.org/alencga1/ontologies/2023/2/PhenOWL/O1> ;
                                                                                                                         <http://www.w3.org/2003/11/swrl#argument2> <http://www.semanticweb.org/alencga1/ontologies/2023/2/PhenOWL/OP1>
                                                                                                                       ] ;
                                                                                                             rdf:rest [ rdf:type <http://www.w3.org/2003/11/swrl#AtomList> ;
                                                                                                                        rdf:first [ rdf:type <http://www.w3.org/2003/11/swrl#IndividualPropertyAtom> ;
                                                                                                                                    <http://www.w3.org/2003/11/swrl#propertyPredicate> :observationOf ;
                                                                                                                                    <http://www.w3.org/2003/11/swrl#argument1> <http://www.semanticweb.org/alencga1/ontologies/2023/2/PhenOWL/O2> ;
                                                                                                                                    <http://www.w3.org/2003/11/swrl#argument2> <http://www.semanticweb.org/alencga1/ontologies/2023/2/PhenOWL/OP2>
                                                                                                                                  ] ;
                                                                                                                        rdf:rest [ rdf:type <http://www.w3.org/2003/11/swrl#AtomList> ;
                                                                                                                                   rdf:first [ rdf:type <http://www.w3.org/2003/11/swrl#ClassAtom> ;
                                                                                                                                               <http://www.w3.org/2003/11/swrl#classPredicate> <https://w3id.org/seas/System> ;
                                                                                                                                               <http://www.w3.org/2003/11/swrl#argument1> <http://www.semanticweb.org/alencga1/ontologies/2023/2/PhenOWL/S1>
                                                                                                                                             ] ;
                                                                                                                                   rdf:rest [ rdf:type <http://www.w3.org/2003/11/swrl#AtomList> ;
                                                                                                                                              rdf:first [ rdf:type <http://www.w3.org/2003/11/swrl#IndividualPropertyAtom> ;
                                                                                                                                                          <http://www.w3.org/2003/11/swrl#propertyPredicate> <https://w3id.org/seas/connectedTo> ;
                                                                                                                                                          <http://www.w3.org/2003/11/swrl#argument1> <http://www.semanticweb.org/alencga1/ontologies/2023/2/PhenOWL/S1> ;
                                                                                                                                                          <http://www.w3.org/2003/11/swrl#argument2> <http://www.semanticweb.org/alencga1/ontologies/2023/2/PhenOWL/S2>
                                                                                                                                                        ] ;
                                                                                                                                              rdf:rest [ rdf:type <http://www.w3.org/2003/11/swrl#AtomList> ;
                                                                                                                                                         rdf:first [ rdf:type <http://www.w3.org/2003/11/swrl#ClassAtom> ;
                                                                                                                                                                     <http://www.w3.org/2003/11/swrl#classPredicate> <http://www.w3.org/2006/time#Instant> ;
                                                                                                                                                                     <http://www.w3.org/2003/11/swrl#argument1> <http://www.semanticweb.org/alencga1/ontologies/2023/2/PhenOWL/t2>
                                                                                                                                                                   ] ;
                                                                                                                                                         rdf:rest [ rdf:type <http://www.w3.org/2003/11/swrl#AtomList> ;
                                                                                                                                                                    rdf:first [ rdf:type <http://www.w3.org/2003/11/swrl#ClassAtom> ;
                                                                                                                                                                                <http://www.w3.org/2003/11/swrl#classPredicate> :PhenomenonOccurrence ;
                                                                                                                                                                                <http://www.w3.org/2003/11/swrl#argument1> <http://www.semanticweb.org/alencga1/ontologies/2023/2/PhenOWL/OP1>
                                                                                                                                                                              ] ;
                                                                                                                                                                    rdf:rest [ rdf:type <http://www.w3.org/2003/11/swrl#AtomList> ;
                                                                                                                                                                               rdf:first [ rdf:type <http://www.w3.org/2003/11/swrl#IndividualPropertyAtom> ;
                                                                                                                                                                                           <http://www.w3.org/2003/11/swrl#propertyPredicate> :fromPhenomenon ;
                                                                                                                                                                                           <http://www.w3.org/2003/11/swrl#argument1> <http://www.semanticweb.org/alencga1/ontologies/2023/2/PhenOWL/OP1> ;
                                                                                                                                                                                           <http://www.w3.org/2003/11/swrl#argument2> <http://www.semanticweb.org/alencga1/ontologies/2023/2/PhenOWL/P1>
                                                                                                                                                                                         ] ;
                                                                                                                                                                               rdf:rest [ rdf:type <http://www.w3.org/2003/11/swrl#AtomList> ;
                                                                                                                                                                                          rdf:first [ rdf:type <http://www.w3.org/2003/11/swrl#ClassAtom> ;
                                                                                                                                                                                                      <http://www.w3.org/2003/11/swrl#classPredicate> :Phenomenon ;
                                                                                                                                                                                                      <http://www.w3.org/2003/11/swrl#argument1> <http://www.semanticweb.org/alencga1/ontologies/2023/2/PhenOWL/P1>
                                                                                                                                                                                                    ] ;
                                                                                                                                                                                          rdf:rest [ rdf:type <http://www.w3.org/2003/11/swrl#AtomList> ;
                                                                                                                                                                                                     rdf:first [ rdf:type <http://www.w3.org/2003/11/swrl#IndividualPropertyAtom> ;
                                                                                                                                                                                                                 <http://www.w3.org/2003/11/swrl#propertyPredicate> <http://purl.org/nemo/gufo#hasBeginPoint> ;
                                                                                                                                                                                                                 <http://www.w3.org/2003/11/swrl#argument1> <http://www.semanticweb.org/alencga1/ontologies/2023/2/PhenOWL/O1> ;
                                                                                                                                                                                                                 <http://www.w3.org/2003/11/swrl#argument2> <http://www.semanticweb.org/alencga1/ontologies/2023/2/PhenOWL/t1>
                                                                                                                                                                                                               ] ;
                                                                                                                                                                                                     rdf:rest [ rdf:type <http://www.w3.org/2003/11/swrl#AtomList> ;
                                                                                                                                                                                                                rdf:first [ rdf:type <http://www.w3.org/2003/11/swrl#IndividualPropertyAtom> ;
                                                                                                                                                                                                                            <http://www.w3.org/2003/11/swrl#propertyPredicate> <http://purl.org/nemo/gufo#hasBeginPoint> ;
                                                                                                                                                                                                                            <http://www.w3.org/2003/11/swrl#argument1> <http://www.semanticweb.org/alencga1/ontologies/2023/2/PhenOWL/O2> ;
                                                                                                                                                                                                                            <http://www.w3.org/2003/11/swrl#argument2> <http://www.semanticweb.org/alencga1/ontologies/2023/2/PhenOWL/t2>
                                                                                                                                                                                                                          ] ;
                                                                                                                                                                                                                rdf:rest [ rdf:type <http://www.w3.org/2003/11/swrl#AtomList> ;
                                                                                                                                                                                                                           rdf:first [ rdf:type <http://www.w3.org/2003/11/swrl#IndividualPropertyAtom> ;
                                                                                                                                                                                                                                       <http://www.w3.org/2003/11/swrl#propertyPredicate> :happensIn ;
                                                                                                                                                                                                                                       <http://www.w3.org/2003/11/swrl#argument1> <http://www.semanticweb.org/alencga1/ontologies/2023/2/PhenOWL/O1> ;
                                                                                                                                                                                                                                       <http://www.w3.org/2003/11/swrl#argument2> <http://www.semanticweb.org/alencga1/ontologies/2023/2/PhenOWL/S1>
                                                                                                                                                                                                                                     ] ;
                                                                                                                                                                                                                           rdf:rest [ rdf:type <http://www.w3.org/2003/11/swrl#AtomList> ;
                                                                                                                                                                                                                                      rdf:first [ rdf:type <http://www.w3.org/2003/11/swrl#IndividualPropertyAtom> ;
                                                                                                                                                                                                                                                  <http://www.w3.org/2003/11/swrl#propertyPredicate> :happensIn ;
                                                                                                                                                                                                                                                  <http://www.w3.org/2003/11/swrl#argument1> <http://www.semanticweb.org/alencga1/ontologies/2023/2/PhenOWL/O2> ;
                                                                                                                                                                                                                                                  <http://www.w3.org/2003/11/swrl#argument2> <http://www.semanticweb.org/alencga1/ontologies/2023/2/PhenOWL/S2>
                                                                                                                                                                                                                                                ] ;
                                                                                                                                                                                                                                      rdf:rest [ rdf:type <http://www.w3.org/2003/11/swrl#AtomList> ;
                                                                                                                                                                                                                                                 rdf:first [ rdf:type <http://www.w3.org/2003/11/swrl#IndividualPropertyAtom> ;
                                                                                                                                                                                                                                                             <http://www.w3.org/2003/11/swrl#propertyPredicate> :fromPhenomenon ;
                                                                                                                                                                                                                                                             <http://www.w3.org/2003/11/swrl#argument1> <http://www.semanticweb.org/alencga1/ontologies/2023/2/PhenOWL/OP2> ;
                                                                                                                                                                                                                                                             <http://www.w3.org/2003/11/swrl#argument2> <http://www.semanticweb.org/alencga1/ontologies/2023/2/PhenOWL/P1>
                                                                                                                                                                                                                                                           ] ;
                                                                                                                                                                                                                                                 rdf:rest rdf:nil
                                                                                                                                                                                                                                               ]
                                                                                                                                                                                                                                    ]
                                                                                                                                                                                                                         ]
                                                                                                                                                                                                              ]
                                                                                                                                                                                                   ]
                                                                                                                                                                                        ]
                                                                                                                                                                             ]
                                                                                                                                                                  ]
                                                                                                                                                       ]
                                                                                                                                            ]
                                                                                                                                 ]
                                                                                                                      ]
                                                                                                           ]
                                                                                                ]
                                                                                     ]
                                                                          ]
                                                               ]
                                                    ]
                                         ] ;
   <http://www.w3.org/2003/11/swrl#head> [ rdf:type <http://www.w3.org/2003/11/swrl#AtomList> ;
                                           rdf:first [ rdf:type <http://www.w3.org/2003/11/swrl#IndividualPropertyAtom> ;
                                                       <http://www.w3.org/2003/11/swrl#propertyPredicate> :hasSTValidPath ;
                                                       <http://www.w3.org/2003/11/swrl#argument1> <http://www.semanticweb.org/alencga1/ontologies/2023/2/PhenOWL/O1> ;
                                                       <http://www.w3.org/2003/11/swrl#argument2> <http://www.semanticweb.org/alencga1/ontologies/2023/2/PhenOWL/O2>
                                                     ] ;
                                           rdf:rest rdf:nil
                                         ]
 ] .

[ <http://swrl.stanford.edu/ontologies/3.3/swrla.owl#isRuleEnabled> "true"^^xsd:boolean ;
   rdfs:comment "If phenomenon happens in one system, it must also happen in its super-system" ;
   rdfs:label "S2 - Observation in System" ;
   rdf:type <http://www.w3.org/2003/11/swrl#Imp> ;
   <http://www.w3.org/2003/11/swrl#body> [ rdf:type <http://www.w3.org/2003/11/swrl#AtomList> ;
                                           rdf:first [ rdf:type <http://www.w3.org/2003/11/swrl#ClassAtom> ;
                                                       <http://www.w3.org/2003/11/swrl#classPredicate> <https://w3id.org/seas/System> ;
                                                       <http://www.w3.org/2003/11/swrl#argument1> <http://www.semanticweb.org/alencga1/ontologies/2023/2/PhenOWL/S2>
                                                     ] ;
                                           rdf:rest [ rdf:type <http://www.w3.org/2003/11/swrl#AtomList> ;
                                                      rdf:first [ rdf:type <http://www.w3.org/2003/11/swrl#ClassAtom> ;
                                                                  <http://www.w3.org/2003/11/swrl#classPredicate> :Observation ;
                                                                  <http://www.w3.org/2003/11/swrl#argument1> <http://www.semanticweb.org/alencga1/ontologies/2023/2/PhenOWL/O1>
                                                                ] ;
                                                      rdf:rest [ rdf:type <http://www.w3.org/2003/11/swrl#AtomList> ;
                                                                 rdf:first [ rdf:type <http://www.w3.org/2003/11/swrl#ClassAtom> ;
                                                                             <http://www.w3.org/2003/11/swrl#classPredicate> <https://w3id.org/seas/System> ;
                                                                             <http://www.w3.org/2003/11/swrl#argument1> <http://www.semanticweb.org/alencga1/ontologies/2023/2/PhenOWL/S1>
                                                                           ] ;
                                                                 rdf:rest [ rdf:type <http://www.w3.org/2003/11/swrl#AtomList> ;
                                                                            rdf:first [ rdf:type <http://www.w3.org/2003/11/swrl#IndividualPropertyAtom> ;
                                                                                        <http://www.w3.org/2003/11/swrl#propertyPredicate> :happensIn ;
                                                                                        <http://www.w3.org/2003/11/swrl#argument1> <http://www.semanticweb.org/alencga1/ontologies/2023/2/PhenOWL/O1> ;
                                                                                        <http://www.w3.org/2003/11/swrl#argument2> <http://www.semanticweb.org/alencga1/ontologies/2023/2/PhenOWL/S1>
                                                                                      ] ;
                                                                            rdf:rest [ rdf:type <http://www.w3.org/2003/11/swrl#AtomList> ;
                                                                                       rdf:first [ rdf:type <http://www.w3.org/2003/11/swrl#IndividualPropertyAtom> ;
                                                                                                   <http://www.w3.org/2003/11/swrl#propertyPredicate> <https://w3id.org/seas/hasSubSystem> ;
                                                                                                   <http://www.w3.org/2003/11/swrl#argument1> <http://www.semanticweb.org/alencga1/ontologies/2023/2/PhenOWL/S2> ;
                                                                                                   <http://www.w3.org/2003/11/swrl#argument2> <http://www.semanticweb.org/alencga1/ontologies/2023/2/PhenOWL/S1>
                                                                                                 ] ;
                                                                                       rdf:rest rdf:nil
                                                                                     ]
                                                                          ]
                                                               ]
                                                    ]
                                         ] ;
   <http://www.w3.org/2003/11/swrl#head> [ rdf:type <http://www.w3.org/2003/11/swrl#AtomList> ;
                                           rdf:first [ rdf:type <http://www.w3.org/2003/11/swrl#IndividualPropertyAtom> ;
                                                       <http://www.w3.org/2003/11/swrl#propertyPredicate> :happensIn ;
                                                       <http://www.w3.org/2003/11/swrl#argument1> <http://www.semanticweb.org/alencga1/ontologies/2023/2/PhenOWL/O1> ;
                                                       <http://www.w3.org/2003/11/swrl#argument2> <http://www.semanticweb.org/alencga1/ontologies/2023/2/PhenOWL/S2>
                                                     ] ;
                                           rdf:rest rdf:nil
                                         ]
 ] .

[ <http://swrl.stanford.edu/ontologies/3.3/swrla.owl#isRuleEnabled> "true"^^xsd:boolean ;
   rdfs:comment "Associates begin point with beginning of time interval" ;
   rdfs:label "s3.3 - inverse time interval beginning" ;
   rdf:type <http://www.w3.org/2003/11/swrl#Imp> ;
   <http://www.w3.org/2003/11/swrl#body> [ rdf:type <http://www.w3.org/2003/11/swrl#AtomList> ;
                                           rdf:first [ rdf:type <http://www.w3.org/2003/11/swrl#ClassAtom> ;
                                                       <http://www.w3.org/2003/11/swrl#classPredicate> <http://www.w3.org/2006/time#Instant> ;
                                                       <http://www.w3.org/2003/11/swrl#argument1> <http://www.semanticweb.org/alencga1/ontologies/2023/2/PhenOWL/t1>
                                                     ] ;
                                           rdf:rest [ rdf:type <http://www.w3.org/2003/11/swrl#AtomList> ;
                                                      rdf:first [ rdf:type <http://www.w3.org/2003/11/swrl#ClassAtom> ;
                                                                  <http://www.w3.org/2003/11/swrl#classPredicate> <http://purl.org/nemo/gufo#ConcreteEntity> ;
                                                                  <http://www.w3.org/2003/11/swrl#argument1> <http://www.semanticweb.org/alencga1/ontologies/2023/2/PhenOWL/GCE>
                                                                ] ;
                                                      rdf:rest [ rdf:type <http://www.w3.org/2003/11/swrl#AtomList> ;
                                                                 rdf:first [ rdf:type <http://www.w3.org/2003/11/swrl#ClassAtom> ;
                                                                             <http://www.w3.org/2003/11/swrl#classPredicate> <http://www.w3.org/2006/time#ProperInterval> ;
                                                                             <http://www.w3.org/2003/11/swrl#argument1> <http://www.semanticweb.org/alencga1/ontologies/2023/2/PhenOWL/PI1>
                                                                           ] ;
                                                                 rdf:rest [ rdf:type <http://www.w3.org/2003/11/swrl#AtomList> ;
                                                                            rdf:first [ rdf:type <http://www.w3.org/2003/11/swrl#IndividualPropertyAtom> ;
                                                                                        <http://www.w3.org/2003/11/swrl#propertyPredicate> :hasTimeInterval ;
                                                                                        <http://www.w3.org/2003/11/swrl#argument1> <http://www.semanticweb.org/alencga1/ontologies/2023/2/PhenOWL/GCE> ;
                                                                                        <http://www.w3.org/2003/11/swrl#argument2> <http://www.semanticweb.org/alencga1/ontologies/2023/2/PhenOWL/PI1>
                                                                                      ] ;
                                                                            rdf:rest [ rdf:type <http://www.w3.org/2003/11/swrl#AtomList> ;
                                                                                       rdf:first [ rdf:type <http://www.w3.org/2003/11/swrl#IndividualPropertyAtom> ;
                                                                                                   <http://www.w3.org/2003/11/swrl#propertyPredicate> <http://www.w3.org/2006/time#hasBeginning> ;
                                                                                                   <http://www.w3.org/2003/11/swrl#argument1> <http://www.semanticweb.org/alencga1/ontologies/2023/2/PhenOWL/PI1> ;
                                                                                                   <http://www.w3.org/2003/11/swrl#argument2> <http://www.semanticweb.org/alencga1/ontologies/2023/2/PhenOWL/t1>
                                                                                                 ] ;
                                                                                       rdf:rest rdf:nil
                                                                                     ]
                                                                          ]
                                                               ]
                                                    ]
                                         ] ;
   <http://www.w3.org/2003/11/swrl#head> [ rdf:type <http://www.w3.org/2003/11/swrl#AtomList> ;
                                           rdf:first [ rdf:type <http://www.w3.org/2003/11/swrl#IndividualPropertyAtom> ;
                                                       <http://www.w3.org/2003/11/swrl#propertyPredicate> <http://purl.org/nemo/gufo#hasBeginPoint> ;
                                                       <http://www.w3.org/2003/11/swrl#argument1> <http://www.semanticweb.org/alencga1/ontologies/2023/2/PhenOWL/GCE> ;
                                                       <http://www.w3.org/2003/11/swrl#argument2> <http://www.semanticweb.org/alencga1/ontologies/2023/2/PhenOWL/t1>
                                                     ] ;
                                           rdf:rest rdf:nil
                                         ]
 ] .

[ <http://swrl.stanford.edu/ontologies/3.3/swrla.owl#isRuleEnabled> "true"^^xsd:boolean ;
   rdfs:comment "Associates begin point with beginning of time interval" ;
   rdfs:label "s3.1 - time interval beginning" ;
   rdf:type <http://www.w3.org/2003/11/swrl#Imp> ;
   <http://www.w3.org/2003/11/swrl#body> [ rdf:type <http://www.w3.org/2003/11/swrl#AtomList> ;
                                           rdf:first [ rdf:type <http://www.w3.org/2003/11/swrl#ClassAtom> ;
                                                       <http://www.w3.org/2003/11/swrl#classPredicate> <http://www.w3.org/2006/time#Instant> ;
                                                       <http://www.w3.org/2003/11/swrl#argument1> <http://www.semanticweb.org/alencga1/ontologies/2023/2/PhenOWL/t1>
                                                     ] ;
                                           rdf:rest [ rdf:type <http://www.w3.org/2003/11/swrl#AtomList> ;
                                                      rdf:first [ rdf:type <http://www.w3.org/2003/11/swrl#ClassAtom> ;
                                                                  <http://www.w3.org/2003/11/swrl#classPredicate> <http://purl.org/nemo/gufo#ConcreteEntity> ;
                                                                  <http://www.w3.org/2003/11/swrl#argument1> <http://www.semanticweb.org/alencga1/ontologies/2023/2/PhenOWL/GCE>
                                                                ] ;
                                                      rdf:rest [ rdf:type <http://www.w3.org/2003/11/swrl#AtomList> ;
                                                                 rdf:first [ rdf:type <http://www.w3.org/2003/11/swrl#ClassAtom> ;
                                                                             <http://www.w3.org/2003/11/swrl#classPredicate> <http://www.w3.org/2006/time#ProperInterval> ;
                                                                             <http://www.w3.org/2003/11/swrl#argument1> <http://www.semanticweb.org/alencga1/ontologies/2023/2/PhenOWL/PI1>
                                                                           ] ;
                                                                 rdf:rest [ rdf:type <http://www.w3.org/2003/11/swrl#AtomList> ;
                                                                            rdf:first [ rdf:type <http://www.w3.org/2003/11/swrl#IndividualPropertyAtom> ;
                                                                                        <http://www.w3.org/2003/11/swrl#propertyPredicate> <http://purl.org/nemo/gufo#hasBeginPoint> ;
                                                                                        <http://www.w3.org/2003/11/swrl#argument1> <http://www.semanticweb.org/alencga1/ontologies/2023/2/PhenOWL/GCE> ;
                                                                                        <http://www.w3.org/2003/11/swrl#argument2> <http://www.semanticweb.org/alencga1/ontologies/2023/2/PhenOWL/t1>
                                                                                      ] ;
                                                                            rdf:rest [ rdf:type <http://www.w3.org/2003/11/swrl#AtomList> ;
                                                                                       rdf:first [ rdf:type <http://www.w3.org/2003/11/swrl#IndividualPropertyAtom> ;
                                                                                                   <http://www.w3.org/2003/11/swrl#propertyPredicate> :hasTimeInterval ;
                                                                                                   <http://www.w3.org/2003/11/swrl#argument1> <http://www.semanticweb.org/alencga1/ontologies/2023/2/PhenOWL/GCE> ;
                                                                                                   <http://www.w3.org/2003/11/swrl#argument2> <http://www.semanticweb.org/alencga1/ontologies/2023/2/PhenOWL/PI1>
                                                                                                 ] ;
                                                                                       rdf:rest rdf:nil
                                                                                     ]
                                                                          ]
                                                               ]
                                                    ]
                                         ] ;
   <http://www.w3.org/2003/11/swrl#head> [ rdf:type <http://www.w3.org/2003/11/swrl#AtomList> ;
                                           rdf:first [ rdf:type <http://www.w3.org/2003/11/swrl#IndividualPropertyAtom> ;
                                                       <http://www.w3.org/2003/11/swrl#propertyPredicate> <http://www.w3.org/2006/time#hasBeginning> ;
                                                       <http://www.w3.org/2003/11/swrl#argument1> <http://www.semanticweb.org/alencga1/ontologies/2023/2/PhenOWL/PI1> ;
                                                       <http://www.w3.org/2003/11/swrl#argument2> <http://www.semanticweb.org/alencga1/ontologies/2023/2/PhenOWL/t1>
                                                     ] ;
                                           rdf:rest rdf:nil
                                         ]
 ] .

[ <http://swrl.stanford.edu/ontologies/3.3/swrla.owl#isRuleEnabled> "true"^^xsd:boolean ;
   rdfs:comment "Associates end point with beginning of time interval" ;
   rdfs:label "s3.2 - time interval end" ;
   rdf:type <http://www.w3.org/2003/11/swrl#Imp> ;
   <http://www.w3.org/2003/11/swrl#body> [ rdf:type <http://www.w3.org/2003/11/swrl#AtomList> ;
                                           rdf:first [ rdf:type <http://www.w3.org/2003/11/swrl#ClassAtom> ;
                                                       <http://www.w3.org/2003/11/swrl#classPredicate> <http://www.w3.org/2006/time#Instant> ;
                                                       <http://www.w3.org/2003/11/swrl#argument1> <http://www.semanticweb.org/alencga1/ontologies/2023/2/PhenOWL/t1>
                                                     ] ;
                                           rdf:rest [ rdf:type <http://www.w3.org/2003/11/swrl#AtomList> ;
                                                      rdf:first [ rdf:type <http://www.w3.org/2003/11/swrl#ClassAtom> ;
                                                                  <http://www.w3.org/2003/11/swrl#classPredicate> <http://purl.org/nemo/gufo#ConcreteEntity> ;
                                                                  <http://www.w3.org/2003/11/swrl#argument1> <http://www.semanticweb.org/alencga1/ontologies/2023/2/PhenOWL/GCE>
                                                                ] ;
                                                      rdf:rest [ rdf:type <http://www.w3.org/2003/11/swrl#AtomList> ;
                                                                 rdf:first [ rdf:type <http://www.w3.org/2003/11/swrl#ClassAtom> ;
                                                                             <http://www.w3.org/2003/11/swrl#classPredicate> <http://www.w3.org/2006/time#ProperInterval> ;
                                                                             <http://www.w3.org/2003/11/swrl#argument1> <http://www.semanticweb.org/alencga1/ontologies/2023/2/PhenOWL/PI1>
                                                                           ] ;
                                                                 rdf:rest [ rdf:type <http://www.w3.org/2003/11/swrl#AtomList> ;
                                                                            rdf:first [ rdf:type <http://www.w3.org/2003/11/swrl#IndividualPropertyAtom> ;
                                                                                        <http://www.w3.org/2003/11/swrl#propertyPredicate> <http://purl.org/nemo/gufo#hasEndPoint> ;
                                                                                        <http://www.w3.org/2003/11/swrl#argument1> <http://www.semanticweb.org/alencga1/ontologies/2023/2/PhenOWL/GCE> ;
                                                                                        <http://www.w3.org/2003/11/swrl#argument2> <http://www.semanticweb.org/alencga1/ontologies/2023/2/PhenOWL/t1>
                                                                                      ] ;
                                                                            rdf:rest [ rdf:type <http://www.w3.org/2003/11/swrl#AtomList> ;
                                                                                       rdf:first [ rdf:type <http://www.w3.org/2003/11/swrl#IndividualPropertyAtom> ;
                                                                                                   <http://www.w3.org/2003/11/swrl#propertyPredicate> :hasTimeInterval ;
                                                                                                   <http://www.w3.org/2003/11/swrl#argument1> <http://www.semanticweb.org/alencga1/ontologies/2023/2/PhenOWL/GCE> ;
                                                                                                   <http://www.w3.org/2003/11/swrl#argument2> <http://www.semanticweb.org/alencga1/ontologies/2023/2/PhenOWL/PI1>
                                                                                                 ] ;
                                                                                       rdf:rest rdf:nil
                                                                                     ]
                                                                          ]
                                                               ]
                                                    ]
                                         ] ;
   <http://www.w3.org/2003/11/swrl#head> [ rdf:type <http://www.w3.org/2003/11/swrl#AtomList> ;
                                           rdf:first [ rdf:type <http://www.w3.org/2003/11/swrl#IndividualPropertyAtom> ;
                                                       <http://www.w3.org/2003/11/swrl#propertyPredicate> <http://www.w3.org/2006/time#hasEnd> ;
                                                       <http://www.w3.org/2003/11/swrl#argument1> <http://www.semanticweb.org/alencga1/ontologies/2023/2/PhenOWL/PI1> ;
                                                       <http://www.w3.org/2003/11/swrl#argument2> <http://www.semanticweb.org/alencga1/ontologies/2023/2/PhenOWL/t1>
                                                     ] ;
                                           rdf:rest rdf:nil
                                         ]
 ] .

[ <http://swrl.stanford.edu/ontologies/3.3/swrla.owl#isRuleEnabled> "true"^^xsd:boolean ;
   rdfs:comment "Associates end point with beginning of time interval" ;
   rdfs:label "s3.4 - inverse time interval end" ;
   rdf:type <http://www.w3.org/2003/11/swrl#Imp> ;
   <http://www.w3.org/2003/11/swrl#body> [ rdf:type <http://www.w3.org/2003/11/swrl#AtomList> ;
                                           rdf:first [ rdf:type <http://www.w3.org/2003/11/swrl#ClassAtom> ;
                                                       <http://www.w3.org/2003/11/swrl#classPredicate> <http://www.w3.org/2006/time#Instant> ;
                                                       <http://www.w3.org/2003/11/swrl#argument1> <http://www.semanticweb.org/alencga1/ontologies/2023/2/PhenOWL/t1>
                                                     ] ;
                                           rdf:rest [ rdf:type <http://www.w3.org/2003/11/swrl#AtomList> ;
                                                      rdf:first [ rdf:type <http://www.w3.org/2003/11/swrl#IndividualPropertyAtom> ;
                                                                  <http://www.w3.org/2003/11/swrl#propertyPredicate> <http://www.w3.org/2006/time#hasEnd> ;
                                                                  <http://www.w3.org/2003/11/swrl#argument1> <http://www.semanticweb.org/alencga1/ontologies/2023/2/PhenOWL/PI1> ;
                                                                  <http://www.w3.org/2003/11/swrl#argument2> <http://www.semanticweb.org/alencga1/ontologies/2023/2/PhenOWL/t1>
                                                                ] ;
                                                      rdf:rest [ rdf:type <http://www.w3.org/2003/11/swrl#AtomList> ;
                                                                 rdf:first [ rdf:type <http://www.w3.org/2003/11/swrl#ClassAtom> ;
                                                                             <http://www.w3.org/2003/11/swrl#classPredicate> <http://purl.org/nemo/gufo#ConcreteEntity> ;
                                                                             <http://www.w3.org/2003/11/swrl#argument1> <http://www.semanticweb.org/alencga1/ontologies/2023/2/PhenOWL/GCE>
                                                                           ] ;
                                                                 rdf:rest [ rdf:type <http://www.w3.org/2003/11/swrl#AtomList> ;
                                                                            rdf:first [ rdf:type <http://www.w3.org/2003/11/swrl#ClassAtom> ;
                                                                                        <http://www.w3.org/2003/11/swrl#classPredicate> <http://www.w3.org/2006/time#ProperInterval> ;
                                                                                        <http://www.w3.org/2003/11/swrl#argument1> <http://www.semanticweb.org/alencga1/ontologies/2023/2/PhenOWL/PI1>
                                                                                      ] ;
                                                                            rdf:rest [ rdf:type <http://www.w3.org/2003/11/swrl#AtomList> ;
                                                                                       rdf:first [ rdf:type <http://www.w3.org/2003/11/swrl#IndividualPropertyAtom> ;
                                                                                                   <http://www.w3.org/2003/11/swrl#propertyPredicate> :hasTimeInterval ;
                                                                                                   <http://www.w3.org/2003/11/swrl#argument1> <http://www.semanticweb.org/alencga1/ontologies/2023/2/PhenOWL/GCE> ;
                                                                                                   <http://www.w3.org/2003/11/swrl#argument2> <http://www.semanticweb.org/alencga1/ontologies/2023/2/PhenOWL/PI1>
                                                                                                 ] ;
                                                                                       rdf:rest rdf:nil
                                                                                     ]
                                                                          ]
                                                               ]
                                                    ]
                                         ] ;
   <http://www.w3.org/2003/11/swrl#head> [ rdf:type <http://www.w3.org/2003/11/swrl#AtomList> ;
                                           rdf:first [ rdf:type <http://www.w3.org/2003/11/swrl#IndividualPropertyAtom> ;
                                                       <http://www.w3.org/2003/11/swrl#propertyPredicate> <http://purl.org/nemo/gufo#hasEndPoint> ;
                                                       <http://www.w3.org/2003/11/swrl#argument1> <http://www.semanticweb.org/alencga1/ontologies/2023/2/PhenOWL/GCE> ;
                                                       <http://www.w3.org/2003/11/swrl#argument2> <http://www.semanticweb.org/alencga1/ontologies/2023/2/PhenOWL/t1>
                                                     ] ;
                                           rdf:rest rdf:nil
                                         ]
 ] .

[ <http://swrl.stanford.edu/ontologies/3.3/swrla.owl#isRuleEnabled> "true"^^xsd:boolean ;
   rdfs:comment "Presence of group of Individuals in both node/system and observation (eq contains)" ;
   rdfs:label "S4.6 - Pr in Obs (eq contains)" ;
   rdf:type <http://www.w3.org/2003/11/swrl#Imp> ;
   <http://www.w3.org/2003/11/swrl#body> [ rdf:type <http://www.w3.org/2003/11/swrl#AtomList> ;
                                           rdf:first [ rdf:type <http://www.w3.org/2003/11/swrl#IndividualPropertyAtom> ;
                                                       <http://www.w3.org/2003/11/swrl#propertyPredicate> <http://www.w3.org/2006/time#intervalContains> ;
                                                       <http://www.w3.org/2003/11/swrl#argument1> <http://www.semanticweb.org/alencga1/ontologies/2023/2/PhenOWL/PI1> ;
                                                       <http://www.w3.org/2003/11/swrl#argument2> <http://www.semanticweb.org/alencga1/ontologies/2023/2/PhenOWL/PI2>
                                                     ] ;
                                           rdf:rest [ rdf:type <http://www.w3.org/2003/11/swrl#AtomList> ;
                                                      rdf:first [ rdf:type <http://www.w3.org/2003/11/swrl#ClassAtom> ;
                                                                  <http://www.w3.org/2003/11/swrl#classPredicate> :Observation ;
                                                                  <http://www.w3.org/2003/11/swrl#argument1> <http://www.semanticweb.org/alencga1/ontologies/2023/2/PhenOWL/O1>
                                                                ] ;
                                                      rdf:rest [ rdf:type <http://www.w3.org/2003/11/swrl#AtomList> ;
                                                                 rdf:first [ rdf:type <http://www.w3.org/2003/11/swrl#ClassAtom> ;
                                                                             <http://www.w3.org/2003/11/swrl#classPredicate> <http://www.opengis.net/ont/geosparql#SpatialObject> ;
                                                                             <http://www.w3.org/2003/11/swrl#argument1> <http://www.semanticweb.org/alencga1/ontologies/2023/2/PhenOWL/SO2>
                                                                           ] ;
                                                                 rdf:rest [ rdf:type <http://www.w3.org/2003/11/swrl#AtomList> ;
                                                                            rdf:first [ rdf:type <http://www.w3.org/2003/11/swrl#IndividualPropertyAtom> ;
                                                                                        <http://www.w3.org/2003/11/swrl#propertyPredicate> :spatialPresenceIn ;
                                                                                        <http://www.w3.org/2003/11/swrl#argument1> <http://www.semanticweb.org/alencga1/ontologies/2023/2/PhenOWL/PR1> ;
                                                                                        <http://www.w3.org/2003/11/swrl#argument2> <http://www.semanticweb.org/alencga1/ontologies/2023/2/PhenOWL/SO2>
                                                                                      ] ;
                                                                            rdf:rest [ rdf:type <http://www.w3.org/2003/11/swrl#AtomList> ;
                                                                                       rdf:first [ rdf:type <http://www.w3.org/2003/11/swrl#ClassAtom> ;
                                                                                                   <http://www.w3.org/2003/11/swrl#classPredicate> <http://www.w3.org/2006/time#ProperInterval> ;
                                                                                                   <http://www.w3.org/2003/11/swrl#argument1> <http://www.semanticweb.org/alencga1/ontologies/2023/2/PhenOWL/PI1>
                                                                                                 ] ;
                                                                                       rdf:rest [ rdf:type <http://www.w3.org/2003/11/swrl#AtomList> ;
                                                                                                  rdf:first [ rdf:type <http://www.w3.org/2003/11/swrl#ClassAtom> ;
                                                                                                              <http://www.w3.org/2003/11/swrl#classPredicate> <https://w3id.org/seas/System> ;
                                                                                                              <http://www.w3.org/2003/11/swrl#argument1> <http://www.semanticweb.org/alencga1/ontologies/2023/2/PhenOWL/S1>
                                                                                                            ] ;
                                                                                                  rdf:rest [ rdf:type <http://www.w3.org/2003/11/swrl#AtomList> ;
                                                                                                             rdf:first [ rdf:type <http://www.w3.org/2003/11/swrl#ClassAtom> ;
                                                                                                                         <http://www.w3.org/2003/11/swrl#classPredicate> :Presence ;
                                                                                                                         <http://www.w3.org/2003/11/swrl#argument1> <http://www.semanticweb.org/alencga1/ontologies/2023/2/PhenOWL/PR1>
                                                                                                                       ] ;
                                                                                                             rdf:rest [ rdf:type <http://www.w3.org/2003/11/swrl#AtomList> ;
                                                                                                                        rdf:first [ rdf:type <http://www.w3.org/2003/11/swrl#ClassAtom> ;
                                                                                                                                    <http://www.w3.org/2003/11/swrl#classPredicate> <http://www.w3.org/2006/time#ProperInterval> ;
                                                                                                                                    <http://www.w3.org/2003/11/swrl#argument1> <http://www.semanticweb.org/alencga1/ontologies/2023/2/PhenOWL/PI2>
                                                                                                                                  ] ;
                                                                                                                        rdf:rest [ rdf:type <http://www.w3.org/2003/11/swrl#AtomList> ;
                                                                                                                                   rdf:first [ rdf:type <http://www.w3.org/2003/11/swrl#IndividualPropertyAtom> ;
                                                                                                                                               <http://www.w3.org/2003/11/swrl#propertyPredicate> :hasTimeInterval ;
                                                                                                                                               <http://www.w3.org/2003/11/swrl#argument1> <http://www.semanticweb.org/alencga1/ontologies/2023/2/PhenOWL/PR1> ;
                                                                                                                                               <http://www.w3.org/2003/11/swrl#argument2> <http://www.semanticweb.org/alencga1/ontologies/2023/2/PhenOWL/PI2>
                                                                                                                                             ] ;
                                                                                                                                   rdf:rest [ rdf:type <http://www.w3.org/2003/11/swrl#AtomList> ;
                                                                                                                                              rdf:first [ rdf:type <http://www.w3.org/2003/11/swrl#IndividualPropertyAtom> ;
                                                                                                                                                          <http://www.w3.org/2003/11/swrl#propertyPredicate> :hasTimeInterval ;
                                                                                                                                                          <http://www.w3.org/2003/11/swrl#argument1> <http://www.semanticweb.org/alencga1/ontologies/2023/2/PhenOWL/O1> ;
                                                                                                                                                          <http://www.w3.org/2003/11/swrl#argument2> <http://www.semanticweb.org/alencga1/ontologies/2023/2/PhenOWL/PI1>
                                                                                                                                                        ] ;
                                                                                                                                              rdf:rest [ rdf:type <http://www.w3.org/2003/11/swrl#AtomList> ;
                                                                                                                                                         rdf:first [ rdf:type <http://www.w3.org/2003/11/swrl#IndividualPropertyAtom> ;
                                                                                                                                                                     <http://www.w3.org/2003/11/swrl#propertyPredicate> :happensIn ;
                                                                                                                                                                     <http://www.w3.org/2003/11/swrl#argument1> <http://www.semanticweb.org/alencga1/ontologies/2023/2/PhenOWL/O1> ;
                                                                                                                                                                     <http://www.w3.org/2003/11/swrl#argument2> <http://www.semanticweb.org/alencga1/ontologies/2023/2/PhenOWL/S1>
                                                                                                                                                                   ] ;
                                                                                                                                                         rdf:rest [ rdf:type <http://www.w3.org/2003/11/swrl#AtomList> ;
                                                                                                                                                                    rdf:first [ rdf:type <http://www.w3.org/2003/11/swrl#IndividualPropertyAtom> ;
                                                                                                                                                                                <http://www.w3.org/2003/11/swrl#propertyPredicate> <http://www.opengis.net/ont/geosparql#rcc8eq> ;
                                                                                                                                                                                <http://www.w3.org/2003/11/swrl#argument1> <http://www.semanticweb.org/alencga1/ontologies/2023/2/PhenOWL/SO2> ;
                                                                                                                                                                                <http://www.w3.org/2003/11/swrl#argument2> <http://www.semanticweb.org/alencga1/ontologies/2023/2/PhenOWL/S1>
                                                                                                                                                                              ] ;
                                                                                                                                                                    rdf:rest rdf:nil
                                                                                                                                                                  ]
                                                                                                                                                       ]
                                                                                                                                            ]
                                                                                                                                 ]
                                                                                                                      ]
                                                                                                           ]
                                                                                                ]
                                                                                     ]
                                                                          ]
                                                               ]
                                                    ]
                                         ] ;
   <http://www.w3.org/2003/11/swrl#head> [ rdf:type <http://www.w3.org/2003/11/swrl#AtomList> ;
                                           rdf:first [ rdf:type <http://www.w3.org/2003/11/swrl#IndividualPropertyAtom> ;
                                                       <http://www.w3.org/2003/11/swrl#propertyPredicate> :observationalPresenceIn ;
                                                       <http://www.w3.org/2003/11/swrl#argument1> <http://www.semanticweb.org/alencga1/ontologies/2023/2/PhenOWL/PR1> ;
                                                       <http://www.w3.org/2003/11/swrl#argument2> <http://www.semanticweb.org/alencga1/ontologies/2023/2/PhenOWL/O1>
                                                     ] ;
                                           rdf:rest rdf:nil
                                         ]
 ] .

[ <http://swrl.stanford.edu/ontologies/3.3/swrla.owl#isRuleEnabled> "true"^^xsd:boolean ;
   rdfs:comment "Presence of group of Individuals in both node/system and observation (ntpp contains)" ;
   rdfs:label "S4.5 - Pr in Obs (nttp contains)" ;
   rdf:type <http://www.w3.org/2003/11/swrl#Imp> ;
   <http://www.w3.org/2003/11/swrl#body> [ rdf:type <http://www.w3.org/2003/11/swrl#AtomList> ;
                                           rdf:first [ rdf:type <http://www.w3.org/2003/11/swrl#IndividualPropertyAtom> ;
                                                       <http://www.w3.org/2003/11/swrl#propertyPredicate> <http://www.w3.org/2006/time#intervalContains> ;
                                                       <http://www.w3.org/2003/11/swrl#argument1> <http://www.semanticweb.org/alencga1/ontologies/2023/2/PhenOWL/PI1> ;
                                                       <http://www.w3.org/2003/11/swrl#argument2> <http://www.semanticweb.org/alencga1/ontologies/2023/2/PhenOWL/PI2>
                                                     ] ;
                                           rdf:rest [ rdf:type <http://www.w3.org/2003/11/swrl#AtomList> ;
                                                      rdf:first [ rdf:type <http://www.w3.org/2003/11/swrl#ClassAtom> ;
                                                                  <http://www.w3.org/2003/11/swrl#classPredicate> :Observation ;
                                                                  <http://www.w3.org/2003/11/swrl#argument1> <http://www.semanticweb.org/alencga1/ontologies/2023/2/PhenOWL/O1>
                                                                ] ;
                                                      rdf:rest [ rdf:type <http://www.w3.org/2003/11/swrl#AtomList> ;
                                                                 rdf:first [ rdf:type <http://www.w3.org/2003/11/swrl#ClassAtom> ;
                                                                             <http://www.w3.org/2003/11/swrl#classPredicate> <http://www.opengis.net/ont/geosparql#SpatialObject> ;
                                                                             <http://www.w3.org/2003/11/swrl#argument1> <http://www.semanticweb.org/alencga1/ontologies/2023/2/PhenOWL/SO2>
                                                                           ] ;
                                                                 rdf:rest [ rdf:type <http://www.w3.org/2003/11/swrl#AtomList> ;
                                                                            rdf:first [ rdf:type <http://www.w3.org/2003/11/swrl#IndividualPropertyAtom> ;
                                                                                        <http://www.w3.org/2003/11/swrl#propertyPredicate> :spatialPresenceIn ;
                                                                                        <http://www.w3.org/2003/11/swrl#argument1> <http://www.semanticweb.org/alencga1/ontologies/2023/2/PhenOWL/PR1> ;
                                                                                        <http://www.w3.org/2003/11/swrl#argument2> <http://www.semanticweb.org/alencga1/ontologies/2023/2/PhenOWL/SO2>
                                                                                      ] ;
                                                                            rdf:rest [ rdf:type <http://www.w3.org/2003/11/swrl#AtomList> ;
                                                                                       rdf:first [ rdf:type <http://www.w3.org/2003/11/swrl#ClassAtom> ;
                                                                                                   <http://www.w3.org/2003/11/swrl#classPredicate> <http://www.w3.org/2006/time#ProperInterval> ;
                                                                                                   <http://www.w3.org/2003/11/swrl#argument1> <http://www.semanticweb.org/alencga1/ontologies/2023/2/PhenOWL/PI1>
                                                                                                 ] ;
                                                                                       rdf:rest [ rdf:type <http://www.w3.org/2003/11/swrl#AtomList> ;
                                                                                                  rdf:first [ rdf:type <http://www.w3.org/2003/11/swrl#ClassAtom> ;
                                                                                                              <http://www.w3.org/2003/11/swrl#classPredicate> <https://w3id.org/seas/System> ;
                                                                                                              <http://www.w3.org/2003/11/swrl#argument1> <http://www.semanticweb.org/alencga1/ontologies/2023/2/PhenOWL/S1>
                                                                                                            ] ;
                                                                                                  rdf:rest [ rdf:type <http://www.w3.org/2003/11/swrl#AtomList> ;
                                                                                                             rdf:first [ rdf:type <http://www.w3.org/2003/11/swrl#ClassAtom> ;
                                                                                                                         <http://www.w3.org/2003/11/swrl#classPredicate> :Presence ;
                                                                                                                         <http://www.w3.org/2003/11/swrl#argument1> <http://www.semanticweb.org/alencga1/ontologies/2023/2/PhenOWL/PR1>
                                                                                                                       ] ;
                                                                                                             rdf:rest [ rdf:type <http://www.w3.org/2003/11/swrl#AtomList> ;
                                                                                                                        rdf:first [ rdf:type <http://www.w3.org/2003/11/swrl#ClassAtom> ;
                                                                                                                                    <http://www.w3.org/2003/11/swrl#classPredicate> <http://www.w3.org/2006/time#ProperInterval> ;
                                                                                                                                    <http://www.w3.org/2003/11/swrl#argument1> <http://www.semanticweb.org/alencga1/ontologies/2023/2/PhenOWL/PI2>
                                                                                                                                  ] ;
                                                                                                                        rdf:rest [ rdf:type <http://www.w3.org/2003/11/swrl#AtomList> ;
                                                                                                                                   rdf:first [ rdf:type <http://www.w3.org/2003/11/swrl#IndividualPropertyAtom> ;
                                                                                                                                               <http://www.w3.org/2003/11/swrl#propertyPredicate> :hasTimeInterval ;
                                                                                                                                               <http://www.w3.org/2003/11/swrl#argument1> <http://www.semanticweb.org/alencga1/ontologies/2023/2/PhenOWL/PR1> ;
                                                                                                                                               <http://www.w3.org/2003/11/swrl#argument2> <http://www.semanticweb.org/alencga1/ontologies/2023/2/PhenOWL/PI2>
                                                                                                                                             ] ;
                                                                                                                                   rdf:rest [ rdf:type <http://www.w3.org/2003/11/swrl#AtomList> ;
                                                                                                                                              rdf:first [ rdf:type <http://www.w3.org/2003/11/swrl#IndividualPropertyAtom> ;
                                                                                                                                                          <http://www.w3.org/2003/11/swrl#propertyPredicate> <http://www.opengis.net/ont/geosparql#rcc8ntpp> ;
                                                                                                                                                          <http://www.w3.org/2003/11/swrl#argument1> <http://www.semanticweb.org/alencga1/ontologies/2023/2/PhenOWL/SO2> ;
                                                                                                                                                          <http://www.w3.org/2003/11/swrl#argument2> <http://www.semanticweb.org/alencga1/ontologies/2023/2/PhenOWL/S1>
                                                                                                                                                        ] ;
                                                                                                                                              rdf:rest [ rdf:type <http://www.w3.org/2003/11/swrl#AtomList> ;
                                                                                                                                                         rdf:first [ rdf:type <http://www.w3.org/2003/11/swrl#IndividualPropertyAtom> ;
                                                                                                                                                                     <http://www.w3.org/2003/11/swrl#propertyPredicate> :hasTimeInterval ;
                                                                                                                                                                     <http://www.w3.org/2003/11/swrl#argument1> <http://www.semanticweb.org/alencga1/ontologies/2023/2/PhenOWL/O1> ;
                                                                                                                                                                     <http://www.w3.org/2003/11/swrl#argument2> <http://www.semanticweb.org/alencga1/ontologies/2023/2/PhenOWL/PI1>
                                                                                                                                                                   ] ;
                                                                                                                                                         rdf:rest [ rdf:type <http://www.w3.org/2003/11/swrl#AtomList> ;
                                                                                                                                                                    rdf:first [ rdf:type <http://www.w3.org/2003/11/swrl#IndividualPropertyAtom> ;
                                                                                                                                                                                <http://www.w3.org/2003/11/swrl#propertyPredicate> :happensIn ;
                                                                                                                                                                                <http://www.w3.org/2003/11/swrl#argument1> <http://www.semanticweb.org/alencga1/ontologies/2023/2/PhenOWL/O1> ;
                                                                                                                                                                                <http://www.w3.org/2003/11/swrl#argument2> <http://www.semanticweb.org/alencga1/ontologies/2023/2/PhenOWL/S1>
                                                                                                                                                                              ] ;
                                                                                                                                                                    rdf:rest rdf:nil
                                                                                                                                                                  ]
                                                                                                                                                       ]
                                                                                                                                            ]
                                                                                                                                 ]
                                                                                                                      ]
                                                                                                           ]
                                                                                                ]
                                                                                     ]
                                                                          ]
                                                               ]
                                                    ]
                                         ] ;
   <http://www.w3.org/2003/11/swrl#head> [ rdf:type <http://www.w3.org/2003/11/swrl#AtomList> ;
                                           rdf:first [ rdf:type <http://www.w3.org/2003/11/swrl#IndividualPropertyAtom> ;
                                                       <http://www.w3.org/2003/11/swrl#propertyPredicate> :observationalPresenceIn ;
                                                       <http://www.w3.org/2003/11/swrl#argument1> <http://www.semanticweb.org/alencga1/ontologies/2023/2/PhenOWL/PR1> ;
                                                       <http://www.w3.org/2003/11/swrl#argument2> <http://www.semanticweb.org/alencga1/ontologies/2023/2/PhenOWL/O1>
                                                     ] ;
                                           rdf:rest rdf:nil
                                         ]
 ] .

[ <http://swrl.stanford.edu/ontologies/3.3/swrla.owl#isRuleEnabled> "true"^^xsd:boolean ;
   rdfs:comment "Presence of group of Individuals in both node/system and observation (tpp contains)" ;
   rdfs:label "S4.4 - Pr in Obs (ttp contains)" ;
   rdf:type <http://www.w3.org/2003/11/swrl#Imp> ;
   <http://www.w3.org/2003/11/swrl#body> [ rdf:type <http://www.w3.org/2003/11/swrl#AtomList> ;
                                           rdf:first [ rdf:type <http://www.w3.org/2003/11/swrl#IndividualPropertyAtom> ;
                                                       <http://www.w3.org/2003/11/swrl#propertyPredicate> <http://www.w3.org/2006/time#intervalContains> ;
                                                       <http://www.w3.org/2003/11/swrl#argument1> <http://www.semanticweb.org/alencga1/ontologies/2023/2/PhenOWL/PI1> ;
                                                       <http://www.w3.org/2003/11/swrl#argument2> <http://www.semanticweb.org/alencga1/ontologies/2023/2/PhenOWL/PI2>
                                                     ] ;
                                           rdf:rest [ rdf:type <http://www.w3.org/2003/11/swrl#AtomList> ;
                                                      rdf:first [ rdf:type <http://www.w3.org/2003/11/swrl#ClassAtom> ;
                                                                  <http://www.w3.org/2003/11/swrl#classPredicate> :Observation ;
                                                                  <http://www.w3.org/2003/11/swrl#argument1> <http://www.semanticweb.org/alencga1/ontologies/2023/2/PhenOWL/O1>
                                                                ] ;
                                                      rdf:rest [ rdf:type <http://www.w3.org/2003/11/swrl#AtomList> ;
                                                                 rdf:first [ rdf:type <http://www.w3.org/2003/11/swrl#IndividualPropertyAtom> ;
                                                                             <http://www.w3.org/2003/11/swrl#propertyPredicate> <http://www.opengis.net/ont/geosparql#rcc8tpp> ;
                                                                             <http://www.w3.org/2003/11/swrl#argument1> <http://www.semanticweb.org/alencga1/ontologies/2023/2/PhenOWL/SO2> ;
                                                                             <http://www.w3.org/2003/11/swrl#argument2> <http://www.semanticweb.org/alencga1/ontologies/2023/2/PhenOWL/S1>
                                                                           ] ;
                                                                 rdf:rest [ rdf:type <http://www.w3.org/2003/11/swrl#AtomList> ;
                                                                            rdf:first [ rdf:type <http://www.w3.org/2003/11/swrl#ClassAtom> ;
                                                                                        <http://www.w3.org/2003/11/swrl#classPredicate> <http://www.opengis.net/ont/geosparql#SpatialObject> ;
                                                                                        <http://www.w3.org/2003/11/swrl#argument1> <http://www.semanticweb.org/alencga1/ontologies/2023/2/PhenOWL/SO2>
                                                                                      ] ;
                                                                            rdf:rest [ rdf:type <http://www.w3.org/2003/11/swrl#AtomList> ;
                                                                                       rdf:first [ rdf:type <http://www.w3.org/2003/11/swrl#IndividualPropertyAtom> ;
                                                                                                   <http://www.w3.org/2003/11/swrl#propertyPredicate> :spatialPresenceIn ;
                                                                                                   <http://www.w3.org/2003/11/swrl#argument1> <http://www.semanticweb.org/alencga1/ontologies/2023/2/PhenOWL/PR1> ;
                                                                                                   <http://www.w3.org/2003/11/swrl#argument2> <http://www.semanticweb.org/alencga1/ontologies/2023/2/PhenOWL/SO2>
                                                                                                 ] ;
                                                                                       rdf:rest [ rdf:type <http://www.w3.org/2003/11/swrl#AtomList> ;
                                                                                                  rdf:first [ rdf:type <http://www.w3.org/2003/11/swrl#ClassAtom> ;
                                                                                                              <http://www.w3.org/2003/11/swrl#classPredicate> <http://www.w3.org/2006/time#ProperInterval> ;
                                                                                                              <http://www.w3.org/2003/11/swrl#argument1> <http://www.semanticweb.org/alencga1/ontologies/2023/2/PhenOWL/PI1>
                                                                                                            ] ;
                                                                                                  rdf:rest [ rdf:type <http://www.w3.org/2003/11/swrl#AtomList> ;
                                                                                                             rdf:first [ rdf:type <http://www.w3.org/2003/11/swrl#ClassAtom> ;
                                                                                                                         <http://www.w3.org/2003/11/swrl#classPredicate> <https://w3id.org/seas/System> ;
                                                                                                                         <http://www.w3.org/2003/11/swrl#argument1> <http://www.semanticweb.org/alencga1/ontologies/2023/2/PhenOWL/S1>
                                                                                                                       ] ;
                                                                                                             rdf:rest [ rdf:type <http://www.w3.org/2003/11/swrl#AtomList> ;
                                                                                                                        rdf:first [ rdf:type <http://www.w3.org/2003/11/swrl#ClassAtom> ;
                                                                                                                                    <http://www.w3.org/2003/11/swrl#classPredicate> :Presence ;
                                                                                                                                    <http://www.w3.org/2003/11/swrl#argument1> <http://www.semanticweb.org/alencga1/ontologies/2023/2/PhenOWL/PR1>
                                                                                                                                  ] ;
                                                                                                                        rdf:rest [ rdf:type <http://www.w3.org/2003/11/swrl#AtomList> ;
                                                                                                                                   rdf:first [ rdf:type <http://www.w3.org/2003/11/swrl#ClassAtom> ;
                                                                                                                                               <http://www.w3.org/2003/11/swrl#classPredicate> <http://www.w3.org/2006/time#ProperInterval> ;
                                                                                                                                               <http://www.w3.org/2003/11/swrl#argument1> <http://www.semanticweb.org/alencga1/ontologies/2023/2/PhenOWL/PI2>
                                                                                                                                             ] ;
                                                                                                                                   rdf:rest [ rdf:type <http://www.w3.org/2003/11/swrl#AtomList> ;
                                                                                                                                              rdf:first [ rdf:type <http://www.w3.org/2003/11/swrl#IndividualPropertyAtom> ;
                                                                                                                                                          <http://www.w3.org/2003/11/swrl#propertyPredicate> :hasTimeInterval ;
                                                                                                                                                          <http://www.w3.org/2003/11/swrl#argument1> <http://www.semanticweb.org/alencga1/ontologies/2023/2/PhenOWL/PR1> ;
                                                                                                                                                          <http://www.w3.org/2003/11/swrl#argument2> <http://www.semanticweb.org/alencga1/ontologies/2023/2/PhenOWL/PI2>
                                                                                                                                                        ] ;
                                                                                                                                              rdf:rest [ rdf:type <http://www.w3.org/2003/11/swrl#AtomList> ;
                                                                                                                                                         rdf:first [ rdf:type <http://www.w3.org/2003/11/swrl#IndividualPropertyAtom> ;
                                                                                                                                                                     <http://www.w3.org/2003/11/swrl#propertyPredicate> :hasTimeInterval ;
                                                                                                                                                                     <http://www.w3.org/2003/11/swrl#argument1> <http://www.semanticweb.org/alencga1/ontologies/2023/2/PhenOWL/O1> ;
                                                                                                                                                                     <http://www.w3.org/2003/11/swrl#argument2> <http://www.semanticweb.org/alencga1/ontologies/2023/2/PhenOWL/PI1>
                                                                                                                                                                   ] ;
                                                                                                                                                         rdf:rest [ rdf:type <http://www.w3.org/2003/11/swrl#AtomList> ;
                                                                                                                                                                    rdf:first [ rdf:type <http://www.w3.org/2003/11/swrl#IndividualPropertyAtom> ;
                                                                                                                                                                                <http://www.w3.org/2003/11/swrl#propertyPredicate> :happensIn ;
                                                                                                                                                                                <http://www.w3.org/2003/11/swrl#argument1> <http://www.semanticweb.org/alencga1/ontologies/2023/2/PhenOWL/O1> ;
                                                                                                                                                                                <http://www.w3.org/2003/11/swrl#argument2> <http://www.semanticweb.org/alencga1/ontologies/2023/2/PhenOWL/S1>
                                                                                                                                                                              ] ;
                                                                                                                                                                    rdf:rest rdf:nil
                                                                                                                                                                  ]
                                                                                                                                                       ]
                                                                                                                                            ]
                                                                                                                                 ]
                                                                                                                      ]
                                                                                                           ]
                                                                                                ]
                                                                                     ]
                                                                          ]
                                                               ]
                                                    ]
                                         ] ;
   <http://www.w3.org/2003/11/swrl#head> [ rdf:type <http://www.w3.org/2003/11/swrl#AtomList> ;
                                           rdf:first [ rdf:type <http://www.w3.org/2003/11/swrl#IndividualPropertyAtom> ;
                                                       <http://www.w3.org/2003/11/swrl#propertyPredicate> :observationalPresenceIn ;
                                                       <http://www.w3.org/2003/11/swrl#argument1> <http://www.semanticweb.org/alencga1/ontologies/2023/2/PhenOWL/PR1> ;
                                                       <http://www.w3.org/2003/11/swrl#argument2> <http://www.semanticweb.org/alencga1/ontologies/2023/2/PhenOWL/O1>
                                                     ] ;
                                           rdf:rest rdf:nil
                                         ]
 ] .

[ <http://swrl.stanford.edu/ontologies/3.3/swrla.owl#isRuleEnabled> "true"^^xsd:boolean ;
   rdfs:comment "If presence of cluster of individuals happens in one spatial region SO2, it must also happen in a region equals to it (SO1):" ;
   rdfs:label "S1.2 - Presence SO eq" ;
   rdf:type <http://www.w3.org/2003/11/swrl#Imp> ;
   <http://www.w3.org/2003/11/swrl#body> [ rdf:type <http://www.w3.org/2003/11/swrl#AtomList> ;
                                           rdf:first [ rdf:type <http://www.w3.org/2003/11/swrl#IndividualPropertyAtom> ;
                                                       <http://www.w3.org/2003/11/swrl#propertyPredicate> :spatialPresenceIn ;
                                                       <http://www.w3.org/2003/11/swrl#argument1> <http://www.semanticweb.org/alencga1/ontologies/2023/2/PhenOWL/PR1> ;
                                                       <http://www.w3.org/2003/11/swrl#argument2> <http://www.semanticweb.org/alencga1/ontologies/2023/2/PhenOWL/SO1>
                                                     ] ;
                                           rdf:rest [ rdf:type <http://www.w3.org/2003/11/swrl#AtomList> ;
                                                      rdf:first [ rdf:type <http://www.w3.org/2003/11/swrl#ClassAtom> ;
                                                                  <http://www.w3.org/2003/11/swrl#classPredicate> <http://www.opengis.net/ont/geosparql#SpatialObject> ;
                                                                  <http://www.w3.org/2003/11/swrl#argument1> <http://www.semanticweb.org/alencga1/ontologies/2023/2/PhenOWL/SO2>
                                                                ] ;
                                                      rdf:rest [ rdf:type <http://www.w3.org/2003/11/swrl#AtomList> ;
                                                                 rdf:first [ rdf:type <http://www.w3.org/2003/11/swrl#ClassAtom> ;
                                                                             <http://www.w3.org/2003/11/swrl#classPredicate> <http://www.opengis.net/ont/geosparql#SpatialObject> ;
                                                                             <http://www.w3.org/2003/11/swrl#argument1> <http://www.semanticweb.org/alencga1/ontologies/2023/2/PhenOWL/SO1>
                                                                           ] ;
                                                                 rdf:rest [ rdf:type <http://www.w3.org/2003/11/swrl#AtomList> ;
                                                                            rdf:first [ rdf:type <http://www.w3.org/2003/11/swrl#ClassAtom> ;
                                                                                        <http://www.w3.org/2003/11/swrl#classPredicate> :Presence ;
                                                                                        <http://www.w3.org/2003/11/swrl#argument1> <http://www.semanticweb.org/alencga1/ontologies/2023/2/PhenOWL/PR1>
                                                                                      ] ;
                                                                            rdf:rest [ rdf:type <http://www.w3.org/2003/11/swrl#AtomList> ;
                                                                                       rdf:first [ rdf:type <http://www.w3.org/2003/11/swrl#IndividualPropertyAtom> ;
                                                                                                   <http://www.w3.org/2003/11/swrl#propertyPredicate> <http://www.opengis.net/ont/geosparql#rcc8eq> ;
                                                                                                   <http://www.w3.org/2003/11/swrl#argument1> <http://www.semanticweb.org/alencga1/ontologies/2023/2/PhenOWL/SO1> ;
                                                                                                   <http://www.w3.org/2003/11/swrl#argument2> <http://www.semanticweb.org/alencga1/ontologies/2023/2/PhenOWL/SO2>
                                                                                                 ] ;
                                                                                       rdf:rest rdf:nil
                                                                                     ]
                                                                          ]
                                                               ]
                                                    ]
                                         ] ;
   <http://www.w3.org/2003/11/swrl#head> [ rdf:type <http://www.w3.org/2003/11/swrl#AtomList> ;
                                           rdf:first [ rdf:type <http://www.w3.org/2003/11/swrl#IndividualPropertyAtom> ;
                                                       <http://www.w3.org/2003/11/swrl#propertyPredicate> :spatialPresenceIn ;
                                                       <http://www.w3.org/2003/11/swrl#argument1> <http://www.semanticweb.org/alencga1/ontologies/2023/2/PhenOWL/PR1> ;
                                                       <http://www.w3.org/2003/11/swrl#argument2> <http://www.semanticweb.org/alencga1/ontologies/2023/2/PhenOWL/SO2>
                                                     ] ;
                                           rdf:rest rdf:nil
                                         ]
 ] .

[ <http://swrl.stanford.edu/ontologies/3.3/swrla.owl#isRuleEnabled> "true"^^xsd:boolean ;
   rdfs:comment "If presence of cluster of individuals happens in one spatial region SO2, it must also happen in a region containing it (SO1)" ;
   rdfs:label "S1.1 - Presence SO ttp" ;
   rdf:type <http://www.w3.org/2003/11/swrl#Imp> ;
   <http://www.w3.org/2003/11/swrl#body> [ rdf:type <http://www.w3.org/2003/11/swrl#AtomList> ;
                                           rdf:first [ rdf:type <http://www.w3.org/2003/11/swrl#IndividualPropertyAtom> ;
                                                       <http://www.w3.org/2003/11/swrl#propertyPredicate> :spatialPresenceIn ;
                                                       <http://www.w3.org/2003/11/swrl#argument1> <http://www.semanticweb.org/alencga1/ontologies/2023/2/PhenOWL/PR1> ;
                                                       <http://www.w3.org/2003/11/swrl#argument2> <http://www.semanticweb.org/alencga1/ontologies/2023/2/PhenOWL/SO1>
                                                     ] ;
                                           rdf:rest [ rdf:type <http://www.w3.org/2003/11/swrl#AtomList> ;
                                                      rdf:first [ rdf:type <http://www.w3.org/2003/11/swrl#ClassAtom> ;
                                                                  <http://www.w3.org/2003/11/swrl#classPredicate> <http://www.opengis.net/ont/geosparql#SpatialObject> ;
                                                                  <http://www.w3.org/2003/11/swrl#argument1> <http://www.semanticweb.org/alencga1/ontologies/2023/2/PhenOWL/SO2>
                                                                ] ;
                                                      rdf:rest [ rdf:type <http://www.w3.org/2003/11/swrl#AtomList> ;
                                                                 rdf:first [ rdf:type <http://www.w3.org/2003/11/swrl#ClassAtom> ;
                                                                             <http://www.w3.org/2003/11/swrl#classPredicate> <http://www.opengis.net/ont/geosparql#SpatialObject> ;
                                                                             <http://www.w3.org/2003/11/swrl#argument1> <http://www.semanticweb.org/alencga1/ontologies/2023/2/PhenOWL/SO1>
                                                                           ] ;
                                                                 rdf:rest [ rdf:type <http://www.w3.org/2003/11/swrl#AtomList> ;
                                                                            rdf:first [ rdf:type <http://www.w3.org/2003/11/swrl#ClassAtom> ;
                                                                                        <http://www.w3.org/2003/11/swrl#classPredicate> :Presence ;
                                                                                        <http://www.w3.org/2003/11/swrl#argument1> <http://www.semanticweb.org/alencga1/ontologies/2023/2/PhenOWL/PR1>
                                                                                      ] ;
                                                                            rdf:rest [ rdf:type <http://www.w3.org/2003/11/swrl#AtomList> ;
                                                                                       rdf:first [ rdf:type <http://www.w3.org/2003/11/swrl#IndividualPropertyAtom> ;
                                                                                                   <http://www.w3.org/2003/11/swrl#propertyPredicate> <http://www.opengis.net/ont/geosparql#rcc8tpp> ;
                                                                                                   <http://www.w3.org/2003/11/swrl#argument1> <http://www.semanticweb.org/alencga1/ontologies/2023/2/PhenOWL/SO1> ;
                                                                                                   <http://www.w3.org/2003/11/swrl#argument2> <http://www.semanticweb.org/alencga1/ontologies/2023/2/PhenOWL/SO2>
                                                                                                 ] ;
                                                                                       rdf:rest rdf:nil
                                                                                     ]
                                                                          ]
                                                               ]
                                                    ]
                                         ] ;
   <http://www.w3.org/2003/11/swrl#head> [ rdf:type <http://www.w3.org/2003/11/swrl#AtomList> ;
                                           rdf:first [ rdf:type <http://www.w3.org/2003/11/swrl#IndividualPropertyAtom> ;
                                                       <http://www.w3.org/2003/11/swrl#propertyPredicate> :spatialPresenceIn ;
                                                       <http://www.w3.org/2003/11/swrl#argument1> <http://www.semanticweb.org/alencga1/ontologies/2023/2/PhenOWL/PR1> ;
                                                       <http://www.w3.org/2003/11/swrl#argument2> <http://www.semanticweb.org/alencga1/ontologies/2023/2/PhenOWL/SO2>
                                                     ] ;
                                           rdf:rest rdf:nil
                                         ]
 ] .

[ <http://swrl.stanford.edu/ontologies/3.3/swrla.owl#isRuleEnabled> "true"^^xsd:boolean ;
   rdfs:comment "If presence of cluster of individuals happens in one spatial region SO2, it must also happen in a region containing it (SO1):" ;
   rdfs:label "S1.3 - Presence SO nttp" ;
   rdf:type <http://www.w3.org/2003/11/swrl#Imp> ;
   <http://www.w3.org/2003/11/swrl#body> [ rdf:type <http://www.w3.org/2003/11/swrl#AtomList> ;
                                           rdf:first [ rdf:type <http://www.w3.org/2003/11/swrl#IndividualPropertyAtom> ;
                                                       <http://www.w3.org/2003/11/swrl#propertyPredicate> <http://www.opengis.net/ont/geosparql#rcc8ntpp> ;
                                                       <http://www.w3.org/2003/11/swrl#argument1> <http://www.semanticweb.org/alencga1/ontologies/2023/2/PhenOWL/SO1> ;
                                                       <http://www.w3.org/2003/11/swrl#argument2> <http://www.semanticweb.org/alencga1/ontologies/2023/2/PhenOWL/SO2>
                                                     ] ;
                                           rdf:rest [ rdf:type <http://www.w3.org/2003/11/swrl#AtomList> ;
                                                      rdf:first [ rdf:type <http://www.w3.org/2003/11/swrl#IndividualPropertyAtom> ;
                                                                  <http://www.w3.org/2003/11/swrl#propertyPredicate> :spatialPresenceIn ;
                                                                  <http://www.w3.org/2003/11/swrl#argument1> <http://www.semanticweb.org/alencga1/ontologies/2023/2/PhenOWL/PR1> ;
                                                                  <http://www.w3.org/2003/11/swrl#argument2> <http://www.semanticweb.org/alencga1/ontologies/2023/2/PhenOWL/SO1>
                                                                ] ;
                                                      rdf:rest [ rdf:type <http://www.w3.org/2003/11/swrl#AtomList> ;
                                                                 rdf:first [ rdf:type <http://www.w3.org/2003/11/swrl#ClassAtom> ;
                                                                             <http://www.w3.org/2003/11/swrl#classPredicate> <http://www.opengis.net/ont/geosparql#SpatialObject> ;
                                                                             <http://www.w3.org/2003/11/swrl#argument1> <http://www.semanticweb.org/alencga1/ontologies/2023/2/PhenOWL/SO2>
                                                                           ] ;
                                                                 rdf:rest [ rdf:type <http://www.w3.org/2003/11/swrl#AtomList> ;
                                                                            rdf:first [ rdf:type <http://www.w3.org/2003/11/swrl#ClassAtom> ;
                                                                                        <http://www.w3.org/2003/11/swrl#classPredicate> <http://www.opengis.net/ont/geosparql#SpatialObject> ;
                                                                                        <http://www.w3.org/2003/11/swrl#argument1> <http://www.semanticweb.org/alencga1/ontologies/2023/2/PhenOWL/SO1>
                                                                                      ] ;
                                                                            rdf:rest [ rdf:type <http://www.w3.org/2003/11/swrl#AtomList> ;
                                                                                       rdf:first [ rdf:type <http://www.w3.org/2003/11/swrl#ClassAtom> ;
                                                                                                   <http://www.w3.org/2003/11/swrl#classPredicate> :Presence ;
                                                                                                   <http://www.w3.org/2003/11/swrl#argument1> <http://www.semanticweb.org/alencga1/ontologies/2023/2/PhenOWL/PR1>
                                                                                                 ] ;
                                                                                       rdf:rest rdf:nil
                                                                                     ]
                                                                          ]
                                                               ]
                                                    ]
                                         ] ;
   <http://www.w3.org/2003/11/swrl#head> [ rdf:type <http://www.w3.org/2003/11/swrl#AtomList> ;
                                           rdf:first [ rdf:type <http://www.w3.org/2003/11/swrl#IndividualPropertyAtom> ;
                                                       <http://www.w3.org/2003/11/swrl#propertyPredicate> :spatialPresenceIn ;
                                                       <http://www.w3.org/2003/11/swrl#argument1> <http://www.semanticweb.org/alencga1/ontologies/2023/2/PhenOWL/PR1> ;
                                                       <http://www.w3.org/2003/11/swrl#argument2> <http://www.semanticweb.org/alencga1/ontologies/2023/2/PhenOWL/SO2>
                                                     ] ;
                                           rdf:rest rdf:nil
                                         ]
 ] .

###  Generated by the OWL API (version 5.1.18) https://github.com/owlcs/owlapi/
